@prefix : <http://w3id.org/meta-share/omtd-share/> .
@prefix owl: <http://www.w3.org/2002/07/owl#> .
@prefix rdf: <http://www.w3.org/1999/02/22-rdf-syntax-ns#> .
@prefix xml: <http://www.w3.org/XML/1998/namespace> .
@prefix xsd: <http://www.w3.org/2001/XMLSchema#> .
@prefix rdfs: <http://www.w3.org/2000/01/rdf-schema#> .
@base <http://w3id.org/meta-share/omtd-share/> .

<http://w3id.org/meta-share/omtd-share/> rdf:type owl:Ontology ;
                                          <http://purl.org/dc/elements/1.1/date> "2015-05-15" ;
                                          <http://purl.org/dc/elements/1.1/description> "OMTD-SHARE ontology for resources related to Text and Data Mining initiated in the framework of the OpenMinTeD project (https://www.openminted.eu). It currently focuses on TDM functions (tasks performed by TDM software), annotation types (types of information extracted or annotated by TDM software), TDM methods (classification of the theoretical method used in the TDM algorithm), and data formats of the resoures that can be processed by TDM software. The ontology is deployed in the OMTD-SHARE metadata schema for the description of such resources (https://openminted.github.io/releases/omtd-share/) and is based on work done previously in the framework of the META-SHARE schema for language resources(http://www.meta-share.org/knowledgebase/homePage) and the FOSTER taxonomy of TDM (https://www.fosteropenscience.eu/resources)." ;
                                          <http://purl.org/dc/elements/1.1/title> "OMTD-SHARE ontology" ;
                                          <http://purl.org/dc/terms/contributor> "Richard Eckart de Castilho" ;
                                          <http://purl.org/dc/terms/creator> "Claire Nedellec" ,
                                                                             "Dimitris Galanis" ,
                                                                             "Katerina Gkirtzou" ,
                                                                             "Marta Villegas" ,
                                                                             "Penny Labropoulou" ,
                                                                             "Petr Knoth" ,
                                                                             "Sophie Aubin" ;
                                          <http://purl.org/dc/terms/issued> "2019-05-15" ;
                                          <http://purl.org/dc/terms/license> <http://purl.org/NET/rdflicense/cc-by4.0> ;
                                          <http://purl.org/vocab/vann/preferredNamespacePrefix> "omtd" ;
                                          rdfs:comment """The OMTD-SHARE ontology is intended for resources related to Text and Data Mining. 
	It currently focuses on TDM functions (tasks performed by TDM software), annotation types (types of information extracted or annotated by TDM software), TDM methods (classification of the theoretical method used in the TDM algorithm), and data formats of the resoures that can be processed by TDM software. The ontology is deployed in the OMTD-SHARE metadata schema for the description of such resources (https://openminted.github.io/releases/omtd-share/). 
	The ontology has been initiated in the framework of the OpenMinTeD project (https://www.openminted.eu). It is based on work done previously in the framework of the META-SHARE schema for language resources(http://www.meta-share.org/knowledgebase/homePage) and the FOSTER taxonomy of TDM (https://www.fosteropenscience.eu/resources).
	The ontology is still in a working status.""" ;
                                          rdfs:label "OMTD-SHARE ontology"@en ;
                                          owl:priorVersion "1.1.0" ;
                                          owl:versionInfo "pre-release 2.0.0" .

#################################################################
#    Annotation properties
#################################################################

###  http://purl.org/dc/elements/1.1/date
<http://purl.org/dc/elements/1.1/date> rdf:type owl:AnnotationProperty .


###  http://purl.org/dc/elements/1.1/description
<http://purl.org/dc/elements/1.1/description> rdf:type owl:AnnotationProperty .


###  http://purl.org/dc/elements/1.1/source
<http://purl.org/dc/elements/1.1/source> rdf:type owl:AnnotationProperty .


###  http://purl.org/dc/elements/1.1/title
<http://purl.org/dc/elements/1.1/title> rdf:type owl:AnnotationProperty .


###  http://purl.org/dc/terms/contributor
<http://purl.org/dc/terms/contributor> rdf:type owl:AnnotationProperty .


###  http://purl.org/dc/terms/creator
<http://purl.org/dc/terms/creator> rdf:type owl:AnnotationProperty .


###  http://purl.org/dc/terms/issued
<http://purl.org/dc/terms/issued> rdf:type owl:AnnotationProperty .


###  http://purl.org/dc/terms/license
<http://purl.org/dc/terms/license> rdf:type owl:AnnotationProperty .


###  http://purl.org/dc/terms/replaces
<http://purl.org/dc/terms/replaces> rdf:type owl:AnnotationProperty .


###  http://purl.org/vocab/vann/preferredNamespacePrefix
<http://purl.org/vocab/vann/preferredNamespacePrefix> rdf:type owl:AnnotationProperty .


###  http://www.w3.org/2000/01/rdf-schema#altLabel
rdfs:altLabel rdf:type owl:AnnotationProperty .


###  http://www.w3.org/2004/02/skos/core#altLabel
<http://www.w3.org/2004/02/skos/core#altLabel> rdf:type owl:AnnotationProperty .


###  http://www.w3.org/2004/02/skos/core#comment
<http://www.w3.org/2004/02/skos/core#comment> rdf:type owl:AnnotationProperty .


###  http://www.w3.org/2004/02/skos/core#definition
<http://www.w3.org/2004/02/skos/core#definition> rdf:type owl:AnnotationProperty .


###  http://www.w3.org/2004/02/skos/core#example
<http://www.w3.org/2004/02/skos/core#example> rdf:type owl:AnnotationProperty .


###  http://www.w3.org/2004/02/skos/core#related
<http://www.w3.org/2004/02/skos/core#related> rdf:type owl:AnnotationProperty .


#################################################################
#    Object Properties
#################################################################

###  http://w3id.org/meta-share/omtd-share/deployedInDomain
:deployedInDomain rdf:type owl:ObjectProperty ;
                  rdfs:subPropertyOf owl:topObjectProperty ;
                  rdfs:domain :Operation ;
                  rdfs:range :Domain ;
                  rdfs:comment "Concept A is used frequently in domain B"@en ;
                  rdfs:label "deployed in domain"@en .


###  http://w3id.org/meta-share/omtd-share/hasAnnotationType
:hasAnnotationType rdf:type owl:ObjectProperty ;
                   rdfs:subPropertyOf owl:topObjectProperty ;
                   rdfs:domain :Annotation ;
                   rdfs:range :AnnotationType ;
                   rdfs:comment "Used to classify annotations"@en ;
                   rdfs:label "has annotation type"@en .


###  http://w3id.org/meta-share/omtd-share/hasDataFormat
:hasDataFormat rdf:type owl:ObjectProperty ;
               rdfs:range :DataFormat ;
               rdfs:label "data format"@en .


###  http://w3id.org/meta-share/omtd-share/hasMethod
:hasMethod rdf:type owl:ObjectProperty ;
           rdfs:range :TdmMethod ;
           rdfs:label "method"@en .


###  http://w3id.org/meta-share/omtd-share/hasMimetype
:hasMimetype rdf:type owl:ObjectProperty ;
             rdfs:subPropertyOf owl:topObjectProperty ;
             rdfs:domain :DataFormat ;
             rdfs:range :Mimetype ;
             rdfs:comment "Relates a data format to the IANA mimetype; it can be the exact or a broader mimetype; unofficial mimetypes are also used, but this relation will be revisited"@en ;
             rdfs:label "has mimetype"@en .


###  http://w3id.org/meta-share/omtd-share/performsOperation
:performsOperation rdf:type owl:ObjectProperty ;
                   rdfs:subPropertyOf owl:topObjectProperty ;
                   rdfs:domain :ComponentType ;
                   rdfs:range :Operation ;
                   rdfs:comment "Component A performs Operation B"@en ;
                   rdfs:label "performs Operation"@en ;
                   <http://www.w3.org/2004/02/skos/core#altLabel> "performs Task"@en .


###  http://www.w3.org/2000/01/rdf-schema#seeAlso
rdfs:seeAlso rdf:type owl:ObjectProperty .


###  http://www.w3.org/2002/07/owl#equivalentClass
owl:equivalentClass rdf:type owl:ObjectProperty ;
                    rdfs:label "owl:equivalentClass" .


###  http://www.w3.org/2004/02/skos/core#closeMatch
<http://www.w3.org/2004/02/skos/core#closeMatch> rdf:type owl:ObjectProperty .


###  http://www.w3.org/2004/02/skos/core#relatedTo
<http://www.w3.org/2004/02/skos/core#relatedTo> rdf:type owl:ObjectProperty .


#################################################################
#    Data properties
#################################################################

###  http://w3id.org/meta-share/omtd-share/documentationUrl
:documentationUrl rdf:type owl:DatatypeProperty ;
                  rdfs:subPropertyOf owl:topDataProperty ;
                  rdfs:domain owl:Thing ;
                  rdfs:range xsd:anyURI ;
                  rdfs:comment "The URL link in which a concept is documented"@en ;
                  rdfs:label "documentation URL"@en .


###  http://w3id.org/meta-share/omtd-share/hasFileExtension
:hasFileExtension rdf:type owl:DatatypeProperty ;
                  rdfs:subPropertyOf owl:topDataProperty ;
                  rdfs:domain :DataFormat ;
                  rdfs:range xsd:string ;
                  rdfs:comment "The file extension usually associated with a specific data format (e.g. txt for plain text files, pdf for PDF files etc.)"@en ;
                  rdfs:label "has file extension"@en .


###  http://www.w3.org/2004/02/skos/core#broadMatch
<http://www.w3.org/2004/02/skos/core#broadMatch> rdf:type owl:DatatypeProperty .


#################################################################
#    Classes
#################################################################

###  http://purl.org/olia/olia-top.owl#Clause
<http://purl.org/olia/olia-top.owl#Clause> rdf:type owl:Class .


###  http://purl.org/olia/olia-top.owl#Constituent
<http://purl.org/olia/olia-top.owl#Constituent> rdf:type owl:Class .


###  http://purl.org/olia/olia-top.owl#Date
<http://purl.org/olia/olia-top.owl#Date> rdf:type owl:Class .


###  http://purl.org/olia/olia-top.owl#DiscourseFeature
<http://purl.org/olia/olia-top.owl#DiscourseFeature> rdf:type owl:Class .


###  http://purl.org/olia/olia-top.owl#Frame
<http://purl.org/olia/olia-top.owl#Frame> rdf:type owl:Class .


###  http://purl.org/olia/olia-top.owl#LexicalRelation
<http://purl.org/olia/olia-top.owl#LexicalRelation> rdf:type owl:Class .


###  http://purl.org/olia/olia-top.owl#MorphosyntacticCategory
<http://purl.org/olia/olia-top.owl#MorphosyntacticCategory> rdf:type owl:Class .


###  http://purl.org/olia/olia-top.owl#MorphosyntacticFeature
<http://purl.org/olia/olia-top.owl#MorphosyntacticFeature> rdf:type owl:Class .


###  http://purl.org/olia/olia-top.owl#NamedEntity
<http://purl.org/olia/olia-top.owl#NamedEntity> rdf:type owl:Class .


###  http://purl.org/olia/olia-top.owl#Phrase
<http://purl.org/olia/olia-top.owl#Phrase> rdf:type owl:Class .


###  http://purl.org/olia/olia-top.owl#PolarityFeature
<http://purl.org/olia/olia-top.owl#PolarityFeature> rdf:type owl:Class .


###  http://purl.org/olia/olia-top.owl#SemanticFeature
<http://purl.org/olia/olia-top.owl#SemanticFeature> rdf:type owl:Class .


###  http://purl.org/olia/olia-top.owl#SemanticRole
<http://purl.org/olia/olia-top.owl#SemanticRole> rdf:type owl:Class .


###  http://purl.org/olia/olia-top.owl#Sentence
<http://purl.org/olia/olia-top.owl#Sentence> rdf:type owl:Class .


###  http://purl.org/olia/olia-top.owl#Stem
<http://purl.org/olia/olia-top.owl#Stem> rdf:type owl:Class .


###  http://purl.org/olia/olia-top.owl#SyntacticCategory
<http://purl.org/olia/olia-top.owl#SyntacticCategory> rdf:type owl:Class .


###  http://purl.org/olia/olia-top.owl#Token
<http://purl.org/olia/olia-top.owl#Token> rdf:type owl:Class .


###  http://purl.org/olia/olia-top.owl#Word
<http://purl.org/olia/olia-top.owl#Word> rdf:type owl:Class .


###  http://vocab.lappsgrid.org/Annotation
<http://vocab.lappsgrid.org/Annotation> rdf:type owl:Class .


###  http://vocab.lappsgrid.org/Constituent
<http://vocab.lappsgrid.org/Constituent> rdf:type owl:Class .


###  http://vocab.lappsgrid.org/Coreference
<http://vocab.lappsgrid.org/Coreference> rdf:type owl:Class .


###  http://vocab.lappsgrid.org/Dependency
<http://vocab.lappsgrid.org/Dependency> rdf:type owl:Class .


###  http://vocab.lappsgrid.org/Document
<http://vocab.lappsgrid.org/Document> rdf:type owl:Class .


###  http://vocab.lappsgrid.org/NamedEntity
<http://vocab.lappsgrid.org/NamedEntity> rdf:type owl:Class .


###  http://vocab.lappsgrid.org/Paragraph
<http://vocab.lappsgrid.org/Paragraph> rdf:type owl:Class .


###  http://vocab.lappsgrid.org/SemanticRole
<http://vocab.lappsgrid.org/SemanticRole> rdf:type owl:Class .


###  http://vocab.lappsgrid.org/Token
<http://vocab.lappsgrid.org/Token> rdf:type owl:Class .


###  http://w3id.org/meta-share/omtd-share/AccessComponent
:AccessComponent rdf:type owl:Class ;
                 rdfs:subClassOf :ComponentType ,
                                 [ rdf:type owl:Restriction ;
                                   owl:onProperty :performsOperation ;
                                   owl:someValuesFrom :ResourceAccess
                                 ] ;
                 rdfs:comment "A component that provides access to data resources, e.g. reads a resource or writes the output of a process in a certain format"@en ;
                 rdfs:label "Access Component"@en .


###  http://w3id.org/meta-share/omtd-share/AclAnthologyCorpusFormat
:AclAnthologyCorpusFormat rdf:type owl:Class ;
                          rdfs:subClassOf :CorpusFormat ,
                                          [ rdf:type owl:Restriction ;
                                            owl:onProperty :hasMimetype ;
                                            owl:hasValue :text_plain
                                          ] ,
                                          [ rdf:type owl:Restriction ;
                                            owl:onProperty :documentationUrl ;
                                            owl:hasValue "https://dkpro.github.io/dkpro-core/releases/1.8.0/docs/format-reference.html#format-AclAnthology"
                                          ] ,
                                          [ rdf:type owl:Restriction ;
                                            owl:onProperty :documentationUrl ;
                                            owl:hasValue "https://dkpro.github.io/dkpro-core/releases/1.8.0/docs/format-reference.html#format-de.tudarmstadt.ukp.dkpro.core.io.aclanthology-asl"
                                          ] ;
                          rdfs:comment "Data format specific to the ACL Anthology Reference Corpus (http://acl-arc.comp.nus.edu.sg/), most probably version 20080325"@en ;
                          rdfs:label "ACL Anthology Corpus format"@en .


###  http://w3id.org/meta-share/omtd-share/AgeBracketDetection
:AgeBracketDetection rdf:type owl:Class ;
                     rdfs:subClassOf :InformationExtraction ;
                     rdfs:comment "The task/process of identifying in a text a segment inside parentheses that describes an age group or age-related utterance"@en ;
                     rdfs:label "Age-bracket detection"@en .


###  http://w3id.org/meta-share/omtd-share/AgriculturalEntity
:AgriculturalEntity rdf:type owl:Class ;
                    rdfs:subClassOf :Domain-specificAnnotation ,
                                    :DomainSpecificAnnotationType ;
                    rdfs:comment "Any kind of annotation pertaining to entities of the agricultural domain; the use of the AGROVOC thesaurus is recommended"@en ;
                    rdfs:label "Agricultural entity"@en .


###  http://w3id.org/meta-share/omtd-share/Agriculture
:Agriculture rdf:type owl:Class ;
             rdfs:subClassOf :Domain ;
             rdfs:comment "The science, art, or practice of cultivating the soil, producing crops, and raising livestock and in varying degrees the preparation and marketing of the resulting products [https://www.merriam-webster.com/dictionary/agriculture]"@en ;
             rdfs:label "Agriculture"@en .


###  http://w3id.org/meta-share/omtd-share/AimedCorpusFormat
:AimedCorpusFormat rdf:type owl:Class ;
                   rdfs:subClassOf :CorpusFormat ,
                                   [ rdf:type owl:Restriction ;
                                     owl:onProperty :documentationUrl ;
                                     owl:hasValue "https://builds.openminted.eu/job/WP%205.2%20-%20Typesystem%20alignment/eu.openminted.interop$mapping-conversion/doclinks/1/components.html#Aimed_Collection_Reader"
                                   ] ;
                   rdfs:comment "Format of the Aimed corpus (225 abstracts from MEDLINE) with the gold standard sentence, protein, protein-protein interaction annotations."@en ;
                   rdfs:label "AIMED corpus format"@en .


###  http://w3id.org/meta-share/omtd-share/Aligner
:Aligner rdf:type owl:Class ;
         rdfs:subClassOf :Annotator ;
         rdfs:comment "A component that detects and annotates equivalence relations between items (corpora, texts, paragraphs, sentences, phrases, words) in two languages"@en ;
         rdfs:label "Aligner"@en .


###  http://w3id.org/meta-share/omtd-share/Alignment
:Alignment rdf:type owl:Class ;
           rdfs:subClassOf :MachineTranslationSupport ;
           rdfs:comment "Establishment of translational equivalences between structural units (words, sentences etc.) of a text in a given language and a text with similar meaning in other language(s)"@en ;
           rdfs:label "Alignment"@en .


###  http://w3id.org/meta-share/omtd-share/Alignment1
:Alignment1 rdf:type owl:Class ;
            rdfs:subClassOf :AnnotationType ;
            rdfs:comment "The translational equivalent between structural units (words, sentences etc.) of a text in a given language and a text with similar meaning in other language(s)"@en ;
            rdfs:label "Alignment"@en .


###  http://w3id.org/meta-share/omtd-share/AllbusVariable
:AllbusVariable rdf:type owl:Class ;
                rdfs:subClassOf :SocialSciencesEntity ;
                rdfs:comment "ALLBUS variable"@en ;
                rdfs:label "ALLBUS variable"@en .


###  http://w3id.org/meta-share/omtd-share/Alto
:Alto rdf:type owl:Class ;
      rdfs:subClassOf :Xml ,
                      [ rdf:type owl:Restriction ;
                        owl:onProperty :hasMimetype ;
                        owl:hasValue :application_xml_alto
                      ] ,
                      [ rdf:type owl:Restriction ;
                        owl:onProperty :documentationUrl ;
                        owl:hasValue "https://en.wikipedia.org/wiki/ALTO_(XML)"
                      ] ;
      rdfs:label "ALTO" .


###  http://w3id.org/meta-share/omtd-share/AlvisEnrichedDocumentFormat
:AlvisEnrichedDocumentFormat rdf:type owl:Class ;
                             rdfs:subClassOf :AnnotationFormat ,
                                             :Xml ,
                                             [ rdf:type owl:Restriction ;
                                               owl:onProperty :hasMimetype ;
                                               owl:hasValue :application_xml
                                             ] ,
                                             [ rdf:type owl:Restriction ;
                                               owl:onProperty :documentationUrl ;
                                               owl:hasValue "http://www.lrec-conf.org/proceedings/lrec2006/pdf/742_pdf.pdf"
                                             ] ;
                             rdfs:comment "Format for linguistic annotations of documents used for the ALVIS framework"@en ;
                             rdfs:label "ALVIS Enriched Document format"@en .


###  http://w3id.org/meta-share/omtd-share/Anafora
:Anafora rdf:type owl:Class ;
         rdfs:subClassOf :AnnotationFormat ,
                         [ rdf:type owl:Restriction ;
                           owl:onProperty :hasMimetype ;
                           owl:hasValue :text_x_anafora
                         ] ,
                         [ rdf:type owl:Restriction ;
                           owl:onProperty :documentationUrl ;
                           owl:hasValue "https://www.ncbi.nlm.nih.gov/pmc/articles/PMC5657237/"
                         ] ;
         rdfs:label "Anafora" .


###  http://w3id.org/meta-share/omtd-share/Analyzer
:Analyzer rdf:type owl:Class ;
          rdfs:subClassOf :ComponentType ;
          rdfs:comment "A component that is used for analyzing an input text in order to extract specific features/information (e.g. word list), or to produce statements over the whole text (e.g. classify it by topic)"@en ;
          rdfs:label "Analyzer"@en ;
          <http://www.w3.org/2004/02/skos/core#altLabel> "Extractor"@en .


###  http://w3id.org/meta-share/omtd-share/AnaphoraAnnotation
:AnaphoraAnnotation rdf:type owl:Class ;
                    rdfs:subClassOf :DiscourseAnnotation ;
                    rdfs:comment "The process/task of marking all linguistic expressions that appear in a certain text or across texts as referring to the same entity and linking it to this entity"@en ;
                    rdfs:label "Anaphora annotation"@en ;
                    <http://www.w3.org/2004/02/skos/core#related> :CoReferenceAnnotation .


###  http://w3id.org/meta-share/omtd-share/AnaphoraResolution
:AnaphoraResolution rdf:type owl:Class ;
                    rdfs:subClassOf :LinguisticAnalysis ;
                    rdfs:comment "The process/task of identifying all linguistic expressions that appear in a certain text or across texts and refer to the same entity"@en ;
                    rdfs:label "Anaphora resolution"@en ;
                    <http://www.w3.org/2004/02/skos/core#related> :CoReferenceResolution .


###  http://w3id.org/meta-share/omtd-share/Annotation
:Annotation rdf:type owl:Class ;
            rdfs:subClassOf :Operation ;
            rdfs:comment "A note by way of explanation or comment added to a text or diagram [OED, https://en.oxforddictionaries.com/definition/annotation]. Text or corpus annotation refers to the interpretative linguistic information grounded in a knowledge resource that is added manually or automatically to a text or corpus respectively."@en ,
                         "The process/task of adding annotations to an item"@en ;
            rdfs:label "Annotation"@en ;
            <http://www.w3.org/2004/02/skos/core#altLabel> "Labeling [en-US]"@en-us ,
                                                           "Labelling"@en ,
                                                           "Tagging"@en .


###  http://w3id.org/meta-share/omtd-share/AnnotationFormat
:AnnotationFormat rdf:type owl:Class ;
                  rdfs:subClassOf :DataFormat ;
                  rdfs:comment "Any format used for annotated files"@en ;
                  rdfs:label "Annotation format"@en .


###  http://w3id.org/meta-share/omtd-share/AnnotationOfCompoundingFeatures
:AnnotationOfCompoundingFeatures rdf:type owl:Class ;
                                 rdfs:subClassOf :MorphologicalAnnotation ;
                                 rdfs:comment "The task/process of marking compounds (single words composed of two or more free morphemes) and their parts"@en ;
                                 rdfs:label "Annotation of compounds"@en ;
                                 owl:deprecated "true"^^xsd:boolean .


###  http://w3id.org/meta-share/omtd-share/AnnotationOfCompounds
:AnnotationOfCompounds rdf:type owl:Class ;
                       rdfs:subClassOf :MorphologicalAnnotation ;
                       <http://purl.org/dc/terms/replaces> :AnnotationOfCompoundingFeatures ;
                       rdfs:comment "The task/process of marking compounds (single words composed of two or more free morphemes) and their parts"@en ;
                       rdfs:label "Annotation of compounds"@en .


###  http://w3id.org/meta-share/omtd-share/AnnotationOfDates
:AnnotationOfDates rdf:type owl:Class ;
                   rdfs:subClassOf :TemporalExpressionsLabelling ;
                   rdfs:comment "The task/process of marking dates in a text"@en ;
                   rdfs:label "Annotation of dates"@en ;
                   <http://www.w3.org/2004/02/skos/core#altLabel> "Date Detection"@en ,
                                                                  "Date Recognition"@en .


###  http://w3id.org/meta-share/omtd-share/AnnotationOfDerivationalFeatures
:AnnotationOfDerivationalFeatures rdf:type owl:Class ;
                                  rdfs:subClassOf :MorphologicalAnnotation ;
                                  rdfs:comment "The task/process of adding annotations relevant to the derivational level of analysis (e.g. recognizing derivational affixes, tagging their meaning etc.)"@en ;
                                  rdfs:label "Annotation of derivational features"@en .


###  http://w3id.org/meta-share/omtd-share/AnnotationOfDocumentStructure
:AnnotationOfDocumentStructure rdf:type owl:Class ;
                               rdfs:subClassOf :StructuralAnnotation ;
                               rdfs:comment "The task/process of annotating the internal structure of a document (e.g. book chapters, sections in a journal article, title, preface, images/figures etc.)"@en ;
                               rdfs:label "Annotation of document structure"@en .


###  http://w3id.org/meta-share/omtd-share/AnnotationOfMeasurements
:AnnotationOfMeasurements rdf:type owl:Class ;
                          rdfs:subClassOf :SemanticAnnotation ;
                          rdfs:comment "The task/process of annotating measurement expressions (e.g. of length, temperature, time, etc.)"@en ;
                          rdfs:label "Annotation of measurements"@en ;
                          <http://www.w3.org/2004/02/skos/core#altLabel> "Quantity detection"@en ,
                                                                         "Quantity extraction"@en .


###  http://w3id.org/meta-share/omtd-share/AnnotationOfMultiWordUnits
:AnnotationOfMultiWordUnits rdf:type owl:Class ;
                            rdfs:subClassOf :MorphologicalAnnotation ;
                            rdfs:comment "The task/process of annotating multi-word units, i.e. combinations of words that are considered as one"@en ;
                            rdfs:label "Annotation of multi-word units"@en .


###  http://w3id.org/meta-share/omtd-share/AnnotationOfNumbers
:AnnotationOfNumbers rdf:type owl:Class ;
                     rdfs:subClassOf :SemanticAnnotation ;
                     rdfs:comment "The task/process of annotating numbers in a text"@en ;
                     rdfs:label "Annotation of numbers"@en ;
                     <http://www.w3.org/2004/02/skos/core#altLabel> "Number detection"@en .


###  http://w3id.org/meta-share/omtd-share/AnnotationOfQuestionTopics
:AnnotationOfQuestionTopics rdf:type owl:Class ;
                            rdfs:subClassOf :SemanticAnnotation ;
                            rdfs:comment "The task/process of attaching tags to the segment of a question that functions as the topic of that question"@en ;
                            rdfs:label "Annotation of question topics"@en ;
                            <http://www.w3.org/2004/02/skos/core#altLabel> "Annotation of question topical targets"@en .


###  http://w3id.org/meta-share/omtd-share/AnnotationOfSpeakerTurns
:AnnotationOfSpeakerTurns rdf:type owl:Class ;
                          rdfs:subClassOf :SpeechAnnotation ;
                          rdfs:comment "The task/process of marking locations in speech where there is a change of speakers"@en ;
                          rdfs:label "Annotation of speaker turns"@en .


###  http://w3id.org/meta-share/omtd-share/AnnotationOfTextualEntailment
:AnnotationOfTextualEntailment rdf:type owl:Class ;
                               rdfs:subClassOf :SemanticAnnotation ;
                               rdfs:comment "The task/process of annotating textual entailments, most usually indicating whether a text entails or contradicts a hypothesis sentence or does neither."@en ;
                               rdfs:label "Annotation of textual entailment"@en .


###  http://w3id.org/meta-share/omtd-share/AnnotationType
:AnnotationType rdf:type owl:Class ;
                rdfs:subClassOf owl:Thing ;
                rdfs:comment "Category/class of the annotations (metadata) that are added to the data/text that is processed"@en ;
                rdfs:label "Annotation type"@en ;
                <http://www.w3.org/2004/02/skos/core#altLabel> "Label"@en ,
                                                               "Tag"@en .


###  http://w3id.org/meta-share/omtd-share/Annotator
:Annotator rdf:type owl:Class ;
           rdfs:subClassOf :Processor ,
                           [ rdf:type owl:Restriction ;
                             owl:onProperty :performsOperation ;
                             owl:someValuesFrom :Annotation
                           ] ;
           rdfs:comment "A component that annotates any data (text, video, audio etc.), i.e. adds any descriptive or analytic notations (structural, linguistic, etc) to raw data"@en ;
           rdfs:label "Annotator"@en ;
           <http://www.w3.org/2004/02/skos/core#altLabel> "Tagger"@en .


###  http://w3id.org/meta-share/omtd-share/AnnotatorOfSemanticRoleLabels
:AnnotatorOfSemanticRoleLabels rdf:type owl:Class ;
                               rdfs:subClassOf :SemanticAnnotator ;
                               rdfs:comment "A component that annotates the tokens of a text with Semantic Role labels"@en ;
                               rdfs:label "Annotator of semantic role labels"@en .


###  http://w3id.org/meta-share/omtd-share/Anonymization
:Anonymization rdf:type owl:Class ;
               rdfs:subClassOf :SupportOperation ;
               rdfs:comment "The task/process through which particular text segments or data units that allow the identification of a person are removed or replaced"@en ;
               rdfs:label "Anonymization"@en ;
               <http://www.w3.org/2004/02/skos/core#altLabel> "Anonymisation [en-UK]"@en-uk .


###  http://w3id.org/meta-share/omtd-share/Argumentation
:Argumentation rdf:type owl:Class ;
               rdfs:subClassOf :DiscourseAnnotation ;
               rdfs:comment "The task/process of marking argumentative structures, components and relations in a text"@en ;
               rdfs:label "Annotation of argumentation"@en .


###  http://w3id.org/meta-share/omtd-share/ArtificialNeuralNetwork
:ArtificialNeuralNetwork rdf:type owl:Class ;
                         rdfs:subClassOf :MachineAndStatisticalLearningMethod ;
                         <http://purl.org/dc/elements/1.1/source> "adapted from wikipedia (https://en.wikipedia.org/wiki/Artificial_neural_network)"@en ;
                         rdfs:comment "A computational model based on a large collection of simple neural units (artificial neurons), loosely analogous to the observed behavior of a biological brain's axons. These systems are self-learning and trained, rather than explicitly programmed."@en ;
                         rdfs:label "Artificial Neural Network"@en .


###  http://w3id.org/meta-share/omtd-share/AssociationRuleLearning
:AssociationRuleLearning rdf:type owl:Class ;
                         rdfs:subClassOf :MachineAndStatisticalLearningMethod ;
                         rdfs:comment "A machine learning method used in recognising relationships among variables in databases and extracted in the form of rules."@en ;
                         rdfs:label "Association Rule Learning"@en ;
                         <http://www.w3.org/2004/02/skos/core#altLabel> "ANN"@en .


###  http://w3id.org/meta-share/omtd-share/AudienceReaction
:AudienceReaction rdf:type owl:Class ;
                  rdfs:subClassOf :DiscourseAnnotationType ;
                  rdfs:comment "The response of the target recipients (audience) to a system, process or event"@en ;
                  rdfs:label "Audience reaction"@en .


###  http://w3id.org/meta-share/omtd-share/AudioFormat
:AudioFormat rdf:type owl:Class ;
             rdfs:subClassOf :DataFormat ;
             rdfs:comment "Any format used for audio files"@en ;
             rdfs:label "Audio format"@en .


###  http://w3id.org/meta-share/omtd-share/AudioSegmentation
:AudioSegmentation rdf:type owl:Class ;
                   rdfs:subClassOf :SpeechAnnotation ;
                   rdfs:comment "The task/process of partitioning audio stream into homogeneous segments and classifying them into speech and non-speech segments"@en ;
                   rdfs:label "Audio segmentation"@en .


###  http://w3id.org/meta-share/omtd-share/AuthorClassification
:AuthorClassification rdf:type owl:Class ;
                      rdfs:subClassOf :InformationExtraction ;
                      rdfs:comment "The task/process of organizing documents into groups/classes on the basis of their author"@en ;
                      rdfs:label "Author classification"@en .


###  http://w3id.org/meta-share/omtd-share/AuthoringSupport
:AuthoringSupport rdf:type owl:Class ;
                  rdfs:subClassOf :Operation ;
                  rdfs:comment "The task/process of providing spelling, grammatical or stylistic suggestions as an aid for the authoring task"@en ;
                  rdfs:label "Authoring support"@en ;
                  <http://www.w3.org/2004/02/skos/core#altLabel> "Structure-Based Authoring Assistant"@en ,
                                                                 "Writing support"@en ;
                  <http://www.w3.org/2004/02/skos/core#definition> "Software for supporting the distributed creation of consistent, high-quality information on an industrial scale. Key components include terminology extraction for legacy information, terminology checking and hyperlinking integrated in standard authoring environments, as well as structural (syntactic) checking of texts to ensure readability, consistency and translatability."@en .


###  http://w3id.org/meta-share/omtd-share/AutomaticHyperlinking
:AutomaticHyperlinking rdf:type owl:Class ;
                       rdfs:subClassOf :InformationExtraction ;
                       rdfs:comment "The identification of hyperlinkable entities (concepts, named entities) in a text and the assignment of hyperlinks (link targets) for each such entity."@en ;
                       rdfs:label "Automatic hyperlinking"@en ;
                       <http://www.w3.org/2004/02/skos/core#definition> "Automatic hyperlinking is the insertion of hyperlinks into text documents by automatic means. The automatic hyperlinking process consists of the identification of hyperlinkable entities (concepts, named entities) in the original text, and the assignment of link targets for each such entity. Named entity recognition is often used for identifying linkable entities, for example geographical locations or organisation names. The assignment of link targets depends on a database with link targets for each entity. In general, there can be several link targets for each entity, for example for a company: its homepage, a map, a stock quote etc. Multiple outgoing hyperlinks from one target are supported by the W3C standard XLINK/XPointer. Automatic hyperlinking is an important technology for enabling the Semantic Web."@en .


###  http://w3id.org/meta-share/omtd-share/AutomaticSubtitling
:AutomaticSubtitling rdf:type owl:Class ;
                     rdfs:subClassOf :NaturalLanguageGeneration ;
                     rdfs:comment "The task/process of automatically adding subtitles to a video"@en ;
                     rdfs:label "Automatic subtitling"@en .


###  http://w3id.org/meta-share/omtd-share/Avro_json
:Avro_json rdf:type owl:Class ;
           rdfs:subClassOf :Json ,
                           [ rdf:type owl:Restriction ;
                             owl:onProperty :documentationUrl ;
                             owl:hasValue "https://avro.apache.org/docs/1.8.1/spec.html"
                           ] ;
           rdfs:label "Avro" .


###  http://w3id.org/meta-share/omtd-share/Bayesian
:Bayesian rdf:type owl:Class ;
          rdfs:subClassOf :MachineAndStatisticalLearningMethod ;
          <http://purl.org/dc/elements/1.1/source> "adapted from Wikipedia (https://en.wikipedia.org/wiki/Bayesian_inference)"@en ;
          rdfs:comment "A method in probability and statistics based on Bayes' theorem, mainly related to statistical inference."@en ;
          rdfs:label "Bayesian"@en .


###  http://w3id.org/meta-share/omtd-share/BelowPosTagging
:BelowPosTagging rdf:type owl:Class ;
                 rdfs:subClassOf :MorphologicalAnnotation ,
                                 :MorphosyntacticTagging ;
                 rdfs:comment "The annotation of words with morphological information besides the part of speech and dependent upon it (e.g. for nouns: gender, number and case; for verbs: tense, number, person etc.)"@en ;
                 rdfs:label "Below Part-of-Speech Tagging"@en ;
                 <http://www.w3.org/2004/02/skos/core#altLabel> "Annotation of morphological features"@en ,
                                                                "B-PoS Tagging"@en ,
                                                                "Below PoS Tagging"@en .


###  http://w3id.org/meta-share/omtd-share/BilingualLexiconInduction
:BilingualLexiconInduction rdf:type owl:Class ;
                           rdfs:subClassOf :KnowledgeAcquisition ,
                                           :SupportOperationForKnowledgeResources ;
                           rdfs:comment "The task/process of inducing word translations from monolingual or comparable corpora in two languages"@en ;
                           rdfs:label "Bilingual lexicon induction"@en .


###  http://w3id.org/meta-share/omtd-share/BinaryCas
:BinaryCas rdf:type owl:Class ;
           rdfs:subClassOf :UimaCasFormat ,
                           [ rdf:type owl:Restriction ;
                             owl:onProperty :hasMimetype ;
                             owl:hasValue :application_x_org_dkpro_uima_binary
                           ] ,
                           [ rdf:type owl:Restriction ;
                             owl:onProperty :documentationUrl ;
                             owl:hasValue "https://dkpro.github.io/dkpro-core/releases/1.8.0/docs/format-reference.html#format-de.tudarmstadt.ukp.dkpro.core.io.bincas-asl"
                           ] ;
           rdfs:comment "Binary format used for CAS data"@en ;
           rdfs:label "Binary CAS"@en ;
           <http://www.w3.org/2004/02/skos/core#altLabel> "UIMA Binary CAS"@en .


###  http://w3id.org/meta-share/omtd-share/BinaryFormat
:BinaryFormat rdf:type owl:Class ;
              rdfs:subClassOf :DataFormat ;
              rdfs:comment "Any format of a computer file in which information is stored in the form of ones and zeros, or in some other binary (two-state) sequence; used mainly for executable files or files that need to be interpreted by a computer program"@en ;
              rdfs:label "Binary format"@en .


###  http://w3id.org/meta-share/omtd-share/BiologicalActivity
:BiologicalActivity rdf:type owl:Class ;
                    rdfs:subClassOf :BiologicalEnity ,
                                    :NamedEntity ;
                    rdfs:comment "Biological activity"@en ;
                    rdfs:label "Biological activity"@en .


###  http://w3id.org/meta-share/omtd-share/BiologicalEnity
:BiologicalEnity rdf:type owl:Class ;
                 rdfs:subClassOf :Domain-specificAnnotation ,
                                 :DomainSpecificAnnotationType ;
                 rdfs:comment "Any kind of annotation pertaining to entities of biology"@en ;
                 rdfs:label "Biological enity"@en .


###  http://w3id.org/meta-share/omtd-share/BiomedicalConceptNormalization
:BiomedicalConceptNormalization rdf:type owl:Class ;
                                rdfs:subClassOf :ConceptNormalization ;
                                rdfs:comment "The task of mapping free-form expressions to medical terms [source: Medical concept normalization in social media posts with recurrent neural networks]"@en ;
                                rdfs:label "Biomedical concept normalization"@en ;
                                <http://www.w3.org/2004/02/skos/core#altLabel> "Biomedical concept normalisation"@en-uk .


###  http://w3id.org/meta-share/omtd-share/Bionlp
:Bionlp rdf:type owl:Class ;
        rdfs:subClassOf :BionlpFormat ,
                        :BionlpFormats ,
                        [ rdf:type owl:Restriction ;
                          owl:onProperty :documentationUrl ;
                          owl:hasValue "https://builds.openminted.eu/job/WP%205.2%20-%20Typesystem%20alignment/eu.openminted.interop$mapping-conversion/doclinks/1/components.html#_bionlp_shared_task_2"
                        ] ;
        rdfs:comment "File format used for the BioNLP Shared Task format"@en ;
        rdfs:label "BioNLP"@en .


###  http://w3id.org/meta-share/omtd-share/BionlpFormat
:BionlpFormat rdf:type owl:Class ;
              rdfs:subClassOf :DocumentFormat ;
              <http://purl.org/dc/terms/replaces> :BionlpFormats ;
              rdfs:comment "Formats used  for BioNLP shared tasks"@en ;
              rdfs:label "BioNLP format"@en .


###  http://w3id.org/meta-share/omtd-share/BionlpFormats
:BionlpFormats rdf:type owl:Class ;
               rdfs:subClassOf :DocumentFormat ;
               rdfs:comment "Formats used  for BioNLP shared tasks"@en ;
               rdfs:label "BioNLP formats"@en ;
               owl:deprecated "true"^^xsd:boolean .


###  http://w3id.org/meta-share/omtd-share/BionlpSt2013A1_a2
:BionlpSt2013A1_a2 rdf:type owl:Class ;
                   rdfs:subClassOf :BionlpFormat ,
                                   :BionlpFormats ,
                                   [ rdf:type owl:Restriction ;
                                     owl:onProperty :documentationUrl ;
                                     owl:hasValue "https://builds.openminted.eu/job/WP%205.2%20-%20Typesystem%20alignment/eu.openminted.interop$mapping-conversion/doclinks/1/components.html#_bionlp_st_2013_a1_a2_1"
                                   ] ;
                   rdfs:comment "Format used in BioNLP Shared Task 2013"@en ;
                   rdfs:label "BioNLP-ST 2013 a1/a2"@en ;
                   <http://www.w3.org/2004/02/skos/core#altLabel> "bioNLP; format-variant=ST2013a1_a2"@en .


###  http://w3id.org/meta-share/omtd-share/Blikiwikipedia
:Blikiwikipedia rdf:type owl:Class ;
                rdfs:subClassOf :WikipediaFormat ,
                                [ rdf:type owl:Restriction ;
                                  owl:onProperty :documentationUrl ;
                                  owl:hasValue "https://dkpro.github.io/dkpro-core/releases/1.8.0/docs/format-reference.html#format-de.tudarmstadt.ukp.dkpro.core.io.bliki-asl"
                                ] ;
                rdfs:comment "The Java Wikipedia API (Bliki engine) is a parser library for converting Wikipedia wikitext notation to HTML."@en ;
                rdfs:label "blikiWikipedia"@en .


###  http://w3id.org/meta-share/omtd-share/BncFormat
:BncFormat rdf:type owl:Class ;
           rdfs:subClassOf :CorpusFormat ,
                           :Xml ,
                           [ rdf:type owl:Restriction ;
                             owl:onProperty :hasMimetype ;
                             owl:hasValue :application_xml
                           ] ,
                           [ rdf:type owl:Restriction ;
                             owl:onProperty :documentationUrl ;
                             owl:hasValue "https://dkpro.github.io/dkpro-core/releases/1.8.0/docs/format-reference.html#format-de.tudarmstadt.ukp.dkpro.core.io.bnc-asl"
                           ] ;
           rdfs:comment "Data format for the XML version of the British National Corpus (http://www.natcorp.ox.ac.uk/)"@en ;
           rdfs:label "BNC format"@en .


###  http://w3id.org/meta-share/omtd-share/BotDetection
:BotDetection rdf:type owl:Class ;
              rdfs:subClassOf :InformationExtraction ;
              rdfs:comment "The task/process of identifying segments of text or speech discourse that have been uttered by bots"@en ;
              rdfs:label "Bot detection"@en .


###  http://w3id.org/meta-share/omtd-share/BrainRegion
:BrainRegion rdf:type owl:Class ;
             rdfs:subClassOf :BiologicalEnity ,
                             :NamedEntity ;
             rdfs:comment "Part of the brain"@en ;
             rdfs:label "Brain region"@en .


###  http://w3id.org/meta-share/omtd-share/Brat
:Brat rdf:type owl:Class ;
      rdfs:subClassOf :AnnotationFormat ,
                      [ rdf:type owl:Restriction ;
                        owl:onProperty :hasMimetype ;
                        owl:hasValue :text_x_brat
                      ] ,
                      [ rdf:type owl:Restriction ;
                        owl:onProperty :documentationUrl ;
                        owl:hasValue "http://brat.nlplab.org/standoff.html"
                      ] ,
                      [ rdf:type owl:Restriction ;
                        owl:onProperty :documentationUrl ;
                        owl:hasValue "https://dkpro.github.io/dkpro-core/releases/1.8.0/docs/format-reference.html#format-de.tudarmstadt.ukp.dkpro.core.io.brat-asl"
                      ] ;
      rdfs:comment "BRAT stand-off format for annotations (BRAT is a online environment for collaborative text annotation, cf. http://brat.nlplab.org/)"@en ;
      rdfs:label "BRAT"@en .


###  http://w3id.org/meta-share/omtd-share/BuildingOfFiniteStateAutomata
:BuildingOfFiniteStateAutomata rdf:type owl:Class ;
                               rdfs:subClassOf :SupportOperation ;
                               rdfs:comment "The task/process of creating Finite State Automata (a mathematical model of computation)"@en ;
                               rdfs:label "Building of finite state automata"@en ;
                               <http://www.w3.org/2004/02/skos/core#related> :FiniteStateTechnology .


###  http://w3id.org/meta-share/omtd-share/Cadixe_json
:Cadixe_json rdf:type owl:Class ;
             rdfs:subClassOf :AnnotationFormat ,
                             :Json ,
                             [ rdf:type owl:Restriction ;
                               owl:onProperty :hasMimetype ;
                               owl:hasValue :application_json
                             ] ,
                             [ rdf:type owl:Restriction ;
                               owl:onProperty :documentationUrl ;
                               owl:hasValue "https://builds.openminted.eu/job/WP%205.2%20-%20Typesystem%20alignment/eu.openminted.interop$mapping-conversion/doclinks/1/components.html#ExportCadixeJSON"
                             ] ;
             rdfs:comment "AlvisAE protocol format"@en ;
             rdfs:label "Cadixe/JSON"@en .


###  http://w3id.org/meta-share/omtd-share/CertaintyLevel
:CertaintyLevel rdf:type owl:Class ;
                rdfs:subClassOf :SemanticAnnotationType ;
                rdfs:comment "Degree of certainty about the validity of what is being asserted in the text"@en ;
                rdfs:label "Certainty level"@en .


###  http://w3id.org/meta-share/omtd-share/CertaintyLevelLabelling
:CertaintyLevelLabelling rdf:type owl:Class ;
                         rdfs:subClassOf :SemanticAnnotation ;
                         rdfs:comment "The task/process of adding to statements in a text annotations that indicate the level of certainty of the author vis-a-vis the statement"@en ;
                         rdfs:label "Certainty level labelling"@en ;
                         <http://www.w3.org/2004/02/skos/core#altLabel> "Certainty level labeling [en-US]"@en-us .


###  http://w3id.org/meta-share/omtd-share/Chat
:Chat rdf:type owl:Class ;
      rdfs:subClassOf :AnnotationFormat ,
                      [ rdf:type owl:Restriction ;
                        owl:onProperty :documentationUrl ;
                        owl:hasValue "http://talkbank.org/manuals/CHAT.pdf"
                      ] ;
      rdfs:comment "CHAT (Codes for the Human Analysis of Transcripts) transcription format; used by CHILDES corpora"@en ;
      rdfs:label "CHAT"@en ;
      <http://www.w3.org/2004/02/skos/core#altLabel> "Codes for the Human Analysis of Transcripts"@en .


###  http://w3id.org/meta-share/omtd-share/Chemical
:Chemical rdf:type owl:Class ;
          rdfs:subClassOf :BiologicalEnity ,
                          :NamedEntity ;
          rdfs:comment "Any substance (as an acid) that is formed when two or more other substances act upon one another or that is used to produce a change in another substance [https://www.merriam-webster.com/dictionary/chemical]"@en ;
          rdfs:label "Chemical"@en .


###  http://w3id.org/meta-share/omtd-share/ChemicalEntity
:ChemicalEntity rdf:type owl:Class ;
                rdfs:subClassOf :Domain-specificAnnotation ,
                                :DomainSpecificAnnotationType ;
                rdfs:comment "Any kind of annotation pertaining to entities from chemistry"@en ;
                rdfs:label "Chemical entity"@en .


###  http://w3id.org/meta-share/omtd-share/Chunk
:Chunk rdf:type owl:Class ;
       rdfs:subClassOf :SyntacticAnnotationType ,
                       [ rdf:type owl:Restriction ;
                         owl:onProperty :documentationUrl ;
                         owl:hasValue "http://dkpro.github.io/dkpro-core/releases/1.8.0/docs/typesystem-reference.html#de.tudarmstadt.ukp.dkpro.core.api.syntax.type.chunk.Chunk"
                       ] ;
       rdfs:comment "Group of words that function together; a chunk normally includes a head and some consecutive (i.e. without gaps) preceding words"@en ;
       rdfs:label "Chunk"@en .


###  http://w3id.org/meta-share/omtd-share/Chunker
:Chunker rdf:type owl:Class ;
         rdfs:subClassOf :Annotator ;
         rdfs:comment "A component that groups tokens of a text into chunks"@en ;
         rdfs:label "Chunker"@en .


###  http://w3id.org/meta-share/omtd-share/Chunking
:Chunking rdf:type owl:Class ;
          rdfs:subClassOf :Parsing ;
          rdfs:comment "The task/process of dividing a sentence into chunks (non-overlapping text segments consisting of a head and preceding function words and/or modifiers)"@en ;
          rdfs:label "Chunking"@en ;
          <http://www.w3.org/2004/02/skos/core#altLabel> "Light parsing"@en ,
                                                         "Shallow Parsing"@en ;
          <http://www.w3.org/2004/02/skos/core#definition> "Shallow parsing refers to a class of techniques for identifying phrasal chunks in texts without assigning deep hierarchical structures. Cascaded finite-state models are often used for shallow parsing. Shallow parsing techniques are used because they are more time-efficient and more error-tolerant than \"\"deep\"\" parsers, and give rise to fewer ambiguities."@en .


###  http://w3id.org/meta-share/omtd-share/Citation
:Citation rdf:type owl:Class ;
          rdfs:subClassOf :ScholarlyAnalyticsEntity ,
                          :ScholarlyCommunicationAnnotation ;
          rdfs:comment "Reference to a book, paper, or author, especially in a scholarly work."@en ;
          rdfs:label "Citation"@en .


###  http://w3id.org/meta-share/omtd-share/Clause
:Clause rdf:type owl:Class ;
        rdfs:subClassOf :StructuralAnnotationType ,
                        [ rdf:type owl:Restriction ;
                          owl:onProperty owl:equivalentClass ;
                          owl:someValuesFrom <http://purl.org/olia/olia-top.owl#Clause>
                        ] ;
        rdfs:comment "A clause is a subdivision of a sentence containing a subject (argument) and predicate. It is possible to have a word that implies or refers to a predicate rather than one explicitly stated. [Pei & Gaynor 1980: 40, http://linguistics-ontology.org/gold/2010/Clause]"@en ;
        rdfs:label "Clause"@en .


###  http://w3id.org/meta-share/omtd-share/ClusteringMethod
:ClusteringMethod rdf:type owl:Class ;
                  rdfs:subClassOf :MachineAndStatisticalLearningMethod ;
                  <http://purl.org/dc/elements/1.1/source> "adapted from wikipedia (https://en.wikipedia.org/wiki/Cluster_analysis)"@en ;
                  rdfs:comment "Any method used in clustering or cluster analysis, i.e. in grouping a set of objects in such a way that objects in the same group (cluster) are more similar (in some sense or another) to each other than to those in other groups (clusters)."@en ;
                  rdfs:label "Clustering Method"@en ;
                  <http://www.w3.org/2004/02/skos/core#example> "k-means, k-nearest neighbours"@en .


###  http://w3id.org/meta-share/omtd-share/CoReferenceAnnotator
:CoReferenceAnnotator rdf:type owl:Class ;
                      rdfs:subClassOf :Annotator ;
                      rdfs:comment "A component that annotates tokens of a text with coreference labels, marking expressions that refer to the same entity in the text"@en ;
                      rdfs:label "Co-reference annotator"@en .


###  http://w3id.org/meta-share/omtd-share/CoReferenceResolution
:CoReferenceResolution rdf:type owl:Class ;
                       rdfs:subClassOf :LinguisticAnalysis ;
                       rdfs:comment "The process/task of determining all linguistic expressions that refer to the same entity in a certain text or across texts."@en ,
                                    "The process/task of identifying all linguistic expressions that appear in a certain text or across texts and refer to the same unique entity in the world"@en ;
                       rdfs:label "Co-reference resolution"@en ;
                       <http://www.w3.org/2004/02/skos/core#altLabel> "Coreference resolution"@en ;
                       <http://www.w3.org/2004/02/skos/core#related> :AnaphoraResolution .


###  http://w3id.org/meta-share/omtd-share/Cochrane
:Cochrane rdf:type owl:Class ;
          rdfs:subClassOf :DocumentFormat ,
                          [ rdf:type owl:Restriction ;
                            owl:onProperty :hasMimetype ;
                            owl:hasValue :text_xCochrane
                          ] ,
                          [ rdf:type owl:Restriction ;
                            owl:onProperty :documentationUrl ;
                            owl:hasValue "https://gate.ac.uk/sale/tao/splitch23.html#sec:creole:pubmed"
                          ] ;
          rdfs:comment "Format used in Cochrane texts"@en ;
          rdfs:label "Cochrane"@en .


###  http://w3id.org/meta-share/omtd-share/CommentFiltering
:CommentFiltering rdf:type owl:Class ;
                  rdfs:subClassOf :SupportOperation ;
                  rdfs:comment "The identification and removal of abusive, bullying, etc. comments from texts"@en ;
                  rdfs:label "Comment filtering"@en .


###  http://w3id.org/meta-share/omtd-share/ComponentType
:ComponentType rdf:type owl:Class ;
               rdfs:subClassOf owl:Thing ;
               rdfs:comment "Specifies the type of a component, in terms of the function/task it performs"@en ;
               rdfs:label "Component type"@en .


###  http://w3id.org/meta-share/omtd-share/Compound
:Compound rdf:type owl:Class ;
          rdfs:subClassOf :MorphologicalAnnotationType ,
                          [ rdf:type owl:Restriction ;
                            owl:onProperty :documentationUrl ;
                            owl:hasValue "http://dkpro.github.io/dkpro-core/releases/1.8.0/docs/typesystem-reference.html#de.tudarmstadt.ukp.dkpro.core.api.segmentation.type.Compound"
                          ] ;
          rdfs:comment "A single word composed of two or more free morphemes"@en ;
          rdfs:label "Compound"@en .


###  http://w3id.org/meta-share/omtd-share/ComputationalArgumentation
:ComputationalArgumentation rdf:type owl:Class ;
                            rdfs:subClassOf :InformationExtraction ;
                            rdfs:comment "The process/task of identifying and representing argumentation in text, so that systems have the ability to use them in tasks, such as automated logical reasoning"@en ;
                            rdfs:label "Computational argumentation"@en .


###  http://w3id.org/meta-share/omtd-share/ComputerAidedTranslation
:ComputerAidedTranslation rdf:type owl:Class ;
                          rdfs:subClassOf :MachineTranslation ;
                          rdfs:comment "A form of translation performed by a human translator with the aid of software programmes"@en ;
                          rdfs:label "Computer-aided translation"@en ;
                          <http://www.w3.org/2004/02/skos/core#altLabel> "CAT"@en ,
                                                                         "Computer-assisted translation"@en ,
                                                                         "MAHT"@en ,
                                                                         "Machine-aided human translation"@en ;
                          <http://www.w3.org/2004/02/skos/core#definition> "Techniques that help to increase the productivity of human translators via suitable computational infrastructure, including translation memories, terminology management, partial machine translation, online lexicons, or other techniques that automate parts of the translator's work, such as speech recognition or accelerated typing techniques applied to human translations."@en .


###  http://w3id.org/meta-share/omtd-share/ConceptNormalization
:ConceptNormalization rdf:type owl:Class ;
                      rdfs:subClassOf :Normalization ;
                      rdfs:comment "The task of mapping free-form expressions to the concepts of a specific domain"@en ;
                      rdfs:label "Concept normalization"@en ;
                      <http://www.w3.org/2004/02/skos/core#altLabel> "Concept normalisation"@en-uk .


###  http://w3id.org/meta-share/omtd-share/Conjugation
:Conjugation rdf:type owl:Class ;
             rdfs:subClassOf :NaturalLanguageGeneration ;
             rdfs:comment "The act of generating (listing in a prescribed order) the various inflectional forms of a word"@en ;
             rdfs:label "Conjugation"@en .


###  http://w3id.org/meta-share/omtd-share/Conll2000
:Conll2000 rdf:type owl:Class ;
           rdfs:subClassOf :ConllFormat ,
                           [ rdf:type owl:Restriction ;
                             owl:onProperty :hasMimetype ;
                             owl:hasValue :text_x_org_dkpro_conll2000
                           ] ,
                           [ rdf:type owl:Restriction ;
                             owl:onProperty :documentationUrl ;
                             owl:hasValue "https://dkpro.github.io/dkpro-core/releases/1.8.0/docs/format-reference.html#format-Conll2000"
                           ] ;
           rdfs:comment "The CoNLL 2000 format represents POS and Chunk tags. Fields in a line are separated by spaces. Sentences are separated by a blank new line."@en ;
           rdfs:label "CoNLL-2000"@en .


###  http://w3id.org/meta-share/omtd-share/Conll2002
:Conll2002 rdf:type owl:Class ;
           rdfs:subClassOf :ConllFormat ,
                           [ rdf:type owl:Restriction ;
                             owl:onProperty :hasMimetype ;
                             owl:hasValue :text_x_org_dkpro_conll2002
                           ] ,
                           [ rdf:type owl:Restriction ;
                             owl:onProperty :documentationUrl ;
                             owl:hasValue "https://dkpro.github.io/dkpro-core/releases/1.8.0/docs/format-reference.html#format-Conll2002"
                           ] ;
           rdfs:comment "The CoNLL 2002 format encodes named entity spans. Fields are separated by a single space. Sentences are separated by a blank new line."@en ;
           rdfs:label "CoNLL-2002"@en .


###  http://w3id.org/meta-share/omtd-share/Conll2003
:Conll2003 rdf:type owl:Class ;
           rdfs:subClassOf :ConllFormat ,
                           [ rdf:type owl:Restriction ;
                             owl:onProperty :hasMimetype ;
                             owl:hasValue :text_x_org_dkpro_conll2003
                           ] ,
                           [ rdf:type owl:Restriction ;
                             owl:onProperty :documentationUrl ;
                             owl:hasValue "https://zoidberg.ukp.informatik.tu-darmstadt.de/jenkins/job/DKPro%20Core%20Documentation%20(GitHub)/de.tudarmstadt.ukp.dkpro.core$de.tudarmstadt.ukp.dkpro.core.doc-asl/doclinks/5/format-reference.html#format-Conll2003"
                           ] ;
           rdfs:comment "The CoNLL 2004 format encodes named entity spans and chunk spans. Fields are separated by a single space. Sentences are separated by a blank new line. Named entities and chunks are encoded in the IOB1 format. I.e. a B prefix is only used if the category of the following span differs from the category of the current span."@en ;
           rdfs:label "CoNLL-2003"@en .


###  http://w3id.org/meta-share/omtd-share/Conll2006
:Conll2006 rdf:type owl:Class ;
           rdfs:subClassOf :ConllFormat ,
                           [ rdf:type owl:Restriction ;
                             owl:onProperty :hasMimetype ;
                             owl:hasValue :text_x_org_dkpro_conll2006
                           ] ,
                           [ rdf:type owl:Restriction ;
                             owl:onProperty :documentationUrl ;
                             owl:hasValue "https://dkpro.github.io/dkpro-core/releases/1.8.0/docs/format-reference.html#format-Conll2006"
                           ] ;
           rdfs:comment "The CoNLL 2006 (aka CoNLL-X) format targets dependency parsing. Columns are tab-separated. Sentences are separated by a blank new line."@en ;
           rdfs:label "CoNLL-2006"@en ;
           <http://www.w3.org/2004/02/skos/core#altLabel> "CoNLL-2007"@en ,
                                                          "CoNLL-X"@en .


###  http://w3id.org/meta-share/omtd-share/Conll2008
:Conll2008 rdf:type owl:Class ;
           rdfs:subClassOf :ConllFormat ,
                           [ rdf:type owl:Restriction ;
                             owl:onProperty :hasMimetype ;
                             owl:hasValue :text_x_org_dkpro_conll2008
                           ] ,
                           [ rdf:type owl:Restriction ;
                             owl:onProperty :documentationUrl ;
                             owl:hasValue "https://zoidberg.ukp.informatik.tu-darmstadt.de/jenkins/job/DKPro%20Core%20Documentation%20(GitHub)/de.tudarmstadt.ukp.dkpro.core$de.tudarmstadt.ukp.dkpro.core.doc-asl/doclinks/5/format-reference.html#format-Conll2008"
                           ] ;
           rdfs:comment "The CoNLL 2008 format targets syntactic and semantic dependencies. Columns are tab-separated. Sentences are separated by a blank new line."@en ;
           rdfs:label "CoNLL-2008"@en .


###  http://w3id.org/meta-share/omtd-share/Conll2009
:Conll2009 rdf:type owl:Class ;
           rdfs:subClassOf :ConllFormat ,
                           [ rdf:type owl:Restriction ;
                             owl:onProperty :hasMimetype ;
                             owl:hasValue :text_x_org_dkpro_conll2009
                           ] ,
                           [ rdf:type owl:Restriction ;
                             owl:onProperty :documentationUrl ;
                             owl:hasValue "https://dkpro.github.io/dkpro-core/releases/1.8.0/docs/format-reference.html#format-Conll2009"
                           ] ;
           rdfs:comment "The CoNLL 2009 format targets semantic role labeling. Columns are tab-separated. Sentences are separated by a blank new line."@en ;
           rdfs:label "CoNLL-2009"@en .


###  http://w3id.org/meta-share/omtd-share/Conll2012
:Conll2012 rdf:type owl:Class ;
           rdfs:subClassOf :ConllFormat ,
                           [ rdf:type owl:Restriction ;
                             owl:onProperty :hasMimetype ;
                             owl:hasValue :text_x_org_dkpro_conll2012
                           ] ,
                           [ rdf:type owl:Restriction ;
                             owl:onProperty :documentationUrl ;
                             owl:hasValue "https://dkpro.github.io/dkpro-core/releases/1.8.0/docs/format-reference.html#format-Conll2012"
                           ] ;
           rdfs:comment "The CoNLL 2012 format targets semantic role labeling and coreference. Columns are tab-separated. Sentences are separated by a blank new line."@en ;
           rdfs:label "CoNLL-2012"@en .


###  http://w3id.org/meta-share/omtd-share/ConllFormat
:ConllFormat rdf:type owl:Class ;
             rdfs:subClassOf :AnnotationFormat ,
                             :TabularFormat ;
             rdfs:comment "Formats used in the CoNLL Shared Tasks"@en ;
             rdfs:label "CoNLL format"@en .


###  http://w3id.org/meta-share/omtd-share/ConllU
:ConllU rdf:type owl:Class ;
        rdfs:subClassOf :ConllFormat ,
                        [ rdf:type owl:Restriction ;
                          owl:onProperty :hasMimetype ;
                          owl:hasValue :text_x_org_dkpro_conllU
                        ] ,
                        [ rdf:type owl:Restriction ;
                          owl:onProperty :documentationUrl ;
                          owl:hasValue "http://universaldependencies.org/docs/format.html"
                        ] ;
        rdfs:comment "Format used for CoNLL."@en ;
        rdfs:label "CoNLL-U"@en .


###  http://w3id.org/meta-share/omtd-share/ConstituencyParser
:ConstituencyParser rdf:type owl:Class ;
                    rdfs:subClassOf :Parser ,
                                    [ rdf:type owl:Restriction ;
                                      owl:onProperty :performsOperation ;
                                      owl:someValuesFrom :ConstituencyParsing
                                    ] ;
                    rdfs:comment "A component that builds a constituency tree from typically token and part-of-speech annotations"@en ;
                    rdfs:label "Constituency parser"@en .


###  http://w3id.org/meta-share/omtd-share/ConstituencyParsing
:ConstituencyParsing rdf:type owl:Class ;
                     rdfs:subClassOf :Parsing ;
                     rdfs:comment "The task/process of identifying and marking constituents (phrases, governed by a head and including function words and/or modifiers ) in a text or text segment"@en ;
                     rdfs:label "Constituency parsing"@en ;
                     <http://www.w3.org/2004/02/skos/core#altLabel> "Natural Language Parsing"@en ,
                                                                    "Phrase parsing"@en ;
                     <http://www.w3.org/2004/02/skos/core#definition> "Parsing (from Latin \"\"pars orationis\"\" = parts of speech) is the syntactic analysis of languages. Natural Language Parsing is the syntactic analysis of natural languages, such as Finnish or Chinese. The objective of Natural Language Parsing is to determine parts of sentences (such as verbs, noun phrases, or relative clauses), and the relationships between them (such as subject or object). Unlike parsing of formally defined artificial languages (such as Java or predicate logic), parsing of natural languages presents problems due to ambiguity, and the productive and creative use of language."@en .


###  http://w3id.org/meta-share/omtd-share/ConstituencyTree
:ConstituencyTree rdf:type owl:Class ;
                  rdfs:subClassOf :SyntacticAnnotationType ;
                  rdfs:comment "An ordered, rooted tree that represents the syntactic structure of a string according to a constituency grammar (= phrase structure grammars). It distinguishes between terminal and non-terminal nodes. The interior nodes are labeled by non-terminal categories of the grammar (phrases), while the leaf nodes are labeled by terminal categories (parts of speech). [adapted from https://en.wikipedia.org/wiki/Parse_tree]"@en ;
                  rdfs:label "Constituency tree"@en .


###  http://w3id.org/meta-share/omtd-share/Constituent
:Constituent rdf:type owl:Class ;
             rdfs:subClassOf :SyntacticAnnotationType ,
                             [ rdf:type owl:Restriction ;
                               owl:onProperty owl:equivalentClass ;
                               owl:someValuesFrom <http://purl.org/olia/olia-top.owl#Constituent>
                             ] ,
                             [ rdf:type owl:Restriction ;
                               owl:onProperty owl:equivalentClass ;
                               owl:someValuesFrom <http://vocab.lappsgrid.org/Constituent>
                             ] ,
                             [ rdf:type owl:Restriction ;
                               owl:onProperty :documentationUrl ;
                               owl:hasValue "http://dkpro.github.io/dkpro-core/releases/1.8.0/docs/typesystem-reference.html#de.tudarmstadt.ukp.dkpro.core.api.syntax.type.constituent.Constituent"
                             ] ;
             rdfs:comment "A word or group of words that function as a single unit in a syntactic structure"@en ;
             rdfs:label "Constituent"@en .


###  http://w3id.org/meta-share/omtd-share/ContentMining
:ContentMining rdf:type owl:Class ;
               rdfs:subClassOf :Operation ,
                               [ rdf:type owl:Restriction ;
                                 owl:onProperty <http://www.w3.org/2004/02/skos/core#closeMatch> ;
                                 owl:someValuesFrom :TextAndDataMining
                               ] ;
               rdfs:comment "The automated analysis of large volumes of content of any form or medium (e.g. text, images, videos, graphs, metadata etc.) that leads to the discovery of previously undiscovered information (e.g. identification of relationships between entities)."@en ;
               rdfs:label "Content Mining"@en ;
               <http://www.w3.org/2004/02/skos/core#related> :TextAndDataMining .


###  http://w3id.org/meta-share/omtd-share/Contradiction
:Contradiction rdf:type owl:Class ;
               rdfs:subClassOf :DiscourseAnnotationType ;
               rdfs:comment "A set of statements that contradict each other (i.e. one of them asserts the truth and the other the falsity of the proposition)"@en ;
               rdfs:label "Contradiction"@en .


###  http://w3id.org/meta-share/omtd-share/ContradictionDetection
:ContradictionDetection rdf:type owl:Class ;
                        rdfs:subClassOf :InformationExtraction ;
                        rdfs:comment "The task/process of identifying conflicting statements (contradictions) in a dataset"@en ;
                        rdfs:label "Contradiction detection"@en .


###  http://w3id.org/meta-share/omtd-share/ContradictionDetector
:ContradictionDetector rdf:type owl:Class ;
                       rdfs:subClassOf :Analyzer ,
                                       [ rdf:type owl:Restriction ;
                                         owl:onProperty :performsOperation ;
                                         owl:someValuesFrom :ContradictionDetection
                                       ] ;
                       rdfs:comment "A component that tries to automatically recognize elements that reveal contradiction in a text"@en ;
                       rdfs:label "Contradiction detector"@en ;
                       <http://www.w3.org/2004/02/skos/core#comment> "could also be an annotator"@en .


###  http://w3id.org/meta-share/omtd-share/ConversationalSystemsBuilding
:ConversationalSystemsBuilding rdf:type owl:Class ;
                               rdfs:subClassOf :OperationWithMultimediaInputOrOutput ;
                               rdfs:altLabel "Chatbots building"@en ,
                                             "Conversational agents building"@en ,
                                             "Dialogue systems building"@en ,
                                             "Embodied agents building"@en ,
                                             "Virtual agents building"@en ;
                               rdfs:comment "All activities related to the creation of conversational/dialogue systems (i.e. computer systems intended to converse with humans, through one or more communication modalities, such as text, speech, graphics, haptics, gestures)"@en ;
                               rdfs:label "Conversational systems building"@en ;
                               <http://www.w3.org/2004/02/skos/core#comment> "I have put all terms together as alternative labels, but maybe they should be distinguished at a later stage"@en .


###  http://w3id.org/meta-share/omtd-share/Converter
:Converter rdf:type owl:Class ;
           rdfs:subClassOf :SupportComponent ,
                           [ rdf:type owl:Restriction ;
                             owl:onProperty :performsOperation ;
                             owl:someValuesFrom :FormatConversion
                           ] ;
           rdfs:comment "A component that performs conversion between formats of a resource"@en ;
           rdfs:label "Converter"@en .


###  http://w3id.org/meta-share/omtd-share/Coreference
:Coreference rdf:type owl:Class ;
             rdfs:subClassOf :DiscourseAnnotationType ,
                             [ rdf:type owl:Restriction ;
                               owl:onProperty owl:equivalentClass ;
                               owl:someValuesFrom <http://vocab.lappsgrid.org/Coreference>
                             ] ;
             rdfs:comment "Coreference is the reference in one expression to the same referent in another expression. [http://www.glossary.sil.org/term/coreference]"@en ;
             rdfs:label "Coreference"@en ;
             <http://www.w3.org/2004/02/skos/core#altLabel> "Co-reference"@en ;
             <http://www.w3.org/2004/02/skos/core#comment> "As defined here it refers more to the phenomenon than the actual annotation types; referent and co-referent might be more appropriate"@en .


###  http://w3id.org/meta-share/omtd-share/CoreferenceAnnotation
:CoreferenceAnnotation rdf:type owl:Class ;
                       rdfs:subClassOf :DiscourseAnnotation ;
                       rdfs:comment "The task/process of attaching tags to a text unit and linking it to other text units that refer to the same entity in the world"@en ;
                       rdfs:label "Coreference annotation"@en ;
                       <http://www.w3.org/2004/02/skos/core#altLabel> "Co-reference annotation"@en ,
                                                                      "Coreference identification"@en ;
                       <http://www.w3.org/2004/02/skos/core#related> :AnaphoraAnnotation .


###  http://w3id.org/meta-share/omtd-share/CorpusFormat
:CorpusFormat rdf:type owl:Class ;
              rdfs:subClassOf :DataFormat ;
              rdfs:comment "A format used by a specific type of corpus (collection of texts)"@en ;
              rdfs:label "Corpus format"@en .


###  http://w3id.org/meta-share/omtd-share/CorpusManagement
:CorpusManagement rdf:type owl:Class ;
                  rdfs:subClassOf :SupportOperation ;
                  rdfs:comment "The task/process of managing corpora, e.g. creating, viewing, etc. through an integrated environment"@en ;
                  rdfs:label "Corpus management"@en .


###  http://w3id.org/meta-share/omtd-share/CorpusViewer
:CorpusViewer rdf:type owl:Class ;
              rdfs:subClassOf :Viewer ,
                              [ rdf:type owl:Restriction ;
                                owl:onProperty :performsOperation ;
                                owl:someValuesFrom :CorpusViewing
                              ] ;
              rdfs:comment "A component that supports humans in accessing the contents of a corpus"@en ;
              rdfs:label "Corpus viewer"@en .


###  http://w3id.org/meta-share/omtd-share/CorpusViewing
:CorpusViewing rdf:type owl:Class ;
               rdfs:subClassOf :Viewing ;
               rdfs:comment "The task/process of viewing the contents of a corpus as performed by human beings"@en ;
               rdfs:label "Corpus viewing"@en .


###  http://w3id.org/meta-share/omtd-share/Crawler
:Crawler rdf:type owl:Class ;
         rdfs:subClassOf :DataCollector ,
                         [ rdf:type owl:Restriction ;
                           owl:onProperty :performsOperation ;
                           owl:someValuesFrom :Crawling
                         ] ;
         rdfs:comment "A component that crawls the web and collects data from various web sites"@en ;
         rdfs:label "Crawler"@en .


###  http://w3id.org/meta-share/omtd-share/Crawling
:Crawling rdf:type owl:Class ;
          rdfs:subClassOf :DataCollection ;
          rdfs:comment "The use of bots that crawl the web (crawlers) in order to spot content that matches user-set criteria and download them to create large datasets"@en ;
          rdfs:label "Web crawling"@en ;
          <http://www.w3.org/2004/02/skos/core#altLabel> "Crawling"@en ,
                                                         "Web Crawling and Spidering"@en ;
          <http://www.w3.org/2004/02/skos/core#definition> "" .


###  http://w3id.org/meta-share/omtd-share/CrossLingualSearch
:CrossLingualSearch rdf:type owl:Class ;
                    rdfs:subClassOf :InformationRetrieval ;
                    rdfs:comment "The ability of a system to retrieve relevant documents in various languages in response to a user query that is formulated in only one language"@en ;
                    rdfs:label "Cross-language Information Retrieval"@en ;
                    <http://www.w3.org/2004/02/skos/core#altLabel> "CLIR"@en ,
                                                                   "Cross-lingual information retrieval"@en ,
                                                                   "Cross-lingual search"@en ,
                                                                   "Translingual information retrieval"@en ;
                    <http://www.w3.org/2004/02/skos/core#definition> "Cross-language information retrieval means using queries in one language to search for documents in a different language. Multilingual information retrieval is a broader term, which includes the case where queries in different languages are used, but only for searching documents in the same language."@en ;
                    <http://www.w3.org/2004/02/skos/core#related> :MultilingualInformationRetrieval .


###  http://w3id.org/meta-share/omtd-share/Crowdsourcing
:Crowdsourcing rdf:type owl:Class ;
               rdfs:subClassOf :TdmMethod ;
               <http://purl.org/dc/elements/1.1/source> <https://www.merriam-webster.com/dictionary/crowdsourcing> ;
               rdfs:comment "The practice of obtaining needed services, ideas, or content by soliciting contributions from a large group of people and especially from the online community rather than from traditional employees or suppliers"@en ;
               rdfs:label "Crowdsourcing"@en .


###  http://w3id.org/meta-share/omtd-share/CrowdsourcingComponent
:CrowdsourcingComponent rdf:type owl:Class ;
                        rdfs:subClassOf :SupportComponent ,
                                        [ rdf:type owl:Restriction ;
                                          owl:onProperty :performsOperation ;
                                          owl:someValuesFrom :SupportOfCrowdsourcingTasks
                                        ] ;
                        rdfs:comment "A component that supports crowdsourcing operations"@en ;
                        rdfs:label "Crowdsourcing component"@en .


###  http://w3id.org/meta-share/omtd-share/Csv
:Csv rdf:type owl:Class ;
     rdfs:subClassOf :TabularFormat ,
                     [ rdf:type owl:Restriction ;
                       owl:onProperty :hasMimetype ;
                       owl:hasValue :text_csv
                     ] ;
     rdfs:comment "Data format with comma-separated values"@en ;
     rdfs:label "CSV"@en ;
     <http://www.w3.org/2004/02/skos/core#altLabel> "Comma-separated values"@en .


###  http://w3id.org/meta-share/omtd-share/DataCollection
:DataCollection rdf:type owl:Class ;
                rdfs:subClassOf :SupportOperation ;
                <http://purl.org/dc/elements/1.1/source> <https://en.wikipedia.org/wiki/Data_collection> ;
                rdfs:comment "The process of gathering and measuring information on targeted variables in an established systematic fashion, which then enables one to answer relevant questions and evaluate outcomes."@en ;
                rdfs:label "Data collection"@en .


###  http://w3id.org/meta-share/omtd-share/DataCollector
:DataCollector rdf:type owl:Class ;
               rdfs:subClassOf :SupportComponent ,
                               [ rdf:type owl:Restriction ;
                                 owl:onProperty :performsOperation ;
                                 owl:someValuesFrom :DataCollection
                               ] ;
               rdfs:comment "A component that collects (retrieves) data from various sources"@en ;
               rdfs:label "Data collector"@en .


###  http://w3id.org/meta-share/omtd-share/DataFormat
:DataFormat rdf:type owl:Class ;
            rdfs:subClassOf owl:Thing ;
            rdfs:comment "The format of a computer file storing data"@en ;
            rdfs:label "Data format"@en ;
            <http://www.w3.org/2004/02/skos/core#altLabel> "Data type"@en ,
                                                           "File format"@en .


###  http://w3id.org/meta-share/omtd-share/DataMasking
:DataMasking rdf:type owl:Class ;
             rdfs:subClassOf :Anonymization ;
             rdfs:comment "The process of hiding original data with modified content (characters or other data) in order to protect data classified as personal identifiable data, or sensitive data [adapted from Wikipedia]"@en ;
             rdfs:label "Data masking"@en .


###  http://w3id.org/meta-share/omtd-share/DataMerger
:DataMerger rdf:type owl:Class ;
            rdfs:subClassOf :SupportComponent ,
                            [ rdf:type owl:Restriction ;
                              owl:onProperty :performsOperation ;
                              owl:someValuesFrom :DataMerging
                            ] ;
            rdfs:comment "A component that supports data merging from various sources"@en ;
            rdfs:label "Data merger"@en .


###  http://w3id.org/meta-share/omtd-share/DataMerging
:DataMerging rdf:type owl:Class ;
             rdfs:subClassOf :SupportOperation ;
             rdfs:comment "The task/process of merging (combining) together data from various sources"@en ;
             rdfs:label "Data merging"@en .


###  http://w3id.org/meta-share/omtd-share/DataSplitter
:DataSplitter rdf:type owl:Class ;
              rdfs:subClassOf :SupportComponent ,
                              [ rdf:type owl:Restriction ;
                                owl:onProperty :performsOperation ;
                                owl:someValuesFrom :DataSplitting
                              ] ;
              rdfs:comment "A component that performs data splitting for cross validation purposes"@en ;
              rdfs:label "Data splitter"@en .


###  http://w3id.org/meta-share/omtd-share/DataSplitting
:DataSplitting rdf:type owl:Class ;
               rdfs:subClassOf :SupportOperation ;
               rdfs:comment "The task/process of splitting (partitioning) available data into parts, usually for cross-validatory purposes, e.g. in order to use one part for training purposes and the other for evaluation."@en ;
               rdfs:label "Data splitting"@en .


###  http://w3id.org/meta-share/omtd-share/DatabaseFormat
:DatabaseFormat rdf:type owl:Class ;
                rdfs:subClassOf :DataFormat ;
                rdfs:comment "Formats used for databases"@en ;
                rdfs:label "Database format"@en .


###  http://w3id.org/meta-share/omtd-share/Datasift_json
:Datasift_json rdf:type owl:Class ;
               rdfs:subClassOf :GateFormat ,
                               :Json ,
                               [ rdf:type owl:Restriction ;
                                 owl:onProperty :hasMimetype ;
                                 owl:hasValue :application_json
                               ] ,
                               [ rdf:type owl:Restriction ;
                                 owl:onProperty :documentationUrl ;
                                 owl:hasValue "https://gate.ac.uk/sale/tao/splitch23.html#x28-59500023.32"
                               ] ;
               rdfs:comment "Common format for social media data from http://datasift.com"@en ;
               rdfs:label "DataSift/JSON"@en .


###  http://w3id.org/meta-share/omtd-share/Date
:Date rdf:type owl:Class ;
      rdfs:subClassOf :NamedEntity ,
                      [ rdf:type owl:Restriction ;
                        owl:onProperty owl:equivalentClass ;
                        owl:someValuesFrom <http://purl.org/olia/olia-top.owl#Date>
                      ] ,
                      [ rdf:type owl:Restriction ;
                        owl:onProperty :documentationUrl ;
                        owl:hasValue "http://dkpro.github.io/dkpro-core/releases/1.8.0/docs/typesystem-reference.html#de.tudarmstadt.ukp.dkpro.core.api.ner.type.Date"
                      ] ;
      rdfs:comment "A text unit that denotes a date, a specific point in time"@en ;
      rdfs:label "Date"@en .


###  http://w3id.org/meta-share/omtd-share/Debugger
:Debugger rdf:type owl:Class ;
          rdfs:subClassOf :SupportComponent ,
                          [ rdf:type owl:Restriction ;
                            owl:onProperty :performsOperation ;
                            owl:someValuesFrom :Debugging
                          ] ;
          rdfs:comment "A component that is used in the debugging process"@en ;
          rdfs:label "Debugger"@en .


###  http://w3id.org/meta-share/omtd-share/Debugging
:Debugging rdf:type owl:Class ;
           rdfs:subClassOf :SupportOperation ;
           rdfs:comment "The task/process of removing errors from a computer programme"@en ;
           rdfs:label "Debugging"@en .


###  http://w3id.org/meta-share/omtd-share/DecisionTrees
:DecisionTrees rdf:type owl:Class ;
               rdfs:subClassOf :MachineAndStatisticalLearningMethod ;
               <http://purl.org/dc/elements/1.1/source> """adapted from  (http://scikit-learn.org/stable/modules/tree.html)
and wikipedia (https://en.wikipedia.org/wiki/Decision_tree)"""@en ;
               rdfs:comment "A non-parametric supervised learning method used for classification and regression. The goal is to create a tree-like graph or model of decisions and their possible consequences by learning simple decision rules inferred from the data features."@en ;
               rdfs:label "Decision Trees"@en .


###  http://w3id.org/meta-share/omtd-share/DeepLearning
:DeepLearning rdf:type owl:Class ;
              rdfs:subClassOf :MachineAndStatisticalLearningMethod ;
              <http://purl.org/dc/elements/1.1/source> "adapted from wikipedia (https://en.wikipedia.org/wiki/Deep_learning)"@en ;
              rdfs:comment "A branch of machine learning based on deep neural networks. A deep neural network (DNN) is an artificial neural network (ANN) with multiple hidden layers of units between the input and output layers."@en ;
              rdfs:label "Deep Learning"@en .


###  http://w3id.org/meta-share/omtd-share/DeepParserPerformanceEvaluation
:DeepParserPerformanceEvaluation rdf:type owl:Class ;
                                 rdfs:subClassOf :Evaluation ;
                                 rdfs:comment "The task/process of measuring the speed and accuracy of deep parsers with respect to a manually parsed test corpus."@en ;
                                 rdfs:label "Deep parser performance evaluation"@en ;
                                 <http://www.w3.org/2004/02/skos/core#definition> "The task of parser evaluation is to measure the speed and accuracy of parsers with respect to a manually parsed test corpus. In the evaluation of so-called deep parsers, which are based on comprehensive linguistic theories, the assignment of the correct semantic analysis plays an important role. Another aspect is the handling and reduction of ambiguities, which is important not only from the linguistic point of view but because it plays a major role in the time and memory requirements of deep parsers. Test data can either be a treebank constructed from naturally occurring data, such as the \"\"Wall Street Corpus\"\", or a \"\"test suite\"\" containing constructed examples which cover all interesting linguistic phenomena. An important issue in deep parser evaluation is the comparison of parsers and grammars based on different linguistic theories."@en .


###  http://w3id.org/meta-share/omtd-share/DeepParsing
:DeepParsing rdf:type owl:Class ;
             rdfs:subClassOf :Parsing ;
             rdfs:comment "The  task/process of building complete parse trees for a sentence [adapted from https://stackoverflow.com/questions/37020577/shallow-parsing-vs-deep-parsing-in-stanford-corenlp-java]"@en ;
             rdfs:label "Deep parsing"@en .


###  http://w3id.org/meta-share/omtd-share/Dependency
:Dependency rdf:type owl:Class ;
            rdfs:subClassOf :SyntacticAnnotationType ,
                            [ rdf:type owl:Restriction ;
                              owl:onProperty owl:equivalentClass ;
                              owl:someValuesFrom <http://vocab.lappsgrid.org/Dependency>
                            ] ,
                            [ rdf:type owl:Restriction ;
                              owl:onProperty :documentationUrl ;
                              owl:hasValue "http://dkpro.github.io/dkpro-core/releases/1.8.0/docs/typesystem-reference.html#de.tudarmstadt.ukp.dkpro.core.api.syntax.type.dependency.Dependency"
                            ] ;
            rdfs:comment "A type of syntactic relation that holds between linguistic units, where we try to recognise the head (governor) and its dependents"@en ;
            rdfs:label "Dependency"@en .


###  http://w3id.org/meta-share/omtd-share/DependencyConversion
:DependencyConversion rdf:type owl:Class ;
                      rdfs:subClassOf :FormatConversion ,
                                      [ rdf:type owl:Restriction ;
                                        owl:onProperty <http://www.w3.org/2004/02/skos/core#relatedTo> ;
                                        owl:someValuesFrom :ConstituencyParsing
                                      ] ,
                                      [ rdf:type owl:Restriction ;
                                        owl:onProperty <http://www.w3.org/2004/02/skos/core#relatedTo> ;
                                        owl:someValuesFrom :DependencyParsing
                                      ] ;
                      rdfs:comment "The task/process of converting constituency structures to dependency trees"@en ;
                      rdfs:label "Dependency conversion"@en .


###  http://w3id.org/meta-share/omtd-share/DependencyConverter
:DependencyConverter rdf:type owl:Class ;
                     rdfs:subClassOf :Converter ,
                                     [ rdf:type owl:Restriction ;
                                       owl:onProperty :performsOperation ;
                                       owl:someValuesFrom :DependencyConversion
                                     ] ;
                     rdfs:comment "A component that converts a constituency tree into a dependency tree"@en ;
                     rdfs:label "Dependency converter"@en .


###  http://w3id.org/meta-share/omtd-share/DependencyParser
:DependencyParser rdf:type owl:Class ;
                  rdfs:subClassOf :Parser ,
                                  [ rdf:type owl:Restriction ;
                                    owl:onProperty :performsOperation ;
                                    owl:someValuesFrom :DependencyParsing
                                  ] ;
                  rdfs:comment "A component that generates a dependency tree from typically token and part-of-speech annotations"@en ;
                  rdfs:label "Dependency parser"@en .


###  http://w3id.org/meta-share/omtd-share/DependencyParsing
:DependencyParsing rdf:type owl:Class ;
                   rdfs:subClassOf :Parsing ;
                   <http://purl.org/dc/elements/1.1/source> "adapted from https://nlp.stanford.edu/software/nndep.shtml"@en ;
                   rdfs:comment "The task/process of identifying and marking the grammatical structure of a sentence, establishing relationships between \"\"head\"\" words and words that modify those heads"@en ;
                   rdfs:label "Dependency parsing"@en .


###  http://w3id.org/meta-share/omtd-share/DependencyTree
:DependencyTree rdf:type owl:Class ;
                rdfs:subClassOf :SyntacticAnnotationType ;
                rdfs:comment "A tree that represents the dependency relations in a sentence, i.e. showing the governor (head) and its dependents with directed links"@en ;
                rdfs:label "Dependency tree"@en .


###  http://w3id.org/meta-share/omtd-share/DerivationalAnalysis
:DerivationalAnalysis rdf:type owl:Class ;
                      rdfs:subClassOf :LinguisticAnalysis ;
                      rdfs:comment "The analysis of a word in order to identify its derivation, i.e. whether and how it has been formed on the basis of another word (e.g. through the use of affixes)"@en ;
                      rdfs:label "Derivational analysis"@en .


###  http://w3id.org/meta-share/omtd-share/DerivationalFeature
:DerivationalFeature rdf:type owl:Class ;
                     rdfs:subClassOf :MorphologicalAnnotationType ;
                     rdfs:comment "Any feature relevant to the derivation process of a word (e.g. marking affixes, their meaning etc.)"@en ;
                     rdfs:label "Derivational feature"@en .


###  http://w3id.org/meta-share/omtd-share/DialogueAct
:DialogueAct rdf:type owl:Class ;
             rdfs:subClassOf :SpeechAct ;
             rdfs:comment "A dialogue act has two main components:  a communicative function and a semantic content.   The semantic content specifies the objects, relations, actions, events, etc. that the dialogue act is about; the communicative function can be viewed as a specification of the way an addressee uses the semantic content to update his or her information state when  he  or  she  understands  the  corresponding  stretch  of dialogue. [http://www.lrec-conf.org/proceedings/lrec2010/pdf/560_Paper.pdf]"@en ;
             rdfs:label "Dialogue act"@en .


###  http://w3id.org/meta-share/omtd-share/DialogueModelling
:DialogueModelling rdf:type owl:Class ;
                   rdfs:subClassOf :LanguageModelling ;
                   rdfs:comment "The task/process of building models of dialogues to be used in dialogue systems"@en ;
                   rdfs:label "Dialogue modelling"@en ;
                   <http://www.w3.org/2004/02/skos/core#altLabel> "Dialog modeling [en-US]"@en-us ;
                   <http://www.w3.org/2004/02/skos/core#definition> "A Dialogue model is a system that simulates the behavior of dialogue participants. This includes formal models that instantiate linguistic theories of dialogue interaction and statistical models of dialogue behaviors."@en .


###  http://w3id.org/meta-share/omtd-share/Diaml
:Diaml rdf:type owl:Class ;
       rdfs:subClassOf :AnnotationFormat ,
                       [ rdf:type owl:Restriction ;
                         owl:onProperty :documentationUrl ;
                         owl:hasValue "https://www.iso.org/standard/51967.html"
                       ] ;
       rdfs:comment "Format following Dialogue Act Markup Language (DiAML) which is defined within the ISO standard 24617-2"@en ;
       rdfs:label "DIAML"@en .


###  http://w3id.org/meta-share/omtd-share/DimensionalityReduction
:DimensionalityReduction rdf:type owl:Class ;
                         rdfs:subClassOf :MachineAndStatisticalLearningMethod ;
                         <http://purl.org/dc/elements/1.1/source> "adapted from Wikipedia (https://en.wikipedia.org/wiki/Dimensionality_reduction)"@en ;
                         rdfs:comment "A method based on reducing the number of random variables under consideration, via obtaining a set of principal variables."@en ;
                         rdfs:label "Dimensionality Reduction"@en .


###  http://w3id.org/meta-share/omtd-share/Disambiguator
:Disambiguator rdf:type owl:Class ;
               rdfs:subClassOf :Analyzer ;
               rdfs:comment "A component that is used to disambiguate between two or more ambiguous items"@en ;
               rdfs:label "Disambiguator"@en .


###  http://w3id.org/meta-share/omtd-share/DiscourceRelation
:DiscourceRelation rdf:type owl:Class ;
                   rdfs:subClassOf :DiscourseAnnotationType ;
                   rdfs:comment "The relation that holds between two segments of discourse; e.g. causal, temporal etc."@en ;
                   rdfs:label "Discource relation"@en .


###  http://w3id.org/meta-share/omtd-share/DiscourseAnalysis
:DiscourseAnalysis rdf:type owl:Class ;
                   rdfs:subClassOf :LinguisticAnalysis ;
                   rdfs:comment "A method of analysing the structure of texts or utterances longer than one sentence, taking into account both their linguistic content and their sociolinguistic context; analysis performed using this method.[OED, https://en.oxforddictionaries.com/definition/discourse_analysis]"@en ;
                   rdfs:label "Discourse analysis"@en .


###  http://w3id.org/meta-share/omtd-share/DiscourseAnnotation
:DiscourseAnnotation rdf:type owl:Class ;
                     rdfs:subClassOf :TextAnnotation ;
                     rdfs:comment "The task/process of adding annotations relevant to discourse, such as discourse structure, discourse markers etc."@en ;
                     rdfs:label "Discourse annotation"@en .


###  http://w3id.org/meta-share/omtd-share/DiscourseAnnotationType
:DiscourseAnnotationType rdf:type owl:Class ;
                         rdfs:subClassOf :AnnotationType ,
                                         [ rdf:type owl:Restriction ;
                                           owl:onProperty owl:equivalentClass ;
                                           owl:someValuesFrom <http://purl.org/olia/olia-top.owl#DiscourseFeature>
                                         ] ;
                         rdfs:comment "Any type of annotation relevant to discourse"@en ;
                         rdfs:label "Discourse annotation type"@en .


###  http://w3id.org/meta-share/omtd-share/DiscourseModelling
:DiscourseModelling rdf:type owl:Class ;
                    rdfs:subClassOf :DiscourseAnnotation ;
                    rdfs:comment "The task/process of building discourse models"@en ;
                    rdfs:label "Discourse modelling"@en ;
                    <http://www.w3.org/2004/02/skos/core#altLabel> "Discourse modeling [en-US]"@en-us ;
                    <http://www.w3.org/2004/02/skos/core#definition> "Discourse modelling describes all aspects of the relations between groups of sentences in monologue (text), dialogue, or multiparty interactions, e.g. text coherence, rhetorical relations, intentional and attentional state, centering, dialogue moves, dialogue acts, argument structures and reference phenomena, to name just a few. Recently, with the growing interest in multimodal discourse processing, discourse models extend their reach beyond the modality speech/language to other modalities like gesture, gaze or haptics, and cover also cross-modal phenomena."@en .


###  http://w3id.org/meta-share/omtd-share/DkproTokenized
:DkproTokenized rdf:type owl:Class ;
                rdfs:subClassOf :AnnotationFormat ,
                                [ rdf:type owl:Restriction ;
                                  owl:onProperty :documentationUrl ;
                                  owl:hasValue "https://dkpro.github.io/dkpro-core/releases/1.8.0/docs/format-reference.html#format-TokenizedText"
                                ] ,
                                [ rdf:type owl:Restriction ;
                                  owl:onProperty :documentationUrl ;
                                  owl:hasValue "https://dkpro.github.io/dkpro-core/releases/1.8.0/docs/format-reference.html#format-de.tudarmstadt.ukp.dkpro.core.io.text-asl"
                                ] ;
                rdfs:comment "DkPro format for tokenized files containing one sentence per line and tokens split by whitespaces."@en ;
                rdfs:label "DKPro tokenized"@en .


###  http://w3id.org/meta-share/omtd-share/DocumentAnnotationType
:DocumentAnnotationType rdf:type owl:Class ;
                        rdfs:subClassOf :AnnotationType ,
                                        [ rdf:type owl:Restriction ;
                                          owl:onProperty owl:equivalentClass ;
                                          owl:someValuesFrom <http://vocab.lappsgrid.org/Document>
                                        ] ;
                        rdfs:comment "Any kind of annotation that is used to describe a document (e.g. identifier, size, location, language etc.)"@en ;
                        rdfs:label "Document annotation type"@en ;
                        <http://www.w3.org/2004/02/skos/core#altLabel> "Document information"@en ,
                                                                       "Document metadata"@en .


###  http://w3id.org/meta-share/omtd-share/DocumentClassifier
:DocumentClassifier rdf:type owl:Class ;
                    rdfs:subClassOf :Analyzer ,
                                    [ rdf:type owl:Restriction ;
                                      owl:onProperty :performsOperation ;
                                      owl:someValuesFrom :TextCategorization
                                    ] ;
                    rdfs:comment "A component that tries to classify a document into one or more categories"@en ;
                    rdfs:label "Document classifier"@en .


###  http://w3id.org/meta-share/omtd-share/DocumentComparison
:DocumentComparison rdf:type owl:Class ;
                    rdfs:subClassOf :SupportOperation ;
                    rdfs:comment "The task/process of comparing different versions of the same document"@en ;
                    rdfs:label "Document comparison"@en .


###  http://w3id.org/meta-share/omtd-share/DocumentFormat
:DocumentFormat rdf:type owl:Class ;
                rdfs:subClassOf :DataFormat ;
                rdfs:comment "Any format used for documents (textual resources)"@en ;
                rdfs:label "Document format"@en .


###  http://w3id.org/meta-share/omtd-share/DocumentImageAnalysis
:DocumentImageAnalysis rdf:type owl:Class ;
                       rdfs:subClassOf :SupportOperation ;
                       rdfs:comment "The processing of images of documents in order to obtain a machine-readable description of the their contents and structure from the pixel data [adapted from https://www.ias.ac.in/article/fulltext/sadh/027/01/0003-0022]"@en ;
                       rdfs:label "Document image analysis"@en ;
                       <http://www.w3.org/2004/02/skos/core#definition> "Document image analysis is the theory and practice of recovering the logical structure of digital images scanned from documents or produced by computer. It includes optical character recognition as one of its subfields, but has more ambitious tasks, both in the breadth (understand diagrams, music scores, images ...), and depth (e.g. the correct interpretation of a scanned mathematical formula)."@en .


###  http://w3id.org/meta-share/omtd-share/DocumentReading
:DocumentReading rdf:type owl:Class ;
                 rdfs:subClassOf :TextToSpeechSynthesis ;
                 rdfs:comment "The task/process of converting the contents of a digital document into speech in order to aid mainly individuals with visual impairments"@en ;
                 rdfs:label "Document reading"@en .


###  http://w3id.org/meta-share/omtd-share/DocumentSection
:DocumentSection rdf:type owl:Class ;
                 rdfs:subClassOf :ScholarlyAnalyticsEntity ,
                                 :ScholarlyCommunicationAnnotation ,
                                 :StructuralAnnotationType ,
                                 [ rdf:type owl:Restriction ;
                                   owl:onProperty :documentationUrl ;
                                   owl:hasValue "http://dkpro.github.io/dkpro-core/releases/1.8.0/docs/typesystem-reference.html#de.tudarmstadt.ukp.dkpro.core.api.segmentation.type.Div"
                                 ] ;
                 rdfs:comment "Any subdivision of a document, e.g. a chapter, abstract, etc."@en ;
                 rdfs:label "Document section"@en .


###  http://w3id.org/meta-share/omtd-share/Domain
:Domain rdf:type owl:Class ;
        rdfs:subClassOf owl:Thing ;
        rdfs:comment "Area of interest or activities"@en ;
        rdfs:label "Domain"@en .


###  http://w3id.org/meta-share/omtd-share/Domain-specificAnnotation
:Domain-specificAnnotation rdf:type owl:Class ;
                           rdfs:subClassOf :AnnotationType ;
                           rdfs:comment "Any kind of annotation that is used for specific domains (e.g. genes and proteins from the biomedical domain, plants from agriculture etc.)"@en ;
                           rdfs:label "Domain-specific annotation type"@en ;
                           owl:deprecated "true"^^xsd:boolean .


###  http://w3id.org/meta-share/omtd-share/DomainSpecificAnnotationType
:DomainSpecificAnnotationType rdf:type owl:Class ;
                              rdfs:subClassOf :AnnotationType ;
                              <http://purl.org/dc/terms/replaces> :DomainSpecificAnnotationType ;
                              rdfs:comment "Any kind of annotation that is used for specific domains (e.g. genes and proteins from the biomedical domain, plants from agriculture etc.)"@en ;
                              rdfs:label "Domain-specific annotation type"@en .


###  http://w3id.org/meta-share/omtd-share/Editing
:Editing rdf:type owl:Class ;
         rdfs:subClassOf :SupportOperation ;
         rdfs:comment "The task/process of changing the contents of a resource"@en ;
         rdfs:label "Editing"@en .


###  http://w3id.org/meta-share/omtd-share/Editor
:Editor rdf:type owl:Class ;
        rdfs:subClassOf :SupportComponent ,
                        [ rdf:type owl:Restriction ;
                          owl:onProperty :performsOperation ;
                          owl:someValuesFrom :Editing
                        ] ;
        rdfs:comment "A component that allows humans to edit the contents of a resource"@en ;
        rdfs:label "Editor"@en .


###  http://w3id.org/meta-share/omtd-share/Emma
:Emma rdf:type owl:Class ;
      rdfs:subClassOf :AnnotationFormat ,
                      :Xml ,
                      [ rdf:type owl:Restriction ;
                        owl:onProperty :hasMimetype ;
                        owl:hasValue :application_emma_xml
                      ] ;
      rdfs:comment "Data format according to the EMMA (Extensible MultiModal Annotation markup language) specifications, cf. https://www.w3.org/TR/2007/CR-emma-20071211/"@en ;
      rdfs:label "EMMA"@en .


###  http://w3id.org/meta-share/omtd-share/Emotion
:Emotion rdf:type owl:Class ;
         rdfs:subClassOf :SemanticAnnotationType ;
         rdfs:comment "An affective state of consciousness in which joy, sorrow, fear, hate, or the like, is experienced, as distinguished from cognitive and volitional states of consciousness [http://www.dictionary.com/browse/emotion]"@en ;
         rdfs:label "Emotion"@en .


###  http://w3id.org/meta-share/omtd-share/EmotionDetection
:EmotionDetection rdf:type owl:Class ;
                  rdfs:subClassOf :InformationExtraction ,
                                  [ rdf:type owl:Restriction ;
                                    owl:onProperty :deployedInDomain ;
                                    owl:someValuesFrom :SocialSciences
                                  ] ;
                  rdfs:label "Emotion recognition"@en ;
                  <http://www.w3.org/2004/02/skos/core#altLabel> "Emotion detection"@en ;
                  <http://www.w3.org/2004/02/skos/core#definition> "The recognition of emotions from text, speech, facial expressions, gestures and/or physiological measures. A key challenge is the appropriate representation of emotional states."@en .


###  http://w3id.org/meta-share/omtd-share/EmotionLabelling
:EmotionLabelling rdf:type owl:Class ;
                  rdfs:subClassOf :InformationExtraction ;
                  rdfs:comment "The process/task of identifying types of feelings (e.g. anger, fear, happiness, sadness, etc.) in the linguistic expression of texts or facial expressions"@en ;
                  rdfs:label "Emotion labelling"@en ;
                  <http://www.w3.org/2004/02/skos/core#altLabel> "Emotion labeling [en-US]"@en-us .


###  http://w3id.org/meta-share/omtd-share/EmotionRecognizer
:EmotionRecognizer rdf:type owl:Class ;
                   rdfs:subClassOf :Analyzer ,
                                   [ rdf:type owl:Restriction ;
                                     owl:onProperty :performsOperation ;
                                     owl:someValuesFrom :EmotionDetection
                                   ] ;
                   rdfs:comment "A component that tries to recognize and annotate emotions (e.g. fear, anger, happiness etc.) from text, video, audio and image"@en ;
                   rdfs:label "Emotion recognizer"@en ;
                   <http://www.w3.org/2004/02/skos/core#altLabel> "Emotion detector"@en ;
                   <http://www.w3.org/2004/02/skos/core#comment> "could also be an annotator"@en .


###  http://w3id.org/meta-share/omtd-share/EnsembleMethod
:EnsembleMethod rdf:type owl:Class ;
                rdfs:subClassOf :MachineAndStatisticalLearningMethod ;
                <http://purl.org/dc/elements/1.1/source> "adapted from Wikipedia (https://en.wikipedia.org/wiki/Ensemble_learning)"@en ;
                rdfs:comment "Any method that uses multiple learning algorithms in an attempt to improve predictive performance not obtainable otherwise with any of the constituent learning algorithms."@en ;
                rdfs:label "Ensemble Method"@en .


###  http://w3id.org/meta-share/omtd-share/EntityLinking
:EntityLinking rdf:type owl:Class ;
               rdfs:subClassOf :SemanticAnnotation ;
               rdfs:comment "The task/process of attaching tags to all the mentions of an entity in a text linking them together with the entity."@en ;
               rdfs:label "Entity linking"@en .


###  http://w3id.org/meta-share/omtd-share/EntityMentionLabelling
:EntityMentionLabelling rdf:type owl:Class ;
                        rdfs:subClassOf :InformationExtraction ;
                        rdfs:label "Entity mention labelling"@en ;
                        <http://www.w3.org/2004/02/skos/core#altLabel> "Entity mention labeling [en-US]"@en-us .


###  http://w3id.org/meta-share/omtd-share/EntityMentionPair
:EntityMentionPair rdf:type owl:Class ;
                   rdfs:subClassOf :Coreference ;
                   rdfs:comment "The pair of an entity and all the mentions of this entity formulated in various ways; used in co-reference resolution"@en ;
                   rdfs:label "Entity-Mention pair"@en .


###  http://w3id.org/meta-share/omtd-share/EntityMentionRecognition
:EntityMentionRecognition rdf:type owl:Class ;
                          rdfs:subClassOf :InformationExtraction ,
                                          [ rdf:type owl:Restriction ;
                                            owl:onProperty <http://www.w3.org/2004/02/skos/core#relatedTo> ;
                                            owl:someValuesFrom :NamedEntityRecognition
                                          ] ;
                          rdfs:comment "The task/process of detecting in a text mentions of a specific class of entities (e.g. biochemical entities, historical persons)"@en ;
                          rdfs:label "Entity mention recognition"@en ;
                          <http://www.w3.org/2004/02/skos/core#altLabel> "Entity mention detection"@en ,
                                                                         "Mention detection"@en ;
                          <http://www.w3.org/2004/02/skos/core#comment> "unclear definition"@en .


###  http://w3id.org/meta-share/omtd-share/Evaluation
:Evaluation rdf:type owl:Class ;
            rdfs:subClassOf :Operation ,
                            :SupportOperation ;
            rdfs:comment "The task/process of assessing the quality of a resource, e.g. based on the contents (for a dataset) or performance (for a tool or service)"@en ;
            rdfs:label "Evaluation"@en .


###  http://w3id.org/meta-share/omtd-share/EvaluationOfBroadCoverageNaturalLanguageParsers
:EvaluationOfBroadCoverageNaturalLanguageParsers rdf:type owl:Class ;
                                                 rdfs:subClassOf :Evaluation ;
                                                 rdfs:comment "The task/process of assessing the quality performance of parsers"@en ;
                                                 rdfs:label "Evaluation of broad-coverage natural language parsers"@en ;
                                                 <http://www.w3.org/2004/02/skos/core#definition> "The taks of parser evaluation is the measure the speed and accuracy of (symbolic or stochastic) parsers with respect to a manually parsed test corpus. Test data can either be a treebank constructed naturally occurring data, such as the \"\"Wall Street Corpus\"\", or a \"\"test suite\"\" containing constructed examples which cover all interesting linguistic phenomena. An important issue in parser evaluation is the comparison of parsers and grammars based on different linguistic theories. Evaluations have focussed on phrase structure or dependency structures."@en .


###  http://w3id.org/meta-share/omtd-share/EvaluationOfMachineTranslationAndTranslationTools
:EvaluationOfMachineTranslationAndTranslationTools rdf:type owl:Class ;
                                                   rdfs:subClassOf :Evaluation ;
                                                   rdfs:comment "The task/process of assessing the quality performance of machine translation tools"@en ;
                                                   rdfs:label "Evaluation of Machine Translation and translation tools"@en ;
                                                   <http://www.w3.org/2004/02/skos/core#altLabel> "Evaluation of MT"@en ,
                                                                                                  "Evaluation of MT Systems"@en ,
                                                                                                  "MT Evaluation"@en ;
                                                   <http://www.w3.org/2004/02/skos/core#definition> "The growing number of MT systems on the market that span a wide range of quality levels has motivated activities towards evaluation standards from national and international organizations. Evaluation of MT systems depends strongly on whether such a system is used for information dissemination, assimilation, or in a conversational context, the types of texts to be translated, whether there is a well-defined and limited application domain and many more factors."@en .


###  http://w3id.org/meta-share/omtd-share/Evaluator
:Evaluator rdf:type owl:Class ;
           rdfs:subClassOf :SupportComponent ,
                           [ rdf:type owl:Restriction ;
                             owl:onProperty :performsOperation ;
                             owl:someValuesFrom :Evaluation
                           ] ;
           rdfs:comment "A component that is used in the evaluation of the performance of a component"@en ;
           rdfs:label "Evaluator"@en .


###  http://w3id.org/meta-share/omtd-share/Event
:Event rdf:type owl:Class ;
       rdfs:subClassOf :SemanticAnnotationType ,
                       [ rdf:type owl:Restriction ;
                         owl:onProperty :documentationUrl ;
                         owl:hasValue "http://dkpro.github.io/dkpro-core/releases/1.8.0/docs/typesystem-reference.html#de.tudarmstadt.ukp.dkpro.core.api.ner.type.Event"
                       ] ;
       rdfs:comment "A thing that happens or takes place, especially one of importance [https://en.oxforddictionaries.com/definition/event]"@en ;
       rdfs:label "Event"@en .


###  http://w3id.org/meta-share/omtd-share/EventDetection
:EventDetection rdf:type owl:Class ;
                rdfs:subClassOf :InformationExtraction ;
                rdfs:comment "The process/task of identifying events in data (text, video, images etc.), usually combined with their classification into types of events and recognition of the event attributes (e.g. time, place, participants and duration)"@en ;
                rdfs:label "Event detection"@en ;
                <http://www.w3.org/2004/02/skos/core#altLabel> "Event extraction"@en .


###  http://w3id.org/meta-share/omtd-share/EventExtractor
:EventExtractor rdf:type owl:Class ;
                rdfs:subClassOf :Analyzer ,
                                [ rdf:type owl:Restriction ;
                                  owl:onProperty :performsOperation ;
                                  owl:someValuesFrom :EventDetection
                                ] ;
                rdfs:comment "A component that tries to extract information related to incidents referred to in a text"@en ;
                rdfs:label "Event extractor"@en ;
                <http://www.w3.org/2004/02/skos/core#comment> "could also be an annotator"@en .


###  http://w3id.org/meta-share/omtd-share/EventLabelling
:EventLabelling rdf:type owl:Class ;
                rdfs:subClassOf :SemanticAnnotation ;
                rdfs:comment "The process/act of marking events and classifying them into types of events in a text"@en ;
                rdfs:label "Event labelling"@en ;
                <http://www.w3.org/2004/02/skos/core#altLabel> "Annotation of events"@en ,
                                                               "Event labeling [en-US]"@en-us .


###  http://w3id.org/meta-share/omtd-share/ExploratorySearch
:ExploratorySearch rdf:type owl:Class ;
                   rdfs:subClassOf :InformationRetrieval ;
                   rdfs:comment "A type of search which, in contrast to traditional lookup search, covers a broad class of activities, such as investigating, evaluating, comparing, and synthesizing"@en ;
                   rdfs:label "Exploratory search"@en .


###  http://w3id.org/meta-share/omtd-share/ExtractionOfDomainSpecificInformation
:ExtractionOfDomainSpecificInformation rdf:type owl:Class ;
                                       rdfs:subClassOf :InformationExtraction ;
                                       rdfs:comment "Extraction of information that pertains to specific domains/disciplines; it can be used combined with \"\"Annotation type\"\" to specify the type of information extracted"@en ,
                                                    "Extraction of information that pertains to specific domains/disciplines; it can be used combined with \"Annotation type\" to specify the type of information extracted"@en ;
                                       rdfs:label "Extraction of domain-specific information"@en .


###  http://w3id.org/meta-share/omtd-share/ExtractionOfFundingInformation
:ExtractionOfFundingInformation rdf:type owl:Class ;
                                rdfs:subClassOf :ExtractionOfDomainSpecificInformation ,
                                                [ rdf:type owl:Restriction ;
                                                  owl:onProperty :deployedInDomain ;
                                                  owl:someValuesFrom :ScholarlyCommunication
                                                ] ;
                                rdfs:comment "The task/process of detecting in a text and extracting information relevant to funding (e.g. funding programme, award, funder etc.)"@en ;
                                rdfs:label "Extraction of funding information"@en ;
                                <http://www.w3.org/2004/02/skos/core#altLabel> "Mining of funding information"@en .


###  http://w3id.org/meta-share/omtd-share/FaceDetection
:FaceDetection rdf:type owl:Class ;
               rdfs:subClassOf :OperationWithMultimediaInputOrOutput ;
               rdfs:comment "The task/process of recognizing that a person appears on a digital image or a video frame from a video source and possibly marking the contours around it"@en ;
               rdfs:label "Face detection"@en .


###  http://w3id.org/meta-share/omtd-share/FaceRecognition
:FaceRecognition rdf:type owl:Class ;
                 rdfs:subClassOf :OperationWithMultimediaInputOrOutput ;
                 rdfs:comment "The task/process of identifying or verifying a person from a digital image or a video frame from a video source [adapted from Wikipedia]"@en ;
                 rdfs:label "Face recognition"@en ;
                 <http://www.w3.org/2004/02/skos/core#altLabel> "Facial recognition"@en .


###  http://w3id.org/meta-share/omtd-share/FaceVerification
:FaceVerification rdf:type owl:Class ;
                  rdfs:subClassOf :OperationWithMultimediaInputOrOutput ;
                  rdfs:comment "The task/process of validating a claimed identity based on the image of a face, and either accepting or rejecting the identity claim [adapted from http://www.idiap.ch/~marcel/labs/faceverif.php]"@en ;
                  rdfs:label "Face verification"@en ;
                  <http://www.w3.org/2004/02/skos/core#altLabel> "Face authentication"@en .


###  http://w3id.org/meta-share/omtd-share/FacialExpressionRecognition
:FacialExpressionRecognition rdf:type owl:Class ;
                             rdfs:subClassOf :SupportOperation ;
                             rdfs:comment "The task/process of detecting emotions on human face based on biometric markers [adapted from https://sightcorp.com/knowledge-base/facial-expression-recognition/]"@en ;
                             rdfs:label "Facial expression recognition"@en ;
                             <http://www.w3.org/2004/02/skos/core#altLabel> "Expression detection"@en ,
                                                                            "Expression recognition"@en ,
                                                                            "Face expression detection"@en ,
                                                                            "Face expression recognition"@en ,
                                                                            "Facial expression detection"@en .


###  http://w3id.org/meta-share/omtd-share/Facility
:Facility rdf:type owl:Class ;
          rdfs:subClassOf :NamedEntity ;
          rdfs:comment "A human-made artifact in the domains of architecture and civil engineering [source: https://www.nltk.org/book/ch07.html]"@en ;
          rdfs:label "Facility"@en .


###  http://w3id.org/meta-share/omtd-share/FactChecking
:FactChecking rdf:type owl:Class ;
              rdfs:subClassOf :InformationExtraction ;
              rdfs:altLabel "Fact-checking"@en ;
              rdfs:comment "The act of checking factual assertions in non-fictional text in order to determine the veracity and correctness of the factual statements in the text [from Wikipedia]"@en ;
              rdfs:label "Fact checking"@en ;
              <http://www.w3.org/2004/02/skos/core#related> :FakeNewsDetection .


###  http://w3id.org/meta-share/omtd-share/FactoredTagLemFormat
:FactoredTagLemFormat rdf:type owl:Class ;
                      rdfs:subClassOf :AnnotationFormat ,
                                      [ rdf:type owl:Restriction ;
                                        owl:onProperty :documentationUrl ;
                                        owl:hasValue "https://builds.openminted.eu/job/WP%205.2%20-%20Typesystem%20alignment/eu.openminted.interop$mapping-conversion/doclinks/1/components.html#_factored_tag_lem_1"
                                      ] ;
                      rdfs:comment "Factored tag lemma format"@en ;
                      rdfs:label "Factored tag lem format"@en .


###  http://w3id.org/meta-share/omtd-share/FakeNewsDetection
:FakeNewsDetection rdf:type owl:Class ;
                   rdfs:subClassOf :InformationExtraction ;
                   rdfs:altLabel "Fake news assessment"@en ,
                                 "Fake news evaluation"@en ;
                   rdfs:comment "The process of detecting whether a certain news item is fake (i.e. a type of news items of yellow journalism or propaganda that consists of deliberate disinformation or hoaxes spread via traditional news media or online social media) [adapted from wikipedia]"@en ;
                   rdfs:label "Fake news detection"@en .


###  http://w3id.org/meta-share/omtd-share/FastInfoset
:FastInfoset rdf:type owl:Class ;
             rdfs:subClassOf :BinaryFormat ,
                             :GateFormat ,
                             [ rdf:type owl:Restriction ;
                               owl:onProperty :hasMimetype ;
                               owl:hasValue :application_fastinfoset
                             ] ,
                             [ rdf:type owl:Restriction ;
                               owl:onProperty :documentationUrl ;
                               owl:hasValue "https://gate.ac.uk/sale/tao/splitch23.html#x28-59400023.31"
                             ] ;
             rdfs:comment "A compressed binary encoding of GATE XML"@en ;
             rdfs:label "Fast Infoset"@en .


###  http://w3id.org/meta-share/omtd-share/FeatureExtraction
:FeatureExtraction rdf:type owl:Class ;
                   rdfs:subClassOf :SupportOperation ;
                   <http://purl.org/dc/elements/1.1/source> <http://scikit-learn.org/stable/modules/feature_extraction.html> ;
                   rdfs:comment "Feature extraction consists in transforming arbitrary data, such as text or images, into numerical features usable for machine learning"@en ;
                   rdfs:label "Feature extraction"@en .


###  http://w3id.org/meta-share/omtd-share/FeatureExtractor
:FeatureExtractor rdf:type owl:Class ;
                  rdfs:subClassOf :SupportComponent ,
                                  [ rdf:type owl:Restriction ;
                                    owl:onProperty :performsOperation ;
                                    owl:someValuesFrom :FeatureExtraction
                                  ] ;
                  rdfs:comment "A component that is used for extracting features"@en ;
                  rdfs:label "Feature extractor"@en ;
                  <http://www.w3.org/2004/02/skos/core#comment> "could also be under analyzer as a general term"@en .


###  http://w3id.org/meta-share/omtd-share/Filter
:Filter rdf:type owl:Class ;
        rdfs:subClassOf :PreOrPostProcessor ;
        rdfs:comment "A component that is used for filtering text input or annotations based on specific criteria"@en ;
        rdfs:label "Filter"@en .


###  http://w3id.org/meta-share/omtd-share/FiniteStateTechnology
:FiniteStateTechnology rdf:type owl:Class ;
                       rdfs:subClassOf :TdmMethod ;
                       rdfs:comment "In data communications, flow control is the process of managing the rate of data transmission between two nodes to prevent a fast sender from overwhelming a slow receiver. It provides a mechanism for the receiver to control the transmission speed, so that the receiving node is not overwhelmed with data from transmitting node."@en ;
                       rdfs:label "Finite state technology"@en ;
                       <http://www.w3.org/2004/02/skos/core#related> :BuildingOfFiniteStateAutomata .


###  http://w3id.org/meta-share/omtd-share/FlowControl
:FlowControl rdf:type owl:Class ;
             rdfs:subClassOf :SupportOperation ;
             <http://purl.org/dc/elements/1.1/source> <https://en.wikipedia.org/wiki/Flow_control_(data)> ;
             rdfs:label "Flow control"@en .


###  http://w3id.org/meta-share/omtd-share/FlowController
:FlowController rdf:type owl:Class ;
                rdfs:subClassOf :SupportComponent ,
                                [ rdf:type owl:Restriction ;
                                  owl:onProperty :performsOperation ;
                                  owl:someValuesFrom :FlowControl
                                ] ;
                rdfs:comment "A component that supports controlling flows"@en ;
                rdfs:label "Flow controller"@en .


###  http://w3id.org/meta-share/omtd-share/Folia
:Folia rdf:type owl:Class ;
       rdfs:subClassOf :AnnotationFormat ,
                       :Xml ,
                       [ rdf:type owl:Restriction ;
                         owl:onProperty :documentationUrl ;
                         owl:hasValue "https://proycon.github.io/folia/"
                       ] ;
       rdfs:comment "FoLiA is an XML-based annotation format, suitable for the representation of linguistically annotated language resources"@en ;
       rdfs:label "FoLiA"@en ;
       <http://www.w3.org/2004/02/skos/core#altLabel> "Format for Linguistic Annotation"@en .


###  http://w3id.org/meta-share/omtd-share/FormatConversion
:FormatConversion rdf:type owl:Class ;
                  rdfs:subClassOf :SupportOperation ;
                  rdfs:comment "The task/process of converting (changing) the format of a resource into another (e.g. PDF to TXT or XML)"@en ;
                  rdfs:label "Format conversion"@en ;
                  <http://www.w3.org/2004/02/skos/core#altLabel> "Data conversion"@en ,
                                                                 "File conversion"@en .


###  http://w3id.org/meta-share/omtd-share/FrameExtraction
:FrameExtraction rdf:type owl:Class ;
                 rdfs:subClassOf :InformationExtraction ;
                 rdfs:comment "The task of recognizing words and phrases that evoke semantic frames as defined in the FrameNet project, and their semantic dependents."@en ;
                 rdfs:label "Frame extraction"@en .


###  http://w3id.org/meta-share/omtd-share/FrameSemanticParsing
:FrameSemanticParsing rdf:type owl:Class ;
                      rdfs:subClassOf :Parsing ,
                                      :SemanticAnnotation ;
                      rdfs:comment "The task/process of recognising and labelling in a text predicate argument structures and the semantic roles of the constituents, in accordance to the frame semantics theory."@en ;
                      rdfs:label "Frame-semantic parsing"@en .


###  http://w3id.org/meta-share/omtd-share/Funding
:Funding rdf:type owl:Class ;
         rdfs:subClassOf :ScholarlyAnalyticsEntity ,
                         :ScholarlyCommunicationAnnotation ;
         rdfs:comment "Annotation related to the funding of a resource (e.g. funder, funding project, etc.)"@en ;
         rdfs:label "Funding"@en .


###  http://w3id.org/meta-share/omtd-share/GateFormat
:GateFormat rdf:type owl:Class ;
            rdfs:subClassOf :DataFormat ;
            rdfs:comment "Formats used for the GATE framework"@en ;
            rdfs:label "GATE format"@en .


###  http://w3id.org/meta-share/omtd-share/GateXml
:GateXml rdf:type owl:Class ;
         rdfs:subClassOf :GateFormat ,
                         :Xml ,
                         [ rdf:type owl:Restriction ;
                           owl:onProperty :hasMimetype ;
                           owl:hasValue :application_xml
                         ] ;
         rdfs:comment "XML-based format for GATE components"@en ;
         rdfs:label "GATE XML"@en .


###  http://w3id.org/meta-share/omtd-share/Gate_twitter_json
:Gate_twitter_json rdf:type owl:Class ;
                   rdfs:subClassOf :GateFormat ,
                                   :Json ,
                                   [ rdf:type owl:Restriction ;
                                     owl:onProperty :hasMimetype ;
                                     owl:hasValue :application_x_json_twitter
                                   ] ,
                                   [ rdf:type owl:Restriction ;
                                     owl:onProperty :documentationUrl ;
                                     owl:hasValue "https://gate.ac.uk/sale/tao/splitch17.html"
                                   ] ;
                   rdfs:comment "A Twitter-style JSON format used for GATE documents"@en ;
                   rdfs:label "GATE/JSON twitter"@en ;
                   <http://www.w3.org/2004/02/skos/core#altLabel> "Twitter/JSON"@en .


###  http://w3id.org/meta-share/omtd-share/GazeteerBasedMatcher
:GazeteerBasedMatcher rdf:type owl:Class ;
                      rdfs:subClassOf :Matcher ,
                                      [ rdf:type owl:Restriction ;
                                        owl:onProperty :performsOperation ;
                                        owl:someValuesFrom :GazeteerBasedMatching
                                      ] ;
                      rdfs:comment "A component that allows matching of elements based on a gazeteer"@en ;
                      rdfs:label "Gazeteer based matcher"@en .


###  http://w3id.org/meta-share/omtd-share/GazeteerBasedMatching
:GazeteerBasedMatching rdf:type owl:Class ;
                       rdfs:subClassOf :Matching ;
                       rdfs:comment "The task/process of performing a comparison between a text/dataset and a gazeteer and identifying in the text/dataset units that are included in the gazeteer"@en ;
                       rdfs:label "Gazeteer based matching"@en ;
                       <http://www.w3.org/2004/02/skos/core#altLabel> "Gazeteer-based matching"@en .


###  http://w3id.org/meta-share/omtd-share/GenderDetection
:GenderDetection rdf:type owl:Class ;
                 rdfs:subClassOf :InformationExtraction ;
                 rdfs:label "Gender detection"@en .


###  http://w3id.org/meta-share/omtd-share/Gene
:Gene rdf:type owl:Class ;
      rdfs:subClassOf :AgriculturalEntity ;
      rdfs:comment "Specific sequence of nucleotides along a molecule of DNA (or, in the case of some viruses, RNA) which represents functional units of heredity [http://artemide.art.uniroma2.it:8081/agrovoc/agrovoc/en/page/c_3214]"@en ;
      rdfs:label "Gene"@en .


###  http://w3id.org/meta-share/omtd-share/GeneFamily
:GeneFamily rdf:type owl:Class ;
            rdfs:subClassOf :AgriculturalEntity ;
            rdfs:comment "A gene family is a set of several similar genes, formed by duplication of a single original gene, and generally with similar biochemical functions [https://en.wikipedia.org/wiki/Gene_family]"@en ;
            rdfs:label "Gene family"@en .


###  http://w3id.org/meta-share/omtd-share/Generator
:Generator rdf:type owl:Class ;
           rdfs:subClassOf :Processor ;
           rdfs:comment "A component that generates (semi-)automatically natural language texts (based on non-linguistic data, keywords, logical forms, knowledge bases...)"@en ;
           rdfs:label "Generator"@en .


###  http://w3id.org/meta-share/omtd-share/Geo-politicalEntity
:Geo-politicalEntity rdf:type owl:Class ;
                     rdfs:subClassOf :NamedEntity ;
                     rdfs:altLabel "GPE"@en ;
                     rdfs:comment "A geographical area associated with some sort of political structure"@en ;
                     rdfs:label "Geo-political entity"@en .


###  http://w3id.org/meta-share/omtd-share/Graf
:Graf rdf:type owl:Class ;
      rdfs:subClassOf :AnnotationFormat ,
                      [ rdf:type owl:Restriction ;
                        owl:onProperty :hasMimetype ;
                        owl:hasValue :application_x_org_dkpro_graf_xml
                      ] ,
                      [ rdf:type owl:Restriction ;
                        owl:onProperty :documentationUrl ;
                        owl:hasValue "http://dl.acm.org/citation.cfm?id=1642060"
                      ] ,
                      [ rdf:type owl:Restriction ;
                        owl:onProperty :documentationUrl ;
                        owl:hasValue "https://zoidberg.ukp.informatik.tu-darmstadt.de/jenkins/job/DKPro%20Core%20Documentation%20(GitHub)/de.tudarmstadt.ukp.dkpro.core$de.tudarmstadt.ukp.dkpro.core.doc-asl/doclinks/5/format-reference.html#format-Graf"
                      ] ;
      rdfs:comment "GrAF (Graph Annotation Format) is an extension of the Linguistic Annotation Framework (LAF)"@en ;
      rdfs:label "GrAF"@en ;
      <http://www.w3.org/2004/02/skos/core#altLabel> "Graph Annotation Format"@en .


###  http://w3id.org/meta-share/omtd-share/GrammarChecker
:GrammarChecker rdf:type owl:Class ;
                rdfs:subClassOf :PreOrPostProcessor ;
                rdfs:comment "A component that corrects grammatical mistakes in a text"@en ;
                rdfs:label "Grammar checker"@en .


###  http://w3id.org/meta-share/omtd-share/GrammarChecking
:GrammarChecking rdf:type owl:Class ;
                 rdfs:subClassOf :AuthoringSupport ;
                 rdfs:label "Grammar checking"@en .


###  http://w3id.org/meta-share/omtd-share/GrapeVariety
:GrapeVariety rdf:type owl:Class ;
              rdfs:subClassOf :AgriculturalEntity ;
              rdfs:comment "A type of grape"@en ;
              rdfs:label "Grape variety"@en .


###  http://w3id.org/meta-share/omtd-share/Habitat
:Habitat rdf:type owl:Class ;
         rdfs:subClassOf :AgriculturalEntity ;
         rdfs:comment "The place or environment where an organism, plant or animal naturally or normally lives and grows"@en ;
         rdfs:label "Habitat"@en .


###  http://w3id.org/meta-share/omtd-share/HandwritingRecognition
:HandwritingRecognition rdf:type owl:Class ;
                        rdfs:subClassOf :SupportOperation ;
                        rdfs:comment "The ability of a computer to receive and interpret intelligible handwritten input from sources such as paper documents, photographs, touch-screens and other devices [from Wikipedia]"@en ;
                        rdfs:label "Handwriting recognition"@en ;
                        <http://www.w3.org/2004/02/skos/core#altLabel> "HWR"@en ;
                        <http://www.w3.org/2004/02/skos/core#definition> "" .


###  http://w3id.org/meta-share/omtd-share/HateSpeechRecognition
:HateSpeechRecognition rdf:type owl:Class ;
                       rdfs:subClassOf :InformationExtraction ;
                       rdfs:altLabel "Hate speech detection"@en ;
                       rdfs:comment "The task of automatically identifying hate speech, i.e. statements intended to demean and brutalize another, or the use of cruel and derogatory language on the basis of real or alleged membership in a social group [adapted from wikipedia]"@en ;
                       rdfs:label "Hate speech recognition"@en .


###  http://w3id.org/meta-share/omtd-share/HistoricalEvent
:HistoricalEvent rdf:type owl:Class ;
                 rdfs:subClassOf :NamedEntity ,
                                 :SocialSciencesEntity ;
                 rdfs:comment "Historical event"@en ;
                 rdfs:label "Historical event"@en .


###  http://w3id.org/meta-share/omtd-share/Html
:Html rdf:type owl:Class ;
      rdfs:subClassOf :DocumentFormat ,
                      [ rdf:type owl:Restriction ;
                        owl:onProperty :hasMimetype ;
                        owl:hasValue :text_html
                      ] ;
      rdfs:comment "HTML format"@en ;
      rdfs:label "HTML"@en .


###  http://w3id.org/meta-share/omtd-share/Html5Microdata
:Html5Microdata rdf:type owl:Class ;
                rdfs:subClassOf :AnnotationFormat ,
                                :Html ,
                                [ rdf:type owl:Restriction ;
                                  owl:onProperty :hasMimetype ;
                                  owl:hasValue :text_html
                                ] ,
                                [ rdf:type owl:Restriction ;
                                  owl:onProperty :documentationUrl ;
                                  owl:hasValue "https://www.w3.org/TR/microdata/"
                                ] ;
                rdfs:comment "Format according to the specifications of HTML5 Microdata"@en ;
                rdfs:label "HTML5 Microdata"@en .


###  http://w3id.org/meta-share/omtd-share/HumanAidedMachineTranslation
:HumanAidedMachineTranslation rdf:type owl:Class ;
                              rdfs:subClassOf :MachineTranslation ;
                              rdfs:comment "The process of performing Machine Translation facilitated by pre-editing or post-editing steps, or interactive human intervention to steer or select from alternative translations"@en ;
                              rdfs:label "Human Aided Machine Translation"@en ;
                              <http://www.w3.org/2004/02/skos/core#altLabel> "HAMT"@en ;
                              <http://www.w3.org/2004/02/skos/core#definition> "We call Human-aided Machine Translation all systems and techniques which rely on real automation of the translation function when porting a text from one language to another. As opposed to full Machine Translation, human-aided MT does not fully rely on computational translation, but assists this process by pre-editing and post-editing steps, possibly also interactive human intervention to steer or select from alternative translations. Translation of real-time spoken language, by contrast, does not allow for human intervention, except for negotiation functions, such as clarification dialogues."@en .


###  http://w3id.org/meta-share/omtd-share/HumanComputerInteraction
:HumanComputerInteraction rdf:type owl:Class ;
                          rdfs:subClassOf :OperationWithMultimediaInputOrOutput ;
                          rdfs:comment "A multi-disciplinary research area focusing on the design and use of computer technology deployed in interfaces between humans and computers"@en ;
                          rdfs:label "Human Computer Interaction"@en ;
                          <http://www.w3.org/2004/02/skos/core#altLabel> "HCI"@en .


###  http://w3id.org/meta-share/omtd-share/HumourDetection
:HumourDetection rdf:type owl:Class ;
                 rdfs:subClassOf :InformationExtraction ;
                 rdfs:altLabel "Humor detection"@en-us ,
                               "Humor recognition"@en-us ,
                               "Humor sensing"@en-us ,
                               "Humour recognition"@en ,
                               "Humour sensing"@en ;
                 rdfs:comment "The task of identifying in a text structures and phrases of humour"@en-us ;
                 rdfs:label "Humour detection"@en .


###  http://w3id.org/meta-share/omtd-share/I2b2
:I2b2 rdf:type owl:Class ;
      rdfs:subClassOf :AnnotationFormat ,
                      [ rdf:type owl:Restriction ;
                        owl:onProperty :documentationUrl ;
                        owl:hasValue "https://builds.openminted.eu/job/WP%205.2%20-%20Typesystem%20alignment/eu.openminted.interop$mapping-conversion/doclinks/1/components.html#I2B2Reader"
                      ] ,
                      [ rdf:type owl:Restriction ;
                        owl:onProperty :documentationUrl ;
                        owl:hasValue "https://www.i2b2.org/NLP/RDoCforPsychiatry/PreviousChallenges.php"
                      ] ;
      rdfs:comment "Format of the I2B2 challenge"@en ;
      rdfs:label "I2B2"@en .


###  http://w3id.org/meta-share/omtd-share/ImageTranslation
:ImageTranslation rdf:type owl:Class ;
                  rdfs:subClassOf :Translation ;
                  rdfs:comment "The automatic extraction of text contained in an image (e.g. by OCR technology), its subsequent translation into another language, followed by a digital image processing step in order to reconstruct the original image with the translated text [adapted from https://en.wikipedia.org/wiki/Image_translation]"@en ;
                  rdfs:label "Image translation"@en .


###  http://w3id.org/meta-share/omtd-share/ImageUnderstanding
:ImageUnderstanding rdf:type owl:Class ;
                    rdfs:subClassOf :TextAndDataMining ;
                    rdfs:comment "Advanced image processing in which artificial-intelligence techniques are used to interpret images by locating, characterizing, and recognizing objects and other features in the scene. [from https://www.encyclopedia.com/computing/dictionaries-thesauruses-pictures-and-press-releases/image-understanding]"@en ;
                    rdfs:label "Image Understanding"@en ;
                    <http://www.w3.org/2004/02/skos/core#definition> "" .


###  http://w3id.org/meta-share/omtd-share/Imscwb
:Imscwb rdf:type owl:Class ;
        rdfs:subClassOf :CorpusFormat ,
                        :TabularFormat ,
                        [ rdf:type owl:Restriction ;
                          owl:onProperty :hasMimetype ;
                          owl:hasValue :text_x_org_dkpro_imscwb
                        ] ,
                        [ rdf:type owl:Restriction ;
                          owl:onProperty :documentationUrl ;
                          owl:hasValue "https://dkpro.github.io/dkpro-core/releases/1.8.0/docs/format-reference.html#format-de.tudarmstadt.ukp.dkpro.core.io.imscwb-asl"
                        ] ;
        rdfs:comment "A tab-separated format with limited markup (e.g. for sentences, documents, but not recursive structures like parse-trees) used by the IMS Open Corpus Workbench."@en ;
        rdfs:label "imsCwb"@en ;
        <http://www.w3.org/2004/02/skos/core#altLabel> "IMS Corpus Workbench"@en .


###  http://w3id.org/meta-share/omtd-share/InformationExtraction
:InformationExtraction rdf:type owl:Class ;
                       rdfs:subClassOf :TextAndDataMining ;
                       rdfs:comment "The process/task of automatically extracting structured information from unstructured and/or semi-structured data"@en ;
                       rdfs:label "Information Extraction"@en ;
                       <http://www.w3.org/2004/02/skos/core#altLabel> "IE & Text Analysis"@en ,
                                                                      "Information Discovery"@en ;
                       <http://www.w3.org/2004/02/skos/core#definition> "The goal of information extraction (IE) is to build systems that find and link relevant information from natural language text ignoring irrelevant information. The information of interest is typically pre-specified in form of uninstantiated frame-like structures also called templates. The templates are domain and task specific. The major task of an IE-system is then the identification of the relevant parts of the text which are used to fill a template's slots."@en .


###  http://w3id.org/meta-share/omtd-share/InformationExtractor
:InformationExtractor rdf:type owl:Class ;
                      rdfs:subClassOf :Analyzer ,
                                      [ rdf:type owl:Restriction ;
                                        owl:onProperty :performsOperation ;
                                        owl:someValuesFrom :InformationExtraction
                                      ] ;
                      rdfs:comment "A component that automatically extracts structured information from unstructured and/or semi-structured machine-readable documents"@en ;
                      rdfs:label "Information extractor"@en .


###  http://w3id.org/meta-share/omtd-share/InformationFiltering
:InformationFiltering rdf:type owl:Class ;
                      rdfs:subClassOf :InformationRetrieval ;
                      rdfs:comment "The process/task of removing (filtering out) redundant or unwanted information from an information stream using (semi)automated or computerized methods prior to presentation to a human user; the selection of the items is based on the correlation between the content of the items and the users preferences (content-based filtering) or the correlation between people with similar preferences (collaborative filtering)"@en ;
                      rdfs:label "Information filtering"@en .


###  http://w3id.org/meta-share/omtd-share/InformationFilteringByRecommenderSystems
:InformationFilteringByRecommenderSystems rdf:type owl:Class ;
                                          rdfs:subClassOf :InformationFiltering ;
                                          rdfs:comment "The delivery of information in the form of suggestions by recommender systems; recommender systems seek to predict the \"\"rating\"\" or \"\"preference\"\" that a user would give to an item"@en ;
                                          rdfs:label "Information filtering by recommender systems"@en .


###  http://w3id.org/meta-share/omtd-share/InformationRetrieval
:InformationRetrieval rdf:type owl:Class ;
                      rdfs:subClassOf :TextAndDataMining ;
                      rdfs:comment "The activity of obtaining information resources relevant to an information need from a collection of information resources; searches can be based on full-text or other content-based indexing"@en ;
                      rdfs:label "Information Retrieval"@en ;
                      <http://www.w3.org/2004/02/skos/core#definition> "Information Retrieval is the process of locating information that fits a user's information need, which is usually expressed as a search query. The fit of the retrieved information with the information need is referred to as \"\"relevance\"\". The information can be retrieved from databases (data retrieval) or from document collections (document retrieval), where documents can either be text documents or other media (audio, video, semi-structured data, multimedia). Success in information retrieval is generally defined by retrieving as much relevant information as possible (measured by \"\"recall\"\") while minimising the irrelevant information retrieved (measured by \"\"precision\"\"). The most widely used information retrieval systems today are Internet search engines."@en .


###  http://w3id.org/meta-share/omtd-share/InformationStorage
:InformationStorage rdf:type owl:Class ;
                    rdfs:subClassOf :SupportOperation ;
                    rdfs:label "Information storage"@en ;
                    <http://www.w3.org/2004/02/skos/core#altLabel> "Data storage"@en ;
                    <http://www.w3.org/2004/02/skos/core#definition> "" .


###  http://w3id.org/meta-share/omtd-share/InlineXml
:InlineXml rdf:type owl:Class ;
           rdfs:subClassOf :AnnotationFormat ,
                           :Xml ,
                           [ rdf:type owl:Restriction ;
                             owl:onProperty :hasMimetype ;
                             owl:hasValue :application_xml
                           ] ,
                           [ rdf:type owl:Restriction ;
                             owl:onProperty :documentationUrl ;
                             owl:hasValue "https://dkpro.github.io/dkpro-core/releases/1.8.0/docs/format-reference.html#format-de.tudarmstadt.ukp.dkpro.core.io.xml-asl"
                           ] ;
           rdfs:comment "Inline XML file format"@en ;
           rdfs:label "Inline XML"@en .


###  http://w3id.org/meta-share/omtd-share/InstanceBasedLearning
:InstanceBasedLearning rdf:type owl:Class ;
                       rdfs:subClassOf :MachineAndStatisticalLearningMethod ;
                       <http://purl.org/dc/elements/1.1/source> "adapted from Wikipedia (https://en.wikipedia.org/wiki/Instance-based_learning)"@en ;
                       rdfs:comment "A family of learning algorithms that, instead of performing explicit generalization, compares new problem instances with instances seen in training, which have been stored in memory."@en ;
                       rdfs:label "Instance-based Learning"@en ;
                       <http://www.w3.org/2004/02/skos/core#example> "Examples of instance-based learning algorithm are the k-nearest neighbor algorithm, kernel machines and RBF networks."@en .


###  http://w3id.org/meta-share/omtd-share/IntraDocumentCoReferenceResolution
:IntraDocumentCoReferenceResolution rdf:type owl:Class ;
                                    rdfs:subClassOf :CoReferenceResolution ;
                                    rdfs:label "Intra-document co-reference resolution"@en ;
                                    <http://www.w3.org/2004/02/skos/core#altLabel> "Intra-document coreference resolution"@en .


###  http://w3id.org/meta-share/omtd-share/IonicChannel
:IonicChannel rdf:type owl:Class ;
              rdfs:subClassOf :BiologicalEnity ,
                              :NamedEntity ;
              rdfs:altLabel "Ion channel"@en ;
              rdfs:comment "A single protein or protein complex that traverses the lipid bilayer of cell membrane and form a channel to facilitate the movement of ions through the membrane according to their electrochemical gradient [http://www.biology-online.org/dictionary/Ion_channel]"@en ;
              rdfs:label "Ionic channel"@en .


###  http://w3id.org/meta-share/omtd-share/IonicConductance
:IonicConductance rdf:type owl:Class ;
                  rdfs:subClassOf :BiologicalEnity ,
                                  :NamedEntity ;
                  rdfs:altLabel "Ion conductance"@en ;
                  rdfs:comment "Ionic conductance"@en ;
                  rdfs:label "Ionic conductance"@en .


###  http://w3id.org/meta-share/omtd-share/IonicCurrent
:IonicCurrent rdf:type owl:Class ;
              rdfs:subClassOf :BiologicalEnity ,
                              :NamedEntity ;
              rdfs:altLabel "Ion current"@en ;
              rdfs:comment "The influx and/or efflux of ions through an ion channel"@en ;
              rdfs:label "Ionic current"@en .


###  http://w3id.org/meta-share/omtd-share/IronyDetection
:IronyDetection rdf:type owl:Class ;
                rdfs:subClassOf :InformationExtraction ;
                rdfs:label "Irony detection"@en ,
                           "The task of identifying in a text segments expressing irony and classifying  them into types"@en .


###  http://w3id.org/meta-share/omtd-share/Jdbc
:Jdbc rdf:type owl:Class ;
      rdfs:subClassOf :DatabaseFormat ,
                      [ rdf:type owl:Restriction ;
                        owl:onProperty :documentationUrl ;
                        owl:hasValue "https://zoidberg.ukp.informatik.tu-darmstadt.de/jenkins/job/DKPro%20Core%20Documentation%20(GitHub)/de.tudarmstadt.ukp.dkpro.core$de.tudarmstadt.ukp.dkpro.core.doc-asl/doclinks/5/format-reference.html#format-Jdbc"
                      ] ;
      rdfs:comment "For JDBC databases"@en ;
      rdfs:label "JDBC"@en ;
      <http://www.w3.org/2004/02/skos/core#altLabel> "JAVA Database Connectivity"@en .


###  http://w3id.org/meta-share/omtd-share/Json
:Json rdf:type owl:Class ;
      rdfs:subClassOf :DataFormat ;
      rdfs:comment "Superclass of JSON formats"@en ;
      rdfs:label "JSON"@en .


###  http://w3id.org/meta-share/omtd-share/Json_genia
:Json_genia rdf:type owl:Class ;
            rdfs:subClassOf :BionlpFormat ,
                            :BionlpFormats ,
                            :Json ,
                            [ rdf:type owl:Restriction ;
                              owl:onProperty :hasMimetype ;
                              owl:hasValue :application_json
                            ] ,
                            [ rdf:type owl:Restriction ;
                              owl:onProperty :documentationUrl ;
                              owl:hasValue "https://builds.openminted.eu/job/WP%205.2%20-%20Typesystem%20alignment/eu.openminted.interop$mapping-conversion/doclinks/1/components.html#GeniaJSONReader"
                            ] ;
            rdfs:comment "JSON format of the Genia dataset"@en ;
            rdfs:label "JSON/Genia"@en .


###  http://w3id.org/meta-share/omtd-share/Kaf
:Kaf rdf:type owl:Class ;
     rdfs:subClassOf :AnnotationFormat ,
                     :Json ,
                     [ rdf:type owl:Restriction ;
                       owl:onProperty :hasMimetype ;
                       owl:hasValue :application_x_kaf_json
                     ] ,
                     [ rdf:type owl:Restriction ;
                       owl:onProperty :documentationUrl ;
                       owl:hasValue "http://kyoto-project.eu/xmlgroup.iit.cnr.it/kyoto/indexdd46.html?option=com_content&view=article&id=141&Itemid=130"
                     ] ;
     rdfs:comment "KAF (also known as Knowledge Annotation Format) is a language neutral annotation format representing both morpho-syntactic and semantic annotation of documents through a stand-off multilayered structure"@en ;
     rdfs:label "KAF"@en ;
     <http://www.w3.org/2004/02/skos/core#altLabel> "KYOTO Annotation Format"@en ,
                                                    "Knowledge Annotation Format"@en .


###  http://w3id.org/meta-share/omtd-share/KeaCorpus
:KeaCorpus rdf:type owl:Class ;
           rdfs:subClassOf :CorpusFormat ,
                           [ rdf:type owl:Restriction ;
                             owl:onProperty :documentationUrl ;
                             owl:hasValue "https://builds.openminted.eu/job/WP%205.2%20-%20Typesystem%20alignment/eu.openminted.interop$mapping-conversion/doclinks/1/components.html#_kea_corpus_1"
                           ] ;
           rdfs:comment "KEA-style (Keyphrase Extraction Algorithm) corpus"@en ;
           rdfs:label "KEA corpus"@en .


###  http://w3id.org/meta-share/omtd-share/KernelMethod
:KernelMethod rdf:type owl:Class ;
              rdfs:subClassOf :MachineAndStatisticalLearningMethod ;
              <http://purl.org/dc/elements/1.1/source> "adapted from wikipedia (https://en.wikipedia.org/wiki/Kernel_method)"@en ;
              rdfs:comment "Any method used in pattern analysis that relies on kernel functions, which enable it to operate in a high-dimensional, implicit feature space without ever computing the coordinates of the data in that space, but rather by simply computing the inner products between the images of all pairs of data in the feature space."@en ;
              rdfs:label "Kernel Method"@en .


###  http://w3id.org/meta-share/omtd-share/Keyword
:Keyword rdf:type owl:Class ;
         rdfs:subClassOf :ScholarlyAnalyticsEntity ,
                         :ScholarlyCommunicationAnnotation ,
                         :SemanticAnnotationType ;
         rdfs:comment "A word or group of words used to describe or index the contents of a document"@en ;
         rdfs:label "Keyword"@en .


###  http://w3id.org/meta-share/omtd-share/KeywordExtraction
:KeywordExtraction rdf:type owl:Class ;
                   rdfs:subClassOf :InformationExtraction ;
                   rdfs:comment "The task/process of identifying keywords (words deemed indicative of the topic/subject) in a text/corpus"@en ;
                   rdfs:label "Keyword extraction"@en ;
                   <http://www.w3.org/2004/02/skos/core#altLabel> "KWS"@en ,
                                                                  "Key phrase Extraction"@en ,
                                                                  "Keyword search"@en ,
                                                                  "Keyword spotting"@en .


###  http://w3id.org/meta-share/omtd-share/KeywordExtractor
:KeywordExtractor rdf:type owl:Class ;
                  rdfs:subClassOf :Analyzer ,
                                  [ rdf:type owl:Restriction ;
                                    owl:onProperty :performsOperation ;
                                    owl:someValuesFrom :KeywordExtraction
                                  ] ;
                  rdfs:comment "A component that tries to extract keywords from a given text"@en ;
                  rdfs:label "Keyword extractor"@en .


###  http://w3id.org/meta-share/omtd-share/KnowledgeAcquisition
:KnowledgeAcquisition rdf:type owl:Class ;
                      rdfs:subClassOf :TextAndDataMining ;
                      rdfs:comment "The process/task of extracting, organising and systematising knowledge usually of a specific domain from external sources so that it can be used in a knowledge-based system"@en ;
                      rdfs:label "Knowledge acquisition"@en .


###  http://w3id.org/meta-share/omtd-share/KnowledgeDiscovery
:KnowledgeDiscovery rdf:type owl:Class ;
                    rdfs:subClassOf :TextAndDataMining ;
                    rdfs:comment "The task/process of automatically searching large volumes of data for patterns that can be considered knowledge about the data"@en ;
                    rdfs:label "Knowledge Discovery"@en ;
                    <http://www.w3.org/2004/02/skos/core#altLabel> "KD"@en ,
                                                                   "KDD"@en ,
                                                                   "Knowledge Discovery in Databases"@en ;
                    <http://www.w3.org/2004/02/skos/core#definition> "Generally, knowledge discovery / data mining is the process of analyzing data from different perspectives and summarizing it into useful information - information that can be used to increase revenue, cuts costs, or both. Data mining software is one of a number of analytical tools for analyzing data. It allows users to analyze data from many different dimensions or angles, categorize it, and summarize the relationships identified. Technically, data mining is the process of finding correlations or patterns among dozens of fields in large relational databases."@en .


###  http://w3id.org/meta-share/omtd-share/KnowledgeRepresentation
:KnowledgeRepresentation rdf:type owl:Class ;
                         rdfs:subClassOf :TextAndDataMining ;
                         rdfs:comment "The task/process of representing information about entities in a form that machines are capable of understanding it"@en ;
                         rdfs:label "Knowledge Representation"@en ;
                         <http://www.w3.org/2004/02/skos/core#altLabel> "KR" ;
                         <http://www.w3.org/2004/02/skos/core#definition> "" .


###  http://w3id.org/meta-share/omtd-share/L2WritingSupport
:L2WritingSupport rdf:type owl:Class ;
                  rdfs:subClassOf :AuthoringSupport ;
                  rdfs:altLabel "L2 writing assistant"@en ;
                  rdfs:label "L2 writing support"@en .


###  http://w3id.org/meta-share/omtd-share/LD_json
:LD_json rdf:type owl:Class ;
         rdfs:subClassOf :DocumentFormat ,
                         :Json ,
                         :LinkedDataFormat ,
                         [ rdf:type owl:Restriction ;
                           owl:onProperty :hasMimetype ;
                           owl:hasValue :application_ld_json
                         ] ;
         rdfs:altLabel "JSON linked data" ,
                       "LD-Json" ;
         rdfs:comment "Data format encoding Linked Data using JSON"@en ;
         rdfs:label "JSON/LD"@en .


###  http://w3id.org/meta-share/omtd-share/LanguageChecking
:LanguageChecking rdf:type owl:Class ;
                  rdfs:subClassOf :AuthoringSupport ;
                  rdfs:comment "The task/process of identifying (and usually correcting) grammatical mistakes in a text"@en ;
                  rdfs:label "Language checking"@en ;
                  <http://www.w3.org/2004/02/skos/core#altLabel> "Proofing"@en ;
                  <http://www.w3.org/2004/02/skos/core#definition> "Language Checking comprises technologies used to detect and/or correct erroneous or inconsistent language use in documents. The scope of language checking technology ranges from general error correction, as performed by spell checkers and grammar chec"@en .


###  http://w3id.org/meta-share/omtd-share/LanguageDetection
:LanguageDetection rdf:type owl:Class ;
                   rdfs:subClassOf :InformationExtraction ;
                   rdfs:label "Language detection"@en .


###  http://w3id.org/meta-share/omtd-share/LanguageIdentification
:LanguageIdentification rdf:type owl:Class ;
                        rdfs:subClassOf :InformationExtraction ,
                                        :SupportOperation ;
                        rdfs:comment "The task/process of guessing what natural language a text or text segment is written in"@en ;
                        rdfs:label "Language identification"@en ;
                        <http://www.w3.org/2004/02/skos/core#altLabel> "Automatic Language Identification"@en ;
                        <http://www.w3.org/2004/02/skos/core#definition> "Automatic Language Identification (LID) is the process of identifying the natural language of a sample of speech or written text by an unknown speaker. Several important applications exist for LID, viz., as a front-end to, e.g., a call router in a telephone-based application or a multi-lingual speech recognition system."@en .


###  http://w3id.org/meta-share/omtd-share/LanguageIdentifier
:LanguageIdentifier rdf:type owl:Class ;
                    rdfs:subClassOf :Analyzer ,
                                    [ rdf:type owl:Restriction ;
                                      owl:onProperty :performsOperation ;
                                      owl:someValuesFrom :LanguageIdentification
                                    ] ;
                    rdfs:comment "A component that identifies the language of a given text based on its contents"@en ;
                    rdfs:label "Language identifier"@en .


###  http://w3id.org/meta-share/omtd-share/LanguageModelling
:LanguageModelling rdf:type owl:Class ;
                   rdfs:subClassOf :SupportOperation ;
                   rdfs:comment "The construction of statistical or Machine Learning language models"@en ;
                   rdfs:label "Language Modelling"@en ;
                   <http://www.w3.org/2004/02/skos/core#altLabel> "LM"@en ,
                                                                  "Language Modeling"@en ;
                   <http://www.w3.org/2004/02/skos/core#definition> "A Statistical Language Models predicts a word given a sequence of already known words (i.e. the history). Ist can also be applied to other sequences of symbols (e.g. DNA). Very often the history contains just the previous two words. This is called a trigram. The parameters of statistical language models are estimated from a set of training examples. Data sparsity and smoothing of the estimates is one of the core problems. The best smoothing technique known so far is Kneser-Ney-Smoothing. Maximum-Entropy techniques are also under investigation and may be the method of choice for long-range language models (beyond trigram). Language models are used in text-compression, speech recognition, information retrieval and information extraction."@en .


###  http://w3id.org/meta-share/omtd-share/LanguageTechnology
:LanguageTechnology rdf:type owl:Class ;
                    rdfs:subClassOf :Operation ;
                    rdfs:comment "Language technology, often called human language technology, studies methods of how computer programs or electronic devices can analyze, produce, modify or respond to human texts and speech. It consists of natural language processing and computational linguistics on the one hand, and speech technology on the other. (from Wikipedia)"@en ;
                    rdfs:label "Language Technology"@en ;
                    <http://www.w3.org/2004/02/skos/core#altLabel> "HLT"@en ,
                                                                   "Human Language Technology"@en ,
                                                                   "LT"@en ;
                    <http://www.w3.org/2004/02/skos/core#definition> "Language technology (LT), also Human Language Technology (HLT), is the cover term for all information technologies specialized for dealing with text and speech in human language. It is also the field of engineering in which LT methods and applications are developed."@en .


###  http://w3id.org/meta-share/omtd-share/Latex
:Latex rdf:type owl:Class ;
       rdfs:subClassOf :DocumentFormat ,
                       [ rdf:type owl:Restriction ;
                         owl:onProperty :hasMimetype ;
                         owl:hasValue :application_xLatex
                       ] ,
                       [ rdf:type owl:Restriction ;
                         owl:onProperty :documentationUrl ;
                         owl:hasValue "https://www.latex-project.org/about/"
                       ] ;
       rdfs:comment "Data format for documents using LaTeX (a high-quality typesetting system very popular for scientific documents)"@en ;
       rdfs:label "LATEX"@en .


###  http://w3id.org/meta-share/omtd-share/Lemma
:Lemma rdf:type owl:Class ;
       rdfs:subClassOf :MorphologicalAnnotationType ,
                       [ rdf:type owl:Restriction ;
                         owl:onProperty :documentationUrl ;
                         owl:hasValue "http://dkpro.github.io/dkpro-core/releases/1.8.0/docs/typesystem-reference.html#de.tudarmstadt.ukp.dkpro.core.api.segmentation.type.Lemma"
                       ] ;
       rdfs:comment "The canonical or citation form used for referring to a word and its inflected forms"@en ;
       rdfs:label "Lemma"@en .


###  http://w3id.org/meta-share/omtd-share/Lemmatization
:Lemmatization rdf:type owl:Class ;
               rdfs:subClassOf :TextAnnotation ,
                               [ rdf:type owl:Restriction ;
                                 owl:onProperty <http://www.w3.org/2004/02/skos/core#closeMatch> ;
                                 owl:someValuesFrom :Stemming
                               ] ;
               rdfs:comment "Lemmatisation  (or lemmatization) in linguistics is the process of grouping together the inflected forms of a word so they can be analysed as a single item, identified by the word's lemma, or dictionary form. [Wikipedia]"@en ;
               rdfs:label "Lemmatization"@en ;
               <http://www.w3.org/2004/02/skos/core#altLabel> "Lemmatisation"@en-uk .


###  http://w3id.org/meta-share/omtd-share/Lemmatizer
:Lemmatizer rdf:type owl:Class ;
            rdfs:subClassOf :Annotator ,
                            [ rdf:type owl:Restriction ;
                              owl:onProperty :performsOperation ;
                              owl:someValuesFrom :Lemmatization
                            ] ;
            rdfs:comment "A component that annotates the tokens of a text with lemma information"@en ;
            rdfs:label "Lemmatizer"@en .


###  http://w3id.org/meta-share/omtd-share/LexicalSemanticRelation
:LexicalSemanticRelation rdf:type owl:Class ;
                         rdfs:subClassOf :SemanticAnnotationType ,
                                         [ rdf:type owl:Restriction ;
                                           owl:onProperty owl:equivalentClass ;
                                           owl:someValuesFrom <http://purl.org/olia/olia-top.owl#LexicalRelation>
                                         ] ;
                         rdfs:comment "A relation holding between two or more words based on their meanings"@en ;
                         rdfs:label "Lexical semantic relation"@en ;
                         <http://www.w3.org/2004/02/skos/core#altLabel> "Semantic relation"@en .


###  http://w3id.org/meta-share/omtd-share/LexicalSimplification
:LexicalSimplification rdf:type owl:Class ;
                       rdfs:subClassOf :NaturalLanguageGeneration ;
                       rdfs:comment "The task of replacing individual words of a text with words that are easier to understand, so that the text as a whole becomes easier to comprehend, e.g. by people with learning disabilities or by children who learn to read [from https://link.springer.com/chapter/10.1007/978-3-642-28601-8_36]"@en ;
                       rdfs:label "Lexical simplification"@en ;
                       <http://www.w3.org/2004/02/skos/core#related> :LexicalSubstitution .


###  http://w3id.org/meta-share/omtd-share/LexicalSubstitution
:LexicalSubstitution rdf:type owl:Class ;
                     rdfs:subClassOf :NaturalLanguageGeneration ;
                     rdfs:comment "The task of identifying a substitute for a word in the context of a clause [from Wikipedia]"@en ;
                     rdfs:label "Lexical substitution"@en ;
                     <http://www.w3.org/2004/02/skos/core#related> :Paraphrasing .


###  http://w3id.org/meta-share/omtd-share/LexiconAccess
:LexiconAccess rdf:type owl:Class ;
               rdfs:subClassOf :SupportOperationForKnowledgeResources ;
               rdfs:comment "The task/process of accessing lexical/conceptual resources (either by humans or computer programs)"@en ;
               rdfs:label "Lexicon access"@en .


###  http://w3id.org/meta-share/omtd-share/LexiconAcquisitionFromCorpora
:LexiconAcquisitionFromCorpora rdf:type owl:Class ;
                               rdfs:subClassOf :KnowledgeAcquisition ,
                                               :SupportOperationForKnowledgeResources ;
                               rdfs:comment "The task/process of constructing lexical resources from corpora"@en ;
                               rdfs:label "Lexicon acquisition from corpora"@en .


###  http://w3id.org/meta-share/omtd-share/LexiconCreation
:LexiconCreation rdf:type owl:Class ;
                 rdfs:subClassOf :SupportOperationForKnowledgeResources ;
                 rdfs:comment "The task/process of constructing lexical resources (e.g. dictionaries, computational lexica, glossaries, etc.)"@en ;
                 rdfs:label "Lexicon creation"@en ;
                 <http://www.w3.org/2004/02/skos/core#altLabel> "Lexicon Development"@en .


###  http://w3id.org/meta-share/omtd-share/LexiconEnhancement
:LexiconEnhancement rdf:type owl:Class ;
                    rdfs:subClassOf :KnowledgeAcquisition ,
                                    :SupportOperationForKnowledgeResources ;
                    rdfs:comment "The task/process of improving (e.g. increasing the size of entries, improving the information, adding new types of information, etc.) a lexicon"@en ;
                    rdfs:label "Lexicon enhancement"@en .


###  http://w3id.org/meta-share/omtd-share/LexiconExtractionFromLexica
:LexiconExtractionFromLexica rdf:type owl:Class ;
                             rdfs:subClassOf :KnowledgeAcquisition ,
                                             :SupportOperationForKnowledgeResources ;
                             rdfs:comment "The task/process of constructing lexical resources based on the restructuring of lexical information contained in lexica (e.g. by parsing definitions or using syntactic information attached to lemmas)"@en ;
                             rdfs:label "Lexicon extraction from lexica"@en .


###  http://w3id.org/meta-share/omtd-share/LexiconExtractorFromCorpora
:LexiconExtractorFromCorpora rdf:type owl:Class ;
                             rdfs:subClassOf :Analyzer ,
                                             [ rdf:type owl:Restriction ;
                                               owl:onProperty :performsOperation ;
                                               owl:someValuesFrom :LexiconAcquisitionFromCorpora
                                             ] ;
                             rdfs:comment "A component that extracts lexical information from corpora in order to produce structured lexical resources"@en ;
                             rdfs:label "Lexicon extractor from corpora"@en .


###  http://w3id.org/meta-share/omtd-share/LexiconExtractorFromLexica
:LexiconExtractorFromLexica rdf:type owl:Class ;
                            rdfs:subClassOf :Analyzer ,
                                            [ rdf:type owl:Restriction ;
                                              owl:onProperty :performsOperation ;
                                              owl:someValuesFrom :LexiconExtractionFromLexica
                                            ] ;
                            rdfs:comment "A component that extracts specific lexical information contained in other lexica"@en ;
                            rdfs:label "Lexicon extractor from lexica"@en .


###  http://w3id.org/meta-share/omtd-share/LexiconFormatConversion
:LexiconFormatConversion rdf:type owl:Class ;
                         rdfs:subClassOf :FormatConversion ,
                                         :SupportOperationForKnowledgeResources ;
                         rdfs:comment "The task/process of converting the format of a lexical/conceptual resource into another (e.g. from TSV to XML)"@en ;
                         rdfs:label "Lexicon format conversion"@en .


###  http://w3id.org/meta-share/omtd-share/LexiconMerging
:LexiconMerging rdf:type owl:Class ;
                rdfs:subClassOf :SupportOperationForKnowledgeResources ;
                rdfs:comment "The task/process of merging (combining together) information coming from various lexical/conceptual resources"@en ;
                rdfs:label "Lexicon merging"@en .


###  http://w3id.org/meta-share/omtd-share/LexiconViewer
:LexiconViewer rdf:type owl:Class ;
               rdfs:subClassOf :Viewer ,
                               [ rdf:type owl:Restriction ;
                                 owl:onProperty :performsOperation ;
                                 owl:someValuesFrom :LexiconViewing
                               ] ;
               rdfs:comment "A component that supports humans in accessing the contents of a lexical/conceptual resource"@en ;
               rdfs:label "Lexicon viewer"@en .


###  http://w3id.org/meta-share/omtd-share/LexiconViewing
:LexiconViewing rdf:type owl:Class ;
                rdfs:subClassOf :SupportOperationForKnowledgeResources ,
                                :Viewing ;
                rdfs:comment "The task/process of viewing the contents of a lexicon as performed by human beings"@en ;
                rdfs:label "Lexicon viewing"@en .


###  http://w3id.org/meta-share/omtd-share/LexiconVisualization
:LexiconVisualization rdf:type owl:Class ;
                      rdfs:subClassOf :SupportOperationForKnowledgeResources ,
                                      :Visualization ;
                      rdfs:comment "The task/process of visualizing information (e.g. using diagrams, 3-d images, word clouds etc.) contained in lexical/conceptual resources"@en ;
                      rdfs:label "Lexicon visualization"@en ;
                      <http://www.w3.org/2004/02/skos/core#altLabel> "Lexicon visualisation"@en-uk .


###  http://w3id.org/meta-share/omtd-share/LifeSciences
:LifeSciences rdf:type owl:Class ;
              rdfs:subClassOf :Domain ;
              rdfs:comment "A branch of science (such as biology, medicine, and sometimes anthropology or sociology) that deals with living organisms and life processes usually used in plural"@en ;
              rdfs:label "Life sciences"@en .


###  http://w3id.org/meta-share/omtd-share/LinguisticAnalysis
:LinguisticAnalysis rdf:type owl:Class ;
                    rdfs:subClassOf :SupportOperation ;
                    rdfs:comment "Any operation that aims at the analysis of language or its structure"@en ;
                    rdfs:label "Linguistic analysis"@en ;
                    <http://www.w3.org/2004/02/skos/core#altLabel> "Language Analysis"@en ,
                                                                   "Language Analysis and Understanding"@en ,
                                                                   "Linguistic research"@en .


###  http://w3id.org/meta-share/omtd-share/LinguisticEntity
:LinguisticEntity rdf:type owl:Class ;
                  rdfs:subClassOf :Domain-specificAnnotation ,
                                  :DomainSpecificAnnotationType ;
                  rdfs:comment "Any kind of annotation pertaining to entities of linguistics; the use of OLIA is recommended"@en ;
                  rdfs:label "Linguistic entity"@en .


###  http://w3id.org/meta-share/omtd-share/LinkedDataFormat
:LinkedDataFormat rdf:type owl:Class ;
                  rdfs:subClassOf :DataFormat ;
                  rdfs:comment "Formats used for linked data"@en ;
                  rdfs:label "Linked data format"@en .


###  http://w3id.org/meta-share/omtd-share/LipTrackingAnalysis
:LipTrackingAnalysis rdf:type owl:Class ;
                     rdfs:subClassOf :SpeechRecognition ;
                     rdfs:comment "The task/process of recognising the lip contour and tracking the movements of lips in lip reading"@en ;
                     rdfs:label "Lip tracking analysis"@en .


###  http://w3id.org/meta-share/omtd-share/Lll
:Lll rdf:type owl:Class ;
     rdfs:subClassOf :AnnotationFormat ,
                     [ rdf:type owl:Restriction ;
                       owl:onProperty :documentationUrl ;
                       owl:hasValue "https://builds.openminted.eu/job/WP%205.2%20-%20Typesystem%20alignment/eu.openminted.interop$mapping-conversion/doclinks/1/components.html#_lll_1"
                     ] ;
     rdfs:comment "Format of the LLL challenge"@en ;
     rdfs:label "LLL"@en .


###  http://w3id.org/meta-share/omtd-share/Localization
:Localization rdf:type owl:Class ;
              rdfs:subClassOf :Translation ;
              rdfs:comment "The process of adapting a product or content to a specific locale or market, including translation of relevant language material but also converting to local measures and currency units, modifications necessary to adapt to cultural differences of the target audience, etc. [adapted from https://www.gala-global.org/industry/intro-language-industry/what-localization]"@en ;
              rdfs:label "Localization"@en ;
              <http://www.w3.org/2004/02/skos/core#altLabel> "Localisation"@en-uk ;
              <http://www.w3.org/2004/02/skos/core#definition> "" .


###  http://w3id.org/meta-share/omtd-share/Location
:Location rdf:type owl:Class ;
          rdfs:subClassOf :NamedEntity ,
                          [ rdf:type owl:Restriction ;
                            owl:onProperty :documentationUrl ;
                            owl:hasValue "http://dkpro.github.io/dkpro-core/releases/1.8.0/docs/typesystem-reference.html#de.tudarmstadt.ukp.dkpro.core.api.ner.type.Location"
                          ] ;
          rdfs:comment "A word or group of words that denotes a geographical entity"@en ;
          rdfs:label "Location"@en .


###  http://w3id.org/meta-share/omtd-share/MachineAndStatisticalLearningMethod
:MachineAndStatisticalLearningMethod rdf:type owl:Class ;
                                     rdfs:subClassOf :TdmMethod ;
                                     rdfs:comment "Methods and techniques used either in machine learning or statistical learning"@en ;
                                     rdfs:label "Machine and Statistical Learning Method"@en .


###  http://w3id.org/meta-share/omtd-share/MachineLearningMethod
:MachineLearningMethod rdf:type owl:Class ;
                       rdfs:subClassOf :TdmMethod ;
                       <http://purl.org/dc/elements/1.1/source> "adapted from https://www.sas.com/en_us/insights/analytics/machine-learning.html"@en ;
                       rdfs:comment "A method of data analysis that automates model building. Using algorithms that iteratively learn from data, machine learning allows computers to find hidden insights without being explicitly programmed where to look."@en ;
                       rdfs:label "Machine Learning Method"@en .


###  http://w3id.org/meta-share/omtd-share/MachineLearningPredictor
:MachineLearningPredictor rdf:type owl:Class ;
                          rdfs:subClassOf :SupportComponent ,
                                          [ rdf:type owl:Restriction ;
                                            owl:onProperty :performsOperation ;
                                            owl:someValuesFrom :Prediction
                                          ] ;
                          rdfs:comment "A component that is used in predicting based on machine learning models"@en ;
                          rdfs:label "Machine Learning predictor"@en ;
                          <http://www.w3.org/2004/02/skos/core#comment> "maybe create another class for predictors, analytics"@en .


###  http://w3id.org/meta-share/omtd-share/MachineTranslation
:MachineTranslation rdf:type owl:Class ;
                    rdfs:subClassOf :Translation ;
                    rdfs:comment "The automatic translation of a text from one language into another performed by software without human involvement"@en ;
                    rdfs:label "Machine Translation"@en ;
                    <http://www.w3.org/2004/02/skos/core#altLabel> "Automated Translation"@en ,
                                                                   "Automatic Translation"@en ,
                                                                   "Computer Translation"@en ,
                                                                   "MT"@en ;
                    <http://www.w3.org/2004/02/skos/core#definition> "Machine Translation (MT) is the fully automatic translation from one human language into another one. Machine translation has been worked on since the 1950s. There are a number of commercial products available and in daily use, but there are still open research problems. Tranfer-based MT has a set of transfer rules for each language pair, so that n*(n-1) rule sets are necessary for MT between n languages. In contract, interlingua-based MT uses a language-independent representation into which all source languages are analysed and from which all target languages is generated. Most practically usable MT systems are tranfser-based. Recently, there have been interestinv developments in statistical MT algorithms which are trained on parallel corpora of translated texts, and are very useful for constructing MT systems for new language pairs."@en .


###  http://w3id.org/meta-share/omtd-share/MachineTranslationSupport
:MachineTranslationSupport rdf:type owl:Class ;
                           rdfs:subClassOf :MachineTranslation ,
                                           :SupportOperation ;
                           rdfs:comment "Any operation that can be used for training or support of Machine Translation tools"@en ;
                           rdfs:label "Machine translation support"@en .


###  http://w3id.org/meta-share/omtd-share/MalletLdaTopicProportions
:MalletLdaTopicProportions rdf:type owl:Class ;
                           rdfs:subClassOf :AnnotationFormat ,
                                           [ rdf:type owl:Restriction ;
                                             owl:onProperty :documentationUrl ;
                                             owl:hasValue "http://dkpro.github.io/dkpro-core/releases/1.8.0/docs/format-reference.html#format-MalletTopicProportions"
                                           ] ,
                                           [ rdf:type owl:Restriction ;
                                             owl:onProperty :documentationUrl ;
                                             owl:hasValue "https://dkpro.github.io/dkpro-core/releases/1.8.0/docs/format-reference.html#format-de.tudarmstadt.ukp.dkpro.core.mallet-asl"
                                           ] ;
                           rdfs:comment "Topic proportions in the shape [\\t]\\t\\t..."@en ;
                           rdfs:label "Mallet LDA Topic Proportions"@en .


###  http://w3id.org/meta-share/omtd-share/MalletLdaTopicProportionsSorted
:MalletLdaTopicProportionsSorted rdf:type owl:Class ;
                                 rdfs:subClassOf :AnnotationFormat ,
                                                 [ rdf:type owl:Restriction ;
                                                   owl:onProperty :documentationUrl ;
                                                   owl:hasValue "https://dkpro.github.io/dkpro-core/releases/1.8.0/docs/format-reference.html#format-MalletTopicsProportionsSorted"
                                                 ] ;
                                 rdfs:comment "Topic proportions in the shape [\\t]\\t\\t... sorted"@en ;
                                 rdfs:label "Mallet LDA Topic Proportions Sorted"@en .


###  http://w3id.org/meta-share/omtd-share/ManagementOfAnnotations
:ManagementOfAnnotations rdf:type owl:Class ;
                         rdfs:subClassOf :CorpusManagement ;
                         rdfs:comment "The task/process of managing (manually or (semi-)automatically) annotated texts, distributing them among annotators and monitoring their work"@en ;
                         rdfs:label "Management of annotations"@en ;
                         <http://www.w3.org/2004/02/skos/core#altLabel> "Management of annotated texts"@en ,
                                                                        "Monitoring of annotated texts"@en ,
                                                                        "Monitoring of annotations"@en .


###  http://w3id.org/meta-share/omtd-share/Marker
:Marker rdf:type owl:Class ;
        rdfs:subClassOf :AgriculturalEntity ;
        rdfs:comment "Marker"@en ;
        rdfs:label "Marker"@en .


###  http://w3id.org/meta-share/omtd-share/Matcher
:Matcher rdf:type owl:Class ;
         rdfs:subClassOf :SupportComponent ,
                         [ rdf:type owl:Restriction ;
                           owl:onProperty :performsOperation ;
                           owl:someValuesFrom :Matching
                         ] ;
         rdfs:comment "A component that allows matching of elements"@en ;
         rdfs:label "Matcher"@en .


###  http://w3id.org/meta-share/omtd-share/Matching
:Matching rdf:type owl:Class ;
          rdfs:subClassOf :SupportOperation ;
          rdfs:comment "The task/performance of identifying similar elements in two resources"@en ;
          rdfs:label "Matching"@en .


###  http://w3id.org/meta-share/omtd-share/Media
:Media rdf:type owl:Class ;
       rdfs:subClassOf :NamedEntity ,
                       :SocialSciencesEntity ;
       rdfs:comment "The main means of mass communication (broadcasting, publishing, and the Internet) regarded collectively [https://en.oxforddictionaries.com/definition/media]"@en ;
       rdfs:label "Media"@en .


###  http://w3id.org/meta-share/omtd-share/MediaWikiMarkup
:MediaWikiMarkup rdf:type owl:Class ;
                 rdfs:subClassOf :WikiFormat ,
                                 :WikiFormats ,
                                 [ rdf:type owl:Restriction ;
                                   owl:onProperty :documentationUrl ;
                                   owl:hasValue "https://www.mediawiki.org/wiki/Help:Formatting"
                                 ] ;
                 rdfs:comment "Wiki markup for formatting"@en ;
                 rdfs:label "Media Wiki markup"@en .


###  http://w3id.org/meta-share/omtd-share/Metabolite
:Metabolite rdf:type owl:Class ;
            rdfs:subClassOf :BiologicalEnity ,
                            :NamedEntity ;
            rdfs:comment "Any substance involved in metabolism (= the chemical processes in the body needed for life) [https://dictionary.cambridge.org/dictionary/english/metabolite]"@en ;
            rdfs:label "Metabolite"@en .


###  http://w3id.org/meta-share/omtd-share/MethodOfResearch
:MethodOfResearch rdf:type owl:Class ;
                  rdfs:subClassOf :NamedEntity ,
                                  :SocialSciencesEntity ;
                  rdfs:altLabel "Research method"@en ;
                  rdfs:comment "Method of research"@en ;
                  rdfs:label "Method of research"@en .


###  http://w3id.org/meta-share/omtd-share/Mimetype
:Mimetype rdf:type owl:Class ;
          rdfs:subClassOf owl:Thing ;
          rdfs:comment "The IANA mimetype that can be used for the data format; it can be the exact or a broader mimetype; unofficial mimetypes are also used, but this will be revisited"@en ;
          rdfs:label "Mimetype"@en .


###  http://w3id.org/meta-share/omtd-share/Miscellaneous
:Miscellaneous rdf:type owl:Class ;
               rdfs:subClassOf :NamedEntity ;
               rdfs:altLabel "MISC"@en ;
               rdfs:comment "A general label for named entities other than the usual ones recognized by a system"@en ;
               rdfs:label "Miscellaneous"@en .


###  http://w3id.org/meta-share/omtd-share/ModelOrganism_species
:ModelOrganism_species rdf:type owl:Class ;
                       rdfs:subClassOf :BiologicalEnity ,
                                       :NamedEntity ;
                       rdfs:comment "Model organism/species"@en ;
                       rdfs:label "Model organism/species"@en .


###  http://w3id.org/meta-share/omtd-share/MorphologicalAnalysis
:MorphologicalAnalysis rdf:type owl:Class ;
                       rdfs:subClassOf :LinguisticAnalysis ;
                       rdfs:comment "The analysis of the structure of words and their relations to other words as regards their form and derivation"@en ;
                       rdfs:label "Morphological analysis"@en ;
                       <http://www.w3.org/2004/02/skos/core#altLabel> "General morphological analyisis"@en ;
                       <http://www.w3.org/2004/02/skos/core#definition> "The technologies for or the process of tracing the inflectional, derivational, and compounding processes in the formation of a given word in order to determine properties such as stem form, part-of-speech and inflectional information. As a crucial preprocessing step, morphological analysis is used in virtually all fields of natural language processing."@en .


###  http://w3id.org/meta-share/omtd-share/MorphologicalAnnotation
:MorphologicalAnnotation rdf:type owl:Class ;
                         rdfs:subClassOf :TextAnnotation ;
                         rdfs:comment "The task/process of adding annotations pertaining to the morphological level of analysis (e.g. gender, number, person etc.)"@en ;
                         rdfs:label "Morphological annotation"@en .


###  http://w3id.org/meta-share/omtd-share/MorphologicalAnnotationType
:MorphologicalAnnotationType rdf:type owl:Class ;
                             rdfs:subClassOf :AnnotationType ;
                             rdfs:comment "Any type of annotation pertaining to the morphological level"@en ;
                             rdfs:label "Morphological annotation type"@en .


###  http://w3id.org/meta-share/omtd-share/MorphologicalFeature
:MorphologicalFeature rdf:type owl:Class ;
                      rdfs:subClassOf :MorphologicalAnnotationType ,
                                      [ rdf:type owl:Restriction ;
                                        owl:onProperty owl:equivalentClass ;
                                        owl:someValuesFrom <http://purl.org/olia/olia-top.owl#MorphosyntacticFeature>
                                      ] ,
                                      [ rdf:type owl:Restriction ;
                                        owl:onProperty :documentationUrl ;
                                        owl:hasValue "http://dkpro.github.io/dkpro-core/releases/1.8.0/docs/typesystem-reference.html#de.tudarmstadt.ukp.dkpro.core.api.lexmorph.type.morph.MorphologicalFeatures"
                                      ] ;
                      rdfs:comment "Property of a word that is expressed in its inflected form; examples include person, tense, gender, case etc."@en ;
                      rdfs:label "Morphological feature"@en ;
                      <http://www.w3.org/2004/02/skos/core#altLabel> "Grammatical category"@en ,
                                                                     "Grammatical feature"@en ,
                                                                     "Morphosyntactic feature"@en .


###  http://w3id.org/meta-share/omtd-share/MorphologicalTagger
:MorphologicalTagger rdf:type owl:Class ;
                     rdfs:subClassOf :Annotator ,
                                     [ rdf:type owl:Restriction ;
                                       owl:onProperty :performsOperation ;
                                       owl:someValuesFrom :MorphologicalAnnotation
                                     ] ;
                     rdfs:comment "A component that annotates tokens of a text with morphological information (part-of-speech and morphological features)"@en ;
                     rdfs:label "Morphological tagger"@en .


###  http://w3id.org/meta-share/omtd-share/MorphosyntacticTagging
:MorphosyntacticTagging rdf:type owl:Class ;
                        rdfs:subClassOf :TextAnnotation ;
                        rdfs:comment "The task/process of adding morphosyntactic tags to words in a text, i.e. part-of-speech and, optionally, morphological features per part-of-speech."@en ;
                        rdfs:label "Morphosyntactic tagging"@en ;
                        <http://www.w3.org/2004/02/skos/core#altLabel> "Morphosyntactic annotation"@en .


###  http://w3id.org/meta-share/omtd-share/MsAccessDatabase
:MsAccessDatabase rdf:type owl:Class ;
                  rdfs:subClassOf :DatabaseFormat ,
                                  [ rdf:type owl:Restriction ;
                                    owl:onProperty :hasMimetype ;
                                    owl:hasValue :application_vnd_msaccess
                                  ] ,
                                  [ rdf:type owl:Restriction ;
                                    owl:onProperty :hasMimetype ;
                                    owl:hasValue :application_xMsaccess
                                  ] ,
                                  [ rdf:type owl:Restriction ;
                                    owl:onProperty :hasFileExtension ;
                                    owl:hasValue "mdb"
                                  ] ;
                  rdfs:comment "Data format for Microsoft Access database"@en ;
                  rdfs:label "MS-Access database"@en .


###  http://w3id.org/meta-share/omtd-share/MsExcel
:MsExcel rdf:type owl:Class ;
         rdfs:subClassOf :AnnotationFormat ,
                         :DocumentFormat ,
                         :TabularFormat ,
                         [ rdf:type owl:Restriction ;
                           owl:onProperty :hasMimetype ;
                           owl:hasValue :application_vnd_msExcel
                         ] ;
         rdfs:comment "Data format for Microsoft Excel documents"@en ;
         rdfs:label "MS-Excel"@en .


###  http://w3id.org/meta-share/omtd-share/MsPowerpoint
:MsPowerpoint rdf:type owl:Class ;
              rdfs:subClassOf :DocumentFormat ,
                              [ rdf:type owl:Restriction ;
                                owl:onProperty :hasMimetype ;
                                owl:hasValue :application_vnd_ms_powerpoint
                              ] ;
              rdfs:comment "Data format for Microsoft Powerpoint files" ;
              rdfs:label "MS-Powerpoint" .


###  http://w3id.org/meta-share/omtd-share/MsWord
:MsWord rdf:type owl:Class ;
        rdfs:subClassOf :DocumentFormat ,
                        [ rdf:type owl:Restriction ;
                          owl:onProperty :hasMimetype ;
                          owl:hasValue :application_msword
                        ] ,
                        [ rdf:type owl:Restriction ;
                          owl:onProperty :hasFileExtension ;
                          owl:hasValue "doc"
                        ] ;
        rdfs:comment "Data format for Microsoft Word documents"@en ;
        rdfs:label "MS-Word"@en .


###  http://w3id.org/meta-share/omtd-share/MultiWordUnit
:MultiWordUnit rdf:type owl:Class ;
               rdfs:subClassOf :StructuralAnnotationType ;
               rdfs:comment "A combination of words that are considered as forming one semantic unit"@en ;
               rdfs:label "Multi-word unit"@en .


###  http://w3id.org/meta-share/omtd-share/MultilingualGeneration
:MultilingualGeneration rdf:type owl:Class ;
                        rdfs:subClassOf :NaturalLanguageGeneration ;
                        rdfs:comment "The task/process of generating content in multiple languages"@en ;
                        rdfs:label "Multilingual generation"@en ;
                        <http://www.w3.org/2004/02/skos/core#definition> "Multilingual generation is the verbalization of a non-linguistic semantic representation in different human languages. The language of choice is usually a parameter to a multilingual generation system. A typical instance of multilingual generation is found in interlingual machine translation, when multiple target languages are involved. Other instances include report generation systems for multiple languages (such as Temsis-Gen) and grammar-based realizers (such as FUF/SURGE)."@en .


###  http://w3id.org/meta-share/omtd-share/MultilingualInformationRetrieval
:MultilingualInformationRetrieval rdf:type owl:Class ;
                                  rdfs:subClassOf :InformationRetrieval ;
                                  rdfs:label "Multilingual Information Retrieval"@en ;
                                  <http://www.w3.org/2004/02/skos/core#altLabel> "MIR"@en ;
                                  <http://www.w3.org/2004/02/skos/core#definition> "Cross-language information retrieval means using queries in one language to search for documents in a different language. Multilingual information retrieval is a broader term, which includes the case where queries in different languages are used, but only for searching documents in the same language."@en ;
                                  <http://www.w3.org/2004/02/skos/core#related> :CrossLingualSearch .


###  http://w3id.org/meta-share/omtd-share/MultimediaAnnotation
:MultimediaAnnotation rdf:type owl:Class ;
                      rdfs:subClassOf :Annotation ;
                      rdfs:label "Multimedia annotation"@en .


###  http://w3id.org/meta-share/omtd-share/MultimediaDevelopment
:MultimediaDevelopment rdf:type owl:Class ;
                       rdfs:subClassOf :OperationWithMultimediaInputOrOutput ;
                       rdfs:label "Multimedia development"@en .


###  http://w3id.org/meta-share/omtd-share/MultimediaDocumentProcessing
:MultimediaDocumentProcessing rdf:type owl:Class ;
                              rdfs:subClassOf :OperationWithMultimediaInputOrOutput ;
                              rdfs:label "Multimedia document processing"@en .


###  http://w3id.org/meta-share/omtd-share/MultimediaInformationExtraction
:MultimediaInformationExtraction rdf:type owl:Class ;
                                 rdfs:subClassOf :InformationExtraction ;
                                 rdfs:comment "The process/task of automatically extracting structured information from multimedia data"@en ;
                                 rdfs:label "Multimedia Information Extraction"@en ;
                                 <http://www.w3.org/2004/02/skos/core#definition> "Multimedia Information Extraction can be considered as an extension of textual information extraction to multimedia documents, in an integrated view."@en .


###  http://w3id.org/meta-share/omtd-share/MultimediaRetrieval
:MultimediaRetrieval rdf:type owl:Class ;
                     rdfs:subClassOf :InformationRetrieval ;
                     rdfs:comment "The activity of obtaining multimedia information resources relevant to an information need from a collection of multimedia information resources"@en ;
                     rdfs:label "Multimedia Retrieval"@en ;
                     <http://www.w3.org/2004/02/skos/core#altLabel> "MMIR"@en ,
                                                                    "MR"@en ,
                                                                    "Multimedia Information Retrieval"@en ,
                                                                    "Multimedia Mining"@en ;
                     <http://www.w3.org/2004/02/skos/core#definition> "The research on multimedia retrieval focuses on the development of tools and techniques to support the easy access to information in digital archives. It exploits the synergy that exists between language & speech technology, image processing and database technology. The results can be used in innovative applications that support various content management tasks, e.g. automatic indexing of large text collections and disclosure of audiovisual archives, search technology and filtering of dynamic information streams. (taken from: http://parlevink.cs.utwente.nl/?page=onderwerp&onderwerpID=2"@en .


###  http://w3id.org/meta-share/omtd-share/MultimodalIntegration
:MultimodalIntegration rdf:type owl:Class ;
                       rdfs:subClassOf :OperationWithMultimediaInputOrOutput ;
                       rdfs:comment "The study of how information from the different sensory modalities, such as sight, sound, touch, smell, self-motion and taste, may be integrated by the nervous system. [from Wikipedia]"@en ;
                       rdfs:label "Multimodal integration"@en ;
                       <http://www.w3.org/2004/02/skos/core#altLabel> "Modality integration"@en ,
                                                                      "Multisensory integration"@en ;
                       <http://www.w3.org/2004/02/skos/core#definition> "Multimodal fusion combines the output of speech understanding, gestures and mimic recognition (if available) to an uniform representation of the user intention."@en .


###  http://w3id.org/meta-share/omtd-share/Naf
:Naf rdf:type owl:Class ;
     rdfs:subClassOf :AnnotationFormat ,
                     [ rdf:type owl:Restriction ;
                       owl:onProperty :documentationUrl ;
                       owl:hasValue "http://wordpress.let.vupr.nl/naf/"
                     ] ,
                     [ rdf:type owl:Restriction ;
                       owl:onProperty :documentationUrl ;
                       owl:hasValue "https://github.com/newsreader/NAF"
                     ] ;
     rdfs:comment "The NAF format is linguistic annotation format designed for complex NLP pipelines. NAF combines strengths of the Linguistic Annotation Framework (LAF) as described in Ide et al. (2003) and the NLP Interchange Format (Hellman et al. 2013, NIF)."@en ;
     rdfs:label "NAF"@en ;
     <http://www.w3.org/2004/02/skos/core#altLabel> "NLP Annotation Format"@en .


###  http://w3id.org/meta-share/omtd-share/NamedEntitityRecognizer
:NamedEntitityRecognizer rdf:type owl:Class ;
                         rdfs:subClassOf :Annotator ,
                                         [ rdf:type owl:Restriction ;
                                           owl:onProperty :performsOperation ;
                                           owl:someValuesFrom :NamedEntityRecognition
                                         ] ;
                         rdfs:comment "A component that seeks to locate and classify elements in a text into pre-defined categories such as the names of persons, organizations, locations, expressions of times, discipline-specific classes, etc"@en ;
                         rdfs:label "Named entitity recognizer"@en .


###  http://w3id.org/meta-share/omtd-share/NamedEntity
:NamedEntity rdf:type owl:Class ;
             rdfs:subClassOf :SemanticAnnotationType ;
             rdfs:comment "A word or phrase referring to an entity, identified and annotated as such with a name (label); examples include organizations, persons, places etc."@en ;
             rdfs:label "Named entity"@en .


###  http://w3id.org/meta-share/omtd-share/NamedEntityDisambiguation
:NamedEntityDisambiguation rdf:type owl:Class ;
                           rdfs:subClassOf :NamedEntityRecognition ;
                           rdfs:comment "The task/process of selecting among candidate entities from a knowledge base (or other information resource) the ones to which the named entities in a text refer to"@en ;
                           rdfs:label "Named Entity Disambiguation"@en ;
                           <http://www.w3.org/2004/02/skos/core#altLabel> "NED"@en .


###  http://w3id.org/meta-share/omtd-share/NamedEntityRecognition
:NamedEntityRecognition rdf:type owl:Class ;
                        rdfs:subClassOf :InformationExtraction ;
                        rdfs:comment "A subtask of information extraction that seeks to locate and classify named entities in text into pre-defined categories such as the names of persons, organizations, locations, expressions of times, quantities, monetary values, percentages, etc."@en ;
                        rdfs:label "Named Entity Recognition"@en ;
                        <http://www.w3.org/2004/02/skos/core#altLabel> "NER"@en ,
                                                                       "NERC"@en ,
                                                                       "Entity Extraction" ,
                                                                       "Entity Identification" ;
                        <http://www.w3.org/2004/02/skos/core#comment> "can also be annotation"@en ;
                        <http://www.w3.org/2004/02/skos/core#definition> "Named entity (NE) recognition is a form of information extraction in which the major task is to identify and classify from NL text every word or sequence of words as being a person-name, organizaton, location, date, time, monetary value, percentage expression. NE recognition has a high impact for a number of applications, like e.g., InterNet search engines, text data mining or answer extraction."@en .


###  http://w3id.org/meta-share/omtd-share/NaturalLanguageGeneration
:NaturalLanguageGeneration rdf:type owl:Class ;
                           rdfs:subClassOf :Operation ;
                           rdfs:comment "The task/process of generating natural language text from some non-linguistic representation of information."@en ;
                           rdfs:label "Natural Language Generation"@en ;
                           <http://www.w3.org/2004/02/skos/core#altLabel> "Generation"@en ,
                                                                          "NLG"@en ,
                                                                          "Synthesis"@en ;
                           <http://www.w3.org/2004/02/skos/core#definition> "Natural Language Generation (NLG) is concerned with turning some usually non-linguistic representation of information and intended effect into fluent text preserving both meaning and intention. NLG systems often identify the content to be verbalized. They structure the document into interrelated sentence-sized chunks, choose appropriate words, aggregate and elide information to ensure fluency, create contextually appropriate referring expressions, such as pronouns, and follow grammatical constraints of the chosen language. All this is achieved using knowledge about the world and the domain of dicsourse, about communication and about languages. NLG components are used for e.g. automatic report generation, document authoring, dialogue, concept-to-speech, multi-modal and machine translation systems. Evaluating the correctness and the appropriateness of generated text is a research theme on its own since there is usually no single correct solution. One important way to tackle the problem consists in creating reference corpora and performing shared evaluation tasks, e.g. on generating referring expressions. However, this is not intended to replace less formal evaluation strategies such as human assessments."@en .


###  http://w3id.org/meta-share/omtd-share/NaturalLanguageUnderstanding
:NaturalLanguageUnderstanding rdf:type owl:Class ;
                              rdfs:subClassOf :InformationExtraction ;
                              rdfs:comment "The comprehension by computers of the structure and meaning of human languages, allowing users to interact with the computer using natural sentences. [adapted from https://www.gartner.com/it-glossary/nlu-natural-language-understanding]"@en ;
                              rdfs:label "Natural Language Understanding"@en ;
                              <http://www.w3.org/2004/02/skos/core#altLabel> "LU"@en ,
                                                                             "Language Understanding"@en ,
                                                                             "Machine Understanding"@en ,
                                                                             "NLU"@en ,
                                                                             "Natural Language Understanding"@en ;
                              <http://www.w3.org/2004/02/skos/core#definition> "" .


###  http://w3id.org/meta-share/omtd-share/NegationDetection
:NegationDetection rdf:type owl:Class ;
                   rdfs:subClassOf :InformationExtraction ;
                   rdfs:comment "The task/process of identifying negative cues (words, phrases) in a text"@en ;
                   rdfs:label "Negation detection"@en .


###  http://w3id.org/meta-share/omtd-share/NegraExport
:NegraExport rdf:type owl:Class ;
             rdfs:subClassOf :AnnotationFormat ,
                             [ rdf:type owl:Restriction ;
                               owl:onProperty :hasMimetype ;
                               owl:hasValue :application_x_org_dkpro_negra3
                             ] ,
                             [ rdf:type owl:Restriction ;
                               owl:onProperty :hasMimetype ;
                               owl:hasValue :application_x_org_dkpro_negra4
                             ] ,
                             [ rdf:type owl:Restriction ;
                               owl:onProperty :documentationUrl ;
                               owl:hasValue "http://www.coli.uni-saarland.de/~thorsten/publications/Brants-CLAUS98.pdf"
                             ] ;
             rdfs:comment "Export format for annotated corpora in the NeGra project"@en ;
             rdfs:label "NeGra export"@en .


###  http://w3id.org/meta-share/omtd-share/Neuron
:Neuron rdf:type owl:Class ;
        rdfs:subClassOf :BiologicalEnity ,
                        :NamedEntity ;
        rdfs:comment "A nerve cell that carries information between the brain and other parts of the body"@en ;
        rdfs:label "Neuron"@en .


###  http://w3id.org/meta-share/omtd-share/NeuroscienceEntity
:NeuroscienceEntity rdf:type owl:Class ;
                    rdfs:subClassOf :Domain-specificAnnotation ,
                                    :DomainSpecificAnnotationType ;
                    rdfs:comment "Any kind of annotation pertaining to entities of neuroscience"@en ;
                    rdfs:label "Neuroscience entity"@en .


###  http://w3id.org/meta-share/omtd-share/NewsGeneration
:NewsGeneration rdf:type owl:Class ;
                rdfs:subClassOf :NaturalLanguageGeneration ;
                rdfs:label "News generation"@en .


###  http://w3id.org/meta-share/omtd-share/Nif
:Nif rdf:type owl:Class ;
     rdfs:subClassOf :AnnotationFormat ,
                     :CorpusFormat ,
                     :RdfFormat ,
                     :RdfFormats ,
                     [ rdf:type owl:Restriction ;
                       owl:onProperty :documentationUrl ;
                       owl:hasValue "http://persistence.uni-leipzig.org/nlp2rdf/"
                     ] ;
     rdfs:comment "The NLP Interchange Format (NIF) is an RDF/OWL-based format that aims to achieve interoperability between Natural Language Processing (NLP) tools, language resources and annotations; it consists of specifications, ontologies and software (overview), which are combined under the version identifier \"NIF 2.0\", but are versioned individually"@en ;
     rdfs:label "NIF"@en ;
     <http://www.w3.org/2004/02/skos/core#altLabel> "NLP Interchage Format"@en .


###  http://w3id.org/meta-share/omtd-share/NlpDevelopmentSupport
:NlpDevelopmentSupport rdf:type owl:Class ;
                       rdfs:subClassOf :SupportOperation ;
                       rdfs:label "NLP Development Support"@en ;
                       <http://www.w3.org/2004/02/skos/core#altLabel> "NLP Development Aid"@en ;
                       <http://www.w3.org/2004/02/skos/core#definition> "" .


###  http://w3id.org/meta-share/omtd-share/Normalization
:Normalization rdf:type owl:Class ;
               rdfs:subClassOf :SupportOperation ;
               rdfs:comment "The task/process of editing a text in order to remove unwanted material (e.g. quotation marks, hyphenations etc.) or to substitute/represent specific items (tokens, dates,  etc.) with normalized values"@en ;
               rdfs:label "Normalization"@en .


###  http://w3id.org/meta-share/omtd-share/NormalizationOfMeasurements
:NormalizationOfMeasurements rdf:type owl:Class ;
                             rdfs:subClassOf :Normalization ;
                             rdfs:comment "The task/process of substituting measurements with normalized values"@en ;
                             rdfs:label "Normalization of measurements"@en .


###  http://w3id.org/meta-share/omtd-share/NormalizationOfNumbers
:NormalizationOfNumbers rdf:type owl:Class ;
                        rdfs:subClassOf :Normalization ;
                        rdfs:comment "The task/process of substituting numbers with normalized values"@en ;
                        rdfs:label "Normalization of numbers"@en .


###  http://w3id.org/meta-share/omtd-share/Normalizer
:Normalizer rdf:type owl:Class ;
            rdfs:subClassOf :PreOrPostProcessor ,
                            [ rdf:type owl:Restriction ;
                              owl:onProperty :performsOperation ;
                              owl:someValuesFrom :Normalization
                            ] ;
            rdfs:comment "A component that removes unwanted material from text (e.g. quotation marks, hyphenations etc.) or performs edits so that specific items (tokens, dates,  etc.) are substituted/represented with normalized values"@en ;
            rdfs:label "Normalizer"@en .


###  http://w3id.org/meta-share/omtd-share/NounPhraseChunking
:NounPhraseChunking rdf:type owl:Class ;
                    rdfs:subClassOf :Chunking ;
                    rdfs:comment "The task/process of identifying noun phrases in a sentence"@en ;
                    rdfs:label "Noun phrase chunking"@en .


###  http://w3id.org/meta-share/omtd-share/OasisPresentation
:OasisPresentation rdf:type owl:Class ;
                   rdfs:subClassOf :DocumentFormat ,
                                   :OpenFormat ,
                                   [ rdf:type owl:Restriction ;
                                     owl:onProperty :hasMimetype ;
                                     owl:hasValue :application_vnd_oasis_opendocument_presentation
                                   ] ;
                   rdfs:label "Oasis Presentation" .


###  http://w3id.org/meta-share/omtd-share/OasisSpreadsheet
:OasisSpreadsheet rdf:type owl:Class ;
                  rdfs:subClassOf :DocumentFormat ,
                                  :OpenFormat ,
                                  :TabularFormat ,
                                  [ rdf:type owl:Restriction ;
                                    owl:onProperty :hasMimetype ;
                                    owl:hasValue :application_vnd_oasis_opendocument_spreadsheet
                                  ] ;
                  rdfs:label "Oasis spreadsheet" .


###  http://w3id.org/meta-share/omtd-share/OasisText
:OasisText rdf:type owl:Class ;
           rdfs:subClassOf :DocumentFormat ,
                           :OpenFormat ,
                           [ rdf:type owl:Restriction ;
                             owl:onProperty :hasMimetype ;
                             owl:hasValue :application_vnd_oasis_opendocument_text
                           ] ;
           rdfs:label "Oasis text" .


###  http://w3id.org/meta-share/omtd-share/Obo
:Obo rdf:type owl:Class ;
     rdfs:subClassOf :RdfFormat ,
                     :RdfFormats ,
                     [ rdf:type owl:Restriction ;
                       owl:onProperty :documentationUrl ;
                       owl:hasValue "http://owlcollab.github.io/oboformat/doc/obo-syntax.html"
                     ] ;
     rdfs:comment "Serialization format for ontologies according to the Open Biomedical Ontologies model."@en ;
     rdfs:label "OBO"@en .


###  http://w3id.org/meta-share/omtd-share/OfficialText
:OfficialText rdf:type owl:Class ;
              rdfs:subClassOf :NamedEntity ,
                              :SocialSciencesEntity ;
              rdfs:comment "Official text"@en ;
              rdfs:label "Official text"@en .


###  http://w3id.org/meta-share/omtd-share/OntologyAcquisition
:OntologyAcquisition rdf:type owl:Class ;
                     rdfs:subClassOf :KnowledgeAcquisition ;
                     rdfs:comment "The task/process of creating an ontology based on other resources (corpora, other lexical resources, etc.)"@en ;
                     rdfs:label "Ontology acquisition"@en .


###  http://w3id.org/meta-share/omtd-share/OntologyEnhancement
:OntologyEnhancement rdf:type owl:Class ;
                     rdfs:subClassOf :KnowledgeAcquisition ;
                     rdfs:comment "The task/process of improving an ontology, typically by adding new relations or entities"@en ;
                     rdfs:label "Ontology enhancement"@en .


###  http://w3id.org/meta-share/omtd-share/OpenFormat
:OpenFormat rdf:type owl:Class ;
            rdfs:subClassOf :DataFormat ;
            rdfs:label "Open format" .


###  http://w3id.org/meta-share/omtd-share/OpenOfficeDocument
:OpenOfficeDocument rdf:type owl:Class ;
                    rdfs:subClassOf :DocumentFormat ,
                                    :OpenFormat ,
                                    :Xml ,
                                    [ rdf:type owl:Restriction ;
                                      owl:onProperty :hasMimetype ;
                                      owl:hasValue :application_vnd_openxmlformats_officedocument_wordprocessingml_document
                                    ] ;
                    rdfs:label "Open office document" .


###  http://w3id.org/meta-share/omtd-share/OpenOfficePresentation
:OpenOfficePresentation rdf:type owl:Class ;
                        rdfs:subClassOf :DocumentFormat ,
                                        :OpenFormat ,
                                        :Xml ,
                                        [ rdf:type owl:Restriction ;
                                          owl:onProperty :hasMimetype ;
                                          owl:hasValue :application_vnd_openxmlformats_officedocument_presentationml_presentation
                                        ] ;
                        rdfs:label "Open office presentation" .


###  http://w3id.org/meta-share/omtd-share/OpenOfficeSpreadsheet
:OpenOfficeSpreadsheet rdf:type owl:Class ;
                       rdfs:subClassOf :DocumentFormat ,
                                       :OpenFormat ,
                                       :TabularFormat ,
                                       :Xml ,
                                       [ rdf:type owl:Restriction ;
                                         owl:onProperty :hasMimetype ;
                                         owl:hasValue :application_vnd_openxmlformats_officedocument_spreadsheetml_sheet
                                       ] ;
                       rdfs:label "Open office spreadsheet" .


###  http://w3id.org/meta-share/omtd-share/Operation
:Operation rdf:type owl:Class ;
           rdfs:subClassOf owl:Thing ;
           rdfs:comment "The action that a software program performs or is meant to perform"@en ;
           rdfs:label "Operation"@en ;
           <http://www.w3.org/2004/02/skos/core#altLabel> "Function"@en ,
                                                          "Task"@en .


###  http://w3id.org/meta-share/omtd-share/OperationWithMultimediaInputOrOutput
:OperationWithMultimediaInputOrOutput rdf:type owl:Class ;
                                      rdfs:subClassOf :Operation ;
                                      rdfs:label "Operation with multimedia input or output"@en .


###  http://w3id.org/meta-share/omtd-share/OptimalCharacterRecognition
:OptimalCharacterRecognition rdf:type owl:Class ;
                             rdfs:subClassOf :SupportOperation ;
                             rdfs:comment "The task/process of converting handwritten or printed material into machine editable text"@en ;
                             rdfs:label "Optical Character Recognition"@en ;
                             <http://www.w3.org/2004/02/skos/core#altLabel> "OCR"@en .


###  http://w3id.org/meta-share/omtd-share/Organism
:Organism rdf:type owl:Class ;
          rdfs:subClassOf :AgriculturalEntity ;
          rdfs:comment "An individual animal, plant, or single-celled life form [https://en.oxforddictionaries.com/definition/organism]"@en ;
          rdfs:label "Organism"@en .


###  http://w3id.org/meta-share/omtd-share/Organization
:Organization rdf:type owl:Class ;
              rdfs:subClassOf :NamedEntity ,
                              [ rdf:type owl:Restriction ;
                                owl:onProperty :documentationUrl ;
                                owl:hasValue "http://dkpro.github.io/dkpro-core/releases/1.8.0/docs/typesystem-reference.html#de.tudarmstadt.ukp.dkpro.core.api.ner.type.Organization"
                              ] ;
              rdfs:comment "A word or group of words that denotes an organization, such as company, association, institution etc."@en ;
              rdfs:label "Organization"@en .


###  http://w3id.org/meta-share/omtd-share/OrthographicTranscription
:OrthographicTranscription rdf:type owl:Class ;
                           rdfs:subClassOf :Transcription ;
                           rdfs:comment "The task/process of transcribing a source language word/phrase or an audio segment into the standard spelling system of a target language"@en ;
                           rdfs:label "Orthographic transcription"@en .


###  http://w3id.org/meta-share/omtd-share/Owl
:Owl rdf:type owl:Class ;
     rdfs:subClassOf :RdfFormat ,
                     :RdfFormats ;
     rdfs:comment "Superclass for formats used for OWL"@en ;
     rdfs:label "OWL"@en .


###  http://w3id.org/meta-share/omtd-share/Owl_xml
:Owl_xml rdf:type owl:Class ;
         rdfs:subClassOf :Owl ,
                         :Xml ,
                         [ rdf:type owl:Restriction ;
                           owl:onProperty :hasMimetype ;
                           owl:hasValue :application_xml
                         ] ;
         rdfs:comment "XML format for OWL ontologies"@en ;
         rdfs:label "OWL/XML"@en .


###  http://w3id.org/meta-share/omtd-share/Paragraph
:Paragraph rdf:type owl:Class ;
           rdfs:subClassOf :StructuralAnnotationType ,
                           [ rdf:type owl:Restriction ;
                             owl:onProperty owl:equivalentClass ;
                             owl:someValuesFrom <http://vocab.lappsgrid.org/Paragraph>
                           ] ;
           rdfs:comment "A division of a text, usually about a single theme, consisting of one or more sentences and marked by a new line, indentation or other conventions."@en ;
           rdfs:label "Paragraph"@en .


###  http://w3id.org/meta-share/omtd-share/ParagraphSplitting
:ParagraphSplitting rdf:type owl:Class ;
                    rdfs:subClassOf :StructuralAnnotation ;
                    rdfs:comment "The task/process of segmenting a text into paragraphs and marking their boundaries"@en ;
                    rdfs:label "Paragraph splitting"@en ;
                    <http://www.w3.org/2004/02/skos/core#altLabel> "Paragraph segmentation"@en .


###  http://w3id.org/meta-share/omtd-share/ParalanguageAnnotation
:ParalanguageAnnotation rdf:type owl:Class ;
                        rdfs:subClassOf :SpeechAnnotation ;
                        rdfs:comment "The task/process of annotating paralinguistic features, i.e. vocal features that accompany speech and contribute to communication but are not generally considered to be part of the language system (e.g. vocal quality, loudness, and tempo); facial expressions and gestures are also considered as paralinguistic features [adapted from https://www.dictionary.com/browse/paralanguage]"@en ;
                        rdfs:label "Paralanguage annotation"@en .


###  http://w3id.org/meta-share/omtd-share/ParallelSentenceExtraction
:ParallelSentenceExtraction rdf:type owl:Class ;
                            rdfs:subClassOf :MachineTranslationSupport ;
                            rdfs:comment "The task/process of identifying parallel sentences (i.e. sentences that have the same sense in different languages) in parallel texts"@en ;
                            rdfs:label "Parallel sentence extraction"@en .


###  http://w3id.org/meta-share/omtd-share/Paraphrasing
:Paraphrasing rdf:type owl:Class ;
              rdfs:subClassOf :SupportOperation ;
              rdfs:comment "A task/process whereby a text fragment is reproduced with another text fragment that conveys the same or similar information"@en ;
              rdfs:label "Paraphrasing"@en .


###  http://w3id.org/meta-share/omtd-share/Parser
:Parser rdf:type owl:Class ;
        rdfs:subClassOf :Annotator ;
        rdfs:comment "A component that takes as input text and returns a form of data structure (e.g. syntactic parse as a tree, or bracketed structure etc.)"@en ;
        rdfs:label "Parser"@en ;
        <http://www.w3.org/2004/02/skos/core#altLabel> "Syntactic analyzer"@en .


###  http://w3id.org/meta-share/omtd-share/Parsing
:Parsing rdf:type owl:Class ;
         rdfs:subClassOf :LinguisticAnalysis ,
                         :TextAnnotation ;
         rdfs:comment "The task/process of recognizing and marking the syntactic structure of a text or text segment"@en ;
         rdfs:label "Parsing"@en ;
         <http://www.w3.org/2004/02/skos/core#altLabel> "Syntactic analysis"@en ,
                                                        "Syntactic annotation"@en ,
                                                        "Syntactic parsing"@en ,
                                                        "Syntactic processing"@en ;
         <http://www.w3.org/2004/02/skos/core#definition> "Parsing (=syntactic analysis) of natural language utterances is still an active reasearch topic due to the inherent difficulties that make the problem much harder than e.g. parsing of programming languages. These difficulties include lexical and structural ambiguity of natural language utterances, complexities introduced by expressive grammar formalisms, the need to cope with illformed input or with deficiencies of the linguistic descriptions."@en .


###  http://w3id.org/meta-share/omtd-share/PartOfSpeech
:PartOfSpeech rdf:type owl:Class ;
              rdfs:subClassOf :AnnotationType ,
                              [ rdf:type owl:Restriction ;
                                owl:onProperty owl:equivalentClass ;
                                owl:someValuesFrom <http://purl.org/olia/olia-top.owl#MorphosyntacticCategory>
                              ] ,
                              [ rdf:type owl:Restriction ;
                                owl:onProperty :documentationUrl ;
                                owl:hasValue "http://dkpro.github.io/dkpro-core/releases/1.8.0/docs/typesystem-reference.html#de.tudarmstadt.ukp.dkpro.core.api.lexmorph.type.pos.POS"
                              ] ;
              rdfs:comment "A division of words based on common grammatical features"@en ;
              rdfs:label "Part of Speech"@en ;
              <http://www.w3.org/2004/02/skos/core#altLabel> "Grammatical category"@en ,
                                                             "Morphosyntactic category"@en ,
                                                             "Word category"@en .


###  http://w3id.org/meta-share/omtd-share/PartOfSpeechTagger
:PartOfSpeechTagger rdf:type owl:Class ;
                    rdfs:subClassOf :MorphologicalTagger ;
                    rdfs:comment "A component that annotates tokens of a text with part-of-speech information"@en ;
                    rdfs:label "Part of speech tagger"@en ;
                    <http://www.w3.org/2004/02/skos/core#altLabel> "PoS tagger"@en .


###  http://w3id.org/meta-share/omtd-share/Pdf
:Pdf rdf:type owl:Class ;
     rdfs:subClassOf :BinaryFormat ,
                     :DocumentFormat ,
                     [ rdf:type owl:Restriction ;
                       owl:onProperty :hasMimetype ;
                       owl:hasValue :application_pdf
                     ] ,
                     [ rdf:type owl:Restriction ;
                       owl:onProperty :hasFileExtension ;
                       owl:hasValue "pdf"
                     ] ;
     rdfs:comment "Data format for PDF files (Portable Document Format)"@en ;
     rdfs:label "PDF"@en .


###  http://w3id.org/meta-share/omtd-share/Person
:Person rdf:type owl:Class ;
        rdfs:subClassOf :NamedEntity ,
                        [ rdf:type owl:Restriction ;
                          owl:onProperty :documentationUrl ;
                          owl:hasValue "http://dkpro.github.io/dkpro-core/releases/1.8.0/docs/typesystem-reference.html#de.tudarmstadt.ukp.dkpro.core.api.ner.type.Person"
                        ] ;
        rdfs:comment "A word or group of words that refers to a person"@en ;
        rdfs:label "Person"@en .


###  http://w3id.org/meta-share/omtd-share/PersonIdentification
:PersonIdentification rdf:type owl:Class ;
                      rdfs:subClassOf :OperationWithMultimediaInputOrOutput ;
                      rdfs:comment "A process that identifies an individual uniquely by using unique personal identification number (PIN) and/or biometrics like fingerprint, face recognition etc."@en ;
                      rdfs:label "Person identification"@en .


###  http://w3id.org/meta-share/omtd-share/PersuasiveExpression
:PersuasiveExpression rdf:type owl:Class ;
                      rdfs:subClassOf :SemanticAnnotationType ;
                      rdfs:comment "A word or phrase used for persuasion purposes"@en ;
                      rdfs:label "Persuasive expression"@en .


###  http://w3id.org/meta-share/omtd-share/PersuasiveExpressionMiner
:PersuasiveExpressionMiner rdf:type owl:Class ;
                           rdfs:subClassOf :Analyzer ,
                                           [ rdf:type owl:Restriction ;
                                             owl:onProperty :performsOperation ;
                                             owl:someValuesFrom :PersuasiveExpressionMining
                                           ] ;
                           rdfs:comment "A component that tries to identify persuasive expressions in a given text"@en ;
                           rdfs:label "Persuasive expression miner"@en ;
                           <http://www.w3.org/2004/02/skos/core#comment> "could also be an annotator"@en .


###  http://w3id.org/meta-share/omtd-share/PersuasiveExpressionMining
:PersuasiveExpressionMining rdf:type owl:Class ;
                            rdfs:subClassOf :InformationExtraction ;
                            rdfs:comment "The task/process of identifying and extracting (especially from political speech texts) pieces of text that aim to persuade"@en ;
                            rdfs:label "Persuasive expression mining"@en .


###  http://w3id.org/meta-share/omtd-share/Phenotype
:Phenotype rdf:type owl:Class ;
           rdfs:subClassOf :AgriculturalEntity ;
           rdfs:comment "The physical appearance or biochemical characteristic of an organism as a result of the interaction of its genotype and the environment [http://www.biology-online.org/dictionary/Phenotype]"@en ;
           rdfs:label "Phenotype"@en .


###  http://w3id.org/meta-share/omtd-share/PhoneticTranscription
:PhoneticTranscription rdf:type owl:Class ;
                       rdfs:subClassOf :Transcription ;
                       rdfs:comment "The visual representation of speech sounds (or phones)"@en ;
                       rdfs:label "Phonetic transcription"@en .


###  http://w3id.org/meta-share/omtd-share/Phrase
:Phrase rdf:type owl:Class ;
        rdfs:subClassOf :StructuralAnnotationType ,
                        [ rdf:type owl:Restriction ;
                          owl:onProperty owl:equivalentClass ;
                          owl:someValuesFrom <http://purl.org/olia/olia-top.owl#Phrase>
                        ] ;
        rdfs:comment "A phrase is a syntactic structure that consists of more than one word but lacks the subject-predicate organization of a clause. [http://www.glossary.sil.org/term/phrase]"@en ;
        rdfs:label "Phrase"@en .


###  http://w3id.org/meta-share/omtd-share/PhraseAlignment
:PhraseAlignment rdf:type owl:Class ;
                 rdfs:subClassOf :Alignment ;
                 rdfs:comment "Alignment at phrase level"@en ;
                 rdfs:label "Phrase alignment"@en .


###  http://w3id.org/meta-share/omtd-share/PhysicoChemicalProperty
:PhysicoChemicalProperty rdf:type owl:Class ;
                         rdfs:subClassOf :AgriculturalEntity ;
                         rdfs:comment "Physical and chemical property of substances"@en ;
                         rdfs:label "Physico-chemical property"@en .


###  http://w3id.org/meta-share/omtd-share/Pls
:Pls rdf:type owl:Class ;
     rdfs:subClassOf :DocumentFormat ,
                     :Xml ,
                     [ rdf:type owl:Restriction ;
                       owl:onProperty :hasMimetype ;
                       owl:hasValue :application_pls_xml
                     ] ,
                     [ rdf:type owl:Restriction ;
                       owl:onProperty :documentationUrl ;
                       owl:hasValue "https://www.iana.org/assignments/media-types/application/pls+xml"
                     ] ;
     rdfs:comment "Data format according to the Pronunciation Lexicon Specification (PLS)"@en ;
     rdfs:label "PLS"@en .


###  http://w3id.org/meta-share/omtd-share/Pml
:Pml rdf:type owl:Class ;
     rdfs:subClassOf :AnnotationFormat ,
                     :Xml ,
                     [ rdf:type owl:Restriction ;
                       owl:onProperty :hasMimetype ;
                       owl:hasValue :application_xml
                     ] ,
                     [ rdf:type owl:Restriction ;
                       owl:onProperty :documentationUrl ;
                       owl:hasValue "http://ufal.mff.cuni.cz/jazz/PML/index_en.html"
                     ] ,
                     [ rdf:type owl:Restriction ;
                       owl:onProperty :documentationUrl ;
                       owl:hasValue "https://builds.openminted.eu/job/WP%205.2%20-%20Typesystem%20alignment/eu.openminted.interop$mapping-conversion/doclinks/1/components.html#_prague_markup_language_1"
                     ] ;
     rdfs:comment "Format according to the Prague Markup Language (http://ufal.mff.cuni.cz/jazz/PML/index_en.html); PML is a generic data format based on XML intended for storing linguistically annotated data, such as the Prague Dependency Treebank, also annotation lexicons, etc."@en ;
     rdfs:label "PML"@en ;
     <http://www.w3.org/2004/02/skos/core#altLabel> "Prague Markup Language"@en .


###  http://w3id.org/meta-share/omtd-share/Polarity
:Polarity rdf:type owl:Class ;
          rdfs:subClassOf :SemanticAnnotationType ,
                          [ rdf:type owl:Restriction ;
                            owl:onProperty owl:equivalentClass ;
                            owl:someValuesFrom <http://purl.org/olia/olia-top.owl#PolarityFeature>
                          ] ;
          rdfs:comment "A feature that distinguishes between positive, negative or neutral; in sentiment analysis, it refers to determining whether the expressed opinion in a document, a sentence or an entity feature/aspect is positive, negative, or neutral. [adapted from Wikipedia]"@en ;
          rdfs:label "Polarity"@en .


###  http://w3id.org/meta-share/omtd-share/PolarityDetection
:PolarityDetection rdf:type owl:Class ;
                   rdfs:subClassOf :InformationExtraction ;
                   rdfs:label "Polarity detection"@en .


###  http://w3id.org/meta-share/omtd-share/PolarityLabelling
:PolarityLabelling rdf:type owl:Class ;
                   rdfs:subClassOf :SemanticAnnotation ;
                   rdfs:comment "The task/process of adding to units of a text (especially in sentiment-intensive texts) tags that indicate polarity (negative, positive, neutral, mixed)"@en ;
                   rdfs:label "Polarity labelling"@en .


###  http://w3id.org/meta-share/omtd-share/PosTagging
:PosTagging rdf:type owl:Class ;
            rdfs:subClassOf :MorphosyntacticTagging ;
            rdfs:comment "The task/process of marking words with the part of speech (word category, e.g. noun, verb etc.) to which they belong"@en ;
            rdfs:label "Part-of-Speech Tagging"@en ;
            <http://www.w3.org/2004/02/skos/core#altLabel> "Grammatical annotation"@en ,
                                                           "Grammatical tagging"@en ,
                                                           "PoS Tagging"@en ;
            <http://www.w3.org/2004/02/skos/core#definition> "The technologies for or the process of determining the correct part-of-speech tag for a word given its local context. The task comprises disambiguation of multiple part-of-speech tags and guessing of the correct part-of-speech tag for unknown words. Part-of-speech tagging is frequently used as a preprocessing step for shallow and deep parsers."@en .


###  http://w3id.org/meta-share/omtd-share/Postscript
:Postscript rdf:type owl:Class ;
            rdfs:subClassOf :DocumentFormat ,
                            [ rdf:type owl:Restriction ;
                              owl:onProperty :hasMimetype ;
                              owl:hasValue :application_postscript
                            ] ,
                            [ rdf:type owl:Restriction ;
                              owl:onProperty :documentationUrl ;
                              owl:hasValue "https://www.iana.org/assignments/media-types/application/postscript"
                            ] ,
                            [ rdf:type owl:Restriction ;
                              owl:onProperty :hasFileExtension ;
                              owl:hasValue "ps"
                            ] ;
            rdfs:comment "Data format for PostScript files"@en ;
            rdfs:label "postscript"@en .


###  http://w3id.org/meta-share/omtd-share/PreOrPostProcessor
:PreOrPostProcessor rdf:type owl:Class ;
                    rdfs:subClassOf :ComponentType ;
                    rdfs:comment "A component that is used at pre- or post-processing stages in order to normalize input/output"@en ;
                    rdfs:label "Pre- or Post-Processor"@en .


###  http://w3id.org/meta-share/omtd-share/Prediction
:Prediction rdf:type owl:Class ;
            rdfs:subClassOf :TextAndDataMining ;
            rdfs:comment "In Machine Learning, it refers to the use of algorithms that learn from previous data in order to make predictions on data (by estimating probabilities from previous data)"@en ;
            rdfs:label "Prediction"@en ;
            <http://www.w3.org/2004/02/skos/core#comment> "needs better definition"@en .


###  http://w3id.org/meta-share/omtd-share/Processor
:Processor rdf:type owl:Class ;
           rdfs:subClassOf :ComponentType ;
           rdfs:comment "A component that is used in processing operations"@en ;
           rdfs:label "Processor"@en .


###  http://w3id.org/meta-share/omtd-share/ProsodicAnnotation
:ProsodicAnnotation rdf:type owl:Class ;
                    rdfs:subClassOf :SpeechAnnotation ;
                    rdfs:label "Prosodic annotation"@en .


###  http://w3id.org/meta-share/omtd-share/ProsodicInformationProcessing
:ProsodicInformationProcessing rdf:type owl:Class ;
                               rdfs:subClassOf :InformationExtraction ;
                               rdfs:label "Prosodic information processing"@en ;
                               <http://www.w3.org/2004/02/skos/core#altLabel> "Prosody information processing"@en ;
                               <http://www.w3.org/2004/02/skos/core#definition> "Prosody can be defined as a feature of speech which extends over more than one segment and is often synonymous with 'suprasegmentals'. Prosodic features include fundamental frequency (F0),relative duration and intensity, and spectral quality. They determine the rhythm and intonation of utterances."@en .


###  http://w3id.org/meta-share/omtd-share/ProsodicSegmentation
:ProsodicSegmentation rdf:type owl:Class ;
                      rdfs:subClassOf :ProsodicAnnotation ;
                      rdfs:label "Prosodic segmentation"@en .


###  http://w3id.org/meta-share/omtd-share/Protein
:Protein rdf:type owl:Class ;
         rdfs:subClassOf :BiologicalEnity ,
                         :NamedEntity ;
         rdfs:comment "Any of various naturally occurring extremely complex substances that consist of amino-acid residues joined by peptide bonds, contain the elements carbon, hydrogen, nitrogen, oxygen, usually sulfur, and occasionally other elements (such as phosphorus or iron), and include many essential biological compounds (such as enzymes, hormones, or antibodies) [https://www.merriam-webster.com/dictionary/protein]"@en ;
         rdfs:label "Protein"@en .


###  http://w3id.org/meta-share/omtd-share/ProteinFamily
:ProteinFamily rdf:type owl:Class ;
               rdfs:subClassOf :AgriculturalEntity ;
               rdfs:comment "A protein family is a group of proteins that share a common evolutionary origin, reflected by their related functions and similarities in sequence or structure [https://www.ebi.ac.uk/training/online/course/introduction-protein-classification-ebi/protein-classification/what-are-protein-families]"@en ;
               rdfs:label "Protein family"@en .


###  http://w3id.org/meta-share/omtd-share/Pseudonymization
:Pseudonymization rdf:type owl:Class ;
                  rdfs:subClassOf :SupportOperation ;
                  rdfs:comment "The processing of personal data in such a way that the data can no longer be attributed to a specific data subject without the use of additional information (from GDPR)"@en ;
                  rdfs:label "Pseudonymization"@en .


###  http://w3id.org/meta-share/omtd-share/Ptb
:Ptb rdf:type owl:Class ;
     rdfs:subClassOf :AnnotationFormat ;
     rdfs:comment "Penn Tree Bank formats"@en ;
     rdfs:label "PTB"@en .


###  http://w3id.org/meta-share/omtd-share/PtbChunked
:PtbChunked rdf:type owl:Class ;
            rdfs:subClassOf :Ptb ,
                            [ rdf:type owl:Restriction ;
                              owl:onProperty :hasMimetype ;
                              owl:hasValue :text_x_org_dkpro_ptbChunked
                            ] ,
                            [ rdf:type owl:Restriction ;
                              owl:onProperty :documentationUrl ;
                              owl:hasValue "https://zoidberg.ukp.informatik.tu-darmstadt.de/jenkins/job/DKPro%20Core%20Documentation%20(GitHub)/de.tudarmstadt.ukp.dkpro.core$de.tudarmstadt.ukp.dkpro.core.doc-asl/doclinks/5/format-reference.html#format-PennTreebankChunked"
                            ] ;
            rdfs:comment "Penn Treebank chunked format"@en ;
            rdfs:label "PTB-chunked"@en ;
            <http://www.w3.org/2004/02/skos/core#altLabel> "Penn Treebank - chunked"@en ,
                                                           "ptb; format-variant=chunked"@en .


###  http://w3id.org/meta-share/omtd-share/PtbCombined
:PtbCombined rdf:type owl:Class ;
             rdfs:subClassOf :Ptb ,
                             [ rdf:type owl:Restriction ;
                               owl:onProperty :hasMimetype ;
                               owl:hasValue :text_x_org_dkpro_ptbCombined
                             ] ,
                             [ rdf:type owl:Restriction ;
                               owl:onProperty :documentationUrl ;
                               owl:hasValue "https://dkpro.github.io/dkpro-core/releases/1.8.0/docs/format-reference.html#format-PennTreebankCombined"
                             ] ;
             rdfs:comment "Penn Treebank combined format"@en ;
             rdfs:label "PTB-combined"@en ;
             <http://www.w3.org/2004/02/skos/core#altLabel> "Penn Treebank - combined"@en ,
                                                            "ptb; format-variant=combined"@en .


###  http://w3id.org/meta-share/omtd-share/Pubmed
:Pubmed rdf:type owl:Class ;
        rdfs:subClassOf :DocumentFormat ,
                        [ rdf:type owl:Restriction ;
                          owl:onProperty :hasMimetype ;
                          owl:hasValue :text_xPubmed
                        ] ,
                        [ rdf:type owl:Restriction ;
                          owl:onProperty :documentationUrl ;
                          owl:hasValue "https://gate.ac.uk/sale/tao/splitch23.html#sec:creole:pubmed"
                        ] ;
        rdfs:comment "Textual format used for PubMed articles"@en ;
        rdfs:label "PubMed"@en .


###  http://w3id.org/meta-share/omtd-share/QuestionAnswering
:QuestionAnswering rdf:type owl:Class ;
                   rdfs:subClassOf :InformationExtraction ,
                                   :KnowledgeDiscovery ;
                   rdfs:comment "The task/process where computer systems try to automatically answer questions posed by users in the form of natural language."@en ;
                   rdfs:label "Answer Extraction"@en ;
                   <http://www.w3.org/2004/02/skos/core#altLabel> "AE"@en ,
                                                                  "QA"@en ,
                                                                  "Question Answering"@en ,
                                                                  "Textual Question Answering"@en ;
                   <http://www.w3.org/2004/02/skos/core#definition> "Answer extraction (AE) aims at retrieving those exact passages of a document that directly answer a given user question. AE is more ambitious than information retrieval and information extraction in that the retrieval results are short phrases, not entire documents, and in that the queries may be arbitrarily specific. It is less ambitious than full-fledged question answering in that the answers are not generated from a knowledge base but looked up in the text of documents." .


###  http://w3id.org/meta-share/omtd-share/QuestionTopicalTarget
:QuestionTopicalTarget rdf:type owl:Class ;
                       rdfs:subClassOf :SemanticAnnotationType ;
                       rdfs:comment "The segment of a question that describes the entity about which the question is made"@en ;
                       rdfs:label "Question Topical Target"@en ;
                       <http://www.w3.org/2004/02/skos/core#altLabel> "QTT"@en ,
                                                                      "Question topic"@en .


###  http://w3id.org/meta-share/omtd-share/RdfFormat
:RdfFormat rdf:type owl:Class ;
           rdfs:subClassOf :DataFormat ;
           <http://purl.org/dc/terms/replaces> :RdfFormats ;
           rdfs:comment "Formats for RDF (Resource Description Framework) resources"@en ;
           rdfs:label "RDF format"@en .


###  http://w3id.org/meta-share/omtd-share/RdfFormats
:RdfFormats rdf:type owl:Class ;
            rdfs:subClassOf :DataFormat ;
            rdfs:comment "Formats for RDF (Resource Description Framework) resources"@en ;
            rdfs:label "RDF formats"@en ;
            owl:deprecated "true"^^xsd:boolean .


###  http://w3id.org/meta-share/omtd-share/Rdf_xml
:Rdf_xml rdf:type owl:Class ;
         rdfs:subClassOf :RdfFormat ,
                         :RdfFormats ,
                         :Xml ,
                         [ rdf:type owl:Restriction ;
                           owl:onProperty :hasMimetype ;
                           owl:hasValue :application_rdf_xml
                         ] ,
                         [ rdf:type owl:Restriction ;
                           owl:onProperty :documentationUrl ;
                           owl:hasValue "https://www.w3.org/TR/REC-rdf-syntax/"
                         ] ;
         rdfs:comment "Data format for RDF (Resource Description Framework) XML format; RDF/XML is a serialisation for RDF"@en ;
         rdfs:label "RDF/XML"@en .


###  http://w3id.org/meta-share/omtd-share/Readability
:Readability rdf:type owl:Class ;
             rdfs:subClassOf :SemanticAnnotationType ,
                             [ rdf:type owl:Restriction ;
                               owl:onProperty :documentationUrl ;
                               owl:hasValue "http://dkpro.github.io/dkpro-core/releases/1.8.0/docs/typesystem-reference.html#de.tudarmstadt.ukp.dkpro.core.type.ReadabilityScore"
                             ] ;
             rdfs:comment "The ease with which a reader can understand a written text. [https://en.wikipedia.org/wiki/Readability]"@en ;
             rdfs:label "Readability"@en .


###  http://w3id.org/meta-share/omtd-share/ReadabilityAnnotation
:ReadabilityAnnotation rdf:type owl:Class ;
                       rdfs:subClassOf :SemanticAnnotation ;
                       rdfs:comment "The process/task of adding readability scores (or any other type of similar annotation) to a text or textual segment showing how easy it is to read and understand its meaning."@en ;
                       rdfs:label "Readability annotation"@en .


###  http://w3id.org/meta-share/omtd-share/ReadabilityAnnotator
:ReadabilityAnnotator rdf:type owl:Class ;
                      rdfs:subClassOf :SemanticAnnotator ;
                      rdfs:comment "A component that annotates the tokens of a text with readability scores"@en ;
                      rdfs:label "Readability annotator"@en .


###  http://w3id.org/meta-share/omtd-share/Reader
:Reader rdf:type owl:Class ;
        rdfs:subClassOf :AccessComponent ,
                        [ rdf:type owl:Restriction ;
                          owl:onProperty :performsOperation ;
                          owl:someValuesFrom :Reading
                        ] ;
        rdfs:comment "A component that reads content of various types (pdf, txt, xml etc.)"@en ;
        rdfs:label "Reader"@en .


###  http://w3id.org/meta-share/omtd-share/Reading
:Reading rdf:type owl:Class ;
         rdfs:subClassOf :ResourceAccess ;
         rdfs:comment "Getting access to the contents of an input resource"@en ;
         rdfs:label "Reading"@en .


###  http://w3id.org/meta-share/omtd-share/RecognizingTextualEntailment
:RecognizingTextualEntailment rdf:type owl:Class ;
                              rdfs:subClassOf :InformationExtraction ,
                                              :KnowledgeDiscovery ;
                              rdfs:comment "A task/process that intends to recognize for two text fragments whether the meaning of one text is entailed in that of the other, i.e. whether the truth of one text fragment follows from that of the other fragment."@en ;
                              rdfs:label "Recognizing Textual Entailment"@en .


###  http://w3id.org/meta-share/omtd-share/RegressionAnalysis
:RegressionAnalysis rdf:type owl:Class ;
                    rdfs:subClassOf :MachineAndStatisticalLearningMethod ;
                    <http://purl.org/dc/elements/1.1/source> "Wikipedia (https://en.wikipedia.org/wiki/Regression_analysis)"@en ;
                    rdfs:comment "A statistical process for estimating the relationships among variables. It includes many techniques for modeling and analyzing several variables, when the focus is on the relationship between a dependent variable and one or more independent variables (or 'predictors')."@en ;
                    rdfs:label "Regression Analysis"@en .


###  http://w3id.org/meta-share/omtd-share/Regularisation
:Regularisation rdf:type owl:Class ;
                rdfs:subClassOf :MachineAndStatisticalLearningMethod ;
                <http://purl.org/dc/elements/1.1/source> "adapted from Wikipedia (https://en.wikipedia.org/wiki/Regularization_(mathematics))"@en ;
                rdfs:comment "A process of introducing additional information in order to solve an ill-posed problem or to prevent overfitting."@en ;
                rdfs:label "Regularisation"@en ;
                <http://www.w3.org/2004/02/skos/core#altLabel> "Regularization"@en .


###  http://w3id.org/meta-share/omtd-share/Relation
:Relation rdf:type owl:Class ;
          rdfs:subClassOf :Domain-specificAnnotation ,
                          :DomainSpecificAnnotationType ;
          rdfs:comment "Any type of relation that holds between two or more entities of a specific domain"@en ;
          rdfs:label "Relation"@en .


###  http://w3id.org/meta-share/omtd-share/RelationExtraction
:RelationExtraction rdf:type owl:Class ;
                    rdfs:subClassOf :InformationExtraction ;
                    rdfs:comment "The process/task of identifying and classifying relation mentions between entities in text and/or data."@en ;
                    rdfs:label "Relation Extraction"@en ;
                    <http://www.w3.org/2004/02/skos/core#altLabel> "Relationship Extraction"@en ;
                    <http://www.w3.org/2004/02/skos/core#comment> "can also be annotation"@en ;
                    <http://www.w3.org/2004/02/skos/core#definition> "Automated or human-assisted acquisition of relations between concepts from textual or other data, usu. within a selected domain."@en .


###  http://w3id.org/meta-share/omtd-share/RepresentationOfSpaceAndTime
:RepresentationOfSpaceAndTime rdf:type owl:Class ;
                              rdfs:subClassOf :InformationExtraction ;
                              rdfs:label "Representation of space and time"@en ;
                              <http://www.w3.org/2004/02/skos/core#definition> "The representation of time and space plays a crucial role in Artificial Intelligence and Computational Linguistics, but also in practical areas such as business intelligence or geographical information systems. Representing time and space properly eases querying and reasoning thereof. <br /> <br /> Geographic information systems use traditional techniques from image processing and CAD, like a pixel/raster or a vector representation of spatial data. Temporal data bases extend tradional relational data models by the notion of <i>valid time</i> and <i>transaction time</i>. <br /> <br /> When we speak of time, we mean a linear, dense, and one-dimensional time. With space, we usually refer to a two- or three-dimensional space, often using a latitude/longitude measurement in degrees in case of a spherical 2D geometry or a system of coordinates/trajectories for a Euclidean 2D/3D space. Classical observable spacetime then refers to a 3+1-dimensional continuum in which physical objects move through time and space (Tegmark 1997). Even abstract events or processes can be seen to take place in 4D spacetime. Physical and abstract 4D entities are usually composed of simpler entities -- here, both time and space are the glue to achieve a decomposition. For instance, Allen (1984) has defined a natural system of 13 temporal topological relations. Randell et al. (1992) came up with a logic (later called RCC) to support qualitative reasoning about space. <br /> <br /> Human natural language usually comes up with means to refer to time and space, for instance through the use of temporal and spatial prepositions, adverbs, or verb tense and aspect (Vendler 1967, Moens &amp; Steedman 1988, Herskovits 1986). Several algorithms exist which compute the temporal structure of a discourse (e.g., Hitzeman et al. 1995). When constructing mental models of space derived from text, it has been shown that the representation is more topological than Euclidean (Langston et al. 1998). <br /> <br /> Within theoretical and computational linguistics, type-logical semantics and categorial grammar have given a rigorous account to tense, aspect, and temporal modification through the use of a possible-worlds semantics (see, e.g., Carpenter 1997). <br /> <br /> Studying time from a formal perspective, focussing on the inherent properties of a theory, has a long tradition in logic (e.g., Hayes 1995), artificial intelligence (e.g., McDermott 1982), description logics (e.g., Bry &amp; Spranger 2003, Lutz 2004), or data base theory (Date et al. 2002). <br /> <br /> Looking from a more practical viewpoint on time, a number of frameworks have been proposed within the World Wide Web Consortium W3C: (i) ISO 8601 is an international standard for date and time representations issued by the International Organization for Standardization (Wolf &amp; Wicksteed 1998); (ii) XSD (XML Schema Datatypes) comes up with a number of built-in primitive datatype for time and date (Peterson et al. 2008); (iii) OWL-Time (formerly DAML-Time; see Hobbs &amp; Pan 2004) is an OWL ontology of temporal concepts and properties for describing the temporal content of Web pages and the temporal properties of Web services. <br /> <br /> Representing changing relationships over time and space is related to the problem of diachronic identity which describes the identification of individuals that look different at different times, but still refer to the same entity. The four-dimensional or perdurantist view assumes that all entities (the perdurants) only exist for some period of time. Entities under this view are sometimes refered to as <i>spacetime worms</i> (Sider 2001), since a 4D trajectory is all one needs to identify/follow a perdurant through time and space. Parts of such a worm are called <i>time slices</i>, encoding cooccurent information that stay constant over the specified period of time. There exist several well-known techniques of extending a relation with time and space: (i) equip the relation with further arguments as is done in temporal data bases; (ii) apply a meta-logical predicate (McCarthy &amp; Hayes 1969); (iii) reifiy the original relation as used in RDF (Manola &amp; Miller 2004). Unfortunately, (i) and (ii) are not applicable to OWL (Smith et al. 2004), whereas (iii) requires ontology rewriting. Welty &amp; Fikes (2006) and Krieger et al. (2008) present alternative approaches compatible with OWL."@en .


###  http://w3id.org/meta-share/omtd-share/ResourceAccess
:ResourceAccess rdf:type owl:Class ;
                rdfs:subClassOf :SupportOperation ;
                rdfs:comment "Any operation that enables accessing a resource"@en ;
                rdfs:label "Resource access"@en .


###  http://w3id.org/meta-share/omtd-share/Reuters21578Sgml
:Reuters21578Sgml rdf:type owl:Class ;
                  rdfs:subClassOf :CorpusFormat ,
                                  [ rdf:type owl:Restriction ;
                                    owl:onProperty :hasMimetype ;
                                    owl:hasValue :application_x_org_dkpro_reuters21578_sgml
                                  ] ,
                                  [ rdf:type owl:Restriction ;
                                    owl:onProperty :documentationUrl ;
                                    owl:hasValue "https://dkpro.github.io/dkpro-core/releases/1.8.0/docs/format-reference.html#format-Reuters21578Sgml"
                                  ] ;
                  rdfs:comment "Reuters-21578 corpus in SGML format"@en ;
                  rdfs:label "Reuters21578 SGML"@en .


###  http://w3id.org/meta-share/omtd-share/Reuters21578Txt
:Reuters21578Txt rdf:type owl:Class ;
                 rdfs:subClassOf :CorpusFormat ,
                                 [ rdf:type owl:Restriction ;
                                   owl:onProperty :hasMimetype ;
                                   owl:hasValue :text_x_org_dkpro_reuters21578
                                 ] ,
                                 [ rdf:type owl:Restriction ;
                                   owl:onProperty :documentationUrl ;
                                   owl:hasValue "https://dkpro.github.io/dkpro-core/releases/1.8.0/docs/format-reference.html#format-Reuters21578Txt"
                                 ] ;
                 rdfs:comment "Reuters-21578 corpus transformed into text format using ExtractReuters in the lucene-benchmarks project"@en ;
                 rdfs:label "Reuters21578 Txt"@en .


###  http://w3id.org/meta-share/omtd-share/Rna
:Rna rdf:type owl:Class ;
     rdfs:subClassOf :AgriculturalEntity ;
     rdfs:altLabel "Ribonucleic acid"@en ;
     rdfs:comment "Any of various nucleic acids that contain ribose and uracil as structural components and are associated with the control of cellular chemical activities"@en ;
     rdfs:label "RNA"@en .


###  http://w3id.org/meta-share/omtd-share/Rtf
:Rtf rdf:type owl:Class ;
     rdfs:subClassOf :DocumentFormat ,
                     [ rdf:type owl:Restriction ;
                       owl:onProperty :hasMimetype ;
                       owl:hasValue :application_rtf
                     ] ,
                     [ rdf:type owl:Restriction ;
                       owl:onProperty :hasFileExtension ;
                       owl:hasValue "rtf"
                     ] ;
     rdfs:comment "Rich Text Format; proprietary data format of Microsoft"@en ;
     rdfs:label "RTF"@en .


###  http://w3id.org/meta-share/omtd-share/RuleBasedMethod
:RuleBasedMethod rdf:type owl:Class ;
                 rdfs:subClassOf :TdmMethod ;
                 rdfs:comment "A type of method that makes use of set(s) of rules to perform the relevant task."@en ;
                 rdfs:label "Rule-based Method"@en .


###  http://w3id.org/meta-share/omtd-share/RumoursStanceClassification
:RumoursStanceClassification rdf:type owl:Class ;
                             rdfs:subClassOf :InformationExtraction ;
                             rdfs:comment "The task of identifying the attitude of a person towards the truthfulness of a rumour"@en ;
                             rdfs:label "Rumours stance classification"@en .


###  http://w3id.org/meta-share/omtd-share/ScholarlyAnalyticsEntity
:ScholarlyAnalyticsEntity rdf:type owl:Class ;
                          rdfs:subClassOf :Domain-specificAnnotation ,
                                          :DomainSpecificAnnotationType ;
                          <http://purl.org/dc/terms/replaces> :ScholarlyCommunicationAnnotation ;
                          rdfs:comment "Any type of annotation that is relevant to scholarly analtyics (e.g. citations, funding information etc.)"@en ;
                          rdfs:label "Scholarly analytics entity"@en .


###  http://w3id.org/meta-share/omtd-share/ScholarlyCommunication
:ScholarlyCommunication rdf:type owl:Class ;
                        rdfs:subClassOf :Domain ;
                        rdfs:comment "Scholarly communication can be defined as the system through which research and other scholarly writings are created, evaluated for quality, disseminated to the scholarly community, and preserved for future use. The system includes both formal means of communication, such as publication in peer-reviewed journals, and informal channels, such as electronic listservs. (Association of College & Research Libraries, Principles and Strategies for the Reform of Scholarly Communication 1, 2003)"@en ;
                        rdfs:label "Scholarly communication"@en .


###  http://w3id.org/meta-share/omtd-share/ScholarlyCommunicationAnnotation
:ScholarlyCommunicationAnnotation rdf:type owl:Class ;
                                  rdfs:subClassOf :Domain-specificAnnotation ,
                                                  :DomainSpecificAnnotationType ;
                                  rdfs:comment "Any type of annotation that is relevant to scholarly analtyics (e.g. citations, funding information etc.)"@en ;
                                  rdfs:label "Scholarly analytics entity"@en ;
                                  owl:deprecated "true"^^xsd:boolean .


###  http://w3id.org/meta-share/omtd-share/ScientificUnit
:ScientificUnit rdf:type owl:Class ;
                rdfs:subClassOf :Domain-specificAnnotation ,
                                :DomainSpecificAnnotationType ,
                                :NamedEntity ;
                rdfs:comment "Scientific unit"@en ;
                rdfs:label "Scientific unit"@en .


###  http://w3id.org/meta-share/omtd-share/ScientificValue
:ScientificValue rdf:type owl:Class ;
                 rdfs:subClassOf :Domain-specificAnnotation ,
                                 :DomainSpecificAnnotationType ,
                                 :NamedEntity ;
                 rdfs:comment "Scientific value"@en ;
                 rdfs:label "Scientific value"@en .


###  http://w3id.org/meta-share/omtd-share/ScriptBasedAnalyser
:ScriptBasedAnalyser rdf:type owl:Class ;
                     rdfs:subClassOf :SupportComponent ,
                                     [ rdf:type owl:Restriction ;
                                       owl:onProperty :performsOperation ;
                                       owl:someValuesFrom :ScriptBasedAnalysis
                                     ] ;
                     rdfs:comment "A component that performs analysis tasks based on a script"@en ;
                     rdfs:label "Script-based analyser"@en .


###  http://w3id.org/meta-share/omtd-share/ScriptBasedAnalysis
:ScriptBasedAnalysis rdf:type owl:Class ;
                     rdfs:subClassOf :SupportOperation ;
                     rdfs:comment "The task/process of analysing a resource following a script"@en ;
                     rdfs:label "Script-based analysis"@en ;
                     <http://www.w3.org/2004/02/skos/core#altLabel> "Script based analysis"@en .


###  http://w3id.org/meta-share/omtd-share/Segmenter
:Segmenter rdf:type owl:Class ;
           rdfs:subClassOf :Annotator ;
           rdfs:comment "A component that segments a text into structural untis (chapters, paragraphs, sentences, words, tokens etc.)"@en ;
           rdfs:label "Segmenter"@en ;
           <http://www.w3.org/2004/02/skos/core#comment> "can also be a support tool"@en .


###  http://w3id.org/meta-share/omtd-share/SemanticAnnotation
:SemanticAnnotation rdf:type owl:Class ;
                    rdfs:subClassOf :TextAnnotation ;
                    rdfs:label "Semantic annotation"@en .


###  http://w3id.org/meta-share/omtd-share/SemanticAnnotationType
:SemanticAnnotationType rdf:type owl:Class ;
                        rdfs:subClassOf :AnnotationType ;
                        rdfs:comment "Any type of annotation pertaining to the semantic level"@en ;
                        rdfs:label "Semantic annotation type"@en .


###  http://w3id.org/meta-share/omtd-share/SemanticAnnotator
:SemanticAnnotator rdf:type owl:Class ;
                   rdfs:subClassOf :Annotator ;
                   rdfs:comment "A component that annotates the tokens of a text with semantic features"@en ;
                   rdfs:label "Semantic annotator"@en .


###  http://w3id.org/meta-share/omtd-share/SemanticClass
:SemanticClass rdf:type owl:Class ;
               rdfs:subClassOf :SemanticAnnotationType ,
                               [ rdf:type owl:Restriction ;
                                 owl:onProperty :documentationUrl ;
                                 owl:hasValue "http://dkpro.github.io/dkpro-core/releases/1.8.0/docs/typesystem-reference.html#de.tudarmstadt.ukp.dkpro.core.api.semantics.type.SemanticField"
                               ] ;
               rdfs:comment "A division of words into classes based on their common semantic features"@en ;
               rdfs:label "Semantic class"@en ;
               <http://www.w3.org/2004/02/skos/core#altLabel> "Semantic type"@en .


###  http://w3id.org/meta-share/omtd-share/SemanticClassLabelling
:SemanticClassLabelling rdf:type owl:Class ;
                        rdfs:subClassOf :SemanticAnnotation ;
                        rdfs:comment "The task/process of classifying words in a text according to a set of semantic classes (types)."@en ;
                        rdfs:label "Semantic class labelling"@en ;
                        <http://www.w3.org/2004/02/skos/core#altLabel> "Semantic class labeling [en-US]"@en-us .


###  http://w3id.org/meta-share/omtd-share/SemanticFrame
:SemanticFrame rdf:type owl:Class ;
               rdfs:subClassOf :SemanticAnnotationType ,
                               [ rdf:type owl:Restriction ;
                                 owl:onProperty owl:equivalentClass ;
                                 owl:someValuesFrom <http://purl.org/olia/olia-top.owl#Frame>
                               ] ,
                               [ rdf:type owl:Restriction ;
                                 owl:onProperty :documentationUrl ;
                                 owl:hasValue "http://dkpro.github.io/dkpro-core/releases/1.8.0/docs/typesystem-reference.html#de.tudarmstadt.ukp.dkpro.core.api.semantics.type.SemanticPredicate"
                               ] ;
               <http://purl.org/dc/elements/1.1/source> <https://framenet.icsi.berkeley.edu/fndrupal/glossary> ;
               rdfs:comment "A schematic representation of a situation involving various participants, props and other conceptual roles, each of which is a frame element"@en ;
               rdfs:label "Semantic frame"@en ;
               <http://www.w3.org/2004/02/skos/core#altLabel> "Frame"@en .


###  http://w3id.org/meta-share/omtd-share/SemanticReasoning
:SemanticReasoning rdf:type owl:Class ;
                   rdfs:subClassOf :InformationExtraction ;
                   rdfs:comment "The inferrence of logical consequences from a set of asserted facts or axioms [from wikipedia]"@en ;
                   rdfs:label "Semantic reasoning"@en .


###  http://w3id.org/meta-share/omtd-share/SemanticRelationLabelling
:SemanticRelationLabelling rdf:type owl:Class ;
                           rdfs:subClassOf :SemanticAnnotation ;
                           rdfs:comment "The task/process of attaching tags indicating the semantic relation that holds between units of a text."@en ;
                           rdfs:label "Semantic relation labelling"@en ;
                           <http://www.w3.org/2004/02/skos/core#altLabel> "Semantic relation labeling [en-US]"@en-us .


###  http://w3id.org/meta-share/omtd-share/SemanticRole
:SemanticRole rdf:type owl:Class ;
              rdfs:subClassOf :SemanticAnnotationType ,
                              [ rdf:type owl:Restriction ;
                                owl:onProperty owl:equivalentClass ;
                                owl:someValuesFrom <http://purl.org/olia/olia-top.owl#SemanticRole>
                              ] ,
                              [ rdf:type owl:Restriction ;
                                owl:onProperty owl:equivalentClass ;
                                owl:someValuesFrom <http://vocab.lappsgrid.org/SemanticRole>
                              ] ,
                              [ rdf:type owl:Restriction ;
                                owl:onProperty :documentationUrl ;
                                owl:hasValue "http://dkpro.github.io/dkpro-core/releases/1.8.0/docs/typesystem-reference.html#de.tudarmstadt.ukp.dkpro.core.api.semantics.type.SemanticArgument"
                              ] ;
              rdfs:comment "A semantic role is the underlying relationship that a participant has with the main verb in a clause [http://www.glossary.sil.org/term/semantic-role]"@en ;
              rdfs:label "Semantic role"@en .


###  http://w3id.org/meta-share/omtd-share/SemanticRoleLabelling
:SemanticRoleLabelling rdf:type owl:Class ;
                       rdfs:subClassOf :SemanticAnnotation ;
                       rdfs:comment "The task/process of attaching labels that correspond to the roles that the arguments of a predicate take in an event"@en ;
                       rdfs:label "Semantic role labelling"@en ;
                       <http://www.w3.org/2004/02/skos/core#altLabel> "Semantic role labeling [en-US]"@en-us .


###  http://w3id.org/meta-share/omtd-share/SemanticSearch
:SemanticSearch rdf:type owl:Class ;
                rdfs:subClassOf :InformationRetrieval ;
                rdfs:comment "A type of search that seeks to improve search accuracy by understanding the searcher's intent and the contextual meaning of terms as they appear in the searchable dataspace, whether on the Web or within a closed system, to generate more relevant results."@en ;
                rdfs:label "Semantic search"@en .


###  http://w3id.org/meta-share/omtd-share/Sentence
:Sentence rdf:type owl:Class ;
          rdfs:subClassOf :StructuralAnnotationType ,
                          [ rdf:type owl:Restriction ;
                            owl:onProperty owl:equivalentClass ;
                            owl:someValuesFrom <http://purl.org/olia/olia-top.owl#Sentence>
                          ] ,
                          [ rdf:type owl:Restriction ;
                            owl:onProperty :documentationUrl ;
                            owl:hasValue "http://dkpro.github.io/dkpro-core/releases/1.8.0/docs/typesystem-reference.html#de.tudarmstadt.ukp.dkpro.core.api.segmentation.type.Sentence"
                          ] ;
          rdfs:comment "A group of words, usually containing a verb, that expresses a thought in the form of a statement, question, instruction, or exclamation and starts with a capital letter when written [https://dictionary.cambridge.org/dictionary/english/sentence]"@en ;
          rdfs:label "Sentence"@en .


###  http://w3id.org/meta-share/omtd-share/SentenceAlignment
:SentenceAlignment rdf:type owl:Class ;
                   rdfs:subClassOf :Alignment ;
                   rdfs:comment "Alignment at sentence level"@en ;
                   rdfs:label "Sentence alignment"@en .


###  http://w3id.org/meta-share/omtd-share/SentenceSplitter
:SentenceSplitter rdf:type owl:Class ;
                  rdfs:subClassOf :Segmenter ;
                  rdfs:comment "A component that splits a text into sentences"@en ;
                  rdfs:label "Sentence splitter"@en .


###  http://w3id.org/meta-share/omtd-share/SentenceSplitting
:SentenceSplitting rdf:type owl:Class ;
                   rdfs:subClassOf :StructuralAnnotation ;
                   rdfs:comment "The task/process of recognizing and tagging sentence boundaries in a text"@en ;
                   rdfs:label "Sentence splitting"@en ;
                   <http://www.w3.org/2004/02/skos/core#altLabel> "Segmentation into sentences"@en ,
                                                                  "Sentence segmentation"@en .


###  http://w3id.org/meta-share/omtd-share/Sentiment
:Sentiment rdf:type owl:Class ;
           rdfs:subClassOf :SemanticAnnotationType ,
                           [ rdf:type owl:Restriction ;
                             owl:onProperty :documentationUrl ;
                             owl:hasValue "http://dkpro.github.io/dkpro-core/releases/1.8.0/docs/typesystem-reference.html#de.tudarmstadt.ukp.dkpro.core.sentiment.type.StanfordSentimentAnnotation"
                           ] ;
           rdfs:comment "The affective state (judgement, feeling) of a person or group towards an entity or event"@en ;
           rdfs:label "Sentiment"@en ;
           <http://www.w3.org/2004/02/skos/core#altLabel> "Opinion"@en .


###  http://w3id.org/meta-share/omtd-share/SentimentAnalysis
:SentimentAnalysis rdf:type owl:Class ;
                   rdfs:subClassOf :InformationExtraction ,
                                   :KnowledgeDiscovery ;
                   rdfs:comment "The process/task of computationally identifying and categorizing opinions expressed in a piece of text, especially in order to determine whether the writer's attitude towards a particular topic, product, etc. is positive, negative, or neutral"@en ;
                   rdfs:label "Sentiment analysis"@en ;
                   <http://www.w3.org/2004/02/skos/core#altLabel> "Opinion extraction"@en ,
                                                                  "Opinion mining"@en ,
                                                                  "Polarity detection"@en ,
                                                                  "Sentiment detection"@en .


###  http://w3id.org/meta-share/omtd-share/SentimentAnalyzer
:SentimentAnalyzer rdf:type owl:Class ;
                   rdfs:subClassOf :Analyzer ,
                                   [ rdf:type owl:Restriction ;
                                     owl:onProperty :performsOperation ;
                                     owl:someValuesFrom :SentimentAnalysis
                                   ] ;
                   rdfs:comment "A component that tries to identify sentences that express the authors negative or positive feelings on something"@en ;
                   rdfs:label "Sentiment analyzer"@en ;
                   <http://www.w3.org/2004/02/skos/core#altLabel> "Opinion mining tool"@en ;
                   <http://www.w3.org/2004/02/skos/core#comment> "could also be an annotator"@en .


###  http://w3id.org/meta-share/omtd-share/SerializedCas
:SerializedCas rdf:type owl:Class ;
               rdfs:subClassOf :UimaCasFormat ,
                               [ rdf:type owl:Restriction ;
                                 owl:onProperty :documentationUrl ;
                                 owl:hasValue "http://dkpro.github.io/dkpro-core/releases/1.8.0/docs/format-reference.html#format-SerializedCas"
                               ] ;
               rdfs:comment "The CAS is the native data model used by UIMA; there are various ways of saving CAS data, using XMI, XCAS, or binary formats; this is for the serialized format"@en ;
               rdfs:label "Serialized CAS"@en .


###  http://w3id.org/meta-share/omtd-share/Sgml
:Sgml rdf:type owl:Class ;
      rdfs:subClassOf :DocumentFormat ,
                      [ rdf:type owl:Restriction ;
                        owl:onProperty :hasMimetype ;
                        owl:hasValue :text_sgml
                      ] ;
      rdfs:comment "SGML format"@en ;
      rdfs:label "SGML"@en .


###  http://w3id.org/meta-share/omtd-share/SignLanguageGeneration
:SignLanguageGeneration rdf:type owl:Class ;
                        rdfs:subClassOf :NaturalLanguageGeneration ,
                                        :OperationWithMultimediaInputOrOutput ;
                        rdfs:comment "The task/process of generating videos in sign language"@en ;
                        rdfs:label "Sign language generation"@en .


###  http://w3id.org/meta-share/omtd-share/SignLanguageRecognition
:SignLanguageRecognition rdf:type owl:Class ;
                         rdfs:subClassOf :OperationWithMultimediaInputOrOutput ;
                         rdfs:comment "The task/process of recognizing from images and videos hand gestures performed in sign language"@en ;
                         rdfs:label "Sign language recognition"@en .


###  http://w3id.org/meta-share/omtd-share/Simplifier
:Simplifier rdf:type owl:Class ;
            rdfs:subClassOf :Generator ;
            rdfs:comment "A component that outputs a simpler rendition of a given item (sentence, text etc.)"@en ;
            rdfs:label "Simplifier"@en .


###  http://w3id.org/meta-share/omtd-share/SocialSciences
:SocialSciences rdf:type owl:Class ;
                rdfs:subClassOf :Domain ;
                rdfs:comment "The social sciences are academic disciplines concerned with the study of the social life of human groups and individuals including anthropology, economics, geography, history, political science, psychology, social studies, and sociology. The social sciences consist of the scientific study of the human aspects of the world.[https://en.wikipedia.org/wiki/Category:Social_sciences]"@en ;
                rdfs:label "Social sciences"@en .


###  http://w3id.org/meta-share/omtd-share/SocialSciencesEntity
:SocialSciencesEntity rdf:type owl:Class ;
                      rdfs:subClassOf :Domain-specificAnnotation ,
                                      :DomainSpecificAnnotationType ;
                      rdfs:comment "Any kind of annotation that pertains to entities of social sciences; the use of TheSoz is recommended"@en ;
                      rdfs:label "Social sciences entity"@en .


###  http://w3id.org/meta-share/omtd-share/SoftwareDevelopmentEnvironment
:SoftwareDevelopmentEnvironment rdf:type owl:Class ;
                                rdfs:subClassOf :SupportComponent ;
                                rdfs:comment "A technology that supports the development of software components and data resources required for their operation"@en ;
                                rdfs:label "Software development environment"@en .


###  http://w3id.org/meta-share/omtd-share/Solr
:Solr rdf:type owl:Class ;
      rdfs:subClassOf :DataFormat ,
                      [ rdf:type owl:Restriction ;
                        owl:onProperty :documentationUrl ;
                        owl:hasValue "https://dkpro.github.io/dkpro-core/releases/1.8.0/docs/format-reference.html#format-de.tudarmstadt.ukp.dkpro.core.io.solr-asl"
                      ] ;
      rdfs:comment "Solr format"@en ;
      rdfs:label "Solr"@en .


###  http://w3id.org/meta-share/omtd-share/SoundEventAnnotation
:SoundEventAnnotation rdf:type owl:Class ;
                      rdfs:subClassOf :SpeechAnnotation ;
                      rdfs:label "Sound event annotation"@en .


###  http://w3id.org/meta-share/omtd-share/SoundToTextAlignment
:SoundToTextAlignment rdf:type owl:Class ;
                      rdfs:subClassOf :SpeechAnnotation ;
                      rdfs:label "Sound-to-Text alignment"@en .


###  http://w3id.org/meta-share/omtd-share/SpatialRoleLabelling
:SpatialRoleLabelling rdf:type owl:Class ;
                      rdfs:subClassOf :SemanticAnnotation ;
                      rdfs:altLabel "Spatial role labeling"@en-us ;
                      rdfs:comment "he task of identifying and classifying the spatial arguments of the spatial expressions mentioned in a sentence"@en ;
                      rdfs:label "Spatial role labelling"@en .


###  http://w3id.org/meta-share/omtd-share/SpeakerDiarization
:SpeakerDiarization rdf:type owl:Class ;
                    rdfs:subClassOf :SpeechAnnotation ;
                    rdfs:comment "Partitioning of audio stream into homogeneous segments according to speaker properties and acoustic conditions"@en ;
                    rdfs:label "Speaker diarization"@en ;
                    <http://www.w3.org/2004/02/skos/core#altLabel> "Speaker diarisation"@en-uk .


###  http://w3id.org/meta-share/omtd-share/SpeakerIdentification
:SpeakerIdentification rdf:type owl:Class ;
                       rdfs:subClassOf :SpeechRecognition ;
                       rdfs:comment "The task/process of identifying/recognizing who the person speaking is"@en ;
                       rdfs:label "Speaker identification"@en ;
                       <http://www.w3.org/2004/02/skos/core#altLabel> "SR"@en ,
                                                                      "Speaker Recognition"@en ,
                                                                      "VR"@en ,
                                                                      "Voice Recognition"@en ;
                       <http://www.w3.org/2004/02/skos/core#definition> "Speaker recognition, which can be classified into identification and verification, is the process of automatically recognizing who is speaking on the basis of individual information included in speech waves. This technique makes it possible to use the speaker's voice to verify their identity and control access to services such as voice dialing, banking by telephone, telephone shopping, database access services, information services, voice mail, security control for confidential information areas, and remote access to computers."@en .


###  http://w3id.org/meta-share/omtd-share/SpeakerVerification
:SpeakerVerification rdf:type owl:Class ;
                     rdfs:subClassOf :SpeechRecognition ;
                     rdfs:comment "The task/process of verifying that a certain person is speaking"@en ;
                     rdfs:label "Speaker verification"@en .


###  http://w3id.org/meta-share/omtd-share/Species
:Species rdf:type owl:Class ;
         rdfs:subClassOf :BiologicalEnity ,
                         :NamedEntity ;
         rdfs:comment "A set of animals or plants in which the members have similar characteristics to each other and can breed with each other"@en ;
         rdfs:label "Species"@en .


###  http://w3id.org/meta-share/omtd-share/SpectralData
:SpectralData rdf:type owl:Class ;
              rdfs:subClassOf :NamedEntity ;
              rdfs:comment "Spectral data is essentially data derived by the use of spectroscopic instruments"@en ;
              rdfs:label "Spectral data"@en .


###  http://w3id.org/meta-share/omtd-share/SpeechAct
:SpeechAct rdf:type owl:Class ;
           rdfs:subClassOf :DiscourseAnnotationType ;
           rdfs:comment "A speech act is an act that a speaker performs when making an utterance, including the following: (a) A general act (illocutionary act) that a speaker performs, analyzable as including: the uttering of words (utterance acts), making reference and predicating (propositional acts), and a particular intention in making the utterance (illocutionary force). (b) An act involved in the illocutionary act, including utterance acts and propositional acts, (c) The production of a particular effect in the addressee (perlocutionary act) [http://www.glossary.sil.org/term/speech-act]"@en ;
           rdfs:label "Speech act"@en .


###  http://w3id.org/meta-share/omtd-share/SpeechAnalysis
:SpeechAnalysis rdf:type owl:Class ;
                rdfs:subClassOf :SpeechRecognition ;
                rdfs:label "Speech analysis"@en .


###  http://w3id.org/meta-share/omtd-share/SpeechAnalytics
:SpeechAnalytics rdf:type owl:Class ;
                 rdfs:subClassOf :TextSpeechDataAnalytics ;
                 rdfs:label "Speech analytics"@en .


###  http://w3id.org/meta-share/omtd-share/SpeechAnnotation
:SpeechAnnotation rdf:type owl:Class ;
                  rdfs:subClassOf :Annotation ;
                  rdfs:label "Speech annotation"@en .


###  http://w3id.org/meta-share/omtd-share/SpeechAssistedVideoControl
:SpeechAssistedVideoControl rdf:type owl:Class ;
                            rdfs:subClassOf :OperationWithMultimediaInputOrOutput ;
                            rdfs:label "Speech-assisted video control"@en .


###  http://w3id.org/meta-share/omtd-share/SpeechEnhancement
:SpeechEnhancement rdf:type owl:Class ;
                   rdfs:subClassOf :SpeechRecognition ;
                   rdfs:comment "The improvement of speech intelligibility by removing background noise from the speech signal"@en ;
                   rdfs:label "Speech Enhancement"@en ;
                   <http://www.w3.org/2004/02/skos/core#definition> "The improvement of speech intelligibility by removing background noise from the speech signal. Due to the complexity of speech acoustics and perception, no simple mathematical error criterion can be applied; instead, algorithms and measures need to be developed which accomodate human perception."@en .


###  http://w3id.org/meta-share/omtd-share/SpeechRecognition
:SpeechRecognition rdf:type owl:Class ;
                   rdfs:subClassOf :OperationWithMultimediaInputOrOutput ;
                   rdfs:comment "The use of computer hardware and software-based techniques to identify and process human voice used tused to identify the words a person has spoken or to authenticate the identity of the person speaking into the system [adapted from https://www.techopedia.com/definition/6044/automatic-speech-recognition-asr]"@en ;
                   rdfs:label "Speech Recognition"@en ;
                   <http://www.w3.org/2004/02/skos/core#altLabel> "ASR"@en ,
                                                                  "Automatic speech recognition"@en ,
                                                                  "Computer speech recognition"@en ,
                                                                  "SR"@en ,
                                                                  "Voice recognition"@en ;
                   <http://www.w3.org/2004/02/skos/core#definition> "Automatic Speech Recognition deals with automatic transcribing spoken language as text which is further processed in application dependent ways. Important applications are dictation, control of machines and devices by speech, information systems, speech translation, aids for disabled persons. An increasingly important application is embedded speech recognition in devices such as mobile phones and PDAs."@en .


###  http://w3id.org/meta-share/omtd-share/SpeechRetrieval
:SpeechRetrieval rdf:type owl:Class ;
                 rdfs:subClassOf :InformationExtraction ;
                 rdfs:label "Speech Retrieval"@en ;
                 <http://www.w3.org/2004/02/skos/core#altLabel> "SDR"@en ,
                                                                "SR"@en ,
                                                                "Spoken Document Retrieval"@en ;
                 <http://www.w3.org/2004/02/skos/core#definition> "Speech Retrieval is the process of retrieving spoken audio material (documents)in response to a search query. Search queries can be spoken or textual. Speech retrieval makes use of techniques from speech recognition, natural language understanding and information retrieval. Possible applications are the indexing of archives of broadcast material, and monitoring of telephone conversations."@en .


###  http://w3id.org/meta-share/omtd-share/SpeechSynthesis
:SpeechSynthesis rdf:type owl:Class ;
                 rdfs:subClassOf :NaturalLanguageGeneration ;
                 rdfs:label "Speech Synthesis"@en ;
                 <http://www.w3.org/2004/02/skos/core#altLabel> "Synthetic Speech Generation"@en .


###  http://w3id.org/meta-share/omtd-share/SpeechSynthesisEvaluation
:SpeechSynthesisEvaluation rdf:type owl:Class ;
                           rdfs:subClassOf :Evaluation ;
                           rdfs:label "Speech Synthesis Evaluation"@en ;
                           <http://www.w3.org/2004/02/skos/core#altLabel> "Evaluation of Speech Synthesis"@en ;
                           <http://www.w3.org/2004/02/skos/core#definition> "Evaluation of speech synthesis traditionally considers intelligibility and naturalness. More recently, expressivity has become an issue with the increasing demand for expressive voices. Due to the multitude of aspects involved, there is no agreed standard for evaluation of speech synthesis systems. Since 2005, the Blizzard Challenge is an annual joint event for comparing speech synthesis technologies with a common database."@en .


###  http://w3id.org/meta-share/omtd-share/SpeechToSpeechTranslation
:SpeechToSpeechTranslation rdf:type owl:Class ;
                           rdfs:subClassOf :Translation ;
                           rdfs:comment "The process by which spoken utterances in one language are automatically translated and spoken aloud in another language"@en ;
                           rdfs:label "Speech-to-Speech translation"@en .


###  http://w3id.org/meta-share/omtd-share/SpeechToTextTranslation
:SpeechToTextTranslation rdf:type owl:Class ;
                         rdfs:subClassOf :Translation ;
                         rdfs:label "Speech-to-Text translation"@en .


###  http://w3id.org/meta-share/omtd-share/SpeechUnderstanding
:SpeechUnderstanding rdf:type owl:Class ;
                     rdfs:subClassOf :SpeechRecognition ;
                     rdfs:label "Speech understanding"@en .


###  http://w3id.org/meta-share/omtd-share/SpellChecking
:SpellChecking rdf:type owl:Class ;
               rdfs:subClassOf :AuthoringSupport ;
               rdfs:comment "The task/process of checking the accuracy of spelling of a word (and usually correcting it) according to the accepted form"@en ;
               rdfs:label "Spell checking"@en ;
               <http://www.w3.org/2004/02/skos/core#altLabel> "Spelling correction"@en ;
               <http://www.w3.org/2004/02/skos/core#definition> "Techniques for the identification of spelling or typing errors in textual documents, which may be applied interactively during the creation of the document, or off-line for existing documents. Spelling correction is an extension in which for each assumed error one or several hypothetical corrections are suggested."@en .


###  http://w3id.org/meta-share/omtd-share/SpellingChecker
:SpellingChecker rdf:type owl:Class ;
                 rdfs:subClassOf :PreOrPostProcessor ;
                 rdfs:comment "A component that corrects spelling mistakes in a text"@en ;
                 rdfs:label "Spelling checker"@en .


###  http://w3id.org/meta-share/omtd-share/SpokenLanguageGeneration
:SpokenLanguageGeneration rdf:type owl:Class ;
                          rdfs:subClassOf :NaturalLanguageGeneration ;
                          rdfs:label "Spoken Language Generation"@en ;
                          <http://www.w3.org/2004/02/skos/core#altLabel> "CTS"@en ,
                                                                         "Concept-to-Speech generation"@en ,
                                                                         "SLG"@en ;
                          <http://www.w3.org/2004/02/skos/core#definition> "Whereas the generation of spoken language from semantic representations can be sequentialized into generation of text followed by text-to-speech, using text as an intermediate representation may lose information that was available in the original input, in particular related to information structure relevant for speech output. An integrated solution can avoid this problem and thereby lead to improved quality and/or simpler system architecture."@en .


###  http://w3id.org/meta-share/omtd-share/SpokenLanguageUnderstanding
:SpokenLanguageUnderstanding rdf:type owl:Class ;
                             rdfs:subClassOf :SpeechRecognition ;
                             rdfs:label "Spoken Language Understanding"@en ;
                             <http://www.w3.org/2004/02/skos/core#definition> "Spoken language understanding is the task of assigning a semantic interpretation to a spoken input, by making use of syntactic and semantic knowledge, which is often specific to a particular application domain. Spoken language understanding can involve dealing with multiple recognition hypotheses from a speech recogniser, taking prosodic properties of utterances into account and having to deal with fragmentary and grammatically incorrect utterances. Commercial speech recognisers often are accompanied by analysis tools. In commercial applications such as dialogue systems and command and control, spoken language understanding generally involves the construction of a task and domain-specific interpretation of the utterance."@en .


###  http://w3id.org/meta-share/omtd-share/StanceDetection
:StanceDetection rdf:type owl:Class ;
                 rdfs:subClassOf :InformationExtraction ;
                 rdfs:comment "The extraction of a subjects reaction to a claim made by a primary actor [http://nlpprogress.com/english/stance_detection.html]"@en ;
                 rdfs:label "Stance detection"@en .


###  http://w3id.org/meta-share/omtd-share/StatisticalLanguageModelling
:StatisticalLanguageModelling rdf:type owl:Class ;
                              rdfs:subClassOf :LanguageModelling ;
                              rdfs:label "Statistical Language Modelling"@en ;
                              <http://www.w3.org/2004/02/skos/core#altLabel> "SLM"@en ,
                                                                             "Statistical Language Modeling"@en .


###  http://w3id.org/meta-share/omtd-share/StatisticalLearningMethod
:StatisticalLearningMethod rdf:type owl:Class ;
                           rdfs:subClassOf :TdmMethod ;
                           <http://purl.org/dc/elements/1.1/source> "\"R: Statistical learning primer\", https://www.pressreader.com/australia/linux-format/20161025/283626759591113"@en ;
                           rdfs:comment "The process of using statistics and techniques related to statistics in order to understand and learn from your data so that you can predict its future."@en ;
                           rdfs:label "Statistical Learning Method"@en .


###  http://w3id.org/meta-share/omtd-share/Stem
:Stem rdf:type owl:Class ;
      rdfs:subClassOf :MorphologicalAnnotationType ,
                      [ rdf:type owl:Restriction ;
                        owl:onProperty owl:equivalentClass ;
                        owl:someValuesFrom <http://purl.org/olia/olia-top.owl#Stem>
                      ] ,
                      [ rdf:type owl:Restriction ;
                        owl:onProperty :documentationUrl ;
                        owl:hasValue "http://dkpro.github.io/dkpro-core/releases/1.8.0/docs/typesystem-reference.html#de.tudarmstadt.ukp.dkpro.core.api.segmentation.type.Stem"
                      ] ;
      rdfs:comment "A stem is the root or roots of a word, together with any derivational affixes, to which inflectional affixes are added. [http://www.glossary.sil.org/term/stem]"@en ;
      rdfs:label "Stem"@en .


###  http://w3id.org/meta-share/omtd-share/Stemmer
:Stemmer rdf:type owl:Class ;
         rdfs:subClassOf :Annotator ,
                         [ rdf:type owl:Restriction ;
                           owl:onProperty :performsOperation ;
                           owl:someValuesFrom :Stemming
                         ] ;
         rdfs:comment "A component that extracts stems from words in a text, usually by removing the most common morphological and inflectional endings from words"@en ;
         rdfs:label "Stemmer"@en .


###  http://w3id.org/meta-share/omtd-share/Stemming
:Stemming rdf:type owl:Class ;
          rdfs:subClassOf :TextAnnotation ,
                          [ rdf:type owl:Restriction ;
                            owl:onProperty <http://www.w3.org/2004/02/skos/core#closeMatch> ;
                            owl:someValuesFrom :Lemmatization
                          ] ;
          rdfs:comment "The task/process of cutting off the ends of words (mainly inflectional affixes but sometimes also derivational affixes) aiming to relate words to a base form."@en ;
          rdfs:label "Stemming"@en ;
          <http://www.w3.org/2004/02/skos/core#altLabel> "" .


###  http://w3id.org/meta-share/omtd-share/StructuralAnnotation
:StructuralAnnotation rdf:type owl:Class ;
                      rdfs:subClassOf :TextAnnotation ;
                      rdfs:comment "The task/process of segmenting a text and recognizing textual structural units (paragraphs, sentences, words etc.)"@en ;
                      rdfs:label "Structural annotation"@en ;
                      <http://www.w3.org/2004/02/skos/core#altLabel> "Segmentation"@en .


###  http://w3id.org/meta-share/omtd-share/StructuralAnnotationType
:StructuralAnnotationType rdf:type owl:Class ;
                          rdfs:subClassOf :AnnotationType ;
                          rdfs:comment "Any type of annotation that pertains to the structure of a document"@en ;
                          rdfs:label "Structural annotation type"@en .


###  http://w3id.org/meta-share/omtd-share/SubcategorizationFrame
:SubcategorizationFrame rdf:type owl:Class ;
                        rdfs:subClassOf :SyntacticAnnotationType ;
                        rdfs:comment "The number and types of syntactic arguments required by a certain lexical item (mainly verbs, but also nouns and adjectives)"@en ;
                        rdfs:label "Subcategorization frame"@en ;
                        <http://www.w3.org/2004/02/skos/core#altLabel> "Argument structure"@en ,
                                                                       "Subcategorisation frame"@en .


###  http://w3id.org/meta-share/omtd-share/Subjectivity
:Subjectivity rdf:type owl:Class ;
              rdfs:subClassOf :SemanticAnnotationType ;
              rdfs:comment "The linguistic expression of somebodys opinions, sentiments, emotions, evaluations, beliefs, speculations (private states, i.e. states that are not open to objective observation or verification). [http://www.mavir.net/docs/JWiebe-Subjectivity-nov2010.pdf]"@en ;
              rdfs:label "Subjectivity"@en .


###  http://w3id.org/meta-share/omtd-share/Summarization
:Summarization rdf:type owl:Class ;
               rdfs:subClassOf :NaturalLanguageGeneration ;
               rdfs:altLabel "ATS"@en ;
               rdfs:comment "The process/task of reducing one or more textual documents with a computer program in order to create a summary that retains the most important points of the original document(s)."@en ;
               rdfs:label "Summarization"@en ;
               <http://www.w3.org/2004/02/skos/core#altLabel> "Automatic Summarisation"@en-uk ,
                                                              "Automatic Summarization"@en ,
                                                              "Automatic Text Summarisation"@en-uk ,
                                                              "Automatic Text Summarization"@en ,
                                                              "Summarisation"@en-uk ,
                                                              "TS"@en ,
                                                              "Text Summarisation"@en-uk ,
                                                              "Text Summarization"@en ;
               <http://www.w3.org/2004/02/skos/core#definition> "Text summarization is the process of distilling the most important information from a source (or sources) to produce an abridged version for a particular user (or users) and task (or tasks). Source: Mani, I. and Maybury, M. T., editors (1999), Advances in Automatic Text Summarization. MIT Press, Cambridge, Massachusetts."@en .


###  http://w3id.org/meta-share/omtd-share/Summarizer
:Summarizer rdf:type owl:Class ;
            rdfs:subClassOf :Generator ,
                            [ rdf:type owl:Restriction ;
                              owl:onProperty :performsOperation ;
                              owl:someValuesFrom :Summarization
                            ] ;
            rdfs:comment "A component that produces a natural language synopsis of a longer text"@en ;
            rdfs:label "Summarizer"@en .


###  http://w3id.org/meta-share/omtd-share/SupportComponent
:SupportComponent rdf:type owl:Class ;
                  rdfs:subClassOf :ComponentType ,
                                  [ rdf:type owl:Restriction ;
                                    owl:onProperty :performsOperation ;
                                    owl:someValuesFrom :SupportOperation
                                  ] ;
                  rdfs:comment "A component that provides support to developers"@en ;
                  rdfs:label "Support component"@en ;
                  <http://www.w3.org/2004/02/skos/core#altLabel> "Helper"@en .


###  http://w3id.org/meta-share/omtd-share/SupportOfCrowdsourcingTasks
:SupportOfCrowdsourcingTasks rdf:type owl:Class ;
                             rdfs:subClassOf :SupportOperation ;
                             rdfs:comment "Any operation that can support tasks that are accomplished through crowdsourcing"@en ;
                             rdfs:label "Support of crowdsourcing tasks"@en ;
                             <http://www.w3.org/2004/02/skos/core#example> "Collection of data, their transformation and organization into crowdsourcing units; automatic generation of reusable crowdsourcing interfaces for specific tasks (e.g. annotation)"@en .


###  http://w3id.org/meta-share/omtd-share/SupportOperation
:SupportOperation rdf:type owl:Class ;
                  rdfs:subClassOf :Operation ;
                  rdfs:comment "Any operation that is used to support LT tasks, either for creating workflows or for executing them"@en ;
                  rdfs:label "Support operation"@en .


###  http://w3id.org/meta-share/omtd-share/SupportOperationForKnowledgeResources
:SupportOperationForKnowledgeResources rdf:type owl:Class ;
                                       rdfs:subClassOf :Operation ;
                                       rdfs:comment "Any operation that intends to support the creation, curation or use of knowledge resource"@en ;
                                       rdfs:label "Support operation for knowledge resources"@en .


###  http://w3id.org/meta-share/omtd-share/SyllableSegmentation
:SyllableSegmentation rdf:type owl:Class ;
                      rdfs:subClassOf :MorphologicalAnnotation ;
                      rdfs:comment "Segmentation of a word into syllables"@en ;
                      rdfs:label "Syllable segmentation"@en .


###  http://w3id.org/meta-share/omtd-share/Synapse
:Synapse rdf:type owl:Class ;
         rdfs:subClassOf :BiologicalEnity ,
                         :NamedEntity ;
         rdfs:comment "A specialized structure or junction that allows cell to cell communication [http://www.biology-online.org/dictionary/Synapse]"@en ;
         rdfs:label "Synapse"@en .


###  http://w3id.org/meta-share/omtd-share/SyntacticAnnotationType
:SyntacticAnnotationType rdf:type owl:Class ;
                         rdfs:subClassOf :AnnotationType ,
                                         [ rdf:type owl:Restriction ;
                                           owl:onProperty owl:equivalentClass ;
                                           owl:someValuesFrom <http://purl.org/olia/olia-top.owl#SyntacticCategory>
                                         ] ;
                         rdfs:comment "Any type of annotation that pertains to the syntactic level"@en ;
                         rdfs:label "Syntactic annotation type"@en .


###  http://w3id.org/meta-share/omtd-share/SyntacticStructureGeneration
:SyntacticStructureGeneration rdf:type owl:Class ;
                              rdfs:subClassOf :NaturalLanguageGeneration ;
                              rdfs:label "Syntactic Structure Generation"@en ;
                              <http://www.w3.org/2004/02/skos/core#definition> "" .


###  http://w3id.org/meta-share/omtd-share/SyntacticoSemanticLink
:SyntacticoSemanticLink rdf:type owl:Class ;
                        rdfs:subClassOf :SemanticAnnotationType ,
                                        :SyntacticAnnotationType ;
                        rdfs:comment "A link between the syntactic unit and the semantic unit (sense) of a word"@en ;
                        rdfs:label "Syntactico-semantic link"@en .


###  http://w3id.org/meta-share/omtd-share/TabularFormat
:TabularFormat rdf:type owl:Class ;
               rdfs:subClassOf :DataFormat ;
               rdfs:comment "Any format based on columns"@en ;
               rdfs:label "Tabular format"@en .


###  http://w3id.org/meta-share/omtd-share/TagsetConversion
:TagsetConversion rdf:type owl:Class ;
                  rdfs:subClassOf :SupportOperation ;
                  rdfs:label "Tagset conversion"@en .


###  http://w3id.org/meta-share/omtd-share/TalkingHeadSynthesis
:TalkingHeadSynthesis rdf:type owl:Class ;
                      rdfs:subClassOf :OperationWithMultimediaInputOrOutput ;
                      rdfs:label "Talking head synthesis"@en .


###  http://w3id.org/meta-share/omtd-share/TaskOrientedTextAnalysisEvaluation
:TaskOrientedTextAnalysisEvaluation rdf:type owl:Class ;
                                    rdfs:subClassOf :Evaluation ;
                                    rdfs:label "Task-oriented text analysis evaluation"@en .


###  http://w3id.org/meta-share/omtd-share/Tcf
:Tcf rdf:type owl:Class ;
     rdfs:subClassOf :AnnotationFormat ,
                     :CorpusFormat ,
                     :Xml ,
                     [ rdf:type owl:Restriction ;
                       owl:onProperty :hasMimetype ;
                       owl:hasValue :text_tcf_xml
                     ] ,
                     [ rdf:type owl:Restriction ;
                       owl:onProperty :documentationUrl ;
                       owl:hasValue "https://weblicht.sfs.uni-tuebingen.de/weblichtwiki/index.php/The_TCF_Format"
                     ] ;
     rdfs:comment "An XML data exchange format developed within the WebLicht architecture to facilitate efficient interoperability between the tools; it allows the various linguistic annotations produced by the tools within WebLicht to be stored in one document; it supports incremental enrichment of linguistic annotations at various levels of analysis in a stand-off XMLbased format"@en ;
     rdfs:label "TCF"@en ;
     <http://www.w3.org/2004/02/skos/core#altLabel> "Text Corpus Format"@en .


###  http://w3id.org/meta-share/omtd-share/TdmMethod
:TdmMethod rdf:type owl:Class ;
           rdfs:subClassOf owl:Thing ;
           rdfs:comment "The method used by a TDM algorithm"@en ;
           rdfs:label "TDM Method"@en .


###  http://w3id.org/meta-share/omtd-share/Tei
:Tei rdf:type owl:Class ;
     rdfs:subClassOf :AnnotationFormat ,
                     :Xml ,
                     [ rdf:type owl:Restriction ;
                       owl:onProperty :hasMimetype ;
                       owl:hasValue :application_tei_xml
                     ] ,
                     [ rdf:type owl:Restriction ;
                       owl:onProperty :documentationUrl ;
                       owl:hasValue "http://www.tei-c.org/index.xml"
                     ] ,
                     [ rdf:type owl:Restriction ;
                       owl:onProperty :documentationUrl ;
                       owl:hasValue "https://www.iana.org/assignments/media-types/application/tei+xml"
                     ] ;
     rdfs:altLabel "Text Encoding Initiative"@en ;
     rdfs:comment "Data format for TEI-encoded (Text Encoding Initiative) texts"@en ;
     rdfs:label "TEI"@en .


###  http://w3id.org/meta-share/omtd-share/TemporalExpression
:TemporalExpression rdf:type owl:Class ;
                    rdfs:subClassOf :SemanticAnnotationType ;
                    rdfs:comment "A linguistic expression (word, group of words, group of numbers etc.) that denotes time (a point in time, duration, frequency)"@en ;
                    rdfs:label "Temporal expression"@en .


###  http://w3id.org/meta-share/omtd-share/TemporalExpressionRecognition
:TemporalExpressionRecognition rdf:type owl:Class ;
                               rdfs:subClassOf :InformationExtraction ;
                               rdfs:comment "The task/process of identifying temporal expressions (also called timex) in a text in order to extract temporal information"@en ;
                               rdfs:label "Temporal expressions recognition"@en .


###  http://w3id.org/meta-share/omtd-share/TemporalExpressionsLabelling
:TemporalExpressionsLabelling rdf:type owl:Class ;
                              rdfs:subClassOf :SemanticAnnotation ;
                              rdfs:comment "The task/process of determining the boundaries of units of text that denote time-related concepts and attaching to them tags that name these concepts (e.g. date, time, duration etc.)"@en ;
                              rdfs:label "Temporal expressions labelling"@en ;
                              <http://www.w3.org/2004/02/skos/core#altLabel> "Annotation of time"@en .


###  http://w3id.org/meta-share/omtd-share/Term
:Term rdf:type owl:Class ;
      rdfs:subClassOf :AnnotationType ;
      rdfs:comment "A term is a designation consisting of one or more words representing a general concept in a special language in a specific subject field [ISO 704:2009]"@en ;
      rdfs:label "Term"@en .


###  http://w3id.org/meta-share/omtd-share/TermExtraction
:TermExtraction rdf:type owl:Class ;
                rdfs:subClassOf :InformationExtraction ;
                rdfs:comment "The act/process of identifying and extracting candidate terms from a domain-specific corpus"@en ;
                rdfs:label "Term extraction"@en ;
                <http://www.w3.org/2004/02/skos/core#altLabel> "Corpus based term recognition"@en ,
                                                               "Term recognition"@en ,
                                                               "Terminology extraction"@en ,
                                                               "Terminology recognition"@en .


###  http://w3id.org/meta-share/omtd-share/TermExtractor
:TermExtractor rdf:type owl:Class ;
               rdfs:subClassOf :Analyzer ,
                               [ rdf:type owl:Restriction ;
                                 owl:onProperty :performsOperation ;
                                 owl:someValuesFrom :TermExtraction
                               ] ;
               rdfs:comment "A component that tries to extract terms from a corpus"@en ;
               rdfs:label "Term extractor"@en ;
               <http://www.w3.org/2004/02/skos/core#altLabel> "Terminology extractor"@en .


###  http://w3id.org/meta-share/omtd-share/TerminologyManagement
:TerminologyManagement rdf:type owl:Class ;
                       rdfs:subClassOf :SupportOperation ;
                       rdfs:label "Terminology management"@en .


###  http://w3id.org/meta-share/omtd-share/TerminologyMarkup
:TerminologyMarkup rdf:type owl:Class ;
                   rdfs:subClassOf :SemanticAnnotation ;
                   rdfs:label "Terminology markup"@en ;
                   <http://www.w3.org/2004/02/skos/core#altLabel> "Annotation of terms"@en ,
                                                                  "Term labelling"@en .


###  http://w3id.org/meta-share/omtd-share/TerminologySearch
:TerminologySearch rdf:type owl:Class ;
                   rdfs:subClassOf :InformationRetrieval ;
                   rdfs:label "Terminology search"@en ;
                   <http://www.w3.org/2004/02/skos/core#altLabel> "Term search"@en .


###  http://w3id.org/meta-share/omtd-share/Tex
:Tex rdf:type owl:Class ;
     rdfs:subClassOf :DocumentFormat ,
                     [ rdf:type owl:Restriction ;
                       owl:onProperty :hasMimetype ;
                       owl:hasValue :application_xTex
                     ] ,
                     [ rdf:type owl:Restriction ;
                       owl:onProperty :documentationUrl ;
                       owl:hasValue "https://en.wikipedia.org/wiki/TeX"
                     ] ;
     rdfs:comment "Data format for documents using Tex (a typesetting system)"@en ;
     rdfs:label "TEX"@en .


###  http://w3id.org/meta-share/omtd-share/Text
:Text rdf:type owl:Class ;
      rdfs:subClassOf :DocumentFormat ,
                      [ rdf:type owl:Restriction ;
                        owl:onProperty :hasMimetype ;
                        owl:hasValue :text_plain
                      ] ,
                      [ rdf:type owl:Restriction ;
                        owl:onProperty :hasFileExtension ;
                        owl:hasValue "txt"
                      ] ;
      rdfs:altLabel "plain text"@en ;
      rdfs:comment "Default value for the format of textual files; a textual file should be human-readable and must not contain binary data"@en ;
      rdfs:label "text/plain"@en .


###  http://w3id.org/meta-share/omtd-share/TextAnalysis
:TextAnalysis rdf:type owl:Class ;
              rdfs:subClassOf :InformationExtraction ;
              rdfs:label "Text analysis"@en .


###  http://w3id.org/meta-share/omtd-share/TextAndDataAnalytics
:TextAndDataAnalytics rdf:type owl:Class ;
                      rdfs:subClassOf :TextSpeechDataAnalytics ,
                                      [ rdf:type owl:Restriction ;
                                        owl:onProperty <http://www.w3.org/2004/02/skos/core#closeMatch> ;
                                        owl:someValuesFrom :TextAndDataMining
                                      ] ;
                      rdfs:comment "The process/task of converting unstructured text and data into high-quality structured data that can be further analysed to extract knowledge, support decision making etc."@en ;
                      rdfs:label "Text and Data Analytics"@en .


###  http://w3id.org/meta-share/omtd-share/TextAndDataMining
:TextAndDataMining rdf:type owl:Class ;
                   rdfs:subClassOf :Operation ;
                   rdfs:comment "The automated processing of unstructured text and/or structured data leading to the extraction of previously hidden knowledge."@en ;
                   rdfs:label "Text and Data Mining"@en ;
                   <http://www.w3.org/2004/02/skos/core#altLabel> "DM"@en ,
                                                                  "Data Mining"@en ,
                                                                  "TDM"@en ,
                                                                  "TM"@en ,
                                                                  "Text Data Mining"@en ,
                                                                  "Text Mining"@en ;
                   <http://www.w3.org/2004/02/skos/core#definition> "Text data mining concerns the application of data mining (knowledge discovery in databases, KDD) to unstructured textual data. The goal of data mining is to discover or derive new information from data, finding patterns across datasets, and/or separating signal from noise. Core text mining algorithms decompose text in meaningful chunks that can then be used for true data mining purposes."@en .


###  http://w3id.org/meta-share/omtd-share/TextAnnotation
:TextAnnotation rdf:type owl:Class ;
                rdfs:subClassOf :Annotation ;
                rdfs:comment "The process/task of adding annotations (notes or comments) to a text; in TDM, the annotations refer mainly to the interpretative linguistic information grounded in a knowledge resource that is added manually or automatically to a text"@en ;
                rdfs:label "Text annotation"@en ;
                <http://www.w3.org/2004/02/skos/core#altLabel> "Linguistic annotation"@en .


###  http://w3id.org/meta-share/omtd-share/TextCategorization
:TextCategorization rdf:type owl:Class ;
                    rdfs:subClassOf :InformationExtraction ,
                                    :KnowledgeDiscovery ;
                    rdfs:comment "The task/process of assigning documents into classes or categories"@en ;
                    rdfs:label "Text categorization"@en ;
                    <http://www.w3.org/2004/02/skos/core#altLabel> "Document categorisation"@en ,
                                                                   "Document categorisation"@en-uk ,
                                                                   "Document categorization"@en ,
                                                                   "Document classification"@en ,
                                                                   "Text categorisation"@en-uk ,
                                                                   "Text classification"@en .


###  http://w3id.org/meta-share/omtd-share/TextCompression
:TextCompression rdf:type owl:Class ;
                 rdfs:subClassOf :SupportOperation ;
                 rdfs:label "Text compression"@en ;
                 <http://www.w3.org/2004/02/skos/core#definition> "Methods for text compression identify and exploit redundancy in text documents in order to obtain a more condensed representation of the information, from which the original data can be recovered without modification (lossless compression). In theory, there is a close relation between compression and prediction: The better a statistical language model can estimate the probability of a word, given some context, the more the text as a whole can be compressed."@en .


###  http://w3id.org/meta-share/omtd-share/TextEncryption
:TextEncryption rdf:type owl:Class ;
                rdfs:subClassOf :Anonymization ;
                rdfs:label "Text encryption"@en ;
                <http://www.w3.org/2004/02/skos/core#definition> "A cryptosystem or cipher system is a method of disguising messages so that only certain people can see through the disguise. Cryptography is the art of creating and using cryptosystems. Cryptanalysis is the art of breaking cryptosystems---seeing through the disguise even when you're not supposed to be able to. Cryptology is the study of both cryptography and cryptanalysis."@en .


###  http://w3id.org/meta-share/omtd-share/TextGeneration
:TextGeneration rdf:type owl:Class ;
                rdfs:subClassOf :NaturalLanguageGeneration ;
                rdfs:label "Text generation"@en .


###  http://w3id.org/meta-share/omtd-share/TextIndexing
:TextIndexing rdf:type owl:Class ;
              rdfs:subClassOf :SupportOperation ;
              rdfs:label "Text indexing"@en .


###  http://w3id.org/meta-share/omtd-share/TextSimilarityAssessment
:TextSimilarityAssessment rdf:type owl:Class ;
                          rdfs:subClassOf :InformationExtraction ;
                          rdfs:altLabel "Text similarity checking"@en ,
                                        "Textual similarity assessment"@en ,
                                        "Textual similarity checking"@en ;
                          rdfs:comment "The task of determining the degree of closeness between two pieces of text"@en ;
                          rdfs:label "Text similarity assessment"@en .


###  http://w3id.org/meta-share/omtd-share/TextSimplification
:TextSimplification rdf:type owl:Class ;
                    rdfs:subClassOf :NaturalLanguageGeneration ;
                    rdfs:comment "The task of replacing textual segments (phrases, clauses, etc.) with other segments that have similar meaning but are easier to understand"@en ;
                    rdfs:label "Text simplification"@en ;
                    <http://www.w3.org/2004/02/skos/core#related> :LexicalSimplification .


###  http://w3id.org/meta-share/omtd-share/TextSpeechDataAnalytics
:TextSpeechDataAnalytics rdf:type owl:Class ;
                         rdfs:subClassOf :Operation ;
                         rdfs:label "Text/Speech/Data analytics"@en ;
                         <http://www.w3.org/2004/02/skos/core#comment> "it could also be a composite concept created by three separate concepts, but for now ok"@en .


###  http://w3id.org/meta-share/omtd-share/TextToSpeechSynthesis
:TextToSpeechSynthesis rdf:type owl:Class ;
                       rdfs:subClassOf :NaturalLanguageGeneration ,
                                       :OperationWithMultimediaInputOrOutput ;
                       rdfs:comment "The task/process of converting speech into natural language text"@en ;
                       rdfs:label "Text-to-Speech Synthesis"@en ;
                       <http://www.w3.org/2004/02/skos/core#altLabel> "TTS"@en ,
                                                                      "Text to Speech Synthesis"@en ;
                       <http://www.w3.org/2004/02/skos/core#definition> "The generation of synthetic speech from text. Typically, a text-to-speech synthesis system performs a text analysis using natural language processing techniques; determines the appropriate phonetic string and prosodic features; and generates a speech signal by employing a concatenative or rule-based synthesis method."@en .


###  http://w3id.org/meta-share/omtd-share/Tgrep2
:Tgrep2 rdf:type owl:Class ;
        rdfs:subClassOf :AnnotationFormat ,
                        [ rdf:type owl:Restriction ;
                          owl:onProperty :hasMimetype ;
                          owl:hasValue :application_x_org_dkpro_tgrep2
                        ] ,
                        [ rdf:type owl:Restriction ;
                          owl:onProperty :documentationUrl ;
                          owl:hasValue "https://dkpro.github.io/dkpro-core/releases/1.8.0/docs/format-reference.html#format-de.tudarmstadt.ukp.dkpro.core.io.tgrep-gpl"
                        ] ;
        rdfs:comment "Format for TGrep2 (search engine for searching syntactic parse trees represented as bracketed structures)"@en ;
        rdfs:label "TGrep2"@en .


###  http://w3id.org/meta-share/omtd-share/TheoreticalFrame
:TheoreticalFrame rdf:type owl:Class ;
                  rdfs:subClassOf :NamedEntity ,
                                  :SocialSciencesEntity ;
                  rdfs:comment "Theoretical frame"@en ;
                  rdfs:label "Theoretical frame"@en .


###  http://w3id.org/meta-share/omtd-share/TigerXml
:TigerXml rdf:type owl:Class ;
          rdfs:subClassOf :AnnotationFormat ,
                          :CorpusFormat ,
                          :Xml ,
                          [ rdf:type owl:Restriction ;
                            owl:onProperty :hasMimetype ;
                            owl:hasValue :application_x_org_dkpro_tiger_xml
                          ] ,
                          [ rdf:type owl:Restriction ;
                            owl:onProperty :documentationUrl ;
                            owl:hasValue "http://www.ims.uni-stuttgart.de/forschung/ressourcen/werkzeuge/TIGERSearch/doc/html/TigerXML.html"
                          ] ,
                          [ rdf:type owl:Restriction ;
                            owl:onProperty :documentationUrl ;
                            owl:hasValue "https://dkpro.github.io/dkpro-core/releases/1.8.0/docs/format-reference.html#format-de.tudarmstadt.ukp.dkpro.core.io.tiger-asl"
                          ] ;
          rdfs:comment "The TIGER XML format was created for encoding syntactic constituency structures in the German TIGER corpus. It has since been used for many other corpora as well. TIGERSearch is a linguistic search engine specifically targetting this format. The format has later been extended to also support semantic frame annotations."@en ;
          rdfs:label "Tiger XML"@en .


###  http://w3id.org/meta-share/omtd-share/Tika
:Tika rdf:type owl:Class ;
      rdfs:subClassOf :DocumentFormat ,
                      [ rdf:type owl:Restriction ;
                        owl:onProperty :hasMimetype ;
                        owl:hasValue :application_tika
                      ] ;
      rdfs:label "Tika" .


###  http://w3id.org/meta-share/omtd-share/Tmx
:Tmx rdf:type owl:Class ;
     rdfs:subClassOf :AnnotationFormat ,
                     :Xml ,
                     [ rdf:type owl:Restriction ;
                       owl:onProperty :hasMimetype ;
                       owl:hasValue :application_xTmx_xml
                     ] ,
                     [ rdf:type owl:Restriction ;
                       owl:onProperty :documentationUrl ;
                       owl:hasValue "http://www.ttt.org/oscarstandards/tmx/tmx14-20020710.htm"
                     ] ;
     rdfs:comment "The purpose of the TMX format is to provide a standard method to describe translation memory data that is being exchanged among tools and/or translation vendors, while introducing little or no loss of critical data during the process."@en ;
     rdfs:label "TMX"@en ;
     <http://www.w3.org/2004/02/skos/core#altLabel> "Translation Memory Exchange"@en .


###  http://w3id.org/meta-share/omtd-share/Token
:Token rdf:type owl:Class ;
       rdfs:subClassOf :StructuralAnnotationType ,
                       [ rdf:type owl:Restriction ;
                         owl:onProperty owl:equivalentClass ;
                         owl:someValuesFrom <http://purl.org/olia/olia-top.owl#Token>
                       ] ,
                       [ rdf:type owl:Restriction ;
                         owl:onProperty owl:equivalentClass ;
                         owl:someValuesFrom <http://vocab.lappsgrid.org/Token>
                       ] ,
                       [ rdf:type owl:Restriction ;
                         owl:onProperty :documentationUrl ;
                         owl:hasValue "http://dkpro.github.io/dkpro-core/releases/1.8.0/docs/typesystem-reference.html#de.tudarmstadt.ukp.dkpro.core.api.segmentation.type.Token"
                       ] ;
       rdfs:comment "A set of characters surrounded by spaces or punctuation marks, as well as punctuation marks themselves"@en ;
       rdfs:label "Token"@en .


###  http://w3id.org/meta-share/omtd-share/Tokenization
:Tokenization rdf:type owl:Class ;
              rdfs:subClassOf :StructuralAnnotation ;
              rdfs:comment "The task/process of recognizing and tagging tokens (words, punctuation marks, digits etc.) in a text"@en ;
              rdfs:label "Tokenization"@en ;
              <http://www.w3.org/2004/02/skos/core#altLabel> "Segmentation"@en ,
                                                             "Segmentation and Tokenisation"@en-uk ,
                                                             "Segmentation and Tokenization"@en ,
                                                             "Tokenisation"@en-uk ;
              <http://www.w3.org/2004/02/skos/core#definition> "Tokenization is commonly seen as an independent process of linguistic analysis, in which the input stream of characters is segmented into an ordered sequence of word-like units, usually called tokens, which function as input items for subsequent steps of linguistic processing. Tokens may correspond to words, numbers, punctuation marks or even proper names.The recognized tokens are usually classified according to their syntax. Since the notion of tokenization seems to have different meanings to different people, some tokenization tools fulfil additional tasks like for instance sentence boundary detection, handling of end-line hyphenations or conjoined clitics and contractions."@en .


###  http://w3id.org/meta-share/omtd-share/Tokenizer
:Tokenizer rdf:type owl:Class ;
           rdfs:subClassOf :Segmenter ;
           rdfs:comment "A component that recognizes and tags tokens (words, punctuation marks, digits etc.) in a text"@en ;
           rdfs:label "Tokenizer"@en .


###  http://w3id.org/meta-share/omtd-share/Topic
:Topic rdf:type owl:Class ;
       rdfs:subClassOf :ScholarlyCommunicationAnnotation ,
                       :SemanticAnnotationType ;
       rdfs:comment "The subject of a text or conversation, what it is about"@en ;
       rdfs:label "Topic"@en .


###  http://w3id.org/meta-share/omtd-share/TopicDetection
:TopicDetection rdf:type owl:Class ;
                rdfs:subClassOf :InformationExtraction ,
                                :KnowledgeDiscovery ,
                                [ rdf:type owl:Restriction ;
                                  owl:onProperty <http://www.w3.org/2004/02/skos/core#closeMatch> ;
                                  owl:someValuesFrom :TextCategorization
                                ] ;
                rdfs:comment "The task/process of identifying the topic of a text or dataset (e.g. by clustering keywords or using topic models)"@en ;
                rdfs:label "Topic Detection"@en ;
                <http://www.w3.org/2004/02/skos/core#altLabel> "TD"@en ,
                                                               "TDT"@en ,
                                                               "TT"@en ,
                                                               "Topic Detection and Tracking"@en ,
                                                               "Topic Tracking"@en ,
                                                               "Topic classification"@en ,
                                                               "Topic extraction"@en ;
                <http://www.w3.org/2004/02/skos/core#definition> "Topic Detection and Tracking (TDT) refers to automatic techniques for discovering, threading, and retrieving topically related material in streams of data."@en .


###  http://w3id.org/meta-share/omtd-share/TopicExtractor
:TopicExtractor rdf:type owl:Class ;
                rdfs:subClassOf :Analyzer ;
                rdfs:comment "A component that guesses the topic of a text"@en ;
                rdfs:label "Topic extractor"@en .


###  http://w3id.org/meta-share/omtd-share/TrainerOfMachineLearningModels
:TrainerOfMachineLearningModels rdf:type owl:Class ;
                                rdfs:subClassOf :SupportComponent ,
                                                [ rdf:type owl:Restriction ;
                                                  owl:onProperty :performsOperation ;
                                                  owl:someValuesFrom :TrainingOfMachineLearningModels
                                                ] ;
                                rdfs:comment "A component that is used in training models for machine learning"@en ;
                                rdfs:label "Trainer of Machine Learning models"@en ;
                                <http://www.w3.org/2004/02/skos/core#altLabel> "ML models trainer"@en ,
                                                                               "ML trainer"@en .


###  http://w3id.org/meta-share/omtd-share/TrainingOfLanguageModels
:TrainingOfLanguageModels rdf:type owl:Class ;
                          rdfs:subClassOf :LanguageModelling ;
                          <http://purl.org/dc/elements/1.1/source> "Adapted from http://homepages.inf.ed.ac.uk/lzhang10/slm.html" ;
                          rdfs:comment "The task/process of training (statistical) language models that  that can estimate the distribution of natural language as accurately as possible."@en ;
                          rdfs:label "Training of language models"@en .


###  http://w3id.org/meta-share/omtd-share/TrainingOfMachineLearningModels
:TrainingOfMachineLearningModels rdf:type owl:Class ;
                                 rdfs:subClassOf :LanguageModelling ;
                                 <http://purl.org/dc/elements/1.1/source> "adapted from http://docs.aws.amazon.com/machine-learning/latest/dg/training-ml-models.html" ;
                                 rdfs:comment "The task/process of creating Machine Learning (ML) models by providing a ML algorithm with training data that help the algorithm discover patterns in data, and construct the appropriate models using these discoveries"@en ;
                                 rdfs:label "Training of Machine Learning models"@en .


###  http://w3id.org/meta-share/omtd-share/TrainingOfNmtModels
:TrainingOfNmtModels rdf:type owl:Class ;
                     rdfs:subClassOf :LanguageModelling ;
                     rdfs:label "Training of NMT models"@en ;
                     <http://www.w3.org/2004/02/skos/core#altLabel> "Training of Neural Machine Translation models"@en .


###  http://w3id.org/meta-share/omtd-share/Transcription
:Transcription rdf:type owl:Class ;
               rdfs:subClassOf :SpeechRecognition ;
               rdfs:label "Transcription"@en ;
               <http://www.w3.org/2004/02/skos/core#altLabel> "Speech transcription"@en ,
                                                              "Speech-to-Text conversion"@en ;
               <http://www.w3.org/2004/02/skos/core#definition> "" .


###  http://w3id.org/meta-share/omtd-share/Translation
:Translation rdf:type owl:Class ;
             rdfs:subClassOf :Operation ;
             rdfs:comment "The task/process of expressing the sense of a sequence of words in one language into another language"@en ;
             rdfs:label "Translation"@en ;
             <http://www.w3.org/2004/02/skos/core#definition> "" .


###  http://w3id.org/meta-share/omtd-share/TranslationMemoryManagement
:TranslationMemoryManagement rdf:type owl:Class ;
                             rdfs:subClassOf :SupportOperation ;
                             rdfs:label "Translation memory management"@en .


###  http://w3id.org/meta-share/omtd-share/TranslationProjectManagement
:TranslationProjectManagement rdf:type owl:Class ;
                              rdfs:subClassOf :SupportOperation ;
                              rdfs:label "Translation project management"@en .


###  http://w3id.org/meta-share/omtd-share/Transliteration
:Transliteration rdf:type owl:Class ;
                 rdfs:subClassOf :SpeechRecognition ;
                 rdfs:label "Transliteration"@en ;
                 <http://www.w3.org/2004/02/skos/core#altLabel> "Script conversion"@en ;
                 <http://www.w3.org/2004/02/skos/core#definition> "" .


###  http://w3id.org/meta-share/omtd-share/TruthLabelling
:TruthLabelling rdf:type owl:Class ;
                rdfs:subClassOf :InformationExtraction ;
                rdfs:altLabel "Truth detection"@en ,
                              "Truth labeling"@en-us ;
                rdfs:comment "The task of assigning a true/false tag to a news item, headline, claim, etc."@en ;
                rdfs:label "Truth labelling"@en .


###  http://w3id.org/meta-share/omtd-share/Tsv
:Tsv rdf:type owl:Class ;
     rdfs:subClassOf :TabularFormat ,
                     [ rdf:type owl:Restriction ;
                       owl:onProperty :hasMimetype ;
                       owl:hasValue :text_tabSeparatedValues
                     ] ;
     rdfs:comment "Format for files with tab-separated values"@en ;
     rdfs:label "TSV"@en ;
     <http://www.w3.org/2004/02/skos/core#altLabel> "Tab-separated values"@en .


###  http://w3id.org/meta-share/omtd-share/Tuepp
:Tuepp rdf:type owl:Class ;
       rdfs:subClassOf :AnnotationFormat ,
                       :CorpusFormat ,
                       :Xml ,
                       [ rdf:type owl:Restriction ;
                         owl:onProperty :hasMimetype ;
                         owl:hasValue :application_x_org_dkpro_tuepp_xml
                       ] ,
                       [ rdf:type owl:Restriction ;
                         owl:onProperty :documentationUrl ;
                         owl:hasValue "http://dkpro.github.io/dkpro-core/releases/1.8.0/docs/format-reference.html#format-de.tudarmstadt.ukp.dkpro.core.io.tuepp-asl"
                       ] ,
                       [ rdf:type owl:Restriction ;
                         owl:onProperty :documentationUrl ;
                         owl:hasValue "https://zoidberg.ukp.informatik.tu-darmstadt.de/jenkins/job/DKPro%20Core%20Documentation%20(GitHub)/de.tudarmstadt.ukp.dkpro.core$de.tudarmstadt.ukp.dkpro.core.doc-asl/doclinks/5/format-reference.html#format-Tuepp"
                       ] ;
       rdfs:comment "Format of the Tubingen Partially Parsed Corpus of Written German (TuPP-D/Z) XML files; TPP D/Z (http://www.sfs.uni-tuebingen.de/de/ascl/ressourcen/corpora/tuepp-dz.html) is a collection of articles from the German newspaper taz (die tageszeitung) annotated and encoded in a XML format."@en ;
       rdfs:label "Tuepp"@en .


###  http://w3id.org/meta-share/omtd-share/Turtle
:Turtle rdf:type owl:Class ;
        rdfs:subClassOf :RdfFormat ,
                        :RdfFormats ,
                        [ rdf:type owl:Restriction ;
                          owl:onProperty :hasMimetype ;
                          owl:hasValue :text_turtle
                        ] ,
                        [ rdf:type owl:Restriction ;
                          owl:onProperty :documentationUrl ;
                          owl:hasValue "https://www.w3.org/TR/turtle/"
                        ] ;
        rdfs:comment "Textual syntax for RDF that allows an RDF graph to be completely written in a compact and natural text form, with abbreviations for common usage patterns and datatypes."@en ;
        rdfs:label "Turtle"@en .


###  http://w3id.org/meta-share/omtd-share/UimaCasFormat
:UimaCasFormat rdf:type owl:Class ;
               rdfs:subClassOf :DataFormat ;
               rdfs:comment "Formats used for the UIMA CAS (Common Analysis System) objects"@en ;
               rdfs:label "UIMA CAS format"@en .


###  http://w3id.org/meta-share/omtd-share/Uima_json
:Uima_json rdf:type owl:Class ;
           rdfs:subClassOf :Json ,
                           :UimaCasFormat ,
                           [ rdf:type owl:Restriction ;
                             owl:onProperty :hasMimetype ;
                             owl:hasValue :application_x_org_dkpro_uima_json
                           ] ,
                           [ rdf:type owl:Restriction ;
                             owl:onProperty :documentationUrl ;
                             owl:hasValue "https://dkpro.github.io/dkpro-core/releases/1.8.0/docs/format-reference.html#format-de.tudarmstadt.ukp.dkpro.core.io.json-asl"
                           ] ;
           rdfs:comment "UIMA serialisation in JSON"@en ;
           rdfs:label "UIMA/JSON"@en .


###  http://w3id.org/meta-share/omtd-share/UnicodeConformTokenizing
:UnicodeConformTokenizing rdf:type owl:Class ;
                          rdfs:subClassOf :SupportOperation ;
                          rdfs:label "Unicode-conform tokenizing"@en ;
                          <http://www.w3.org/2004/02/skos/core#definition> "" .


###  http://w3id.org/meta-share/omtd-share/UserAuthentication
:UserAuthentication rdf:type owl:Class ;
                    rdfs:subClassOf :SupportOperation ;
                    rdfs:label "User authentication"@en .


###  http://w3id.org/meta-share/omtd-share/Validation
:Validation rdf:type owl:Class ;
            rdfs:subClassOf :Operation ,
                            :SupportOperation ;
            rdfs:comment "The task/process of confirming that a system/data resource meets the specifications and fulfills its intended purpose"@en ;
            rdfs:label "Validation"@en .


###  http://w3id.org/meta-share/omtd-share/Validator
:Validator rdf:type owl:Class ;
           rdfs:subClassOf :SupportComponent ,
                           [ rdf:type owl:Restriction ;
                             owl:onProperty :performsOperation ;
                             owl:someValuesFrom :Validation
                           ] ;
           rdfs:comment "A component used to confirm that a system/resource meets the specifications and fulfills its intended purpose"@en ;
           rdfs:label "Validator"@en .


###  http://w3id.org/meta-share/omtd-share/VariablesDectector
:VariablesDectector rdf:type owl:Class ;
                    rdfs:subClassOf :Analyzer ;
                    rdfs:altLabel "Variables detection component"@en ;
                    rdfs:comment "A component that tries to identify variables (in social sciences) in a text"@en ;
                    rdfs:label "Variables dectector"@en .


###  http://w3id.org/meta-share/omtd-share/Viewer
:Viewer rdf:type owl:Class ;
        rdfs:subClassOf :SupportComponent ,
                        [ rdf:type owl:Restriction ;
                          owl:onProperty :performsOperation ;
                          owl:someValuesFrom :Viewing
                        ] ;
        rdfs:comment "A component that supports humans in accessing the contents of a resource"@en ;
        rdfs:label "Viewer"@en .


###  http://w3id.org/meta-share/omtd-share/Viewing
:Viewing rdf:type owl:Class ;
         rdfs:subClassOf :SupportOperation ;
         rdfs:comment "The task/process of viewing the contents of a resource as performed by human beings"@en ;
         rdfs:label "Viewing"@en .


###  http://w3id.org/meta-share/omtd-share/Visualiser
:Visualiser rdf:type owl:Class ;
            rdfs:subClassOf :SupportComponent ,
                            [ rdf:type owl:Restriction ;
                              owl:onProperty :performsOperation ;
                              owl:someValuesFrom :Visualization
                            ] ;
            rdfs:comment "A component or interface that renders the contents of a resource in a graphic way for visualisation purposes"@en ;
            rdfs:label "Visualiser"@en .


###  http://w3id.org/meta-share/omtd-share/Visualization
:Visualization rdf:type owl:Class ;
               rdfs:subClassOf :Operation ,
                               :SupportOperation ;
               rdfs:comment "The representation of an object, situation, or set of information as a chart, diagram or any other image that helps end users understand the contents or message"@en ;
               rdfs:label "Visualization"@en ;
               <http://www.w3.org/2004/02/skos/core#altLabel> "Presentation and Visualisation"@en ,
                                                              "Visualisation"@en .


###  http://w3id.org/meta-share/omtd-share/Web1t
:Web1t rdf:type owl:Class ;
       rdfs:subClassOf :CorpusFormat ,
                       [ rdf:type owl:Restriction ;
                         owl:onProperty :hasMimetype ;
                         owl:hasValue :text_x_org_dkpro_ngram
                       ] ,
                       [ rdf:type owl:Restriction ;
                         owl:onProperty :documentationUrl ;
                         owl:hasValue "https://catalog.ldc.upenn.edu/LDC2006T13"
                       ] ,
                       [ rdf:type owl:Restriction ;
                         owl:onProperty :documentationUrl ;
                         owl:hasValue "https://zoidberg.ukp.informatik.tu-darmstadt.de/jenkins/job/DKPro%20Core%20Documentation%20(GitHub)/de.tudarmstadt.ukp.dkpro.core$de.tudarmstadt.ukp.dkpro.core.doc-asl/doclinks/5/format-reference.html#format-Web1T"
                       ] ;
       rdfs:comment "File format used by the Web1T n-gram corpus, a huge collection of n-grams collected from the internet."@en ;
       rdfs:label "Web1T"@en .


###  http://w3id.org/meta-share/omtd-share/WebAnnotationFormat
:WebAnnotationFormat rdf:type owl:Class ;
                     rdfs:subClassOf :AnnotationFormat ,
                                     :Json ,
                                     [ rdf:type owl:Restriction ;
                                       owl:onProperty :hasMimetype ;
                                       owl:hasValue :application_anno_json
                                     ] ,
                                     [ rdf:type owl:Restriction ;
                                       owl:onProperty :hasMimetype ;
                                       owl:hasValue :application_ld_json_profile_http_www_w3_org_ns_anno_jsonld
                                     ] ,
                                     [ rdf:type owl:Restriction ;
                                       owl:onProperty :documentationUrl ;
                                       owl:hasValue "https://www.w3.org/TR/annotation-model/"
                                     ] ;
                     rdfs:comment "A structured model and format to enable annotations to be shared and reused across different hardware and software platforms."@en ;
                     rdfs:label "Web annotation format"@en .


###  http://w3id.org/meta-share/omtd-share/WheatRelatedSpecies
:WheatRelatedSpecies rdf:type owl:Class ;
                     rdfs:subClassOf :AgriculturalEntity ,
                                     :Species ;
                     rdfs:comment "Wheat-related species"@en ;
                     rdfs:label "Wheat-related species"@en .


###  http://w3id.org/meta-share/omtd-share/WikiFormat
:WikiFormat rdf:type owl:Class ;
            rdfs:subClassOf :DataFormat ;
            <http://purl.org/dc/terms/replaces> :WikiFormats ;
            rdfs:comment "Superclass for wiki formats"@en ;
            rdfs:label "Wiki format"@en .


###  http://w3id.org/meta-share/omtd-share/WikiFormats
:WikiFormats rdf:type owl:Class ;
             rdfs:subClassOf :DataFormat ;
             rdfs:comment "Superclass for wiki formats"@en ;
             rdfs:label "Wiki formats"@en ;
             owl:deprecated "true"^^xsd:boolean .


###  http://w3id.org/meta-share/omtd-share/WikipediaArticle
:WikipediaArticle rdf:type owl:Class ;
                  rdfs:subClassOf :WikipediaFormat ,
                                  [ rdf:type owl:Restriction ;
                                    owl:onProperty :documentationUrl ;
                                    owl:hasValue "https://zoidberg.ukp.informatik.tu-darmstadt.de/jenkins/job/DKPro%20Core%20Documentation%20(GitHub)/de.tudarmstadt.ukp.dkpro.core$de.tudarmstadt.ukp.dkpro.core.doc-asl/doclinks/5/format-reference.html#format-WikipediaArticle"
                                  ] ;
                  rdfs:comment "Format for wikipedia articles"@en ;
                  rdfs:label "Wikipedia article"@en .


###  http://w3id.org/meta-share/omtd-share/WikipediaArticleInfo
:WikipediaArticleInfo rdf:type owl:Class ;
                      rdfs:subClassOf :WikipediaFormat ,
                                      [ rdf:type owl:Restriction ;
                                        owl:onProperty :documentationUrl ;
                                        owl:hasValue "https://dkpro.github.io/dkpro-core/releases/1.8.0/docs/format-reference.html#format-WikipediaArticleInfo"
                                      ] ;
                      rdfs:comment "Format of general article infos"@en ;
                      rdfs:label "Wikipedia article info"@en .


###  http://w3id.org/meta-share/omtd-share/WikipediaDiscussion
:WikipediaDiscussion rdf:type owl:Class ;
                     rdfs:subClassOf :WikipediaFormat ,
                                     [ rdf:type owl:Restriction ;
                                       owl:onProperty :documentationUrl ;
                                       owl:hasValue "https://dkpro.github.io/dkpro-core/releases/1.8.0/docs/format-reference.html#format-WikipediaDiscussion"
                                     ] ;
                     rdfs:comment "Format for wikipedia discussion pages"@en ;
                     rdfs:label "Wikipedia discussion"@en .


###  http://w3id.org/meta-share/omtd-share/WikipediaFormat
:WikipediaFormat rdf:type owl:Class ;
                 rdfs:subClassOf :DataFormat ;
                 rdfs:comment "Formats used for wikipedia"@en ;
                 rdfs:label "Wikipedia format"@en .


###  http://w3id.org/meta-share/omtd-share/WikipediaLink
:WikipediaLink rdf:type owl:Class ;
               rdfs:subClassOf :WikipediaFormat ,
                               [ rdf:type owl:Restriction ;
                                 owl:onProperty :documentationUrl ;
                                 owl:hasValue "https://dkpro.github.io/dkpro-core/releases/1.8.0/docs/format-reference.html#format-WikipediaLink"
                               ] ;
               rdfs:comment "Format for wikipedia links"@en ;
               rdfs:label "Wikipedia link"@en .


###  http://w3id.org/meta-share/omtd-share/WikipediaPage
:WikipediaPage rdf:type owl:Class ;
               rdfs:subClassOf :WikipediaFormat ,
                               [ rdf:type owl:Restriction ;
                                 owl:onProperty :documentationUrl ;
                                 owl:hasValue "https://dkpro.github.io/dkpro-core/releases/1.8.0/docs/format-reference.html#format-WikipediaPage"
                               ] ;
               rdfs:comment "Format of wikipedia pages in the database (articles, discussions, etc)"@en ;
               rdfs:label "Wikipedia page"@en .


###  http://w3id.org/meta-share/omtd-share/WikipediaQuery
:WikipediaQuery rdf:type owl:Class ;
                rdfs:subClassOf :WikipediaFormat ,
                                [ rdf:type owl:Restriction ;
                                  owl:onProperty :documentationUrl ;
                                  owl:hasValue "https://dkpro.github.io/dkpro-core/releases/1.8.0/docs/format-reference.html#format-WikipediaQuery"
                                ] ;
                rdfs:comment "Reads all article pages that match a query created by the numerous parameters of this class."@en ;
                rdfs:label "Wikipedia query"@en .


###  http://w3id.org/meta-share/omtd-share/WikipediaRevision
:WikipediaRevision rdf:type owl:Class ;
                   rdfs:subClassOf :WikipediaFormat ,
                                   [ rdf:type owl:Restriction ;
                                     owl:onProperty :documentationUrl ;
                                     owl:hasValue "https://dkpro.github.io/dkpro-core/releases/1.8.0/docs/format-reference.html#format-WikipediaRevision"
                                   ] ;
                   rdfs:comment "Format for wikipedia revision pages"@en ;
                   rdfs:label "Wikipedia revision"@en .


###  http://w3id.org/meta-share/omtd-share/WikipediaRevisionPair
:WikipediaRevisionPair rdf:type owl:Class ;
                       rdfs:subClassOf :WikipediaFormat ,
                                       [ rdf:type owl:Restriction ;
                                         owl:onProperty :documentationUrl ;
                                         owl:hasValue "https://dkpro.github.io/dkpro-core/releases/1.8.0/docs/format-reference.html#format-WikipediaRevisionPair"
                                       ] ;
                       rdfs:comment "Pairs of adjacent revisions of all articles"@en ;
                       rdfs:label "Wikipedia revision pair"@en .


###  http://w3id.org/meta-share/omtd-share/WikipediaTemplateFilteredArticle
:WikipediaTemplateFilteredArticle rdf:type owl:Class ;
                                  rdfs:subClassOf :WikipediaFormat ,
                                                  [ rdf:type owl:Restriction ;
                                                    owl:onProperty :documentationUrl ;
                                                    owl:hasValue "https://dkpro.github.io/dkpro-core/releases/1.8.0/docs/format-reference.html#format-WikipediaTemplateFilteredArticle"
                                                  ] ;
                                  rdfs:comment "Format for wikipedia pages that contain or do not contain the templates specified in the template whitelist and template blacklist"@en ;
                                  rdfs:label "Wikipedia template filtered article"@en .


###  http://w3id.org/meta-share/omtd-share/Word
:Word rdf:type owl:Class ;
      rdfs:subClassOf :MorphologicalAnnotationType ,
                      :StructuralAnnotationType ,
                      [ rdf:type owl:Restriction ;
                        owl:onProperty owl:equivalentClass ;
                        owl:someValuesFrom <http://purl.org/olia/olia-top.owl#Word>
                      ] ;
      rdfs:comment """A word is a unit which is a constituent at the phrase level and above. It is sometimes identifiable according to such criteria as (a) being the minimal possible unit in a reply, (b) having features such as a regular stress pattern, and phonological changes conditioned by or blocked at word boundaries, (c) being the largest unit resistant to insertion of new constituents within its boundaries, or (d) being the smallest constituent that can be moved within a sentence without making the sentence ungrammatical. A word is sometimes placed, in a hierarchy of grammatical constituents, above the morpheme level and below the phrase level. [http://www.glossary.sil.org/term/word]
In annotation, words are often used as equivalent to tokens; thus, for instance, punctuation marks (traditionally not considered as words) will also be annotated as \"word\"."""@en ;
      rdfs:label "Word"@en .


###  http://w3id.org/meta-share/omtd-share/WordAlignment
:WordAlignment rdf:type owl:Class ;
               rdfs:subClassOf :Alignment ;
               rdfs:comment "Alignment at word level"@en ;
               rdfs:label "Word alignment"@en .


###  http://w3id.org/meta-share/omtd-share/WordSegmentation
:WordSegmentation rdf:type owl:Class ;
                  rdfs:subClassOf :MorphologicalAnnotation ;
                  rdfs:comment "The task/process of segmenting (cutting) a word into root and affixes"@en ;
                  rdfs:label "Word segmentation"@en .


###  http://w3id.org/meta-share/omtd-share/WordSense
:WordSense rdf:type owl:Class ;
           rdfs:subClassOf :SemanticAnnotationType ,
                           [ rdf:type owl:Restriction ;
                             owl:onProperty :documentationUrl ;
                             owl:hasValue "http://dkpro.github.io/dkpro-core/releases/1.8.0/docs/typesystem-reference.html#de.tudarmstadt.ukp.dkpro.core.api.semantics.type.WordSense"
                           ] ;
           rdfs:comment "Corresponds to the structural part of a lexical entry that contains the relevant semantic, grammatical, and anthropological information for a lexical unit. [adapted from http://www.glossary.sil.org/term/sense]"@en ;
           rdfs:label "Word sense"@en .


###  http://w3id.org/meta-share/omtd-share/WordSenseDisambiguation
:WordSenseDisambiguation rdf:type owl:Class ;
                         rdfs:subClassOf :SupportOperation ;
                         rdfs:comment "The process/task of identifying which sense of a word with multiple meanings is used in a particular context; the selection of the sense is made from a list of the word's senses."@en ;
                         rdfs:label "Word Sense Disambiguation"@en ;
                         <http://www.w3.org/2004/02/skos/core#altLabel> "WSD"@en ;
                         <http://www.w3.org/2004/02/skos/core#definition> "Word Sense Disambiguation is a subtask of semantic tagging, which consists of assigning a semantic class (sense) to a lexical item as specified by a semantic lexicon. If the semantic lexicon specifies more than one sense for a particular lexical item, a disambiguation procedure is needed to decide upon the most appropriate sense(s) for any given instance of the lexical item in text. WSD is not a self-contained application, but it may be included as an integrated part of a semantic processor."@en .


###  http://w3id.org/meta-share/omtd-share/WordSenseDisambiguator
:WordSenseDisambiguator rdf:type owl:Class ;
                        rdfs:subClassOf :Disambiguator ,
                                        [ rdf:type owl:Restriction ;
                                          owl:onProperty :performsOperation ;
                                          owl:someValuesFrom :WordSenseDisambiguation
                                        ] ;
                        rdfs:comment "A component that tries to identify which sense of a word (i.e. meaning) is used in a sentence, when the word has multiple meanings"@en ;
                        rdfs:label "Word sense disambiguator"@en ;
                        <http://www.w3.org/2004/02/skos/core#comment> "could also be an annotator and a support component (used in a lot of processes)"@en .


###  http://w3id.org/meta-share/omtd-share/WordSenseInduction
:WordSenseInduction rdf:type owl:Class ;
                    rdfs:subClassOf :SupportOperation ;
                    rdfs:altLabel "WSI"@en ;
                    rdfs:comment "The task of automatically identifying the senses of a word"@en ;
                    rdfs:label "Word sense induction"@en ;
                    <http://www.w3.org/2004/02/skos/core#related> :WordSenseDisambiguation .


###  http://w3id.org/meta-share/omtd-share/Writer
:Writer rdf:type owl:Class ;
        rdfs:subClassOf :AccessComponent ,
                        [ rdf:type owl:Restriction ;
                          owl:onProperty :performsOperation ;
                          owl:someValuesFrom :Writing
                        ] ;
        rdfs:comment "A component that writes processing results in various formats"@en ;
        rdfs:label "Writer"@en .


###  http://w3id.org/meta-share/omtd-share/Writing
:Writing rdf:type owl:Class ;
         rdfs:subClassOf :ResourceAccess ;
         rdfs:comment "The task/process of producing the output results of a process/workflow in various formats"@en ;
         rdfs:label "Writing"@en .


###  http://w3id.org/meta-share/omtd-share/Xces
:Xces rdf:type owl:Class ;
      rdfs:subClassOf :AnnotationFormat ,
                      :Xml ,
                      [ rdf:type owl:Restriction ;
                        owl:onProperty :hasMimetype ;
                        owl:hasValue :application_xXces_xml
                      ] ;
      rdfs:comment "Data format for documents and corpora using the XCES standard (Corpus Encoding Standard for XML), cf. http://www.xces.org/"@en ;
      rdfs:label "XCES"@en .


###  http://w3id.org/meta-share/omtd-share/XcesIlspVariant
:XcesIlspVariant rdf:type owl:Class ;
                 rdfs:subClassOf :Xces ,
                                 [ rdf:type owl:Restriction ;
                                   owl:onProperty :hasMimetype ;
                                   owl:hasValue :application_xXces_xml
                                 ] ;
                 rdfs:comment "A variant of XCES implemented for documents"@en ;
                 rdfs:label "XCES ILSP variant"@en ;
                 <http://www.w3.org/2004/02/skos/core#altLabel> "xces; format-variant=ilsp"@en .


###  http://w3id.org/meta-share/omtd-share/Xhtml
:Xhtml rdf:type owl:Class ;
       rdfs:subClassOf :DocumentFormat ,
                       :Xml ,
                       [ rdf:type owl:Restriction ;
                         owl:onProperty :hasMimetype ;
                         owl:hasValue :application_xhtml_xml
                       ] ,
                       [ rdf:type owl:Restriction ;
                         owl:onProperty :documentationUrl ;
                         owl:hasValue "https://www.w3.org/TR/xhtml1/"
                       ] ,
                       [ rdf:type owl:Restriction ;
                         owl:onProperty :hasFileExtension ;
                         owl:hasValue "html"
                       ] ;
       rdfs:comment "Data format for XHTML (Extensible HyperText Markup Language)"@en ;
       rdfs:label "XHTML"@en .


###  http://w3id.org/meta-share/omtd-share/Xmi
:Xmi rdf:type owl:Class ;
     rdfs:subClassOf :DocumentFormat ,
                     :Xml ,
                     [ rdf:type owl:Restriction ;
                       owl:onProperty :hasMimetype ;
                       owl:hasValue :application_vnd_xmi_xml
                     ] ,
                     [ rdf:type owl:Restriction ;
                       owl:onProperty :documentationUrl ;
                       owl:hasValue "https://www.iana.org/assignments/media-types/application/vnd.xmi+xml"
                     ] ,
                     [ rdf:type owl:Restriction ;
                       owl:onProperty :hasFileExtension ;
                       owl:hasValue "xmi"
                     ] ;
     rdfs:comment "Data format for the XML Metadata Interchange (XMI), which is an Object Management Group (OMG) standard for exchanging metadata information via Extensible Markup Language (XML)"@en ;
     rdfs:label "XMI"@en .


###  http://w3id.org/meta-share/omtd-share/Xml
:Xml rdf:type owl:Class ;
     rdfs:subClassOf :DataFormat ;
     rdfs:comment "Superclass for grouping together XML formats"@en ;
     rdfs:label "XML"@en .


###  http://w3id.org/meta-share/omtd-share/XmlBioc
:XmlBioc rdf:type owl:Class ;
         rdfs:subClassOf :Xml ,
                         [ rdf:type owl:Restriction ;
                           owl:onProperty :hasMimetype ;
                           owl:hasValue :application_xml
                         ] ,
                         [ rdf:type owl:Restriction ;
                           owl:onProperty :documentationUrl ;
                           owl:hasValue "http://bioc.sourceforge.net/"
                         ] ;
         rdfs:comment "BioC is a simple format to share text data and annotations."@en ;
         rdfs:label "XML BioC"@en .


###  http://w3id.org/meta-share/omtd-share/Xpath
:Xpath rdf:type owl:Class ;
       rdfs:subClassOf :Xml ,
                       [ rdf:type owl:Restriction ;
                         owl:onProperty :hasMimetype ;
                         owl:hasValue :application_xml
                       ] ,
                       [ rdf:type owl:Restriction ;
                         owl:onProperty :documentationUrl ;
                         owl:hasValue "https://www.w3.org/TR/xpath/"
                       ] ,
                       [ rdf:type owl:Restriction ;
                         owl:onProperty :documentationUrl ;
                         owl:hasValue "https://zoidberg.ukp.informatik.tu-darmstadt.de/jenkins/job/DKPro%20Core%20Documentation%20(GitHub)/de.tudarmstadt.ukp.dkpro.core$de.tudarmstadt.ukp.dkpro.core.doc-asl/doclinks/5/format-reference.html#format-XmlXPath"
                       ] ;
       rdfs:comment "XPath is a language for addressing parts of an XML document, designed to be used by both XSLT and XPointer."@en ;
       rdfs:label "XPath"@en .


###  http://w3id.org/meta-share/omtd-share/aif
:aif rdf:type owl:Class ;
     rdfs:subClassOf :AudioFormat ,
                     [ rdf:type owl:Restriction ;
                       owl:onProperty :hasMimetype ;
                       owl:hasValue :audio_aiff
                     ] ,
                     [ rdf:type owl:Restriction ;
                       owl:onProperty :hasFileExtension ;
                       owl:hasValue "aif"
                     ] ;
     rdfs:label "aif" .


###  http://w3id.org/meta-share/omtd-share/basic
:basic rdf:type owl:Class ;
       rdfs:subClassOf :AudioFormat ,
                       [ rdf:type owl:Restriction ;
                         owl:onProperty :hasMimetype ;
                         owl:hasValue :audio_basic
                       ] ,
                       [ rdf:type owl:Restriction ;
                         owl:onProperty :hasFileExtension ;
                         owl:hasValue "au"
                       ] ,
                       [ rdf:type owl:Restriction ;
                         owl:onProperty :hasFileExtension ;
                         owl:hasValue "snd"
                       ] ;
       rdfs:label "basic" .


###  http://w3id.org/meta-share/omtd-share/mp3
:mp3 rdf:type owl:Class ;
     rdfs:subClassOf :AudioFormat ,
                     [ rdf:type owl:Restriction ;
                       owl:onProperty :hasMimetype ;
                       owl:hasValue :audio_mpeg3
                     ] ,
                     [ rdf:type owl:Restriction ;
                       owl:onProperty :hasMimetype ;
                       owl:hasValue :audio_x_mpeg3
                     ] ,
                     [ rdf:type owl:Restriction ;
                       owl:onProperty :hasFileExtension ;
                       owl:hasValue "mp3"
                     ] ;
     rdfs:label "audio mp3"@en .


###  http://w3id.org/meta-share/omtd-share/mpg
:mpg rdf:type owl:Class ;
     rdfs:subClassOf :AudioFormat ,
                     [ rdf:type owl:Restriction ;
                       owl:onProperty :hasMimetype ;
                       owl:hasValue :audio_mpa
                     ] ,
                     [ rdf:type owl:Restriction ;
                       owl:onProperty :hasMimetype ;
                       owl:hasValue :audio_mpa_robust
                     ] ,
                     [ rdf:type owl:Restriction ;
                       owl:onProperty :hasMimetype ;
                       owl:hasValue :audio_mpeg
                     ] ,
                     [ rdf:type owl:Restriction ;
                       owl:onProperty :hasFileExtension ;
                       owl:hasValue "mpg"
                     ] ;
     rdfs:label "audio mpg" .


###  http://w3id.org/meta-share/omtd-share/wav
:wav rdf:type owl:Class ;
     rdfs:subClassOf :AudioFormat ,
                     [ rdf:type owl:Restriction ;
                       owl:onProperty :hasMimetype ;
                       owl:hasValue :audio_vnd_wave
                     ] ,
                     [ rdf:type owl:Restriction ;
                       owl:onProperty :hasMimetype ;
                       owl:hasValue :audio_wav
                     ] ,
                     [ rdf:type owl:Restriction ;
                       owl:onProperty :hasMimetype ;
                       owl:hasValue :audio_wave
                     ] ,
                     [ rdf:type owl:Restriction ;
                       owl:onProperty :hasMimetype ;
                       owl:hasValue :audio_x_wav
                     ] ,
                     [ rdf:type owl:Restriction ;
                       owl:onProperty :hasFileExtension ;
                       owl:hasValue "wav"
                     ] ;
     rdfs:label "audio wav"@en .


#################################################################
#    Individuals
#################################################################

###  http://w3id.org/meta-share/omtd-share/application_anno_json
:application_anno_json rdf:type owl:NamedIndividual ,
                                :Mimetype ;
                       rdfs:label "application/anno+json" .


###  http://w3id.org/meta-share/omtd-share/application_emma_xml
:application_emma_xml rdf:type owl:NamedIndividual ,
                               :Mimetype ;
                      rdfs:label "application/emma+xml" .


###  http://w3id.org/meta-share/omtd-share/application_fastinfoset
:application_fastinfoset rdf:type owl:NamedIndividual ,
                                  :Mimetype ;
                         rdfs:label "application/fastinfoset" .


###  http://w3id.org/meta-share/omtd-share/application_json
:application_json rdf:type owl:NamedIndividual ,
                           :Mimetype ;
                  rdfs:label "application/json" .


###  http://w3id.org/meta-share/omtd-share/application_ld_json
:application_ld_json rdf:type owl:NamedIndividual ,
                              :Mimetype ;
                     rdfs:label "application/ld+json" .


###  http://w3id.org/meta-share/omtd-share/application_ld_json_profile_http_www_w3_org_ns_anno_jsonld
:application_ld_json_profile_http_www_w3_org_ns_anno_jsonld rdf:type owl:NamedIndividual ,
                                                                     :Mimetype ;
                                                            rdfs:label "application/ld+json;profile=\"http://www.w3.org/ns/anno.jsonld\"" .


###  http://w3id.org/meta-share/omtd-share/application_msword
:application_msword rdf:type owl:NamedIndividual ,
                             :Mimetype ;
                    rdfs:label "application/msword" .


###  http://w3id.org/meta-share/omtd-share/application_pdf
:application_pdf rdf:type owl:NamedIndividual ,
                          :Mimetype ;
                 rdfs:label "application/pdf" .


###  http://w3id.org/meta-share/omtd-share/application_pls_xml
:application_pls_xml rdf:type owl:NamedIndividual ,
                              :Mimetype ;
                     rdfs:label "application/pls+xml" .


###  http://w3id.org/meta-share/omtd-share/application_postscript
:application_postscript rdf:type owl:NamedIndividual ,
                                 :Mimetype ;
                        rdfs:label "application/postscript" .


###  http://w3id.org/meta-share/omtd-share/application_rdf_xml
:application_rdf_xml rdf:type owl:NamedIndividual ,
                              :Mimetype ;
                     rdfs:label "application/rdf+xml" .


###  http://w3id.org/meta-share/omtd-share/application_rtf
:application_rtf rdf:type owl:NamedIndividual ,
                          :Mimetype ;
                 rdfs:label "application/rtf" .


###  http://w3id.org/meta-share/omtd-share/application_tei_xml
:application_tei_xml rdf:type owl:NamedIndividual ,
                              :Mimetype ;
                     rdfs:label "application/tei+xml" .


###  http://w3id.org/meta-share/omtd-share/application_tika
:application_tika rdf:type owl:NamedIndividual ,
                           :Mimetype ;
                  rdfs:label "application/tika" .


###  http://w3id.org/meta-share/omtd-share/application_vnd_msExcel
:application_vnd_msExcel rdf:type owl:NamedIndividual ,
                                  :Mimetype ;
                         rdfs:label "application/vnd.msExcel" .


###  http://w3id.org/meta-share/omtd-share/application_vnd_ms_powerpoint
:application_vnd_ms_powerpoint rdf:type owl:NamedIndividual ,
                                        :Mimetype ;
                               rdfs:label "application/vnd.ms-powerpoint" .


###  http://w3id.org/meta-share/omtd-share/application_vnd_msaccess
:application_vnd_msaccess rdf:type owl:NamedIndividual ,
                                   :Mimetype ;
                          rdfs:label "application/vnd.msaccess" .


###  http://w3id.org/meta-share/omtd-share/application_vnd_oasis_opendocument_presentation
:application_vnd_oasis_opendocument_presentation rdf:type owl:NamedIndividual ,
                                                          :Mimetype ;
                                                 rdfs:label "application/vnd.oasis.opendocument.presentation" .


###  http://w3id.org/meta-share/omtd-share/application_vnd_oasis_opendocument_spreadsheet
:application_vnd_oasis_opendocument_spreadsheet rdf:type owl:NamedIndividual ,
                                                         :Mimetype ;
                                                rdfs:label "application/vnd.oasis.opendocument.spreadsheet" .


###  http://w3id.org/meta-share/omtd-share/application_vnd_oasis_opendocument_text
:application_vnd_oasis_opendocument_text rdf:type owl:NamedIndividual ,
                                                  :Mimetype ;
                                         rdfs:label "application/vnd.oasis.opendocument.text" .


###  http://w3id.org/meta-share/omtd-share/application_vnd_openxmlformats_officedocument_presentationml_presentation
:application_vnd_openxmlformats_officedocument_presentationml_presentation rdf:type owl:NamedIndividual ,
                                                                                    :Mimetype ;
                                                                           rdfs:label "application/vnd.openxmlformats-officedocument.presentationml.presentation" .


###  http://w3id.org/meta-share/omtd-share/application_vnd_openxmlformats_officedocument_spreadsheetml_sheet
:application_vnd_openxmlformats_officedocument_spreadsheetml_sheet rdf:type owl:NamedIndividual ,
                                                                            :Mimetype ;
                                                                   rdfs:label "application/vnd.openxmlformats-officedocument.spreadsheetml.sheet" .


###  http://w3id.org/meta-share/omtd-share/application_vnd_openxmlformats_officedocument_wordprocessingml_document
:application_vnd_openxmlformats_officedocument_wordprocessingml_document rdf:type owl:NamedIndividual ,
                                                                                  :Mimetype ;
                                                                         rdfs:label "application/vnd.openxmlformats-officedocument.wordprocessingml.document" .


###  http://w3id.org/meta-share/omtd-share/application_vnd_xmi_xml
:application_vnd_xmi_xml rdf:type owl:NamedIndividual ,
                                  :Mimetype ;
                         rdfs:label "application/vnd.xmi+xml" .


###  http://w3id.org/meta-share/omtd-share/application_xLatex
:application_xLatex rdf:type owl:NamedIndividual ,
                             :Mimetype ;
                    rdfs:label "application/x-latex" .


###  http://w3id.org/meta-share/omtd-share/application_xMsaccess
:application_xMsaccess rdf:type owl:NamedIndividual ,
                                :Mimetype ;
                       rdfs:label "application/x-msaccess" .


###  http://w3id.org/meta-share/omtd-share/application_xTex
:application_xTex rdf:type owl:NamedIndividual ,
                           :Mimetype ;
                  rdfs:label "application/x-tex" .


###  http://w3id.org/meta-share/omtd-share/application_xTmx_xml
:application_xTmx_xml rdf:type owl:NamedIndividual ,
                               :Mimetype ;
                      rdfs:label "application/x-tmx+xml" .


###  http://w3id.org/meta-share/omtd-share/application_xXces_xml
:application_xXces_xml rdf:type owl:NamedIndividual ,
                                :Mimetype ;
                       rdfs:label "application/x-xces+xml" .


###  http://w3id.org/meta-share/omtd-share/application_xXml_alvis
:application_xXml_alvis rdf:type owl:NamedIndividual ,
                                 :Mimetype ;
                        rdfs:label "application/x-xml+alvis" .


###  http://w3id.org/meta-share/omtd-share/application_x_json_twitter
:application_x_json_twitter rdf:type owl:NamedIndividual ,
                                     :Mimetype ;
                            rdfs:label "application/x-json-twitter" .


###  http://w3id.org/meta-share/omtd-share/application_x_kaf_json
:application_x_kaf_json rdf:type owl:NamedIndividual ,
                                 :Mimetype ;
                        rdfs:label "application/x-kaf+json" .


###  http://w3id.org/meta-share/omtd-share/application_x_org_dkpro_graf_xml
:application_x_org_dkpro_graf_xml rdf:type owl:NamedIndividual ,
                                           :Mimetype ;
                                  rdfs:label "application/x.org.dkpro.graf+xml" .


###  http://w3id.org/meta-share/omtd-share/application_x_org_dkpro_negra3
:application_x_org_dkpro_negra3 rdf:type owl:NamedIndividual ,
                                         :Mimetype ;
                                rdfs:label "application/x.org.dkpro.negra3" .


###  http://w3id.org/meta-share/omtd-share/application_x_org_dkpro_negra4
:application_x_org_dkpro_negra4 rdf:type owl:NamedIndividual ,
                                         :Mimetype ;
                                rdfs:label "application/x.org.dkpro.negra4" .


###  http://w3id.org/meta-share/omtd-share/application_x_org_dkpro_reuters21578_sgml
:application_x_org_dkpro_reuters21578_sgml rdf:type owl:NamedIndividual ,
                                                    :Mimetype ;
                                           rdfs:label "application/x.org.dkpro.reuters21578+sgml" .


###  http://w3id.org/meta-share/omtd-share/application_x_org_dkpro_tgrep2
:application_x_org_dkpro_tgrep2 rdf:type owl:NamedIndividual ,
                                         :Mimetype ;
                                rdfs:label "application/x.org.dkpro.tgrep2" .


###  http://w3id.org/meta-share/omtd-share/application_x_org_dkpro_tiger_xml
:application_x_org_dkpro_tiger_xml rdf:type owl:NamedIndividual ,
                                            :Mimetype ;
                                   rdfs:label "application/x.org.dkpro.tiger+xml" .


###  http://w3id.org/meta-share/omtd-share/application_x_org_dkpro_tuepp_xml
:application_x_org_dkpro_tuepp_xml rdf:type owl:NamedIndividual ,
                                            :Mimetype ;
                                   rdfs:label "application/x.org.dkpro.tuepp+xml" .


###  http://w3id.org/meta-share/omtd-share/application_x_org_dkpro_uima_binary
:application_x_org_dkpro_uima_binary rdf:type owl:NamedIndividual ,
                                              :Mimetype ;
                                     rdfs:label "application/x.org.dkpro.uima+binary" .


###  http://w3id.org/meta-share/omtd-share/application_x_org_dkpro_uima_json
:application_x_org_dkpro_uima_json rdf:type owl:NamedIndividual ,
                                            :Mimetype ;
                                   rdfs:label "application/x.org.dkpro.uima+json" .


###  http://w3id.org/meta-share/omtd-share/application_xhtml_xml
:application_xhtml_xml rdf:type owl:NamedIndividual ,
                                :Mimetype ;
                       rdfs:label "application/xhtml+xml" .


###  http://w3id.org/meta-share/omtd-share/application_xml
:application_xml rdf:type owl:NamedIndividual ,
                          :Mimetype ;
                 rdfs:label "application/xml" .


###  http://w3id.org/meta-share/omtd-share/application_xml_alto
:application_xml_alto rdf:type owl:NamedIndividual ,
                               :Mimetype ;
                      rdfs:label "application/xml+alto" .


###  http://w3id.org/meta-share/omtd-share/audio_aiff
:audio_aiff rdf:type owl:NamedIndividual ,
                     :Mimetype ;
            rdfs:label "audio/aiff" .


###  http://w3id.org/meta-share/omtd-share/audio_basic
:audio_basic rdf:type owl:NamedIndividual ,
                      :Mimetype ;
             rdfs:label "audio/basic" .


###  http://w3id.org/meta-share/omtd-share/audio_mpa
:audio_mpa rdf:type owl:NamedIndividual ,
                    :Mimetype ;
           rdfs:label "audio/MPA" .


###  http://w3id.org/meta-share/omtd-share/audio_mpa_robust
:audio_mpa_robust rdf:type owl:NamedIndividual ,
                           :Mimetype ;
                  rdfs:label "audio/mpa-robust" .


###  http://w3id.org/meta-share/omtd-share/audio_mpeg
:audio_mpeg rdf:type owl:NamedIndividual ,
                     :Mimetype ;
            rdfs:label "audio/mpeg" .


###  http://w3id.org/meta-share/omtd-share/audio_mpeg3
:audio_mpeg3 rdf:type owl:NamedIndividual ,
                      :Mimetype ;
             rdfs:label "audio/mpeg3" .


###  http://w3id.org/meta-share/omtd-share/audio_vnd_wave
:audio_vnd_wave rdf:type owl:NamedIndividual ,
                         :Mimetype ;
                rdfs:label "audio/vnd.wave" .


###  http://w3id.org/meta-share/omtd-share/audio_wav
:audio_wav rdf:type owl:NamedIndividual ,
                    :Mimetype ;
           rdfs:label "audio/wav" .


###  http://w3id.org/meta-share/omtd-share/audio_wave
:audio_wave rdf:type owl:NamedIndividual ,
                     :Mimetype ;
            rdfs:label "audio/wave" .


###  http://w3id.org/meta-share/omtd-share/audio_x_mpeg3
:audio_x_mpeg3 rdf:type owl:NamedIndividual ,
                        :Mimetype ;
               rdfs:label "audio/x-mpeg3" .


###  http://w3id.org/meta-share/omtd-share/audio_x_wav
:audio_x_wav rdf:type owl:NamedIndividual ,
                      :Mimetype ;
             rdfs:label "audio/x-wav" .


###  http://w3id.org/meta-share/omtd-share/text_csv
:text_csv rdf:type owl:NamedIndividual ,
                   :Mimetype ;
          rdfs:label "text/csv" .


###  http://w3id.org/meta-share/omtd-share/text_html
:text_html rdf:type owl:NamedIndividual ,
                    :Mimetype ;
           rdfs:label "text/html" .


###  http://w3id.org/meta-share/omtd-share/text_plain
:text_plain rdf:type owl:NamedIndividual ,
                     :Mimetype ;
            rdfs:label "text/plain" .


###  http://w3id.org/meta-share/omtd-share/text_sgml
:text_sgml rdf:type owl:NamedIndividual ,
                    :Mimetype ;
           rdfs:label "text/sgml" .


###  http://w3id.org/meta-share/omtd-share/text_tabSeparatedValues
:text_tabSeparatedValues rdf:type owl:NamedIndividual ,
                                  :Mimetype ;
                         rdfs:label "text/tab-separated-values" .


###  http://w3id.org/meta-share/omtd-share/text_tcf_xml
:text_tcf_xml rdf:type owl:NamedIndividual ,
                       :Mimetype ;
              rdfs:label "text/tcf+xml" .


###  http://w3id.org/meta-share/omtd-share/text_turtle
:text_turtle rdf:type owl:NamedIndividual ,
                      :Mimetype ;
             rdfs:label "text/turtle" .


###  http://w3id.org/meta-share/omtd-share/text_xCochrane
:text_xCochrane rdf:type owl:NamedIndividual ,
                         :Mimetype ;
                rdfs:label "text/x-cochrane" .


###  http://w3id.org/meta-share/omtd-share/text_xPubmed
:text_xPubmed rdf:type owl:NamedIndividual ,
                       :Mimetype ;
              rdfs:label "text/x-pubmed" .


###  http://w3id.org/meta-share/omtd-share/text_x_anafora
:text_x_anafora rdf:type owl:NamedIndividual ,
                         :Mimetype ;
                rdfs:label "text/x-anafora" .


###  http://w3id.org/meta-share/omtd-share/text_x_brat
:text_x_brat rdf:type owl:NamedIndividual ,
                      :Mimetype ;
             rdfs:label "text/x-brat" .


###  http://w3id.org/meta-share/omtd-share/text_x_org_dkpro_conll2000
:text_x_org_dkpro_conll2000 rdf:type owl:NamedIndividual ,
                                     :Mimetype ;
                            rdfs:label "text/x.org.dkpro.conll-2000" .


###  http://w3id.org/meta-share/omtd-share/text_x_org_dkpro_conll2002
:text_x_org_dkpro_conll2002 rdf:type owl:NamedIndividual ,
                                     :Mimetype ;
                            rdfs:label "text/x.org.dkpro.conll-2002" .


###  http://w3id.org/meta-share/omtd-share/text_x_org_dkpro_conll2003
:text_x_org_dkpro_conll2003 rdf:type owl:NamedIndividual ,
                                     :Mimetype ;
                            rdfs:label "text/x.org.dkpro.conll-2003" .


###  http://w3id.org/meta-share/omtd-share/text_x_org_dkpro_conll2006
:text_x_org_dkpro_conll2006 rdf:type owl:NamedIndividual ,
                                     :Mimetype ;
                            rdfs:label "text/x.org.dkpro.conll-2006" .


###  http://w3id.org/meta-share/omtd-share/text_x_org_dkpro_conll2008
:text_x_org_dkpro_conll2008 rdf:type owl:NamedIndividual ,
                                     :Mimetype ;
                            rdfs:label "text/x.org.dkpro.conll-2008" .


###  http://w3id.org/meta-share/omtd-share/text_x_org_dkpro_conll2009
:text_x_org_dkpro_conll2009 rdf:type owl:NamedIndividual ,
                                     :Mimetype ;
                            rdfs:label "text/x.org.dkpro.conll-2009" .


###  http://w3id.org/meta-share/omtd-share/text_x_org_dkpro_conll2012
:text_x_org_dkpro_conll2012 rdf:type owl:NamedIndividual ,
                                     :Mimetype ;
                            rdfs:label "text/x.org.dkpro.conll-2012" .


###  http://w3id.org/meta-share/omtd-share/text_x_org_dkpro_conllU
:text_x_org_dkpro_conllU rdf:type owl:NamedIndividual ,
                                  :Mimetype ;
                         rdfs:label "text/x.org.dkpro.conll-u" .


###  http://w3id.org/meta-share/omtd-share/text_x_org_dkpro_imscwb
:text_x_org_dkpro_imscwb rdf:type owl:NamedIndividual ,
                                  :Mimetype ;
                         rdfs:label "text/x.org.dkpro.imscwb" .


###  http://w3id.org/meta-share/omtd-share/text_x_org_dkpro_ngram
:text_x_org_dkpro_ngram rdf:type owl:NamedIndividual ,
                                 :Mimetype ;
                        rdfs:label "text/x.org.dkpro.ngram" .


###  http://w3id.org/meta-share/omtd-share/text_x_org_dkpro_ptbChunked
:text_x_org_dkpro_ptbChunked rdf:type owl:NamedIndividual ,
                                      :Mimetype ;
                             rdfs:label "text/x.org.dkpro.ptb-chunked" .


###  http://w3id.org/meta-share/omtd-share/text_x_org_dkpro_ptbCombined
:text_x_org_dkpro_ptbCombined rdf:type owl:NamedIndividual ,
                                       :Mimetype ;
                              rdfs:label "text/x.org.dkpro.ptb-combined" .


###  http://w3id.org/meta-share/omtd-share/text_x_org_dkpro_reuters21578
:text_x_org_dkpro_reuters21578 rdf:type owl:NamedIndividual ,
                                        :Mimetype ;
                               rdfs:label "text/x.org.dkpro.reuters21578" .


###  http://w3id.org/meta-share/omtd-share/text_xml
:text_xml rdf:type owl:NamedIndividual ,
                   :Mimetype ;
          rdfs:label "text/xml" .


###  Generated by the OWL API (version 5.1.11) https://github.com/owlcs/owlapi/
