@prefix : <http://w3id.org/meta-share/omtd-share/> .
@prefix dc: <http://purl.org/dc/elements/1.1/> .
@prefix dct: <http://purl.org/dc/terms/> .
@prefix grddl: <http://www.w3.org/2003/g/data-view#> .
@prefix owl: <http://www.w3.org/2002/07/owl#> .
@prefix rdf: <http://www.w3.org/1999/02/22-rdf-syntax-ns#> .
@prefix rdfs: <http://www.w3.org/2000/01/rdf-schema#> .
@prefix skos: <http://www.w3.org/2004/02/skos/core#> .
@prefix xsd: <http://www.w3.org/2001/XMLSchema#> .

<http://w3id.org/meta-share/omtd-share/> a owl:Ontology .

:FactChecking a skos:Concept;
  rdfs:label "Fact checking"@en;
  skos:altLabel "Fact-checking"@en;
  skos:broader :InformationExtraction;
  skos:definition "The act of checking factual assertions in non-fictional text in order to determine the veracity and correctness of the factual statements in the text [from Wikipedia]"@en;
  skos:inScheme :OperationScheme;
  skos:prefLabel "Fact checking"@en;
  skos:related :FakeNewsDetection .

:Mimetype a skos:Concept;
  rdfs:label "Mimetype"@en;
  skos:inScheme :MimeTypeScheme;
  skos:prefLabel "Mimetype"@en;
  skos:topConceptOf :MimeTypeScheme .

:TdmMethod a skos:Concept;
  rdfs:label "TDM/LT Method"@en;
  skos:definition "The method used by a TDM/LT algorithm"@en;
  skos:inScheme :TdmMethodScheme;
  skos:narrower :Crowdsourcing, :FiniteStateTechnology, :MachineAndStatisticalLearningMethod,
    :MachineLearningMethod, :RuleBasedMethod, :StatisticalLearningMethod;
  skos:prefLabel "TDM/LT Method"@en;
  skos:topConceptOf :TdmMethodScheme .

:VideoFormat a skos:Concept;
  skos:broader :DataFormat;
  skos:definition "Any format used for video files"@en;
  skos:inScheme :DataFormatScheme;
  skos:narrower :avi, :mp4 .

:ParallelSentenceExtraction a skos:Concept;
  rdfs:label "Parallel sentence extraction"@en;
  skos:broader :MachineTranslationSupport;
  skos:definition "The task/process of identifying parallel sentences (i.e. sentences that have the same sense in different languages) in parallel texts"@en;
  skos:inScheme :OperationScheme;
  skos:prefLabel "Parallel sentence extraction"@en .

:ComponentType a skos:Concept;
  rdfs:label "Component type"@en;
  skos:definition "Specifies the type of a component, in terms of the function/task it performs"@en;
  skos:inScheme :ComponentTypeScheme;
  skos:narrower :AccessComponent, :Analyzer, :PreOrPostProcessor, :Processor, :SupportComponent;
  skos:prefLabel "Component type"@en;
  skos:topConceptOf :ComponentTypeScheme .

:CorpusFormat a skos:Concept;
  rdfs:label "Corpus format"@en;
  skos:broader :DataFormat;
  skos:definition "A format used by a specific type of corpus (collection of texts)"@en;
  skos:inScheme :DataFormatScheme;
  skos:narrower :AclAnthologyCorpusFormat, :AimedCorpusFormat, :BncFormat, :Imscwb,
    :KeaCorpus, :MOSESFormat, :Nif, :Reuters21578Sgml, :Reuters21578Txt, :Tcf, :TigerXml,
    :Tuepp, :WARC, :Web1t;
  skos:prefLabel "Corpus format"@en .

:FeatureExtraction skos:inScheme :ModelFunctionScheme .

:FrequencyCount skos:inScheme :ModelFunctionScheme .

:QuestionAnswering skos:inScheme :ModelFunctionScheme .

:Summarization skos:inScheme :ModelFunctionScheme .

:ZeroShotClassification skos:inScheme :ModelFunctionScheme .

:Zip :hasFileExtension "zip"@en .

:ConllFormat a skos:Concept;
  rdfs:label "CoNLL format"@en;
  skos:broader :AnnotationFormat, :TabularFormat;
  skos:definition "Formats used in the CoNLL Shared Tasks"@en;
  skos:inScheme :DataFormatScheme;
  skos:narrower :Conll2000, :Conll2002, :Conll2003, :Conll2006, :Conll2008, :Conll2009,
    :Conll2012, :ConllU;
  skos:prefLabel "CoNLL format"@en .

:DiscourseAnalysis a skos:Concept;
  rdfs:label "Discourse analysis"@en;
  skos:broader :LinguisticAnalysis;
  skos:definition "A method of analysing the structure of texts or utterances longer than one sentence, taking into account both their linguistic content and their sociolinguistic context; analysis performed using this method.[OED, https://en.oxforddictionaries.com/definition/discourse_analysis]"@en;
  skos:inScheme :OperationScheme;
  skos:prefLabel "Discourse analysis"@en .

:DocumentFormat a skos:Concept;
  rdfs:label "Document format"@en;
  skos:broader :DataFormat;
  skos:definition "Any format used for documents (textual resources)"@en;
  skos:inScheme :DataFormatScheme;
  skos:narrower :BionlpFormat, :BionlpFormats, :Cochrane, :Html, :LD_json, :Latex, :MsExcel,
    :MsPowerpoint, :MsWord, :OasisPresentation, :OasisSpreadsheet, :OasisText, :OpenOfficeDocument,
    :OpenOfficePresentation, :OpenOfficeSpreadsheet, :Pdf, :Pls, :Postscript, :Pubmed,
    :Rtf, :Sgml, :Tex, :Text, :Tika, :Xhtml, :Xmi;
  skos:prefLabel "Document format"@en .

:NamedEntityRecognition a skos:Concept;
  rdfs:label "Named Entity Recognition"@en;
  skos:altLabel "Entity Identification"@en, "Entity Recognition"@en, "Entity extraction"@en,
    "NER"@en, "NERC"@en;
  skos:definition "A subtask of information extraction that seeks to locate and classify named entities in text into pre-defined categories such as the names of persons, organizations, locations, expressions of times, quantities, monetary values, percentages, etc."@en,
    "Named entity (NE) recognition is a form of information extraction in which the major task is to identify and classify from NL text every word or sequence of words as being a person-name, organizaton, location, date, time, monetary value, percentage expression. NE recognition has a high impact for a number of applications, like e.g., InterNet search engines, text data mining or answer extraction."@en;
  skos:editorialNote "can also be annotation"@en;
  skos:inScheme :OperationScheme;
  skos:narrower :NamedEntityDisambiguation;
  skos:prefLabel "Named Entity Recognition"@en .

:FacialExpressionRecognition skos:broader :OperationWithMultimediaInputOrOutput .

:SemanticAnnotation a skos:Concept;
  rdfs:label "Semantic annotation"@en;
  skos:broader :TextAnnotation;
  skos:inScheme :OperationScheme;
  skos:narrower :AnnotationOfMeasurements, :AnnotationOfNumbers, :AnnotationOfQuestionTopics,
    :AnnotationOfTextualEntailment, :CertaintyLevelLabelling, :EntityLinking, :EventLabelling,
    :FrameSemanticParsing, :PolarityLabelling, :SemanticClassLabelling, :SemanticRelationLabelling,
    :SemanticRoleLabelling, :SpatialRoleLabelling, :TemporalExpressionsLabelling, :TerminologyMarkup;
  skos:prefLabel "Semantic annotation"@en .

:KnowledgeAcquisition a skos:Concept;
  rdfs:label "Knowledge acquisition"@en;
  skos:broader :TextAndDataMining;
  skos:definition "The process/task of extracting, organising and systematising knowledge usually of a specific domain from external sources so that it can be used in a knowledge-based system"@en;
  skos:inScheme :OperationScheme;
  skos:narrower :BilingualLexiconInduction, :LexiconAcquisitionFromCorpora, :LexiconEnhancement,
    :LexiconExtractionFromLexica, :OntologyAcquisition, :OntologyEnhancement;
  skos:prefLabel "Knowledge acquisition"@en .

:CoreferenceAnnotation a skos:Concept;
  rdfs:label "Coreference annotation"@en;
  skos:altLabel "Co-reference annotation"@en, "Coreference identification"@en;
  skos:broader :DiscourseAnnotation;
  skos:definition "The task/process of attaching tags to a text unit and linking it to other text units that refer to the same entity in the world"@en;
  skos:inScheme :OperationScheme;
  skos:prefLabel "Coreference annotation"@en;
  skos:related :AnaphoraAnnotation .

:SupportOperation a skos:Concept;
  rdfs:label "Support operation"@en;
  skos:broader :Operation;
  skos:definition "Any operation that is used to support LT tasks, either for creating workflows or for executing them"@en;
  skos:inScheme :OperationScheme;
  skos:narrower :BuildingOfFiniteStateAutomata, :CommentFiltering, :CorpusManagement,
    :DataCollection, :DataMerging, :DataSplitting, :Debugging, :Editing, :FeatureExtraction,
    :FillMask, :FlowControl, :FormatConversion, :InformationStorage, :LanguageModelling,
    :LinguisticAnalysis, :MachineTranslationSupport, :Matching, :NlpDevelopmentSupport,
    :Normalization, :ResourceAccess, :ScriptBasedAnalysis, :SupportOfCrowdsourcingTasks,
    :SupportOperationForKnowledgeResources, :TagsetConversion, :TerminologyManagement,
    :TranslationMemoryManagement, :TranslationProjectManagement, :UnicodeConformTokenizing,
    :UserAuthentication, :Validation, :Viewing, :Visualization, :ZeroShotClassification;
  skos:prefLabel "Support operation"@en .

:audio_flac rdfs:label "audio/flac" .

:Search a skos:Concept .

:OasisSpreadsheet a skos:Concept;
  :hasMimetype :application_vnd_oasis_opendocument_spreadsheet;
  rdfs:label "Oasis spreadsheet"@en;
  skos:broader :DocumentFormat, :OpenFormat, :TabularFormat;
  skos:inScheme :DataFormatScheme;
  skos:prefLabel "Oasis spreadsheet"@en .

:avi a skos:Concept;
  :hasFileExtension "avi";
  :hasMimetype :video_avi;
  rdfs:label "AVI"@en;
  skos:altLabel "Audio Video Interleave"@en;
  skos:broader :VideoFormat;
  skos:inScheme :DataFormatScheme;
  skos:prefLabel "AVI"@en .

:UimaCasFormat a skos:Concept;
  rdfs:label "UIMA CAS format"@en;
  skos:broader :DataFormat;
  skos:definition "Formats used for the UIMA CAS (Common Analysis System) objects"@en;
  skos:inScheme :DataFormatScheme;
  skos:narrower :BinaryCas, :SerializedCas, :Uima_json;
  skos:prefLabel "UIMA CAS format"@en .

:application_x_org_dkpro_graf_xml a owl:NamedIndividual, skos:Concept;
  rdfs:label "application/x.org.dkpro.graf+xml" .

:ContentMining a skos:Concept;
  rdfs:label "Content Mining"@en;
  skos:broader :Operation;
  skos:definition "The automated analysis of large volumes of content of any form or medium (e.g. text, images, videos, graphs, metadata etc.) that leads to the discovery of previously undiscovered information (e.g. identification of relationships between entities)."@en;
  skos:inScheme :OperationScheme;
  skos:prefLabel "Content Mining"@en;
  skos:related :TextAndDataMining .

:Blikiwikipedia :documentationUrl "https://dkpro.github.io/dkpro-core/releases/1.8.0/docs/format-reference.html#format-de.tudarmstadt.ukp.dkpro.core.io.bliki-asl";
  skos:broader :WikipediaFormat .

:TextProcessingCollection a skos:Collection;
  rdfs:label "Text Processing Collection"@en;
  skos:member :Alignment, :AnaphoraAnnotation, :AnaphoraResolution, :AnnotationOfCompounds,
    :AnnotationOfDates, :AnnotationOfDerivationalFeatures, :AnnotationOfDocumentStructure,
    :AnnotationOfMeasurements, :AnnotationOfMultiWordUnits, :AnnotationOfNumbers, :AnnotationOfQuestionTopics,
    :AnnotationOfTextualEntailment, :Anonymization, :Argumentation, :AuthorClassification,
    :AuthoringSupport, :BelowPosTagging, :BiomedicalConceptNormalization, :BuildingOfFiniteStateAutomata,
    :CertaintyLevelLabelling, :Chunking, :CoReferenceResolution, :CommentFiltering, :ConceptNormalization,
    :ConstituencyParsing, :CoreferenceAnnotation, :Crawling, :DataCollection, :DataMasking,
    :DataMerging, :DataSplitting, :DeepParserPerformanceEvaluation, :DeepParsing, :DependencyParsing,
    :DerivationalAnalysis, :DiscourseAnalysis, :DiscourseAnnotation, :DiscourseModelling,
    :DocumentComparison, :Editing, :EntityLinking, :EvaluationOfBroadCoverageNaturalLanguageParsers,
    :EventLabelling, :FrameSemanticParsing, :GrammarChecking, :IntraDocumentCoReferenceResolution,
    :L2WritingSupport, :LanguageChecking, :LanguageIdentification, :Lemmatization, :LinguisticAnalysis,
    :MorphologicalAnalysis, :MorphologicalAnnotation, :MorphosyntacticTagging, :NamedEntityDisambiguation,
    :NamedEntityRecognition, :Normalization, :NormalizationOfMeasurements, :NormalizationOfNumbers,
    :NounPhraseChunking, :ParagraphSplitting, :Paraphrasing, :Parsing, :PhraseAlignment,
    :PolarityLabelling, :PosTagging, :Pseudonymization, :ReadabilityAnnotation, :RecognizingTextualEntailment,
    :RelationExtraction, :SemanticAnnotation, :SemanticClassLabelling, :SemanticRelationLabelling,
    :SemanticRoleLabelling, :SentenceAlignment, :SentenceSimilarityAssessment, :SentenceSplitting,
    :SentimentAnalysis, :SpatialRoleLabelling, :SpellChecking, :Stemming, :StructuralAnnotation,
    :Summarization, :SyllableSegmentation, :TaskOrientedTextAnalysisEvaluation, :TemporalExpressionsLabelling,
    :TerminologyMarkup, :TextAndDataAnalytics, :TextAnnotation, :TextCategorization, :TextCompression,
    :TextEncryption, :TextIndexing, :TextSimilarityAssessment, :TextSimplification, :Tokenization,
    :TopicDetection, :Transliteration, :UnicodeConformTokenizing, :WordAlignment, :WordSegmentation,
    :WordSenseDisambiguation, :WordSenseInduction;
  skos:prefLabel "Text Processing Collection"@en .

:application_rdf_xml skos:broader :Mimetype .

:AnnotationFormat a skos:Concept;
  rdfs:label "Annotation format"@en;
  skos:broader :DataFormat;
  skos:definition "Any format used for annotated files"@en;
  skos:inScheme :DataFormatScheme;
  skos:narrower :ANNIS, :AlvisEnrichedDocumentFormat, :Anafora, :BLAST, :Brat, :Cadixe_json,
    :Chat, :ConllFormat, :Diaml, :DkproTokenized, :EAF, :Emma, :FactoredTagLemFormat,
    :Folia, :Graf, :Html5Microdata, :I2b2, :InlineXml, :Kaf, :Lll, :MalletLdaTopicProportions,
    :MalletLdaTopicProportionsSorted, :MsExcel, :Naf, :NegraExport, :Nif, :Pml, :Ptb,
    :Tcf, :Tei, :Tgrep2, :TigerXml, :Tmx, :Tuepp, :WebAnnotationFormat, :Xces;
  skos:prefLabel "Annotation format"@en .

:RepresentationOfSpaceAndTime a skos:Concept;
  rdfs:label "Representation of space and time"@en;
  skos:broader :InformationExtraction;
  skos:definition "The representation of time and space plays a crucial role in Artificial Intelligence and Computational Linguistics, but also in practical areas such as business intelligence or geographical information systems. Representing time and space properly eases querying and reasoning thereof. <br /> <br /> Geographic information systems use traditional techniques from image processing and CAD, like a pixel/raster or a vector representation of spatial data. Temporal data bases extend tradional relational data models by the notion of <i>valid time</i> and <i>transaction time</i>. <br /> <br /> When we speak of time, we mean a linear, dense, and one-dimensional time. With space, we usually refer to a two- or three-dimensional space, often using a latitude/longitude measurement in degrees in case of a spherical 2D geometry or a system of coordinates/trajectories for a Euclidean 2D/3D space. Classical observable spacetime then refers to a 3+1-dimensional continuum in which physical objects move through time and space (Tegmark 1997). Even abstract events or processes can be seen to take place in 4D spacetime. Physical and abstract 4D entities are usually composed of simpler entities -- here, both time and space are the glue to achieve a decomposition. For instance, Allen (1984) has defined a natural system of 13 temporal topological relations. Randell et al. (1992) came up with a logic (later called RCC) to support qualitative reasoning about space. <br /> <br /> Human natural language usually comes up with means to refer to time and space, for instance through the use of temporal and spatial prepositions, adverbs, or verb tense and aspect (Vendler 1967, Moens &amp; Steedman 1988, Herskovits 1986). Several algorithms exist which compute the temporal structure of a discourse (e.g., Hitzeman et al. 1995). When constructing mental models of space derived from text, it has been shown that the representation is more topological than Euclidean (Langston et al. 1998). <br /> <br /> Within theoretical and computational linguistics, type-logical semantics and categorial grammar have given a rigorous account to tense, aspect, and temporal modification through the use of a possible-worlds semantics (see, e.g., Carpenter 1997). <br /> <br /> Studying time from a formal perspective, focussing on the inherent properties of a theory, has a long tradition in logic (e.g., Hayes 1995), artificial intelligence (e.g., McDermott 1982), description logics (e.g., Bry &amp; Spranger 2003, Lutz 2004), or data base theory (Date et al. 2002). <br /> <br /> Looking from a more practical viewpoint on time, a number of frameworks have been proposed within the World Wide Web Consortium W3C: (i) ISO 8601 is an international standard for date and time representations issued by the International Organization for Standardization (Wolf &amp; Wicksteed 1998); (ii) XSD (XML Schema Datatypes) comes up with a number of built-in primitive datatype for time and date (Peterson et al. 2008); (iii) OWL-Time (formerly DAML-Time; see Hobbs &amp; Pan 2004) is an OWL ontology of temporal concepts and properties for describing the temporal content of Web pages and the temporal properties of Web services. <br /> <br /> Representing changing relationships over time and space is related to the problem of diachronic identity which describes the identification of individuals that look different at different times, but still refer to the same entity. The four-dimensional or perdurantist view assumes that all entities (the perdurants) only exist for some period of time. Entities under this view are sometimes refered to as <i>spacetime worms</i> (Sider 2001), since a 4D trajectory is all one needs to identify/follow a perdurant through time and space. Parts of such a worm are called <i>time slices</i>, encoding cooccurent information that stay constant over the specified period of time. There exist several well-known techniques of extending a relation with time and space: (i) equip the relation with further arguments as is done in temporal data bases; (ii) apply a meta-logical predicate (McCarthy &amp; Hayes 1969); (iii) reifiy the original relation as used in RDF (Manola &amp; Miller 2004). Unfortunately, (i) and (ii) are not applicable to OWL (Smith et al. 2004), whereas (iii) requires ontology rewriting. Welty &amp; Fikes (2006) and Krieger et al. (2008) present alternative approaches compatible with OWL."@en;
  skos:inScheme :OperationScheme;
  skos:prefLabel "Representation of space and time"@en .

:Localization a skos:Concept;
  rdfs:label "Localization"@en;
  skos:altLabel "Localisation"@en-uk;
  skos:broader :Translation;
  skos:definition "The process of adapting a product or content to a specific locale or market, including translation of relevant language material but also converting to local measures and currency units, modifications necessary to adapt to cultural differences of the target audience, etc. [adapted from https://www.gala-global.org/industry/intro-language-industry/what-localization]"@en;
  skos:inScheme :OperationScheme;
  skos:prefLabel "Localization"@en .

:Validation a skos:Concept;
  rdfs:label "Validation"@en;
  skos:broader :Operation, :SupportOperation;
  skos:definition "The task/process of confirming that a system/data resource meets the specifications and fulfills its intended purpose"@en;
  skos:inScheme :OperationScheme;
  skos:prefLabel "Validation"@en .

:Json a skos:Concept;
  rdfs:label "JSON"@en;
  skos:broader :DataFormat;
  skos:definition "Superclass of JSON formats"@en;
  skos:inScheme :DataFormatScheme;
  skos:narrower :Avro_json, :Cadixe_json, :Datasift_json, :Gate_twitter_json, :JsonL,
    :Json_genia, :Kaf, :LD_json, :Uima_json, :WebAnnotationFormat;
  skos:prefLabel "JSON"@en .

:NlpDevelopmentSupport a skos:Concept;
  rdfs:label "NLP Development Support"@en;
  skos:altLabel "NLP Development Aid"@en;
  skos:broader :SupportOperation;
  skos:definition "";
  skos:inScheme :OperationScheme;
  skos:prefLabel "NLP Development Support"@en .

:HandwritingRecognition a skos:Concept;
  rdfs:label "Handwriting recognition"@en;
  skos:altLabel "HWR"@en;
  skos:broader :OperationWithMultimediaInputOrOutput;
  skos:definition "The ability of a computer to receive and interpret intelligible handwritten input from sources such as paper documents, photographs, touch-screens and other devices [from Wikipedia]"@en;
  skos:inScheme :OperationScheme;
  skos:prefLabel "Handwriting recognition"@en .

:Annotator a skos:Concept;
  :performsOperation :Annotation;
  rdfs:label "Annotator"@en;
  skos:altLabel "Tagger"@en;
  skos:broader :Processor;
  skos:definition "A component that annotates any data (text, video, audio etc.), i.e. adds any descriptive or analytic notations (structural, linguistic, etc) to raw data"@en;
  skos:inScheme :ComponentTypeScheme;
  skos:narrower :Aligner, :Chunker, :CoReferenceAnnotator, :Lemmatizer, :MorphologicalTagger,
    :NamedEntitityRecognizer, :Parser, :Segmenter, :SemanticAnnotator, :Stemmer;
  skos:prefLabel "Annotator"@en .

:GrammarChecker a skos:Concept;
  rdfs:label "Grammar checker"@en;
  skos:broader :PreOrPostProcessor;
  skos:definition "A component that corrects grammatical mistakes in a text"@en;
  skos:inScheme :ComponentTypeScheme;
  skos:prefLabel "Grammar checker"@en .

:SemanticRoleLabelling a skos:Concept;
  rdfs:label "Semantic role labelling"@en;
  skos:altLabel "Semantic role labeling [en-US]"@en-us;
  skos:broader :SemanticAnnotation;
  skos:definition "The task/process of attaching labels that correspond to the roles that the arguments of a predicate take in an event"@en;
  skos:inScheme :OperationScheme;
  skos:prefLabel "Semantic role labelling"@en .

:Parser a skos:Concept;
  rdfs:label "Parser"@en;
  skos:altLabel "Syntactic analyzer"@en;
  skos:broader :Annotator;
  skos:definition "A component that takes as input text and returns a form of data structure (e.g. syntactic parse as a tree, or bracketed structure etc.)"@en;
  skos:inScheme :ComponentTypeScheme;
  skos:narrower :ConstituencyParser, :DependencyParser;
  skos:prefLabel "Parser"@en .

:StructuralAnnotationType a skos:Concept;
  rdfs:label "Structural annotation type"@en;
  skos:broader :AnnotationType;
  skos:definition "Any type of annotation that pertains to the structure of a document"@en;
  skos:inScheme :AnnotationTypeScheme;
  skos:narrower :Clause, :DocumentSection, :MultiWordUnit, :Paragraph, :Phrase, :Sentence,
    :Token, :Word;
  skos:prefLabel "Structural annotation type"@en .

:ImageVideoProcessingCollection a skos:Collection;
  rdfs:label "Image / Video Processing Collection"@en;
  skos:member :AvatarSynthesis, :DocumentImageAnalysis, :EmotionGeneration, :FaceDetection,
    :FaceRecognition, :FaceVerification, :FacialExpressionRecognition, :HandwritingRecognition,
    :ImageClassification, :ImageGeneration, :ImageProcessing, :ImageSegmentation, :ImageTranslation,
    :ImageUnderstanding, :MultimediaAnnotation, :MultimediaDevelopment, :MultimediaDocumentProcessing,
    :MultimediaInformationExtraction, :MultimodalIntegration, :ObjectDetection, :OpticalCharacterRecognition,
    :PersonIdentification, :SignLanguageGeneration, :SignLanguageRecognition, :TextToImageGeneration;
  skos:prefLabel "Image / Video Processing Collection"@en .

:KeaCorpus skos:prefLabel "KEA corpus"@en .

:MultimodalSynthesis a skos:Concept;
  rdfs:label "Multimodal synthesis"@en .

:SupportComponent a skos:Concept;
  :performsOperation :SupportOperation;
  rdfs:label "Support component"@en;
  skos:altLabel "Helper"@en;
  skos:broader :ComponentType;
  skos:definition "A component that provides support to developers"@en;
  skos:inScheme :ComponentTypeScheme;
  skos:narrower :Converter, :CrowdsourcingComponent, :DataCollector, :DataMerger, :DataSplitter,
    :Debugger, :Editor, :Evaluator, :FeatureExtractor, :FlowController, :MachineLearningPredictor,
    :Matcher, :ScriptBasedAnalyser, :SoftwareDevelopmentEnvironment, :TrainerOfMachineLearningModels,
    :Validator, :Viewer, :Visualiser;
  skos:prefLabel "Support component"@en .

:AnnotationOfDates a skos:Concept;
  rdfs:label "Annotation of dates"@en;
  skos:altLabel "Date Detection"@en, "Date Recognition"@en;
  skos:broader :TemporalExpressionsLabelling;
  skos:definition "The task/process of marking dates in a text"@en;
  skos:inScheme :OperationScheme;
  skos:prefLabel "Annotation of dates"@en .

:OperationWithMultimediaInputOrOutput a skos:Concept;
  rdfs:label "Operation with multimedia input or output"@en;
  skos:broader :Operation;
  skos:inScheme :OperationScheme;
  skos:narrower :AudioProcessing, :EmotionGeneration, :FaceDetection, :FaceRecognition,
    :FaceVerification, :HumanComputerInteraction, :ImageClassification, :ImageGeneration,
    :ImageProcessing, :ImageSegmentation, :MultimediaDevelopment, :MultimediaDocumentProcessing,
    :MultimodalIntegration, :ObjectDetection, :PersonIdentification, :SignLanguageGeneration,
    :SignLanguageRecognition, :SpeechAssistedVideoControl, :SpeechRecognition, :TalkingHeadSynthesis;
  skos:prefLabel "Operation with multimedia input or output"@en .

:application_rdf_xml skos:inScheme :MimeTypeScheme;
  a skos:Concept .

:Tei a skos:Concept;
  :documentationUrl "http://www.tei-c.org/index.xml", "https://www.iana.org/assignments/media-types/application/tei+xml";
  :hasMimetype :application_tei_xml;
  rdfs:label "TEI"@en;
  skos:altLabel "Text Encoding Initiative"@en;
  skos:broader :AnnotationFormat, :Xml;
  skos:definition "Data format for TEI-encoded (Text Encoding Initiative) texts"@en;
  skos:inScheme :DataFormatScheme;
  skos:prefLabel "TEI"@en .

:ParagraphSplitting a skos:Concept;
  rdfs:label "Paragraph splitting"@en;
  skos:altLabel "Paragraph segmentation"@en;
  skos:broader :StructuralAnnotation;
  skos:definition "The task/process of segmenting a text into paragraphs and marking their boundaries"@en;
  skos:inScheme :OperationScheme;
  skos:prefLabel "Paragraph splitting"@en .

:SyntacticAnnotationType a skos:Concept;
  rdfs:label "Syntactic annotation type"@en;
  owl:equivalentClass <http://purl.org/olia/olia-top.owl#SyntacticCategory>;
  skos:broader :AnnotationType;
  skos:definition "Any type of annotation that pertains to the syntactic level"@en;
  skos:inScheme :AnnotationTypeScheme;
  skos:narrower :Chunk, :ConstituencyTree, :Constituent, :Dependency, :DependencyTree,
    :SubcategorizationFrame, :SyntacticoSemanticLink;
  skos:prefLabel "Syntactic annotation type"@en .

:Analyzer a skos:Concept;
  rdfs:label "Analyzer"@en;
  skos:altLabel "Extractor"@en;
  skos:broader :ComponentType;
  skos:definition "A component that is used for analyzing an input text in order to extract specific features/information (e.g. word list), or to produce statements over the whole text (e.g. classify it by topic)"@en;
  skos:inScheme :ComponentTypeScheme;
  skos:narrower :ContradictionDetector, :Disambiguator, :DocumentClassifier, :EmotionRecognizer,
    :EventExtractor, :InformationExtractor, :KeywordExtractor, :LanguageIdentifier, :LexiconExtractorFromCorpora,
    :LexiconExtractorFromLexica, :PersuasiveExpressionMiner, :SentimentAnalyzer, :TermExtractor,
    :TopicExtractor, :VariablesDectector;
  skos:prefLabel "Analyzer"@en .

:EmotionLabelling a skos:Concept;
  rdfs:label "Emotion labelling"@en;
  skos:altLabel "Emotion labeling [en-US]"@en-us;
  skos:broader :InformationExtraction;
  skos:definition "The process/task of identifying types of feelings (e.g. anger, fear, happiness, sadness, etc.) in the linguistic expression of texts or facial expressions"@en;
  skos:inScheme :OperationScheme;
  skos:prefLabel "Emotion labelling"@en .

:ImageFormat a skos:Concept;
  rdfs:label "Image format"@en;
  skos:broader :DataFormat;
  skos:definition "Any format used for image files"@en;
  skos:inScheme :DataFormatScheme;
  skos:narrower :bmp, :gif, :jpg, :png, :svg, :tiff;
  skos:prefLabel "Image format"@en .

:Lll a skos:Concept;
  :documentationUrl "https://builds.openminted.eu/job/WP%205.2%20-%20Typesystem%20alignment/eu.openminted.interop$mapping-conversion/doclinks/1/components.html#_lll_1";
  rdfs:label "LLL"@en;
  skos:broader :AnnotationFormat;
  skos:definition "Format of the LLL challenge"@en;
  skos:inScheme :DataFormatScheme;
  skos:prefLabel "LLL"@en .

:Operation a skos:Concept;
  rdfs:label "Operation"@en;
  skos:altLabel "Function"@en, "Task"@en;
  skos:definition "The action that a software program performs or is meant to perform, and, in a broader sense, the application area where this software or relevant resources can be deployed"@en;
  skos:inScheme :OperationScheme;
  skos:narrower :Annotation, :AuthoringSupport, :ContentMining, :Evaluation, :LanguageTechnology,
    :NaturalLanguageGeneration, :NaturalLanguageUnderstanding, :OperationWithMultimediaInputOrOutput,
    :SupportOperation, :TextAndDataMining, :TextSpeechDataAnalytics, :Translation;
  skos:prefLabel "Operation"@en;
  skos:topConceptOf :OperationScheme .

:KeaCorpus skos:definition "KEA-style (Keyphrase Extraction Algorithm) corpus"@en .

:OfficialText skos:broader :SocialSciencesEntity .

:FillMask skos:broader :ModelFunction .

:image_png skos:broader :Mimetype .

:AllbusVariable a skos:Concept;
  rdfs:label "ALLBUS variable"@en;
  skos:broader :SocialSciencesEntity;
  skos:inScheme :AnnotationTypeScheme;
  skos:prefLabel "ALLBUS variable"@en .

:FiniteStateTechnology a skos:Concept;
  rdfs:label "Finite state technology"@en;
  skos:broader :TdmMethod;
  skos:definition "In data communications, flow control is the process of managing the rate of data transmission between two nodes to prevent a fast sender from overwhelming a slow receiver. It provides a mechanism for the receiver to control the transmission speed, so that the receiving node is not overwhelmed with data from transmitting node."@en;
  skos:inScheme :TdmMethodScheme;
  skos:prefLabel "Finite state technology"@en;
  skos:related :BuildingOfFiniteStateAutomata .

:TextToSpeechSynthesis a skos:Concept;
  rdfs:label "Text-to-Speech Synthesis"@en;
  owl:equivalentClass :SpeechSynthesis;
  skos:altLabel "TTS"@en, "Text to Speech Synthesis"@en;
  skos:broader :NaturalLanguageGeneration;
  skos:definition "The generation of synthetic speech from text. Typically, a text-to-speech synthesis system performs a text analysis using natural language processing techniques; determines the appropriate phonetic string and prosodic features; and generates a speech signal by employing a concatenative or rule-based synthesis method."@en,
    "The task/process of converting speech into natural language text"@en;
  skos:inScheme :OperationScheme;
  skos:narrower :DocumentReading;
  skos:prefLabel "Text-to-Speech Synthesis"@en .

:application_vnd_openxmlformats_officedocument_presentationml_presentation skos:inScheme
    :MimeTypeScheme .

:Paraphrasing a skos:Concept;
  rdfs:label "Paraphrasing"@en;
  skos:broader :NaturalLanguageGeneration;
  skos:definition "A task/process whereby a text fragment is reproduced with another text fragment that conveys the same or similar information"@en;
  skos:inScheme :OperationScheme;
  skos:prefLabel "Paraphrasing"@en .

:FacialExpressionRecognition skos:altLabel "Facial expression detection"@en .

:ChemicalEntity a skos:Concept;
  rdfs:label "Chemical entity"@en;
  skos:broader :DomainSpecificAnnotationType;
  skos:definition "Any kind of annotation pertaining to entities from chemistry"@en;
  skos:inScheme :AnnotationTypeScheme;
  skos:prefLabel "Chemical entity"@en .

:LanguageDetection a skos:Concept;
  rdfs:label "Language detection"@en .

:Reader a skos:Concept;
  :performsOperation :Reading;
  rdfs:label "Reader"@en;
  skos:broader :AccessComponent;
  skos:definition "A component that reads content of various types (pdf, txt, xml etc.)"@en;
  skos:inScheme :ComponentTypeScheme;
  skos:prefLabel "Reader"@en .

:LinguisticAnalysis a skos:Concept;
  rdfs:label "Linguistic analysis"@en;
  skos:altLabel "Language Analysis"@en, "Language Analysis and Understanding"@en, "Linguistic research"@en;
  skos:broader :SupportOperation;
  skos:definition "Any operation that aims at the analysis of language or its structure"@en;
  skos:inScheme :OperationScheme;
  skos:narrower :AnaphoraResolution, :CoReferenceResolution, :DerivationalAnalysis,
    :DiscourseAnalysis, :MorphologicalAnalysis, :Parsing;
  skos:prefLabel "Linguistic analysis"@en .

:audio_basic skos:inScheme :MimeTypeScheme .

:MorphologicalAnnotation a skos:Concept;
  rdfs:label "Morphological annotation"@en;
  skos:broader :TextAnnotation;
  skos:definition "The task/process of adding annotations pertaining to the morphological level of analysis (e.g. gender, number, person etc.)"@en;
  skos:inScheme :OperationScheme;
  skos:narrower :AnnotationOfCompounds, :AnnotationOfDerivationalFeatures, :AnnotationOfMultiWordUnits,
    :BelowPosTagging, :SyllableSegmentation, :WordSegmentation;
  skos:prefLabel "Morphological annotation"@en .

:BiologicalEnity a skos:Concept;
  rdfs:label "Biological enity"@en;
  skos:broader :DomainSpecificAnnotationType;
  skos:definition "Any kind of annotation pertaining to entities of biology"@en;
  skos:inScheme :AnnotationTypeScheme;
  skos:narrower :BiologicalActivity, :BrainRegion, :Chemical, :IonicChannel, :IonicConductance,
    :IonicCurrent, :Metabolite, :ModelOrganism_species, :Neuron, :Protein, :Species, :Synapse;
  skos:prefLabel "Biological enity"@en .

:Evaluation a skos:Concept;
  rdfs:label "Evaluation"@en;
  skos:broader :Operation;
  skos:definition "The task/process of assessing the quality of a resource, e.g. based on the contents (for a dataset) or performance (for a tool or service)"@en;
  skos:inScheme :OperationScheme;
  skos:narrower :DeepParserPerformanceEvaluation, :EvaluationOfBroadCoverageNaturalLanguageParsers,
    :EvaluationOfMachineTranslationAndTranslationTools, :SpeechSynthesisEvaluation, :TaskOrientedTextAnalysisEvaluation;
  skos:prefLabel "Evaluation"@en .

:audio_flac skos:altLabel "audio/x-flac" .

:PackageFormat a skos:Concept;
  rdfs:label "Package format"@en;
  skos:broader :DataFormat;
  skos:definition "The package format of the distribution in which one or more data files are grouped together, e.g. to enable a set of related files to be downloaded together."@en;
  skos:inScheme :DataFormatScheme;
  skos:prefLabel "Package format"@en .

:Date a skos:Concept;
  :documentationUrl "http://dkpro.github.io/dkpro-core/releases/1.8.0/docs/typesystem-reference.html#de.tudarmstadt.ukp.dkpro.core.api.ner.type.Date";
  rdfs:label "Date"@en;
  owl:equivalentClass <http://purl.org/olia/olia-top.owl#Date>;
  skos:broader :NamedEntity;
  skos:definition "A text unit that denotes a date, a specific point in time"@en;
  skos:inScheme :AnnotationTypeScheme;
  skos:prefLabel "Date"@en .

:SpeakerIdentification a skos:Concept;
  rdfs:label "Speaker identification"@en;
  skos:altLabel "SR"@en, "Speaker Recognition"@en, "VR"@en, "Voice Recognition"@en;
  skos:broader :SpeechRecognition;
  skos:definition "Speaker recognition, which can be classified into identification and verification, is the process of automatically recognizing who is speaking on the basis of individual information included in speech waves. This technique makes it possible to use the speaker's voice to verify their identity and control access to services such as voice dialing, banking by telephone, telephone shopping, database access services, information services, voice mail, security control for confidential information areas, and remote access to computers."@en,
    "The task/process of identifying/recognizing who the person speaking is"@en;
  skos:inScheme :OperationScheme;
  skos:prefLabel "Speaker identification"@en .

:Html5Microdata a skos:Concept;
  :documentationUrl "https://www.w3.org/TR/microdata/";
  :hasMimetype :text_html;
  rdfs:label "HTML5 Microdata"@en;
  skos:broader :AnnotationFormat, :Html;
  skos:definition "Format according to the specifications of HTML5 Microdata"@en;
  skos:inScheme :DataFormatScheme;
  skos:prefLabel "HTML5 Microdata"@en .

:Alto a skos:Concept;
  :documentationUrl "https://en.wikipedia.org/wiki/ALTO_(XML)";
  :hasMimetype :application_xml_alto;
  skos:broader :Xml;
  skos:inScheme :DataFormatScheme .

:FillMask skos:inScheme :ModelFunctionScheme .

:VideoFormat skos:prefLabel "Video format"@en .

:WikipediaRevision a skos:Concept;
  :documentationUrl "https://dkpro.github.io/dkpro-core/releases/1.8.0/docs/format-reference.html#format-WikipediaRevision";
  rdfs:label "Wikipedia revision"@en;
  skos:broader :WikipediaFormat;
  skos:definition "Format for wikipedia revision pages"@en;
  skos:inScheme :DataFormatScheme;
  skos:prefLabel "Wikipedia revision"@en .

:ModelFunction a skos:Concept;
  rdfs:label "Model function"@en;
  skos:definition "A subset of functions specific to models"@en;
  skos:narrower :Annotation, :AudioProcessing, :DialogueModelling, :FeatureExtraction,
    :FillMask, :ImageGeneration, :ImageProcessing, :ImageSegmentation, :QuestionAnswering,
    :Summarization, :TextGeneration, :ZeroShotClassification;
  skos:prefLabel "Model function"@en;
  skos:topConceptOf :ModelFunctionScheme .

:FaceRecognition a skos:Concept;
  rdfs:label "Face recognition"@en;
  skos:altLabel "Facial recognition"@en;
  skos:broader :OperationWithMultimediaInputOrOutput;
  skos:definition "The task/process of identifying or verifying a person from a digital image or a video frame from a video source [adapted from Wikipedia]"@en;
  skos:inScheme :OperationScheme;
  skos:prefLabel "Face recognition"@en .

:MachineTranslationSupport a skos:Concept .

:TextSimilarityAssessment a skos:Concept;
  rdfs:label "Text similarity assessment"@en;
  skos:altLabel "Text similarity checking"@en, "Textual similarity assessment"@en, "Textual similarity checking"@en;
  skos:definition "The task of determining the degree of closeness between two pieces of text"@en;
  skos:inScheme :OperationScheme;
  skos:narrower :SentenceSimilarityAssessment;
  skos:prefLabel "Text similarity assessment"@en .

:application_vnd_openxmlformats_officedocument_spreadsheetml_sheet a skos:Concept .

:NamedEntitityRecognizer a skos:Concept;
  :performsOperation :NamedEntityRecognition;
  rdfs:label "Named entitity recognizer"@en;
  skos:broader :Annotator;
  skos:definition "A component that seeks to locate and classify elements in a text into pre-defined categories such as the names of persons, organizations, locations, expressions of times, discipline-specific classes, etc"@en;
  skos:inScheme :ComponentTypeScheme;
  skos:prefLabel "Named entitity recognizer"@en .

:DimensionalityReduction a skos:Concept;
  dc:source "adapted from Wikipedia (https://en.wikipedia.org/wiki/Dimensionality_reduction)"@en;
  rdfs:label "Dimensionality Reduction"@en;
  skos:broader :MachineAndStatisticalLearningMethod;
  skos:definition "A method based on reducing the number of random variables under consideration, via obtaining a set of principal variables."@en;
  skos:inScheme :TdmMethodScheme;
  skos:prefLabel "Dimensionality Reduction"@en .

:Species a skos:Concept;
  rdfs:label "Species"@en;
  skos:broader :BiologicalEnity, :NamedEntity;
  skos:definition "A set of animals or plants in which the members have similar characteristics to each other and can breed with each other"@en;
  skos:inScheme :AnnotationTypeScheme;
  skos:narrower :WheatRelatedSpecies;
  skos:prefLabel "Species"@en .

:SupportOperationCollection a skos:Collection;
  rdfs:label "Support operation Collection"@en;
  skos:member :BilingualLexiconInduction, :BuildingOfFiniteStateAutomata, :CommentFiltering,
    :CorpusManagement, :CorpusViewing, :Crawling, :DataCollection, :DataMerging, :DataSplitting,
    :Debugging, :DeepParserPerformanceEvaluation, :DependencyConversion, :DialogueModelling,
    :Editing, :Evaluation, :EvaluationOfBroadCoverageNaturalLanguageParsers, :EvaluationOfMachineTranslationAndTranslationTools,
    :FeatureExtraction, :FillMask, :FlowControl, :FormatConversion, :FrequencyCount, :GazeteerBasedMatching,
    :InformationStorage, :LanguageModelling, :LexiconAccess, :LexiconAcquisitionFromCorpora,
    :LexiconCreation, :LexiconEnhancement, :LexiconExtractionFromLexica, :LexiconFormatConversion,
    :LexiconMerging, :LexiconViewing, :LexiconVisualization, :MachineTranslationSupport,
    :ManagementOfAnnotations, :Matching, :NlpDevelopmentSupport, :ParallelSentenceExtraction,
    :Reading, :ResourceAccess, :ScriptBasedAnalysis, :SpeechSynthesisEvaluation, :StatisticalLanguageModelling,
    :SupportOfCrowdsourcingTasks, :SupportOperation, :SupportOperationForKnowledgeResources,
    :TagsetConversion, :TaskOrientedTextAnalysisEvaluation, :TerminologyManagement, :TrainingOfLanguageModels,
    :TrainingOfMachineLearningModels, :TrainingOfNmtModels, :TranslationMemoryManagement,
    :TranslationProjectManagement, :UnicodeConformTokenizing, :UserAuthentication, :Validation,
    :Viewing, :Visualization, :Writing, :ZeroShotClassification;
  skos:prefLabel "Support operation Collection"@en .

:AudioProcessing skos:inScheme :ModelFunctionScheme .

:DialogueModelling skos:inScheme :ModelFunctionScheme .

:SemanticClassLabelling skos:inScheme :ModelFunctionScheme .

:SoundToTextAlignment skos:inScheme :ModelFunctionScheme .

:SpatialRoleLabelling skos:inScheme :ModelFunctionScheme .

:Chunking skos:inScheme :ModelFunctionScheme .

:PolarityLabelling skos:inScheme :ModelFunctionScheme .

:CertaintyLevelLabelling skos:inScheme :ModelFunctionScheme .

:Stemming skos:inScheme :ModelFunctionScheme .

:ProsodicAnnotation skos:inScheme :ModelFunctionScheme .

:SpeechAnnotation skos:inScheme :ModelFunctionScheme .

:SyllableSegmentation skos:inScheme :ModelFunctionScheme .

:WordSegmentation skos:inScheme :ModelFunctionScheme .

:AnaphoraAnnotation skos:inScheme :ModelFunctionScheme .

:DependencyParsing skos:inScheme :ModelFunctionScheme .

:DiscourseModelling skos:inScheme :ModelFunctionScheme .

:AnnotationOfDocumentStructure skos:inScheme :ModelFunctionScheme .

:AnnotationOfQuestionTopics skos:inScheme :ModelFunctionScheme .

:AnnotationOfDerivationalFeatures skos:inScheme :ModelFunctionScheme .

:Concordancing a skos:Concept .

:SpeakerDiarization skos:inScheme :ModelFunctionScheme .

:ClusteringMethod a skos:Concept;
  dc:source "adapted from wikipedia (https://en.wikipedia.org/wiki/Cluster_analysis)"@en;
  rdfs:label "Clustering Method"@en;
  skos:broader :MachineAndStatisticalLearningMethod;
  skos:definition "Any method used in clustering or cluster analysis, i.e. in grouping a set of objects in such a way that objects in the same group (cluster) are more similar (in some sense or another) to each other than to those in other groups (clusters)."@en;
  skos:example "k-means, k-nearest neighbours"@en;
  skos:inScheme :TdmMethodScheme;
  skos:prefLabel "Clustering Method"@en .

:OpenOfficeSpreadsheet a skos:Concept;
  :hasMimetype :application_vnd_openxmlformats_officedocument_spreadsheetml_sheet;
  rdfs:label "Open office spreadsheet"@en;
  skos:broader :DocumentFormat, :OpenFormat, :TabularFormat, :Xml;
  skos:inScheme :DataFormatScheme;
  skos:prefLabel "Open office spreadsheet"@en .

:Polarity a skos:Concept;
  rdfs:label "Polarity"@en;
  owl:equivalentClass <http://purl.org/olia/olia-top.owl#PolarityFeature>;
  skos:broader :SemanticAnnotationType;
  skos:definition "A feature that distinguishes between positive, negative or neutral; in sentiment analysis, it refers to determining whether the expressed opinion in a document, a sentence or an entity feature/aspect is positive, negative, or neutral. [adapted from Wikipedia]"@en;
  skos:inScheme :AnnotationTypeScheme;
  skos:prefLabel "Polarity"@en .

:CrossLingualSearch a skos:Concept;
  rdfs:label "Cross-language Information Retrieval"@en;
  skos:altLabel "CLIR"@en, "Cross-lingual information retrieval"@en, "Cross-lingual search"@en,
    "Translingual information retrieval"@en;
  skos:broader :InformationRetrieval;
  skos:definition "Cross-language information retrieval means using queries in one language to search for documents in a different language. Multilingual information retrieval is a broader term, which includes the case where queries in different languages are used, but only for searching documents in the same language."@en,
    "The ability of a system to retrieve relevant documents in various languages in response to a user query that is formulated in only one language"@en;
  skos:inScheme :OperationScheme;
  skos:prefLabel "Cross-language Information Retrieval"@en;
  skos:related :MultilingualInformationRetrieval .

:hasFileExtension rdfs:subPropertyOf owl:topDataProperty .

:NaturalLanguageGenerationCollection a skos:Collection;
  rdfs:label "Natural Language Generation Collection"@en;
  skos:member :Conjugation, :DataToTextGeneration, :DocumentReading, :LexicalSimplification,
    :LexicalSubstitution, :MultilingualGeneration, :NaturalLanguageGeneration, :NewsGeneration,
    :Paraphrasing, :SignLanguageGeneration, :SpeechSynthesis, :SpokenLanguageGeneration,
    :Summarization, :SyntacticStructureGeneration, :TextCompression, :TextGeneration,
    :TextSimplification, :TextToSpeechSynthesis, :TextToTextGeneration;
  skos:prefLabel "Natural Language Generation Collection"@en .

:SoundEventAnnotation skos:inScheme :ModelFunctionScheme .

:ProsodicBoundary a skos:Concept;
  rdfs:label "Prosodic boundary"@en;
  skos:broader :SpeechAnnotationType;
  skos:inScheme :AnnotationTypeScheme;
  skos:prefLabel "Prosodic boundary"@en .

:DataSplitting a skos:Concept;
  rdfs:label "Data splitting"@en;
  skos:broader :SupportOperation;
  skos:definition "The task/process of splitting (partitioning) available data into parts, usually for cross-validatory purposes, e.g. in order to use one part for training purposes and the other for evaluation."@en;
  skos:inScheme :OperationScheme;
  skos:prefLabel "Data splitting"@en .

:image_jpeg skos:broader :Mimetype .

:Token a skos:Concept;
  :documentationUrl "http://dkpro.github.io/dkpro-core/releases/1.8.0/docs/typesystem-reference.html#de.tudarmstadt.ukp.dkpro.core.api.segmentation.type.Token";
  rdfs:label "Token"@en;
  owl:equivalentClass <http://purl.org/olia/olia-top.owl#Token>, <http://vocab.lappsgrid.org/Token>;
  skos:broader :StructuralAnnotationType;
  skos:definition "A set of characters surrounded by spaces or punctuation marks, as well as punctuation marks themselves"@en;
  skos:inScheme :AnnotationTypeScheme;
  skos:prefLabel "Token"@en .

:TextAnnotation a skos:Concept;
  rdfs:label "Text annotation"@en;
  skos:altLabel "Linguistic annotation"@en;
  skos:broader :Annotation;
  skos:definition "The process/task of adding annotations (notes or comments) to a text; in TDM, the annotations refer mainly to the interpretative linguistic information grounded in a knowledge resource that is added manually or automatically to a text"@en;
  skos:inScheme :OperationScheme;
  skos:narrower :DiscourseAnnotation, :Lemmatization, :MorphologicalAnnotation, :MorphosyntacticTagging,
    :Parsing, :ReadabilityAnnotation, :SemanticAnnotation, :Stemming, :StructuralAnnotation;
  skos:prefLabel "Text annotation"@en .

:GrammarChecking rdfs:label "Grammar checking"@en .

:DataSplitter a skos:Concept;
  :performsOperation :DataSplitting;
  rdfs:label "Data splitter"@en;
  skos:broader :SupportComponent;
  skos:definition "A component that performs data splitting for cross validation purposes"@en;
  skos:inScheme :ComponentTypeScheme;
  skos:prefLabel "Data splitter"@en .

:text_x_brat a owl:NamedIndividual, skos:Concept;
  rdfs:label "text/x-brat" .

:Rna a skos:Concept;
  rdfs:label "RNA"@en;
  skos:altLabel "Ribonucleic acid"@en;
  skos:broader :AgriculturalEntity;
  skos:definition "Any of various nucleic acids that contain ribose and uracil as structural components and are associated with the control of cellular chemical activities"@en;
  skos:inScheme :AnnotationTypeScheme;
  skos:prefLabel "RNA"@en .

:SentimentAnalyzer a skos:Concept;
  :performsOperation :SentimentAnalysis;
  rdfs:label "Sentiment analyzer"@en;
  skos:altLabel "Opinion mining tool"@en;
  skos:broader :Analyzer;
  skos:definition "A component that tries to identify sentences that express the author’s negative or positive feelings on something"@en;
  skos:editorialNote "could also be an annotator"@en;
  skos:inScheme :ComponentTypeScheme;
  skos:prefLabel "Sentiment analyzer"@en .

:DataFormat a skos:Concept;
  rdfs:label "Data format"@en;
  skos:altLabel "Data type"@en, "File format"@en;
  skos:definition "The format of a computer file storing data"@en;
  skos:inScheme :DataFormatScheme;
  skos:narrower :AnnotationFormat, :AudioFormat, :BinaryFormat, :CorpusFormat, :DatabaseFormat,
    :DocumentFormat, :GateFormat, :ImageFormat, :Json, :LinkedDataFormat, :MLModelFormat,
    :OpenFormat, :PackageFormat, :RdfFormat, :RdfFormats, :Solr, :TabularFormat, :UimaCasFormat,
    :VideoFormat, :WikiFormat, :WikiFormats, :WikipediaFormat, :Xml;
  skos:prefLabel "Data format"@en;
  skos:topConceptOf :DataFormatScheme .

:ImageTranslation a skos:Concept;
  rdfs:label "Image translation"@en;
  skos:broader :Translation;
  skos:definition "The automatic extraction of text contained in an image (e.g. by OCR technology), its subsequent translation into another language, followed by a digital image processing step in order to reconstruct the original image with the translated text [adapted from https://en.wikipedia.org/wiki/Image_translation]"@en;
  skos:inScheme :OperationScheme;
  skos:prefLabel "Image translation"@en .

:LanguageIdentifier :performsOperation :LanguageIdentification .

:SentenceAlignment skos:broader :Alignment .

:NaturalLanguageUnderstanding a skos:Concept;
  rdfs:label "Natural Language Understanding"@en;
  skos:altLabel "LU"@en, "Language Understanding"@en, "Machine Understanding"@en, "NLU"@en,
    "Natural Language Understanding"@en;
  skos:broader :Operation;
  skos:definition "", "The comprehension by computers of the structure and meaning of human languages, allowing users to interact with the computer using natural sentences. [adapted from https://www.gartner.com/it-glossary/nlu-natural-language-understanding]"@en;
  skos:inScheme :OperationScheme;
  skos:narrower :SpeechUnderstanding;
  skos:prefLabel "Natural Language Understanding"@en .

:TdmMethodScheme a skos:ConceptScheme;
  rdfs:label "TDM/LT Method Taxonomy"@en;
  skos:hasTopConcept :TdmMethod;
  skos:prefLabel "TDM/LT Method Taxonomy"@en .

:KeaCorpus a skos:Concept;
  :documentationUrl "https://builds.openminted.eu/job/WP%205.2%20-%20Typesystem%20alignment/eu.openminted.interop$mapping-conversion/doclinks/1/components.html#_kea_corpus_1";
  rdfs:label "KEA corpus"@en;
  skos:broader :CorpusFormat .

:Blikiwikipedia a skos:Concept;
  skos:inScheme :DataFormatScheme;
  skos:prefLabel "blikiWikipedia"@en .

:application_xXces_xml rdfs:label "application/x-xces+xml";
  skos:broader :Mimetype .

:LanguageProficiencyLevel skos:broader :AnnotationType;
  skos:inScheme :AnnotationTypeScheme .

:text_x_anafora a skos:Concept;
  skos:inScheme :MimeTypeScheme .

:ProsodicInformationProcessing skos:broader :InformationExtraction .

:TextIndexing a skos:Concept;
  rdfs:label "Text indexing"@en;
  skos:inScheme :OperationScheme;
  skos:prefLabel "Text indexing"@en .

:TextCompression skos:broader :SupportOperation .

:ReadabilityAnnotation a skos:Concept;
  rdfs:label "Readability annotation"@en;
  skos:broader :TextAnnotation;
  skos:definition "The process/task of adding readability scores (or any other type of similar annotation) to a text or textual segment showing how easy it is to read and understand its meaning."@en;
  skos:inScheme :OperationScheme;
  skos:prefLabel "Readability annotation"@en .

:Nif a skos:Concept;
  :documentationUrl "http://persistence.uni-leipzig.org/nlp2rdf/";
  rdfs:label "NIF"@en;
  skos:altLabel "NLP Interchage Format"@en;
  skos:broader :AnnotationFormat, :CorpusFormat, :RdfFormat, :RdfFormats;
  skos:definition "The NLP Interchange Format (NIF) is an RDF/OWL-based format that aims to achieve interoperability between Natural Language Processing (NLP) tools, language resources and annotations; it consists of specifications, ontologies and software (overview), which are combined under the version identifier \"NIF 2.0\", but are versioned individually"@en;
  skos:inScheme :DataFormatScheme;
  skos:prefLabel "NIF"@en .

:GazeteerBasedMatcher a skos:Concept;
  :performsOperation :GazeteerBasedMatching;
  rdfs:label "Gazeteer based matcher"@en;
  skos:broader :Matcher;
  skos:definition "A component that allows matching of elements based on a gazeteer"@en;
  skos:inScheme :ComponentTypeScheme;
  skos:prefLabel "Gazeteer based matcher"@en .

:Turtle a skos:Concept;
  :documentationUrl "https://www.w3.org/TR/turtle/";
  :hasMimetype :text_turtle;
  rdfs:label "Turtle"@en;
  skos:broader :RdfFormat, :RdfFormats;
  skos:definition "Textual syntax for RDF that allows an RDF graph to be completely written in a compact and natural text form, with abbreviations for common usage patterns and datatypes."@en;
  skos:inScheme :DataFormatScheme;
  skos:prefLabel "Turtle"@en .

:Rdf_xml a skos:Concept;
  :documentationUrl "https://www.w3.org/TR/REC-rdf-syntax/";
  :hasMimetype :application_rdf_xml;
  rdfs:label "RDF/XML"@en;
  skos:broader :RdfFormat, :RdfFormats, :Xml;
  skos:definition "Data format for RDF (Resource Description Framework) XML format; RDF/XML is a serialisation for RDF"@en;
  skos:inScheme :DataFormatScheme;
  skos:prefLabel "RDF/XML"@en .

:text_x_org_dkpro_conll2003 a skos:Concept;
  rdfs:label "text/x.org.dkpro.conll-2003";
  skos:broader :Mimetype;
  skos:inScheme :MimeTypeScheme .

:MultilingualInformationRetrieval a skos:Concept;
  rdfs:label "Multilingual Information Retrieval"@en;
  skos:altLabel "MIR"@en;
  skos:broader :InformationRetrieval;
  skos:definition "Cross-language information retrieval means using queries in one language to search for documents in a different language. Multilingual information retrieval is a broader term, which includes the case where queries in different languages are used, but only for searching documents in the same language."@en;
  skos:inScheme :OperationScheme;
  skos:prefLabel "Multilingual Information Retrieval"@en;
  skos:related :CrossLingualSearch .

:MorphologicalAnalysis a skos:Concept;
  rdfs:label "Morphological analysis"@en;
  skos:altLabel "General morphological analyisis"@en;
  skos:broader :LinguisticAnalysis;
  skos:definition "The analysis of the structure of words and their relations to other words as regards their form and derivation"@en,
    "The technologies for or the process of tracing the inflectional, derivational, and compounding processes in the formation of a given word in order to determine properties such as stem form, part-of-speech and inflectional information. As a crucial preprocessing step, morphological analysis is used in virtually all fields of natural language processing."@en;
  skos:inScheme :OperationScheme;
  skos:prefLabel "Morphological analysis"@en .

:Prediction a skos:Concept;
  rdfs:label "Prediction"@en;
  skos:broader :TextAndDataMining;
  skos:definition "In Machine Learning, it refers to the use of algorithms that learn from previous data in order to make predictions on data (by estimating probabilities from previous data)"@en;
  skos:inScheme :OperationScheme;
  skos:prefLabel "Prediction"@en .

:TextSpeechDataAnalytics a skos:Concept;
  rdfs:label "Text/Speech/Data analytics"@en;
  skos:broader :Operation;
  skos:editorialNote "it could also be a composite concept created by three separate concepts, but for now ok"@en;
  skos:inScheme :OperationScheme;
  skos:narrower :SpeechAnalytics, :TextAndDataAnalytics;
  skos:prefLabel "Text/Speech/Data analytics"@en .

:image_png skos:inScheme :MimeTypeScheme .

:text_x_org_dkpro_ptbCombined a skos:Concept;
  rdfs:label "text/x.org.dkpro.ptb-combined";
  skos:broader :Mimetype;
  skos:inScheme :MimeTypeScheme .

:Clause a skos:Concept;
  rdfs:label "Clause"@en;
  owl:equivalentClass <http://purl.org/olia/olia-top.owl#Clause>;
  skos:broader :StructuralAnnotationType;
  skos:definition "A clause is a subdivision of a sentence containing a subject (argument) and predicate. It is possible to have a word that implies or refers to a predicate rather than one explicitly stated. [Pei & Gaynor 1980: 40, http://linguistics-ontology.org/gold/2010/Clause]"@en;
  skos:inScheme :AnnotationTypeScheme;
  skos:prefLabel "Clause"@en .

:audio_mpa_robust a skos:Concept;
  rdfs:label "audio/mpa-robust";
  skos:broader :Mimetype;
  skos:inScheme :MimeTypeScheme .

:text_x_org_dkpro_conll2002 a skos:Concept;
  rdfs:label "text/x.org.dkpro.conll-2002";
  skos:broader :Mimetype;
  skos:inScheme :MimeTypeScheme .

:MachineTranslationSupport skos:broader :SupportOperation;
  skos:definition "Any operation that can be used for training or support of Machine Translation tools"@en;
  skos:narrower :ParallelSentenceExtraction;
  skos:prefLabel "Machine translation support"@en .

:hasFileExtension rdfs:comment "The file extension usually associated with a specific data format (e.g. txt for plain text files, pdf for PDF files etc.)"@en .

:text_sgml a skos:Concept;
  skos:broader :Mimetype;
  skos:inScheme :MimeTypeScheme .

:DocumentSection a skos:Concept;
  :documentationUrl "http://dkpro.github.io/dkpro-core/releases/1.8.0/docs/typesystem-reference.html#de.tudarmstadt.ukp.dkpro.core.api.segmentation.type.Div";
  rdfs:label "Document section"@en;
  skos:broader :ScholarlyAnalyticsEntity, :StructuralAnnotationType;
  skos:definition "Any subdivision of a document, e.g. a chapter, abstract, etc."@en;
  skos:inScheme :AnnotationTypeScheme;
  skos:prefLabel "Document section"@en .

:ConstituencyParsing skos:inScheme :ModelFunctionScheme .

:SemanticAnnotator a skos:Concept;
  rdfs:label "Semantic annotator"@en;
  skos:broader :Annotator;
  skos:definition "A component that annotates the tokens of a text with semantic features"@en;
  skos:inScheme :ComponentTypeScheme;
  skos:narrower :AnnotatorOfSemanticRoleLabels, :ReadabilityAnnotator;
  skos:prefLabel "Semantic annotator"@en .

:SocialSciencesEntity a skos:Concept;
  rdfs:label "Social sciences entity"@en;
  skos:broader :DomainSpecificAnnotationType;
  skos:definition "Any kind of annotation that pertains to entities of social sciences; the use of TheSoz is recommended"@en;
  skos:inScheme :AnnotationTypeScheme;
  skos:narrower :AllbusVariable, :HistoricalEvent, :Media, :MethodOfResearch, :OfficialText,
    :TheoreticalFrame;
  skos:prefLabel "Social sciences entity"@en .

:LanguageDetection skos:inScheme :OperationScheme;
  skos:prefLabel "Language detection"@en .

:DependencyConversion a skos:Concept;
  rdfs:label "Dependency conversion"@en;
  skos:broader :FormatConversion;
  skos:definition "The task/process of converting constituency structures to dependency trees"@en;
  skos:inScheme :OperationScheme;
  skos:prefLabel "Dependency conversion"@en;
  skos:related :ConstituencyParsing, :DependencyParsing .

:DecisionTrees a skos:Concept;
  dc:source """adapted from  (http://scikit-learn.org/stable/modules/tree.html)
and wikipedia (https://en.wikipedia.org/wiki/Decision_tree)"""@en;
  rdfs:label "Decision Trees"@en;
  skos:broader :MachineAndStatisticalLearningMethod;
  skos:definition "A non-parametric supervised learning method used for classification and regression. The goal is to create a tree-like graph or model of decisions and their possible consequences by learning simple decision rules inferred from the data features."@en;
  skos:inScheme :TdmMethodScheme;
  skos:prefLabel "Decision Trees"@en .

:HumanComputerInteractionCollection a skos:Collection;
  rdfs:label "Human Computer Interaction Collection"@en;
  skos:member :AvatarSynthesis, :ConversationalSystemsBuilding, :HumanComputerInteraction;
  skos:prefLabel "Human Computer Interaction Collection"@en .

:ScientificValue a skos:Concept;
  rdfs:label "Scientific value"@en;
  skos:broader :DomainSpecificAnnotationType, :NamedEntity;
  skos:inScheme :AnnotationTypeScheme;
  skos:prefLabel "Scientific value"@en .

:FactoredTagLemFormat a skos:Concept;
  :documentationUrl "https://builds.openminted.eu/job/WP%205.2%20-%20Typesystem%20alignment/eu.openminted.interop$mapping-conversion/doclinks/1/components.html#_factored_tag_lem_1";
  rdfs:label "Factored tag lem format"@en;
  skos:broader :AnnotationFormat;
  skos:definition "Factored tag lemma format"@en;
  skos:inScheme :DataFormatScheme;
  skos:prefLabel "Factored tag lem format"@en .

:NegationDetection a skos:Concept;
  rdfs:label "Negation detection"@en;
  skos:broader :InformationExtraction;
  skos:definition "The task/process of identifying negative cues (words, phrases) in a text"@en;
  skos:inScheme :OperationScheme;
  skos:prefLabel "Negation detection"@en .

:application_rdf_xml rdfs:label "application/rdf+xml" .

:PartOfSpeechTagger a skos:Concept;
  rdfs:label "Part of speech tagger"@en;
  skos:altLabel "PoS tagger"@en;
  skos:definition "A component that annotates tokens of a text with part-of-speech information"@en;
  skos:inScheme :ComponentTypeScheme;
  skos:prefLabel "Part of speech tagger"@en .

:FillMask skos:prefLabel "Fill mask"@en .

:Anonymization skos:broader :SupportOperation .

:OfficialText rdfs:label "Official text"@en;
  skos:inScheme :AnnotationTypeScheme;
  skos:prefLabel "Official text"@en .

:TemporalExpression rdfs:label "Temporal expression"@en;
  skos:broader :SemanticAnnotationType;
  skos:prefLabel "Temporal expression"@en .

:image_jpeg a skos:Concept;
  rdfs:label "image/jpeg" .

:application_x_org_dkpro_negra3 a skos:Concept;
  rdfs:label "application/x.org.dkpro.negra3";
  skos:inScheme :MimeTypeScheme .

:audio_basic a skos:Concept;
  skos:broader :Mimetype .

:LanguageIdentification skos:broader :SupportOperation .

:NamedEntityRecognition skos:broader :InformationExtraction .

:FacialExpressionRecognition a skos:Concept;
  skos:altLabel "Expression detection"@en, "Expression recognition"@en, "Face expression recognition"@en;
  skos:inScheme :OperationScheme;
  skos:prefLabel "Facial expression recognition"@en .

:Paraphrasing skos:broader :SupportOperation .

:GrammarChecking skos:inScheme :OperationScheme;
  skos:prefLabel "Grammar checking"@en .

:LanguageProficiencyLevel a skos:Concept .

:TextCategorization skos:broader :KnowledgeDiscovery .

:application_vnd_openxmlformats_officedocument_spreadsheetml_sheet rdfs:label "application/vnd.openxmlformats-officedocument.spreadsheetml.sheet";
  skos:inScheme :MimeTypeScheme .

:TextIndexing skos:broader :SupportOperation .

:TextSimilarityAssessment skos:broader :InformationExtraction .

:Transliteration skos:broader :SpeechRecognition .

:TopicDetection skos:broader :InformationExtraction .

:WordSenseInduction skos:broader :SupportOperation .

:SoftwareDevelopmentEnvironment a skos:Concept;
  rdfs:label "Software development environment"@en;
  skos:broader :SupportComponent;
  skos:definition "A technology that supports the development of software components and data resources required for their operation"@en;
  skos:inScheme :ComponentTypeScheme;
  skos:prefLabel "Software development environment"@en .

:AuthoringSupport a skos:Concept;
  rdfs:label "Authoring support"@en;
  skos:altLabel "Structure-Based Authoring Assistant"@en, "Writing support"@en;
  skos:broader :Operation;
  skos:definition "Software for supporting the distributed creation of consistent, high-quality information on an industrial scale. Key components include terminology extraction for legacy information, terminology checking and hyperlinking integrated in standard authoring environments, as well as structural (syntactic) checking of texts to ensure readability, consistency and translatability."@en,
    "The task/process of providing spelling, grammatical or stylistic suggestions as an aid for the authoring task"@en;
  skos:inScheme :OperationScheme;
  skos:narrower :GrammarChecking, :L2WritingSupport, :LanguageChecking, :SpellChecking;
  skos:prefLabel "Authoring support"@en .

:TopicExtractor a skos:Concept;
  rdfs:label "Topic extractor"@en;
  skos:broader :Analyzer;
  skos:definition "A component that guesses the topic of a text"@en;
  skos:inScheme :ComponentTypeScheme;
  skos:prefLabel "Topic extractor"@en .

:TrainerOfMachineLearningModels a skos:Concept;
  :performsOperation :TrainingOfMachineLearningModels;
  rdfs:label "Trainer of Machine Learning models"@en;
  skos:altLabel "ML models trainer"@en, "ML trainer"@en;
  skos:broader :SupportComponent;
  skos:definition "A component that is used in training models for machine learning"@en;
  skos:inScheme :ComponentTypeScheme;
  skos:prefLabel "Trainer of Machine Learning models"@en .

:PhoneticTranscription a skos:Concept;
  rdfs:label "Phonetic transcription"@en;
  skos:broader :Transcription;
  skos:definition "The visual representation of speech sounds (or phones)"@en;
  skos:inScheme :OperationScheme;
  skos:prefLabel "Phonetic transcription"@en .

:Xml a skos:Concept;
  rdfs:label "XML"@en;
  skos:broader :DataFormat;
  skos:definition "Superclass for grouping together XML formats"@en;
  skos:inScheme :DataFormatScheme;
  skos:narrower :Alto, :AlvisEnrichedDocumentFormat, :BncFormat, :EAF, :Emma, :Folia,
    :GateXml, :InlineXml, :OpenOfficeDocument, :OpenOfficePresentation, :OpenOfficeSpreadsheet,
    :Owl_xml, :Pls, :Pml, :Rdf_xml, :SDL_tm_xliff, :Tbx, :Tcf, :Tei, :TigerXml, :Tmx,
    :Tuepp, :Xces, :Xhtml, :Xmi, :XmlBioc, :Xpath;
  skos:prefLabel "XML"@en .

:Conll2000 a skos:Concept;
  :documentationUrl "https://dkpro.github.io/dkpro-core/releases/1.8.0/docs/format-reference.html#format-Conll2000";
  :hasMimetype :text_x_org_dkpro_conll2000;
  rdfs:label "CoNLL-2000"@en;
  skos:broader :ConllFormat;
  skos:definition "The CoNLL 2000 format represents POS and Chunk tags. Fields in a line are separated by spaces. Sentences are separated by a blank new line."@en;
  skos:inScheme :DataFormatScheme;
  skos:prefLabel "CoNLL-2000"@en .

:LanguageDetection skos:broader :InformationExtraction .

:application_vnd_oasis_opendocument_presentation a skos:Concept;
  rdfs:label "application/vnd.oasis.opendocument.presentation";
  skos:broader :Mimetype;
  skos:inScheme :MimeTypeScheme .

:EventDetection a skos:Concept;
  rdfs:label "Event detection"@en;
  skos:altLabel "Event extraction"@en;
  skos:broader :InformationExtraction;
  skos:definition "The process/task of identifying events in data (text, video, images etc.), usually combined with their classification into types of events and recognition of the event attributes (e.g. time, place, participants and duration)"@en;
  skos:inScheme :OperationScheme;
  skos:prefLabel "Event detection"@en .

:ScientificUnit a skos:Concept;
  rdfs:label "Scientific unit"@en;
  skos:inScheme :AnnotationTypeScheme;
  skos:prefLabel "Scientific unit"@en .

:StanceDetection a skos:Concept;
  rdfs:label "Stance detection"@en;
  skos:broader :InformationExtraction;
  skos:definition "The extraction of a subject’s reaction to a claim made by a primary actor [http://nlpprogress.com/english/stance_detection.html]"@en;
  skos:inScheme :OperationScheme;
  skos:prefLabel "Stance detection"@en .

:ExtractionOfDomainSpecificInformation a skos:Concept;
  rdfs:label "Extraction of domain-specific information"@en;
  skos:broader :InformationExtraction;
  skos:definition "Extraction of information that pertains to specific domains/disciplines; it can be used combined with \"\"Annotation type\"\" to specify the type of information extracted"@en,
    "Extraction of information that pertains to specific domains/disciplines; it can be used combined with \"Annotation type\" to specify the type of information extracted"@en;
  skos:inScheme :OperationScheme;
  skos:narrower :ExtractionOfFundingInformation;
  skos:prefLabel "Extraction of domain-specific information"@en .

:BilingualLexiconInduction a skos:Concept;
  rdfs:label "Bilingual lexicon induction"@en;
  skos:broader :KnowledgeAcquisition, :SupportOperationForKnowledgeResources;
  skos:definition "The task/process of inducing word translations from monolingual or comparable corpora in two languages"@en;
  skos:inScheme :OperationScheme;
  skos:prefLabel "Bilingual lexicon induction"@en .

:AnnotationType a skos:Concept;
  rdfs:label "Annotation type"@en;
  skos:altLabel "Label"@en, "Tag"@en;
  skos:closeMatch <http://vocab.lappsgrid.org/Annotation>;
  skos:definition "Category/class of the annotations (metadata) that are added to the data/text that is processed"@en;
  skos:inScheme :AnnotationTypeScheme;
  skos:narrower :Alignment1, :DiscourseAnnotationType, :DocumentAnnotationType, :DomainSpecificAnnotationType,
    :LanguageCode, :LanguageProficiencyLevel, :ModalityAnnotationType, :MorphologicalAnnotationType,
    :PartOfSpeech, :QuantititativeInformation, :SemanticAnnotationType, :SpeechAnnotationType,
    :StructuralAnnotationType, :SyntacticAnnotationType, :Term;
  skos:prefLabel "Annotation type"@en;
  skos:scopeNote "A note by way of explanation or comment added to a text or diagram [OED, https://en.oxforddictionaries.com/definition/annotation]. Text or corpus annotation refers to the interpretative linguistic information grounded in a knowledge resource that is added manually or automatically to a text or corpus respectively."@en;
  skos:topConceptOf :AnnotationTypeScheme .

:DocumentReading a skos:Concept;
  rdfs:label "Document reading"@en;
  skos:broader :TextToSpeechSynthesis;
  skos:definition "The task/process of converting the contents of a digital document into speech in order to aid mainly individuals with visual impairments"@en;
  skos:inScheme :OperationScheme;
  skos:prefLabel "Document reading"@en .

:ExploratorySearch a skos:Concept;
  rdfs:label "Exploratory search"@en;
  skos:broader :InformationRetrieval;
  skos:definition "A type of search which, in contrast to traditional lookup search, covers a broad class of activities, such as investigating, evaluating, comparing, and synthesizing"@en;
  skos:inScheme :OperationScheme;
  skos:prefLabel "Exploratory search"@en .

:InformationExtractionAndInformationRetrievalCollection a skos:Collection;
  rdfs:label "Information Extraction and Information Retrieval Collection"@en;
  skos:member :AgeBracketDetection, :AuthorClassification, :AutomaticHyperlinking, :BilingualLexiconInduction,
    :BotDetection, :ComputationalArgumentation, :ContentMining, :ContradictionDetection,
    :CrossLingualSearch, :EmotionDetection, :EmotionLabelling, :EntityMentionLabelling,
    :EntityMentionRecognition, :EventDetection, :ExploratorySearch, :ExtractionOfDomainSpecificInformation,
    :ExtractionOfFundingInformation, :ExtractionOfQuantitativeInformation, :FactChecking,
    :FakeNewsDetection, :FrameExtraction, :GenderDetection, :HateSpeechRecognition, :HumourDetection,
    :InformationExtraction, :InformationFiltering, :InformationFilteringByRecommenderSystems,
    :InformationRetrieval, :IronyDetection, :KeywordExtraction, :KnowledgeAcquisition,
    :KnowledgeDiscovery, :KnowledgeRepresentation, :LanguageDetection, :LexiconAcquisitionFromCorpora,
    :LexiconEnhancement, :LexiconExtractionFromLexica, :MultilingualInformationRetrieval,
    :MultimediaInformationExtraction, :MultimediaRetrieval, :NegationDetection, :OntologyAcquisition,
    :OntologyEnhancement, :PersuasiveExpressionMining, :PolarityDetection, :Prediction,
    :QuestionAnswering, :RecognizingTextualEntailment, :RelationExtraction, :RepresentationOfSpaceAndTime,
    :RumoursStanceClassification, :SemanticReasoning, :SemanticSearch, :SpeechAnalytics,
    :SpeechRetrieval, :StanceDetection, :TableQuestionAnswering, :TemporalExpressionRecognition,
    :TermExtraction, :TerminologySearch, :TextAnalysis, :TextAndDataAnalytics, :TextAndDataMining,
    :TruthLabelling, :VerbalAggressionAnalysis;
  skos:prefLabel "Information Extraction and Information Retrieval Collection"@en .

:text_x_anafora skos:broader :Mimetype .

:ArgumentMining a skos:Concept .

:Search rdfs:label "Search"@en .

:SupportOperationForKnowledgeResources a skos:Concept;
  rdfs:label "Support operation for knowledge resources"@en;
  skos:broader :SupportOperation;
  skos:definition "Any operation that intends to support the creation, curation or use of knowledge resource"@en;
  skos:inScheme :OperationScheme;
  skos:narrower :BilingualLexiconInduction, :LexiconAccess, :LexiconAcquisitionFromCorpora,
    :LexiconCreation, :LexiconEnhancement, :LexiconExtractionFromLexica, :LexiconFormatConversion,
    :LexiconMerging, :LexiconViewing, :LexiconVisualization;
  skos:prefLabel "Support operation for knowledge resources"@en .

:ImageSegmentation a skos:Concept;
  rdfs:label "Image segmentation"@en;
  skos:broader :ModelFunction, :OperationWithMultimediaInputOrOutput;
  skos:inScheme :OperationScheme;
  skos:prefLabel "Image segmentation"@en .

:audio_x_wav skos:inScheme :MimeTypeScheme .

:Cochrane a skos:Concept;
  :documentationUrl "https://gate.ac.uk/sale/tao/splitch23.html#sec:creole:pubmed";
  :hasMimetype :text_xCochrane;
  rdfs:label "Cochrane"@en;
  skos:broader :DocumentFormat;
  skos:definition "Format used in Cochrane texts"@en;
  skos:inScheme :DataFormatScheme;
  skos:prefLabel "Cochrane"@en .

:MalletLdaTopicProportionsSorted a skos:Concept;
  :documentationUrl "https://dkpro.github.io/dkpro-core/releases/1.8.0/docs/format-reference.html#format-MalletTopicsProportionsSorted";
  rdfs:label "Mallet LDA Topic Proportions Sorted"@en;
  skos:broader :AnnotationFormat;
  skos:definition "Topic proportions in the shape [\\t]\\t\\t... sorted"@en;
  skos:inScheme :DataFormatScheme;
  skos:prefLabel "Mallet LDA Topic Proportions Sorted"@en .

:Readability a skos:Concept;
  :documentationUrl "http://dkpro.github.io/dkpro-core/releases/1.8.0/docs/typesystem-reference.html#de.tudarmstadt.ukp.dkpro.core.type.ReadabilityScore";
  rdfs:label "Readability"@en;
  skos:broader :SemanticAnnotationType;
  skos:definition "The ease with which a reader can understand a written text. [https://en.wikipedia.org/wiki/Readability]"@en;
  skos:inScheme :AnnotationTypeScheme;
  skos:prefLabel "Readability"@en .

:LexiconCreation a skos:Concept;
  rdfs:label "Lexicon creation"@en;
  skos:altLabel "Lexicon Development"@en;
  skos:broader :SupportOperationForKnowledgeResources;
  skos:definition "The task/process of constructing lexical resources (e.g. dictionaries, computational lexica, glossaries, etc.)"@en;
  skos:inScheme :OperationScheme;
  skos:prefLabel "Lexicon creation"@en .

:TextAndDataAnalytics a skos:Concept;
  rdfs:label "Text and Data Analytics"@en;
  skos:broader :TextSpeechDataAnalytics;
  skos:definition "The process/task of converting unstructured text and data into high-quality structured data that can be further analysed to extract knowledge, support decision making etc."@en;
  skos:inScheme :OperationScheme;
  skos:prefLabel "Text and Data Analytics"@en;
  skos:related :TextAndDataMining .

:LanguageProficiencyLevel rdfs:label "Language proficiency level"@en;
  skos:prefLabel "Language proficiency level"@en .

:Annotation a skos:Concept;
  rdfs:label "Annotation"@en;
  skos:altLabel "Labeling [en-US]"@en-us, "Labelling"@en, "Tagging"@en;
  skos:broader :ModelFunction, :Operation;
  skos:definition "The process/task of adding annotations (i.e. labels that act as notes, comments, explanations, etc.) to an item"@en;
  skos:inScheme :OperationScheme;
  skos:narrower :MultimediaAnnotation, :SpeechAnnotation, :TextAnnotation;
  skos:prefLabel "Annotation"@en;
  skos:scopeNote "A note by way of explanation or comment added to a text or diagram [OED, https://en.oxforddictionaries.com/definition/annotation]. Text or corpus annotation refers to the interpretative linguistic information grounded in a knowledge resource that is added manually or automatically to a text or corpus respectively."@en .

:DerivationalAnalysis a skos:Concept;
  rdfs:label "Derivational analysis"@en;
  skos:broader :LinguisticAnalysis;
  skos:definition "The analysis of a word in order to identify its derivation, i.e. whether and how it has been formed on the basis of another word (e.g. through the use of affixes)"@en;
  skos:inScheme :OperationScheme;
  skos:prefLabel "Derivational analysis"@en .

:hasMimetype a owl:ObjectProperty;
  rdfs:comment "Relates a data format to the IANA mimetype; it can be the exact or a broader mimetype; unofficial mimetypes are also used, but this relation will be revisited"@en;
  rdfs:label "has mimetype"@en;
  rdfs:range _:node1fu4q14cjx30 .

_:node1fu4q14cjx30 a owl:Class .

:hasMimetype rdfs:subPropertyOf owl:topObjectProperty .

:png a skos:Concept;
  :hasFileExtension "png";
  :hasMimetype :image_png;
  rdfs:label "PNG"@en;
  skos:altLabel "Portable Network Graphics"@en;
  skos:broader :ImageFormat;
  skos:inScheme :DataFormatScheme;
  skos:prefLabel "PNG"@en .

:SpeechRetrieval a skos:Concept;
  rdfs:label "Speech Retrieval"@en;
  skos:altLabel "SDR"@en, "SR"@en, "Spoken Document Retrieval"@en;
  skos:broader :InformationExtraction;
  skos:definition "Speech Retrieval is the process of retrieving spoken audio material (documents)in response to a search query. Search queries can be spoken or textual. Speech retrieval makes use of techniques from speech recognition, natural language understanding and information retrieval. Possible applications are the indexing of archives of broadcast material, and monitoring of telephone conversations."@en;
  skos:inScheme :OperationScheme;
  skos:prefLabel "Speech Retrieval"@en .

:application_vnd_openxmlformats_officedocument_presentationml_presentation a skos:Concept;
  skos:broader :Mimetype .

:application_fastinfoset a skos:Concept;
  rdfs:label "application/fastinfoset";
  skos:broader :Mimetype;
  skos:inScheme :MimeTypeScheme .

:Tex a skos:Concept;
  :documentationUrl "https://en.wikipedia.org/wiki/TeX";
  :hasMimetype :application_xTex;
  rdfs:label "TEX"@en;
  skos:broader :DocumentFormat;
  skos:definition "Data format for documents using Tex (a typesetting system)"@en;
  skos:inScheme :DataFormatScheme;
  skos:prefLabel "TEX"@en .

:Conll2012 a skos:Concept;
  :documentationUrl "https://dkpro.github.io/dkpro-core/releases/1.8.0/docs/format-reference.html#format-Conll2012";
  :hasMimetype :text_x_org_dkpro_conll2012;
  rdfs:label "CoNLL-2012"@en;
  skos:broader :ConllFormat;
  skos:definition "The CoNLL 2012 format targets semantic role labeling and coreference. Columns are tab-separated. Sentences are separated by a blank new line."@en;
  skos:inScheme :DataFormatScheme;
  skos:prefLabel "CoNLL-2012"@en .

:SpeakerVerification a skos:Concept;
  rdfs:label "Speaker verification"@en;
  skos:broader :SpeechRecognition;
  skos:definition "The task/process of verifying that a certain person is speaking"@en;
  skos:inScheme :OperationScheme;
  skos:prefLabel "Speaker verification"@en .

:BionlpFormats a skos:Concept;
  rdfs:label "BioNLP formats"@en;
  owl:deprecated true;
  skos:broader :DocumentFormat;
  skos:definition "Formats used  for BioNLP shared tasks"@en;
  skos:inScheme :DataFormatScheme;
  skos:narrower :Bionlp, :BionlpSt2013A1_a2, :Json_genia;
  skos:prefLabel "BioNLP formats"@en .

:SpeechToTextTranslation a skos:Concept;
  rdfs:label "Speech-to-Text translation"@en;
  skos:inScheme :OperationScheme;
  skos:prefLabel "Speech-to-Text translation"@en .

:MachineTranslationSupport rdfs:label "Machine translation support"@en;
  skos:broader :MachineTranslation .

:NounPhraseChunking a skos:Concept;
  rdfs:label "Noun phrase chunking"@en;
  skos:broader :Chunking;
  skos:definition "The task/process of identifying noun phrases in a sentence"@en;
  skos:inScheme :OperationScheme;
  skos:prefLabel "Noun phrase chunking"@en .

:HumanAidedMachineTranslation a skos:Concept;
  rdfs:label "Human Aided Machine Translation"@en;
  skos:altLabel "HAMT"@en;
  skos:definition "The process of performing Machine Translation facilitated by pre-editing or post-editing steps, or interactive human intervention to steer or select from alternative translations"@en,
    "We call Human-aided Machine Translation all systems and techniques which rely on real automation of the translation function when porting a text from one language to another. As opposed to full Machine Translation, human-aided MT does not fully rely on computational translation, but assists this process by pre-editing and post-editing steps, possibly also interactive human intervention to steer or select from alternative translations. Translation of real-time spoken language, by contrast, does not allow for human intervention, except for negotiation functions, such as clarification dialogues."@en;
  skos:inScheme :OperationScheme;
  skos:prefLabel "Human Aided Machine Translation"@en .

:ComputerAidedTranslation skos:broader :MachineTranslation .

:PtbCombined a skos:Concept;
  :documentationUrl "https://dkpro.github.io/dkpro-core/releases/1.8.0/docs/format-reference.html#format-PennTreebankCombined";
  :hasMimetype :text_x_org_dkpro_ptbCombined;
  rdfs:label "PTB-combined"@en;
  skos:altLabel "Penn Treebank - combined"@en, "ptb; format-variant=combined"@en;
  skos:broader :Ptb;
  skos:definition "Penn Treebank combined format"@en;
  skos:inScheme :DataFormatScheme;
  skos:prefLabel "PTB-combined"@en .

:DataMasking a skos:Concept;
  rdfs:label "Data masking"@en;
  skos:broader :Anonymization;
  skos:definition "The process of hiding original data with modified content (characters or other data) in order to protect data classified as personal identifiable data, or sensitive data [adapted from Wikipedia]"@en;
  skos:inScheme :OperationScheme;
  skos:prefLabel "Data masking"@en .

:AnnotationOfMeasurements a skos:Concept;
  rdfs:label "Annotation of measurements"@en;
  skos:altLabel "Quantity detection"@en, "Quantity extraction"@en;
  skos:broader :SemanticAnnotation;
  skos:definition "The task/process of annotating measurement expressions (e.g. of length, temperature, time, etc.)"@en;
  skos:inScheme :OperationScheme;
  skos:prefLabel "Annotation of measurements"@en .

:TranslationProjectManagement a skos:Concept;
  rdfs:label "Translation project management"@en;
  skos:broader :SupportOperation;
  skos:inScheme :OperationScheme;
  skos:prefLabel "Translation project management"@en .

:MorphologicalTagger a skos:Concept;
  :performsOperation :MorphologicalAnnotation;
  rdfs:label "Morphological tagger"@en;
  skos:broader :Annotator;
  skos:definition "A component that annotates tokens of a text with morphological information (part-of-speech and morphological features)"@en;
  skos:inScheme :ComponentTypeScheme;
  skos:narrower :PartOfSpeechTagger;
  skos:prefLabel "Morphological tagger"@en .

:FaceDetection a skos:Concept;
  rdfs:label "Face detection"@en;
  skos:broader :OperationWithMultimediaInputOrOutput;
  skos:definition "The task/process of recognizing that a person appears on a digital image or a video frame from a video source and possibly marking the contours around it"@en;
  skos:inScheme :OperationScheme;
  skos:prefLabel "Face detection"@en .

:Writing a skos:Concept;
  rdfs:label "Writing"@en;
  skos:broader :ResourceAccess;
  skos:definition "The task/process of producing the output results of a process/workflow in various formats"@en;
  skos:inScheme :OperationScheme;
  skos:prefLabel "Writing"@en .

:SpeechProcessingCollection a skos:Collection;
  rdfs:label "Speech Processing Collection"@en;
  skos:member :AnnotationOfSpeakerTurns, :AudioProcessing, :AudioSegmentation, :AutomaticSubtitling,
    :DocumentReading, :LipTrackingAnalysis, :MultimediaInformationExtraction, :OrthographicTranscription,
    :ParalanguageAnnotation, :PhoneticTranscription, :ProsodicAnnotation, :ProsodicInformationProcessing,
    :ProsodicSegmentation, :SoundEventAnnotation, :SoundToTextAlignment, :SpeakerDiarization,
    :SpeakerIdentification, :SpeakerVerification, :SpeechAnalysis, :SpeechAnalytics, :SpeechAnnotation,
    :SpeechEnhancement, :SpeechRecognition, :SpeechRetrieval, :SpeechSynthesis, :SpeechSynthesisEvaluation,
    :SpeechToSpeechTranslation, :SpeechToTextTranslation, :SpeechUnderstanding, :SpokenLanguageGeneration,
    :SpokenLanguageUnderstanding, :TextToSpeechSynthesis, :Transcription;
  skos:prefLabel "Speech Processing Collection"@en .

:FillMask skos:broader :SupportOperation .

:MultimodalSynthesis skos:inScheme :OperationScheme .

:TaskOrientedTextAnalysisEvaluation a skos:Concept;
  rdfs:label "Task-oriented text analysis evaluation"@en;
  skos:broader :Evaluation;
  skos:inScheme :OperationScheme;
  skos:prefLabel "Task-oriented text analysis evaluation"@en .

:GrammarChecking skos:broader :AuthoringSupport .

:Facility a skos:Concept;
  rdfs:label "Facility"@en;
  skos:broader :NamedEntity;
  skos:definition "A human-made artifact in the domains of architecture and civil engineering [source: https://www.nltk.org/book/ch07.html]"@en;
  skos:inScheme :AnnotationTypeScheme;
  skos:prefLabel "Facility"@en .

:DocumentImageAnalysis a skos:Concept;
  rdfs:label "Document image analysis"@en;
  skos:broader :OperationWithMultimediaInputOrOutput;
  skos:definition "Document image analysis is the theory and practice of recovering the logical structure of digital images scanned from documents or produced by computer. It includes optical character recognition as one of its subfields, but has more ambitious tasks, both in the breadth (understand diagrams, music scores, images ...), and depth (e.g. the correct interpretation of a scanned mathematical formula)."@en,
    "The processing of images of documents in order to obtain a machine-readable description of the their contents and structure from the pixel data [adapted from https://www.ias.ac.in/article/fulltext/sadh/027/01/0003-0022]"@en;
  skos:inScheme :OperationScheme;
  skos:prefLabel "Document image analysis"@en .

:ReadabilityAnnotator a skos:Concept;
  rdfs:label "Readability annotator"@en;
  skos:broader :SemanticAnnotator;
  skos:definition "A component that annotates the tokens of a text with readability scores"@en;
  skos:inScheme :ComponentTypeScheme;
  skos:prefLabel "Readability annotator"@en .

:SpeechSynthesisEvaluation a skos:Concept;
  rdfs:label "Speech Synthesis Evaluation"@en;
  skos:altLabel "Evaluation of Speech Synthesis"@en;
  skos:broader :Evaluation;
  skos:definition "Evaluation of speech synthesis traditionally considers intelligibility and naturalness. More recently, expressivity has become an issue with the increasing demand for expressive voices. Due to the multitude of aspects involved, there is no agreed standard for evaluation of speech synthesis systems. Since 2005, the Blizzard Challenge is an annual joint event for comparing speech synthesis technologies with a common database."@en;
  skos:inScheme :OperationScheme;
  skos:prefLabel "Speech Synthesis Evaluation"@en .

:application_vnd_openxmlformats_officedocument_presentationml_presentation rdfs:label
    "application/vnd.openxmlformats-officedocument.presentationml.presentation" .

:Conll2002 a skos:Concept;
  :documentationUrl "https://dkpro.github.io/dkpro-core/releases/1.8.0/docs/format-reference.html#format-Conll2002";
  :hasMimetype :text_x_org_dkpro_conll2002;
  rdfs:label "CoNLL-2002"@en;
  skos:broader :ConllFormat;
  skos:definition "The CoNLL 2002 format encodes named entity spans. Fields are separated by a single space. Sentences are separated by a blank new line."@en;
  skos:inScheme :DataFormatScheme;
  skos:prefLabel "CoNLL-2002"@en .

:Media a skos:Concept;
  rdfs:label "Media"@en;
  skos:broader :NamedEntity, :SocialSciencesEntity;
  skos:definition "The main means of mass communication (broadcasting, publishing, and the Internet) regarded collectively [https://en.oxforddictionaries.com/definition/media]"@en;
  skos:inScheme :AnnotationTypeScheme;
  skos:prefLabel "Media"@en .

:SpeechAssistedVideoControl a skos:Concept;
  rdfs:label "Speech-assisted video control"@en;
  skos:broader :OperationWithMultimediaInputOrOutput;
  skos:inScheme :OperationScheme;
  skos:prefLabel "Speech-assisted video control"@en .

:application_xml_alto a skos:Concept;
  rdfs:label "application/xml+alto";
  skos:broader :Mimetype;
  skos:inScheme :MimeTypeScheme .

:application_xLatex a skos:Concept;
  rdfs:label "application/x-latex";
  skos:broader :Mimetype;
  skos:inScheme :MimeTypeScheme .

:IonicConductance a skos:Concept;
  rdfs:label "Ionic conductance"@en;
  skos:altLabel "Ion conductance"@en;
  skos:broader :BiologicalEnity, :NamedEntity;
  skos:definition "Ionic conductance"@en;
  skos:inScheme :AnnotationTypeScheme;
  skos:prefLabel "Ionic conductance"@en .

:Alignment1 a skos:Concept;
  rdfs:label "Alignment"@en;
  skos:broader :AnnotationType;
  skos:definition "The translational equivalent between structural units (words, sentences etc.) of a text in a given language and a text with similar meaning in other language(s)"@en;
  skos:inScheme :AnnotationTypeScheme;
  skos:prefLabel "Alignment"@en .

:Generator a skos:Concept;
  rdfs:label "Generator"@en;
  skos:broader :Processor;
  skos:definition "A component that generates (semi-)automatically natural language texts (based on non-linguistic data, keywords, logical forms, knowledge bases...)"@en;
  skos:inScheme :ComponentTypeScheme;
  skos:narrower :Simplifier, :Summarizer;
  skos:prefLabel "Generator"@en .

:GenderDetection a skos:Concept;
  rdfs:label "Gender detection"@en;
  skos:broader :InformationExtraction;
  skos:inScheme :OperationScheme;
  skos:prefLabel "Gender detection"@en .

:image_png a skos:Concept;
  rdfs:label "image/png" .

:FillMask rdfs:label "Fill mask"@en .

:hasFileExtension rdfs:domain _:node1fu7rlrd8x2;
  rdfs:label "has file extension"@en;
  rdfs:range xsd:string .

:HumanAidedMachineTranslation skos:broader :MachineTranslation .

:Alignment skos:broader :MachineTranslationSupport .

:SpeechToTextTranslation skos:broader :Translation .

:SentenceAlignment a skos:Concept;
  rdfs:label "Sentence alignment"@en;
  skos:inScheme :OperationScheme .

:MethodOfResearch a skos:Concept;
  rdfs:label "Method of research"@en;
  skos:altLabel "Research method"@en;
  skos:broader :NamedEntity, :SocialSciencesEntity;
  skos:inScheme :AnnotationTypeScheme;
  skos:prefLabel "Method of research"@en .

:UserAuthentication a skos:Concept;
  rdfs:label "User authentication"@en;
  skos:broader :SupportOperation;
  skos:inScheme :OperationScheme;
  skos:prefLabel "User authentication"@en .

<http://w3id.org/meta-share/omtd-share/> dc:description """OMTD-SHARE ontology for resources related to Language Technology (LT) and Text and Data Mining. 
It was initiated in the framework of the OpenMinTeD project (https://www.openminted.eu) focusing on functions (tasks performed by software components), annotation types (types of information extracted or annotated by such software), methods (classification of the theoretical method used in the algorithm), and data formats of the resoures that can be processed by such software, based on metadata elements used in the META-SHARE metadata schema (http://www.meta-share.org/knowledgebase/homePage) and the FOSTER taxonomy of TDM (https://www.fosteropenscience.eu/resources).
Version 2 has been enriched with work done in the European Language Grid and other LT-related projects and has added LT-related terms in the ontology."""@en;
  dc:title "OMTD-SHARE ontology";
  dct:contributor "Richard Eckart de Castilho";
  dct:creator "Claire Nedellec", "Dimitris Galanis", "Katerina Gkirtzou", "Marta Villegas",
    "Penny Labropoulou", "Petr Knoth", "Sophie Aubin";
  dct:issued "2019-05-15";
  dct:license <http://purl.org/NET/rdflicense/cc-by4.0>;
  <http://purl.org/vocab/vann/preferredNamespacePrefix> "omtd";
  owl:priorVersion "1.1.0";
  owl:versionInfo "pre-release 2.0.0" .

:AccessComponent a skos:Concept;
  :performsOperation :ResourceAccess;
  rdfs:label "Access Component"@en;
  skos:broader :ComponentType;
  skos:definition "A component that provides access to data resources, e.g. reads a resource or writes the output of a process in a certain format"@en;
  skos:inScheme :ComponentTypeScheme;
  skos:narrower :Reader, :Writer;
  skos:prefLabel "Access Component"@en .

:BiologicalActivity a skos:Concept;
  rdfs:label "Biological activity"@en;
  skos:broader :BiologicalEnity, :NamedEntity;
  skos:inScheme :AnnotationTypeScheme;
  skos:prefLabel "Biological activity"@en .

:AudioFormat a skos:Concept;
  rdfs:label "Audio format"@en;
  skos:broader :DataFormat;
  skos:definition "Any format used for audio files"@en;
  skos:inScheme :DataFormatScheme;
  skos:narrower :RawAudioFormat, :aif, :basic, :flac, :mp3, :mpg, :wav;
  skos:prefLabel "Audio format"@en .

:ImageProcessing skos:inScheme :ModelFunctionScheme .

:ImageSegmentation skos:inScheme :ModelFunctionScheme .

:ImageGeneration skos:inScheme :ModelFunctionScheme .

:TextToImageGeneration skos:inScheme :ModelFunctionScheme .

:TextGeneration skos:inScheme :ModelFunctionScheme .

:zip :hasMimetype :zip .

:PolarityDetection a skos:Concept;
  rdfs:label "Polarity detection"@en;
  skos:broader :InformationExtraction;
  skos:inScheme :OperationScheme;
  skos:prefLabel "Polarity detection"@en;
  skos:related :PolarityLabelling .

:LexiconExtractionFromLexica a skos:Concept;
  rdfs:label "Lexicon extraction from lexica"@en;
  skos:broader :KnowledgeAcquisition, :SupportOperationForKnowledgeResources;
  skos:definition "The task/process of constructing lexical resources based on the restructuring of lexical information contained in lexica (e.g. by parsing definitions or using syntactic information attached to lemmas)"@en;
  skos:inScheme :OperationScheme;
  skos:prefLabel "Lexicon extraction from lexica"@en .

:ObjectDetection a skos:Concept;
  rdfs:label "Object detection"@en;
  skos:broader :OperationWithMultimediaInputOrOutput;
  skos:inScheme :OperationScheme;
  skos:prefLabel "Object detection"@en .

:LanguageIdentifier rdfs:label "Language identifier"@en .

:ProsodicInformationProcessing a skos:Concept;
  rdfs:label "Prosodic information processing"@en;
  skos:altLabel "Prosody information processing"@en;
  skos:definition "Prosody can be defined as a feature of speech which extends over more than one segment and is often synonymous with 'suprasegmentals'. Prosodic features include fundamental frequency (F0),relative duration and intensity, and spectral quality. They determine the rhythm and intonation of utterances."@en;
  skos:inScheme :OperationScheme;
  skos:prefLabel "Prosodic information processing"@en .

:application_x_org_dkpro_uima_json skos:broader :Mimetype;
  skos:inScheme :MimeTypeScheme .

:DeepParsing a skos:Concept;
  rdfs:label "Deep parsing"@en;
  skos:broader :Parsing;
  skos:definition "The  task/process of building complete parse trees for a sentence [adapted from https://stackoverflow.com/questions/37020577/shallow-parsing-vs-deep-parsing-in-stanford-corenlp-java]"@en;
  skos:inScheme :OperationScheme;
  skos:prefLabel "Deep parsing"@en .

:HateSpeechRecognition a skos:Concept;
  rdfs:label "Hate speech recognition"@en;
  skos:altLabel "Hate speech detection"@en;
  skos:broader :InformationExtraction;
  skos:definition "The task of automatically identifying hate speech, i.e. statements intended to demean and brutalize another, or the use of cruel and derogatory language on the basis of real or alleged membership in a social group [adapted from wikipedia]"@en;
  skos:inScheme :OperationScheme;
  skos:prefLabel "Hate speech recognition"@en .

:SyntacticoSemanticLink a skos:Concept;
  rdfs:label "Syntactico-semantic link"@en;
  skos:broader :SemanticAnnotationType, :SyntacticAnnotationType;
  skos:definition "A link between the syntactic unit and the semantic unit (sense) of a word"@en;
  skos:inScheme :AnnotationTypeScheme;
  skos:prefLabel "Syntactico-semantic link"@en .

:text_xPubmed a skos:Concept;
  rdfs:label "text/x-pubmed";
  skos:broader :Mimetype;
  skos:inScheme :MimeTypeScheme .

:AutomaticSubtitling a skos:Concept;
  rdfs:label "Automatic subtitling"@en;
  skos:broader :NaturalLanguageGeneration;
  skos:definition "The task/process of automatically adding subtitles to a video"@en;
  skos:inScheme :OperationScheme;
  skos:prefLabel "Automatic subtitling"@en .

:LexiconViewing a skos:Concept;
  rdfs:label "Lexicon viewing"@en;
  skos:broader :SupportOperationForKnowledgeResources, :Viewing;
  skos:definition "The task/process of viewing the contents of a lexicon as performed by human beings"@en;
  skos:inScheme :OperationScheme;
  skos:prefLabel "Lexicon viewing"@en .

:SpectralData a skos:Concept;
  rdfs:label "Spectral data"@en;
  skos:broader :NamedEntity;
  skos:definition "Spectral data is essentially data derived by the use of spectroscopic instruments"@en;
  skos:inScheme :AnnotationTypeScheme;
  skos:prefLabel "Spectral data"@en .

:AlvisEnrichedDocumentFormat a skos:Concept;
  :documentationUrl "http://www.lrec-conf.org/proceedings/lrec2006/pdf/742_pdf.pdf";
  :hasMimetype :application_xml;
  rdfs:label "ALVIS Enriched Document format"@en;
  skos:broader :AnnotationFormat, :Xml;
  skos:definition "Format for linguistic annotations of documents used for the ALVIS framework"@en;
  skos:inScheme :DataFormatScheme;
  skos:prefLabel "ALVIS Enriched Document format"@en .

:WikiFormats a skos:Concept;
  rdfs:label "Wiki formats"@en;
  owl:deprecated true;
  skos:broader :DataFormat;
  skos:definition "Superclass for wiki formats"@en;
  skos:inScheme :DataFormatScheme;
  skos:narrower :MediaWikiMarkup;
  skos:prefLabel "Wiki formats"@en .

:MultimediaRetrieval a skos:Concept;
  rdfs:label "Multimedia Retrieval"@en;
  skos:altLabel "MMIR"@en, "MR"@en, "Multimedia Information Retrieval"@en, "Multimedia Mining"@en;
  skos:broader :InformationRetrieval;
  skos:definition "The activity of obtaining multimedia information resources relevant to an information need from a collection of multimedia information resources"@en,
    "The research on multimedia retrieval focuses on the development of tools and techniques to support the easy access to information in digital archives. It exploits the synergy that exists between language & speech technology, image processing and database technology. The results can be used in innovative applications that support various content management tasks, e.g. automatic indexing of large text collections and disclosure of audiovisual archives, search technology and filtering of dynamic information streams. (taken from: http://parlevink.cs.utwente.nl/?page=onderwerp&onderwerpID=2"@en;
  skos:inScheme :OperationScheme;
  skos:prefLabel "Multimedia Retrieval"@en .

:Contradiction a skos:Concept;
  rdfs:label "Contradiction"@en;
  skos:broader :DiscourseAnnotationType;
  skos:definition "A set of statements that contradict each other (i.e. one of them asserts the truth and the other the falsity of the proposition)"@en;
  skos:inScheme :AnnotationTypeScheme;
  skos:prefLabel "Contradiction"@en .

:MorphosyntacticTagging a skos:Concept;
  rdfs:label "Morphosyntactic tagging"@en;
  skos:altLabel "Morphosyntactic annotation"@en;
  skos:broader :TextAnnotation;
  skos:definition "The task/process of adding morphosyntactic tags to words in a text, i.e. part-of-speech and, optionally, morphological features per part-of-speech."@en;
  skos:inScheme :OperationScheme;
  skos:narrower :BelowPosTagging, :PosTagging;
  skos:prefLabel "Morphosyntactic tagging"@en .

:Json_genia a skos:Concept;
  :documentationUrl "https://builds.openminted.eu/job/WP%205.2%20-%20Typesystem%20alignment/eu.openminted.interop$mapping-conversion/doclinks/1/components.html#GeniaJSONReader";
  :hasMimetype :application_json;
  rdfs:label "JSON/Genia"@en;
  skos:broader :BionlpFormat, :BionlpFormats, :Json;
  skos:definition "JSON format of the Genia dataset"@en;
  skos:inScheme :DataFormatScheme;
  skos:prefLabel "JSON/Genia"@en .

:CrowdsourcingComponent a skos:Concept;
  :performsOperation :SupportOfCrowdsourcingTasks;
  rdfs:label "Crowdsourcing component"@en;
  skos:broader :SupportComponent;
  skos:definition "A component that supports crowdsourcing operations"@en;
  skos:inScheme :ComponentTypeScheme;
  skos:prefLabel "Crowdsourcing component"@en .

:WikipediaPage a skos:Concept;
  :documentationUrl "https://dkpro.github.io/dkpro-core/releases/1.8.0/docs/format-reference.html#format-WikipediaPage";
  rdfs:label "Wikipedia page"@en;
  skos:broader :WikipediaFormat;
  skos:definition "Format of wikipedia pages in the database (articles, discussions, etc)"@en;
  skos:inScheme :DataFormatScheme;
  skos:prefLabel "Wikipedia page"@en .

:Frequency a skos:Concept;
  rdfs:label "Frequency"@en;
  skos:broader :QuantititativeInformation;
  skos:inScheme :AnnotationTypeScheme;
  skos:prefLabel "Frequency"@en .

:LanguageModelling a skos:Concept;
  rdfs:label "Language Modelling"@en;
  skos:altLabel "LM"@en, "Language Modeling"@en;
  skos:broader :SupportOperation;
  skos:definition "A Statistical Language Models predicts a word given a sequence of already known words (i.e. the history). Ist can also be applied to other sequences of symbols (e.g. DNA). Very often the history contains just the previous two words. This is called a trigram. The parameters of statistical language models are estimated from a set of training examples. Data sparsity and smoothing of the estimates is one of the core problems. The best smoothing technique known so far is Kneser-Ney-Smoothing. Maximum-Entropy techniques are also under investigation and may be the method of choice for long-range language models (beyond trigram). Language models are used in text-compression, speech recognition, information retrieval and information extraction."@en,
    "The construction of statistical or Machine Learning language models"@en;
  skos:inScheme :OperationScheme;
  skos:narrower :DialogueModelling, :StatisticalLanguageModelling, :TrainingOfLanguageModels,
    :TrainingOfMachineLearningModels, :TrainingOfNmtModels;
  skos:prefLabel "Language Modelling"@en .

:BncFormat a skos:Concept;
  :documentationUrl "https://dkpro.github.io/dkpro-core/releases/1.8.0/docs/format-reference.html#format-de.tudarmstadt.ukp.dkpro.core.io.bnc-asl";
  :hasMimetype :application_xml;
  rdfs:label "BNC format"@en;
  skos:broader :CorpusFormat, :Xml;
  skos:definition "Data format for the XML version of the British National Corpus (http://www.natcorp.ox.ac.uk/)"@en;
  skos:inScheme :DataFormatScheme;
  skos:prefLabel "BNC format"@en .

:NamedEntity a skos:Concept;
  rdfs:label "Named entity"@en;
  skos:broader :SemanticAnnotationType;
  skos:definition "A word or phrase referring to an entity, identified and annotated as such with a name (label); examples include organizations, persons, places etc."@en;
  skos:inScheme :AnnotationTypeScheme;
  skos:narrower :BiologicalActivity, :BrainRegion, :Chemical, :Date, :Facility, :Geo-politicalEntity,
    :HistoricalEvent, :IonicChannel, :IonicConductance, :IonicCurrent, :Location, :Media,
    :Metabolite, :MethodOfResearch, :Miscellaneous, :ModelOrganism_species, :Neuron, :OfficialText,
    :Organization, :Person, :Protein, :ScientificUnit, :ScientificValue, :Species, :SpectralData,
    :Synapse, :TheoreticalFrame;
  skos:prefLabel "Named entity"@en .

:EventExtractor a skos:Concept;
  :performsOperation :EventDetection;
  rdfs:label "Event extractor"@en;
  skos:broader :Analyzer;
  skos:definition "A component that tries to extract information related to incidents referred to in a text"@en;
  skos:editorialNote "could also be an annotator"@en;
  skos:inScheme :ComponentTypeScheme;
  skos:prefLabel "Event extractor"@en .

:Owl a skos:Concept;
  rdfs:label "OWL"@en;
  skos:broader :RdfFormat, :RdfFormats;
  skos:definition "Superclass for formats used for OWL"@en;
  skos:inScheme :DataFormatScheme;
  skos:narrower :Owl_xml;
  skos:prefLabel "OWL"@en .

:Conll2006 a skos:Concept;
  :documentationUrl "https://dkpro.github.io/dkpro-core/releases/1.8.0/docs/format-reference.html#format-Conll2006";
  :hasMimetype :text_x_org_dkpro_conll2006;
  rdfs:label "CoNLL-2006"@en;
  skos:altLabel "CoNLL-2007"@en, "CoNLL-X"@en;
  skos:broader :ConllFormat;
  skos:definition "The CoNLL 2006 (aka CoNLL-X) format targets dependency parsing. Columns are tab-separated. Sentences are separated by a blank new line."@en;
  skos:inScheme :DataFormatScheme;
  skos:prefLabel "CoNLL-2006"@en .

:WikipediaQuery a skos:Concept;
  :documentationUrl "https://dkpro.github.io/dkpro-core/releases/1.8.0/docs/format-reference.html#format-WikipediaQuery";
  rdfs:label "Wikipedia query"@en;
  skos:broader :WikipediaFormat;
  skos:definition "Reads all article pages that match a query created by the numerous parameters of this class."@en;
  skos:inScheme :DataFormatScheme;
  skos:prefLabel "Wikipedia query"@en .

:TerminologyMarkup a skos:Concept;
  rdfs:label "Terminology markup"@en;
  skos:altLabel "Annotation of terms"@en, "Term labelling"@en;
  skos:broader :SemanticAnnotation;
  skos:inScheme :OperationScheme;
  skos:prefLabel "Terminology markup"@en .

:PersuasiveExpressionMining a skos:Concept;
  rdfs:label "Persuasive expression mining"@en;
  skos:broader :InformationExtraction;
  skos:definition "The task/process of identifying and extracting (especially from political speech texts) pieces of text that aim to persuade"@en;
  skos:inScheme :OperationScheme;
  skos:prefLabel "Persuasive expression mining"@en .

:NormalizationOfMeasurements a skos:Concept;
  rdfs:label "Normalization of measurements"@en;
  skos:broader :Normalization;
  skos:definition "The task/process of substituting measurements with normalized values"@en;
  skos:inScheme :OperationScheme;
  skos:prefLabel "Normalization of measurements"@en .

:LanguageChecking a skos:Concept;
  rdfs:label "Language checking"@en;
  skos:altLabel "Proofing"@en;
  skos:broader :AuthoringSupport;
  skos:definition "Language Checking comprises technologies used to detect and/or correct erroneous or inconsistent language use in documents. The scope of language checking technology ranges from general error correction, as performed by spell checkers and grammar checkers"@en,
    "The task/process of identifying (and usually correcting) grammatical mistakes in a text"@en;
  skos:inScheme :OperationScheme;
  skos:prefLabel "Language checking"@en .

:DiscourseAnnotationType a skos:Concept;
  rdfs:label "Discourse annotation type"@en;
  owl:equivalentClass <http://purl.org/olia/olia-top.owl#DiscourseFeature>;
  skos:broader :AnnotationType;
  skos:definition "Any type of annotation relevant to discourse"@en;
  skos:inScheme :AnnotationTypeScheme;
  skos:narrower :AudienceReaction, :Contradiction, :Coreference, :DiscourseRelation,
    :SpeechAct;
  skos:prefLabel "Discourse annotation type"@en .

:Imscwb a skos:Concept;
  :documentationUrl "https://dkpro.github.io/dkpro-core/releases/1.8.0/docs/format-reference.html#format-de.tudarmstadt.ukp.dkpro.core.io.imscwb-asl";
  :hasMimetype :text_x_org_dkpro_imscwb;
  rdfs:label "imsCwb"@en;
  skos:altLabel "IMS Corpus Workbench"@en;
  skos:broader :CorpusFormat, :TabularFormat;
  skos:definition "A tab-separated format with limited markup (e.g. for sentences, documents, but not recursive structures like parse-trees) used by the IMS Open Corpus Workbench."@en;
  skos:inScheme :DataFormatScheme;
  skos:prefLabel "imsCwb"@en .

:bmp a skos:Concept;
  :hasFileExtension "bmp";
  :hasMimetype :image_bmp;
  rdfs:label "BMP"@en;
  skos:altLabel "Bitmap Graphics"@en;
  skos:broader :ImageFormat;
  skos:inScheme :DataFormatScheme;
  skos:prefLabel "BMP"@en .

:TabularFormat a skos:Concept;
  rdfs:label "Tabular format"@en;
  skos:broader :DataFormat;
  skos:definition "Any format based on columns"@en;
  skos:inScheme :DataFormatScheme;
  skos:narrower :ConllFormat, :Csv, :Imscwb, :MsExcel, :OasisSpreadsheet, :OpenOfficeSpreadsheet,
    :Tsv;
  skos:prefLabel "Tabular format"@en .

:LanguageCode a skos:Concept;
  rdfs:label "Language code"@en;
  skos:broader :AnnotationType;
  skos:inScheme :AnnotationTypeScheme;
  skos:prefLabel "Language code"@en .

:Postscript a skos:Concept;
  :documentationUrl "https://www.iana.org/assignments/media-types/application/postscript";
  :hasFileExtension "ps";
  :hasMimetype :application_postscript;
  rdfs:label "postscript"@en;
  skos:broader :DocumentFormat;
  skos:definition "Data format for PostScript files"@en;
  skos:inScheme :DataFormatScheme;
  skos:prefLabel "postscript"@en .

:ModalityAnnotationType a skos:Concept;
  rdfs:label "Modality annotation type"@en;
  skos:broader :AnnotationType;
  skos:inScheme :AnnotationTypeScheme;
  skos:narrower :BodyMovement, :FacialExpression, :GazeEyeMovement, :HeadMovement, :LipMovement;
  skos:prefLabel "Modality annotation type"@en .

:RdfFormat a skos:Concept;
  dct:replaces :RdfFormats;
  rdfs:label "RDF format"@en;
  skos:broader :DataFormat;
  skos:definition "Formats for RDF (Resource Description Framework) resources"@en;
  skos:inScheme :DataFormatScheme;
  skos:narrower :Nif, :Obo, :Owl, :Rdf_xml, :Turtle;
  skos:prefLabel "RDF format"@en .

:Gate_twitter_json a skos:Concept;
  :documentationUrl "https://gate.ac.uk/sale/tao/splitch17.html";
  :hasMimetype :application_x_json_twitter;
  rdfs:label "GATE/JSON twitter"@en;
  skos:altLabel "Twitter/JSON"@en;
  skos:broader :GateFormat, :Json;
  skos:definition "A Twitter-style JSON format used for GATE documents"@en;
  skos:inScheme :DataFormatScheme;
  skos:prefLabel "GATE/JSON twitter"@en .

:Pls a skos:Concept;
  :documentationUrl "https://www.iana.org/assignments/media-types/application/pls+xml";
  :hasMimetype :application_pls_xml;
  rdfs:label "PLS"@en;
  skos:broader :DocumentFormat, :Xml;
  skos:definition "Data format according to the Pronunciation Lexicon Specification (PLS)"@en;
  skos:inScheme :DataFormatScheme;
  skos:prefLabel "PLS"@en .

:TextCategorization a skos:Concept;
  rdfs:label "Text categorization"@en;
  skos:altLabel "Document categorisation"@en, "Document categorisation"@en-uk, "Document categorization"@en,
    "Document classification"@en, "Text categorisation"@en-uk, "Text classification"@en;
  skos:broader :InformationExtraction;
  skos:definition "The task/process of assigning documents into classes or categories"@en;
  skos:inScheme :OperationScheme;
  skos:prefLabel "Text categorization"@en .

:ConceptNormalization a skos:Concept;
  rdfs:label "Concept normalization"@en;
  skos:altLabel "Concept normalisation"@en-uk;
  skos:broader :Normalization;
  skos:definition "The task of mapping free-form expressions to the concepts of a specific domain"@en;
  skos:inScheme :OperationScheme;
  skos:narrower :BiomedicalConceptNormalization;
  skos:prefLabel "Concept normalization"@en .

:OpticalCharacterRecognition a skos:Concept;
  rdfs:label "Optical Character Recognition"@en;
  skos:altLabel "OCR"@en;
  skos:broader :SupportOperation;
  skos:definition "The task/process of converting handwritten or printed material into machine editable text"@en;
  skos:inScheme :OperationScheme;
  skos:prefLabel "Optical Character Recognition"@en .

:Tokenization a skos:Concept;
  rdfs:label "Tokenization"@en;
  skos:altLabel "Segmentation"@en, "Segmentation and Tokenisation"@en-uk, "Segmentation and Tokenization"@en,
    "Tokenisation"@en-uk;
  skos:broader :StructuralAnnotation;
  skos:definition "The task/process of recognizing and tagging tokens (words, punctuation marks, digits etc.) in a text"@en,
    "Tokenization is commonly seen as an independent process of linguistic analysis, in which the input stream of characters is segmented into an ordered sequence of word-like units, usually called tokens, which function as input items for subsequent steps of linguistic processing. Tokens may correspond to words, numbers, punctuation marks or even proper names.The recognized tokens are usually classified according to their syntax. Since the notion of tokenization seems to have different meanings to different people, some tokenization tools fulfil additional tasks like for instance sentence boundary detection, handling of end-line hyphenations or conjoined clitics and contractions."@en;
  skos:inScheme :OperationScheme;
  skos:prefLabel "Tokenization"@en .

:WikiFormat a skos:Concept;
  dct:replaces :WikiFormats;
  rdfs:label "Wiki format"@en;
  skos:broader :DataFormat;
  skos:definition "Superclass for wiki formats"@en;
  skos:inScheme :DataFormatScheme;
  skos:narrower :MediaWikiMarkup;
  skos:prefLabel "Wiki format"@en .

:PhoneticTranscription1 a skos:Concept;
  rdfs:label "Phonetic transcription"@en;
  skos:broader :Transcription1;
  skos:inScheme :AnnotationTypeScheme;
  skos:prefLabel "Phonetic transcription"@en .

:AimedCorpusFormat a skos:Concept;
  :documentationUrl "https://builds.openminted.eu/job/WP%205.2%20-%20Typesystem%20alignment/eu.openminted.interop$mapping-conversion/doclinks/1/components.html#Aimed_Collection_Reader";
  rdfs:label "AIMED corpus format"@en;
  skos:broader :CorpusFormat;
  skos:definition "Format of the Aimed corpus (225 abstracts from MEDLINE) with the gold standard sentence, protein, protein-protein interaction annotations."@en;
  skos:inScheme :DataFormatScheme;
  skos:prefLabel "AIMED corpus format"@en .

:Writer a skos:Concept;
  :performsOperation :Writing;
  rdfs:label "Writer"@en;
  skos:broader :AccessComponent;
  skos:definition "A component that writes processing results in various formats"@en;
  skos:inScheme :ComponentTypeScheme;
  skos:prefLabel "Writer"@en .

:CBOR a skos:Concept;
  :documentationUrl "https://cbor.io/spec.html", "https://www.rfc-editor.org/rfc/rfc8949.html";
  rdfs:label "CBOR"@en;
  skos:altLabel "Concise Binary Object Representation"@en;
  skos:broader :BinaryFormat;
  skos:definition "Concise Binary Object Representation (CBOR) data format; defined as an ISO standard (RFC 8949, https://cbor.io/spec.html)"@en;
  skos:inScheme :DataFormatScheme;
  skos:prefLabel "CBOR"@en .

:AnnotationOfSpeakerTurns a skos:Concept;
  rdfs:label "Annotation of speaker turns"@en;
  skos:broader :SpeechAnnotation;
  skos:definition "The task/process of marking locations in speech where there is a change of speakers"@en;
  skos:inScheme :OperationScheme;
  skos:prefLabel "Annotation of speaker turns"@en .

:SpeechRecognition a skos:Concept;
  rdfs:label "Speech Recognition"@en;
  skos:altLabel "ASR"@en, "Automatic speech recognition"@en, "Computer speech recognition"@en,
    "SR"@en, "Voice recognition"@en;
  skos:broader :OperationWithMultimediaInputOrOutput;
  skos:definition "Automatic Speech Recognition deals with automatic transcribing spoken language as text which is further processed in application dependent ways. Important applications are dictation, control of machines and devices by speech, information systems, speech translation, aids for disabled persons. An increasingly important application is embedded speech recognition in devices such as mobile phones and PDAs."@en,
    "The use of computer hardware and software-based techniques to identify and process human voice used tused to identify the words a person has spoken or to authenticate the identity of the person speaking into the system [adapted from https://www.techopedia.com/definition/6044/automatic-speech-recognition-asr]"@en;
  skos:inScheme :OperationScheme;
  skos:narrower :LipTrackingAnalysis, :SpeakerIdentification, :SpeakerVerification,
    :SpeechAnalysis, :SpeechEnhancement, :SpeechUnderstanding, :SpokenLanguageUnderstanding,
    :Transcription;
  skos:prefLabel "Speech Recognition"@en .

:application_x_org_dkpro_uima_json a skos:Concept;
  rdfs:label "application/x.org.dkpro.uima+json" .

:SemanticAnnotationType a skos:Concept;
  rdfs:label "Semantic annotation type"@en;
  skos:broader :AnnotationType;
  skos:definition "Any type of annotation pertaining to the semantic level"@en;
  skos:inScheme :AnnotationTypeScheme;
  skos:narrower :CertaintyLevel, :Emotion, :Event, :Keyword, :LexicalSemanticRelation,
    :NamedEntity, :PersuasiveExpression, :Polarity, :QuestionTopicalTarget, :Readability,
    :SemanticClass, :SemanticFrame, :SemanticRole, :Sentiment, :Subjectivity, :SyntacticoSemanticLink,
    :TemporalExpression, :TextualEntailment, :Topic, :VerbalAggressionTarget, :WordSense;
  skos:prefLabel "Semantic annotation type"@en .

:MultimodalSynthesis skos:broader :OperationWithMultimediaInputOrOutput;
  skos:definition "The generation of a multimodal output resource"@en;
  skos:prefLabel "Multimodal synthesis"@en;
  skos:related :MultimodalIntegration .

:ImageVideoProcessingCollection skos:member :MultimodalSynthesis .

:LanguageIdentifier skos:inScheme :ComponentTypeScheme .

:OperationWithMultimediaInputOrOutput skos:narrower :MultimodalSynthesis .

:TextToTextGeneration skos:inScheme :ModelFunctionScheme .

:Matcher a skos:Concept;
  :performsOperation :Matching;
  rdfs:label "Matcher"@en;
  skos:broader :SupportComponent;
  skos:definition "A component that allows matching of elements"@en;
  skos:inScheme :ComponentTypeScheme;
  skos:narrower :GazeteerBasedMatcher;
  skos:prefLabel "Matcher"@en .

:Summarization a skos:Concept;
  rdfs:label "Summarization"@en;
  skos:altLabel "ATS"@en, "Automatic Summarisation"@en-uk, "Automatic Summarization"@en,
    "Automatic Text Summarisation"@en-uk, "Automatic Text Summarization"@en, "Summarisation"@en-uk,
    "TS"@en, "Text Summarisation"@en-uk, "Text Summarization"@en;
  skos:broader :ModelFunction, :NaturalLanguageGeneration;
  skos:definition "Text summarization is the process of distilling the most important information from a source (or sources) to produce an abridged version for a particular user (or users) and task (or tasks). Source: Mani, I. and Maybury, M. T., editors (1999), Advances in Automatic Text Summarization. MIT Press, Cambridge, Massachusetts."@en,
    "The process/task of reducing one or more textual documents with a computer program in order to create a summary that retains the most important points of the original document(s)."@en;
  skos:inScheme :OperationScheme;
  skos:prefLabel "Summarization"@en .

:FacialExpressionRecognition rdfs:label "Facial expression recognition"@en .

:QuestionAnswering a skos:Concept;
  rdfs:label "Question Answering"@en;
  skos:altLabel "AE"@en, "Answer Extraction"@en, "QA"@en, "Textual Question Answering"@en;
  skos:broader :InformationExtraction, :KnowledgeDiscovery, :ModelFunction;
  skos:definition "Question answering or Answer extraction (AE) aims at retrieving those exact passages of a document that directly answer a given user question. AE is more ambitious than information retrieval and information extraction in that the retrieval results are short phrases, not entire documents, and in that the queries may be arbitrarily specific. It is less ambitious than full-fledged question answering in that the answers are not generated from a knowledge base but looked up in the text of documents."@en,
    "The task/process where computer systems try to automatically answer questions posed by users in the form of natural language."@en;
  skos:inScheme :OperationScheme;
  skos:prefLabel "Question Answering"@en .

:DataCollector a skos:Concept;
  :performsOperation :DataCollection;
  rdfs:label "Data collector"@en;
  skos:broader :SupportComponent;
  skos:definition "A component that collects (retrieves) data from various sources"@en;
  skos:inScheme :ComponentTypeScheme;
  skos:narrower :Crawler;
  skos:prefLabel "Data collector"@en .

:LexiconViewer a skos:Concept;
  :performsOperation :LexiconViewing;
  rdfs:label "Lexicon viewer"@en;
  skos:broader :Viewer;
  skos:definition "A component that supports humans in accessing the contents of a lexical/conceptual resource"@en;
  skos:inScheme :ComponentTypeScheme;
  skos:prefLabel "Lexicon viewer"@en .

:Anafora a skos:Concept;
  :documentationUrl "https://www.ncbi.nlm.nih.gov/pmc/articles/PMC5657237/";
  :hasMimetype :text_x_anafora;
  rdfs:label "Anafora"@en;
  skos:broader :AnnotationFormat;
  skos:inScheme :DataFormatScheme;
  skos:prefLabel "Anafora"@en .

:Tokenizer a skos:Concept;
  rdfs:label "Tokenizer"@en;
  skos:broader :Segmenter;
  skos:definition "A component that recognizes and tags tokens (words, punctuation marks, digits etc.) in a text"@en;
  skos:inScheme :ComponentTypeScheme;
  skos:prefLabel "Tokenizer"@en .

:TextEncryption a skos:Concept;
  rdfs:label "Text encryption"@en;
  skos:broader :Anonymization;
  skos:definition "A cryptosystem or cipher system is a method of disguising messages so that only certain people can see through the disguise. Cryptography is the art of creating and using cryptosystems. Cryptanalysis is the art of breaking cryptosystems---seeing through the disguise even when you're not supposed to be able to. Cryptology is the study of both cryptography and cryptanalysis."@en;
  skos:inScheme :OperationScheme;
  skos:prefLabel "Text encryption"@en .

:jpg a skos:Concept;
  :hasFileExtension "jpeg", "jpg";
  :hasMimetype :image_jpeg;
  rdfs:label "JPEG"@en;
  skos:altLabel "JPG"@en;
  skos:broader :ImageFormat;
  skos:inScheme :DataFormatScheme;
  skos:prefLabel "JPEG"@en .

:TigerXml a skos:Concept;
  :documentationUrl "http://www.ims.uni-stuttgart.de/forschung/ressourcen/werkzeuge/TIGERSearch/doc/html/TigerXML.html",
    "https://dkpro.github.io/dkpro-core/releases/1.8.0/docs/format-reference.html#format-de.tudarmstadt.ukp.dkpro.core.io.tiger-asl";
  :hasMimetype :application_x_org_dkpro_tiger_xml;
  rdfs:label "Tiger XML"@en;
  skos:broader :AnnotationFormat, :CorpusFormat, :Xml;
  skos:definition "The TIGER XML format was created for encoding syntactic constituency structures in the German TIGER corpus. It has since been used for many other corpora as well. TIGERSearch is a linguistic search engine specifically targetting this format. The format has later been extended to also support semantic frame annotations."@en;
  skos:inScheme :DataFormatScheme;
  skos:prefLabel "Tiger XML"@en .

:XcesIlspVariant a skos:Concept;
  :hasMimetype :application_xXces_xml;
  rdfs:label "XCES ILSP variant"@en;
  skos:altLabel "xces; format-variant=ilsp"@en;
  skos:broader :Xces;
  skos:definition "A variant of XCES implemented for documents"@en;
  skos:inScheme :DataFormatScheme;
  skos:prefLabel "XCES ILSP variant"@en .

:Emma a skos:Concept;
  :hasMimetype :application_emma_xml;
  rdfs:label "EMMA"@en;
  skos:broader :AnnotationFormat, :Xml;
  skos:definition "Data format according to the EMMA (Extensible MultiModal Annotation markup language) specifications, cf. https://www.w3.org/TR/2007/CR-emma-20071211/"@en;
  skos:inScheme :DataFormatScheme;
  skos:prefLabel "EMMA"@en .

:Solr a skos:Concept;
  :documentationUrl "https://dkpro.github.io/dkpro-core/releases/1.8.0/docs/format-reference.html#format-de.tudarmstadt.ukp.dkpro.core.io.solr-asl";
  rdfs:label "Solr"@en;
  skos:broader :DataFormat;
  skos:definition "Solr format"@en;
  skos:inScheme :DataFormatScheme;
  skos:prefLabel "Solr"@en .

:KnowledgeDiscovery a skos:Concept;
  rdfs:label "Knowledge Discovery"@en;
  skos:altLabel "KD"@en, "KDD"@en, "Knowledge Discovery in Databases"@en;
  skos:broader :TextAndDataMining;
  skos:definition "Generally, knowledge discovery / data mining is the process of analyzing data from different perspectives and summarizing it into useful information - information that can be used to increase revenue, cuts costs, or both. Data mining software is one of a number of analytical tools for analyzing data. It allows users to analyze data from many different dimensions or angles, categorize it, and summarize the relationships identified. Technically, data mining is the process of finding correlations or patterns among dozens of fields in large relational databases."@en,
    "The task/process of automatically searching large volumes of data for patterns that can be considered knowledge about the data"@en;
  skos:inScheme :OperationScheme;
  skos:narrower :QuestionAnswering, :RecognizingTextualEntailment;
  skos:prefLabel "Knowledge Discovery"@en .

:Blikiwikipedia rdfs:label "blikiWikipedia"@en .

:Datasift_json a skos:Concept;
  :documentationUrl "https://gate.ac.uk/sale/tao/splitch23.html#x28-59500023.32";
  :hasMimetype :application_json;
  rdfs:label "DataSift/JSON"@en;
  skos:broader :GateFormat, :Json;
  skos:definition "Common format for social media data from http://datasift.com"@en;
  skos:inScheme :DataFormatScheme;
  skos:prefLabel "DataSift/JSON"@en .

:Lemmatizer a skos:Concept;
  :performsOperation :Lemmatization;
  rdfs:label "Lemmatizer"@en;
  skos:broader :Annotator;
  skos:definition "A component that annotates the tokens of a text with lemma information"@en;
  skos:inScheme :ComponentTypeScheme;
  skos:prefLabel "Lemmatizer"@en .

:Reuters21578Txt a skos:Concept;
  :documentationUrl "https://dkpro.github.io/dkpro-core/releases/1.8.0/docs/format-reference.html#format-Reuters21578Txt";
  :hasMimetype :text_x_org_dkpro_reuters21578;
  rdfs:label "Reuters21578 Txt"@en;
  skos:broader :CorpusFormat;
  skos:definition "Reuters-21578 corpus transformed into text format using ExtractReuters in the lucene-benchmarks project"@en;
  skos:inScheme :DataFormatScheme;
  skos:prefLabel "Reuters21578 Txt"@en .

:MOSESFormat a skos:Concept;
  rdfs:label "MOSES plain text format"@en;
  skos:broader :CorpusFormat;
  skos:definition "MOSES format for aligned corpora (monolingual plain text files with language on file extension)"@en;
  skos:inScheme :DataFormatScheme;
  skos:prefLabel "MOSES plain text format"@en .

:Web1t a skos:Concept;
  :documentationUrl "https://catalog.ldc.upenn.edu/LDC2006T13", "https://zoidberg.ukp.informatik.tu-darmstadt.de/jenkins/job/DKPro%20Core%20Documentation%20(GitHub)/de.tudarmstadt.ukp.dkpro.core$de.tudarmstadt.ukp.dkpro.core.doc-asl/doclinks/5/format-reference.html#format-Web1T";
  :hasMimetype :text_x_org_dkpro_ngram;
  rdfs:label "Web1T"@en;
  skos:broader :CorpusFormat;
  skos:definition "File format used by the Web1T n-gram corpus, a huge collection of n-grams collected from the internet."@en;
  skos:inScheme :DataFormatScheme;
  skos:prefLabel "Web1T"@en .

:Metabolite a skos:Concept;
  rdfs:label "Metabolite"@en;
  skos:broader :BiologicalEnity, :NamedEntity;
  skos:definition "Any substance involved in metabolism (= the chemical processes in the body needed for life) [https://dictionary.cambridge.org/dictionary/english/metabolite]"@en;
  skos:inScheme :AnnotationTypeScheme;
  skos:prefLabel "Metabolite"@en .

:Gene a skos:Concept;
  rdfs:label "Gene"@en;
  skos:broader :AgriculturalEntity;
  skos:definition "Specific sequence of nucleotides along a molecule of DNA (or, in the case of some viruses, RNA) which represents functional units of heredity [http://artemide.art.uniroma2.it:8081/agrovoc/agrovoc/en/page/c_3214]"@en;
  skos:inScheme :AnnotationTypeScheme;
  skos:prefLabel "Gene"@en .

:Parsing a skos:Concept;
  rdfs:label "Parsing"@en;
  skos:altLabel "Syntactic analysis"@en, "Syntactic annotation"@en, "Syntactic parsing"@en,
    "Syntactic processing"@en;
  skos:broader :LinguisticAnalysis, :TextAnnotation;
  skos:definition "Parsing (=syntactic analysis) of natural language utterances is still an active reasearch topic due to the inherent difficulties that make the problem much harder than e.g. parsing of programming languages. These difficulties include lexical and structural ambiguity of natural language utterances, complexities introduced by expressive grammar formalisms, the need to cope with illformed input or with deficiencies of the linguistic descriptions."@en,
    "The task/process of recognizing and marking the syntactic structure of a text or text segment"@en;
  skos:inScheme :OperationScheme;
  skos:narrower :Chunking, :ConstituencyParsing, :DeepParsing, :DependencyParsing, :FrameSemanticParsing;
  skos:prefLabel "Parsing"@en .

:Kaf a skos:Concept;
  :documentationUrl "http://kyoto-project.eu/xmlgroup.iit.cnr.it/kyoto/indexdd46.html?option=com_content&view=article&id=141&Itemid=130";
  :hasMimetype :application_x_kaf_json;
  rdfs:label "KAF"@en;
  skos:altLabel "KYOTO Annotation Format"@en, "Knowledge Annotation Format"@en;
  skos:broader :AnnotationFormat, :Json;
  skos:definition "KAF (also known as Knowledge Annotation Format) is a language neutral annotation format representing both morpho-syntactic and semantic annotation of documents through a stand-off multilayered structure"@en;
  skos:inScheme :DataFormatScheme;
  skos:prefLabel "KAF"@en .

:LexicalSemanticRelation a skos:Concept;
  rdfs:label "Lexical semantic relation"@en;
  owl:equivalentClass <http://purl.org/olia/olia-top.owl#LexicalRelation>;
  skos:altLabel "Semantic relation"@en;
  skos:broader :SemanticAnnotationType;
  skos:definition "A relation holding between two or more words based on their meanings"@en;
  skos:inScheme :AnnotationTypeScheme;
  skos:prefLabel "Lexical semantic relation"@en .

:application_vnd_msExcel a skos:Concept;
  rdfs:label "application/vnd.msExcel";
  skos:broader :Mimetype;
  skos:inScheme :MimeTypeScheme .

:Evaluator a skos:Concept;
  :performsOperation :Evaluation;
  rdfs:label "Evaluator"@en;
  skos:broader :SupportComponent;
  skos:definition "A component that is used in the evaluation of the performance of a component"@en;
  skos:inScheme :ComponentTypeScheme;
  skos:prefLabel "Evaluator"@en .

:Stem a skos:Concept;
  :documentationUrl "http://dkpro.github.io/dkpro-core/releases/1.8.0/docs/typesystem-reference.html#de.tudarmstadt.ukp.dkpro.core.api.segmentation.type.Stem";
  rdfs:label "Stem"@en;
  owl:equivalentClass <http://purl.org/olia/olia-top.owl#Stem>;
  skos:broader :MorphologicalAnnotationType;
  skos:definition "A stem is the root or roots of a word, together with any derivational affixes, to which inflectional affixes are added. [http://www.glossary.sil.org/term/stem]"@en;
  skos:inScheme :AnnotationTypeScheme;
  skos:prefLabel "Stem"@en .

:Paragraph a skos:Concept;
  rdfs:label "Paragraph"@en;
  owl:equivalentClass <http://vocab.lappsgrid.org/Paragraph>;
  skos:broader :StructuralAnnotationType;
  skos:definition "A division of a text, usually about a single theme, consisting of one or more sentences and marked by a new line, indentation or other conventions."@en;
  skos:inScheme :AnnotationTypeScheme;
  skos:prefLabel "Paragraph"@en .

:text_x_org_dkpro_conllU a skos:Concept;
  rdfs:label "text/x.org.dkpro.conll-u";
  skos:broader :Mimetype;
  skos:inScheme :MimeTypeScheme .

:VerbalAggressionTarget a skos:Concept;
  rdfs:label "Verbal aggression target"@en;
  skos:altLabel "Verbal attack target"@en;
  skos:broader :SemanticAnnotationType;
  skos:definition "The target of verbal attacks"@en;
  skos:inScheme :AnnotationTypeScheme;
  skos:prefLabel "Verbal aggression target"@en .

:ScholarlyAnalyticsEntity a skos:Concept;
  dct:replaces :ScholarlyCommunicationAnnotation;
  rdfs:label "Scholarly analytics entity"@en;
  skos:broader :DomainSpecificAnnotationType;
  skos:definition "Any type of annotation that is relevant to scholarly analtyics (e.g. citations, funding information etc.)"@en;
  skos:inScheme :AnnotationTypeScheme;
  skos:narrower :Citation, :DocumentSection, :Funding, :Keyword;
  skos:prefLabel "Scholarly analytics entity"@en .

skos:Concept a owl:Class .

:SemanticRole a skos:Concept;
  :documentationUrl "http://dkpro.github.io/dkpro-core/releases/1.8.0/docs/typesystem-reference.html#de.tudarmstadt.ukp.dkpro.core.api.semantics.type.SemanticArgument";
  rdfs:label "Semantic role"@en;
  owl:equivalentClass <http://purl.org/olia/olia-top.owl#SemanticRole>, <http://vocab.lappsgrid.org/SemanticRole>;
  skos:broader :SemanticAnnotationType;
  skos:definition "A semantic role is the underlying relationship that a participant has with the main verb in a clause [http://www.glossary.sil.org/term/semantic-role]"@en;
  skos:inScheme :AnnotationTypeScheme;
  skos:prefLabel "Semantic role"@en .

:PtbChunked a skos:Concept;
  :documentationUrl "https://zoidberg.ukp.informatik.tu-darmstadt.de/jenkins/job/DKPro%20Core%20Documentation%20(GitHub)/de.tudarmstadt.ukp.dkpro.core$de.tudarmstadt.ukp.dkpro.core.doc-asl/doclinks/5/format-reference.html#format-PennTreebankChunked";
  :hasMimetype :text_x_org_dkpro_ptbChunked;
  rdfs:label "PTB-chunked"@en;
  skos:altLabel "Penn Treebank - chunked"@en, "ptb; format-variant=chunked"@en;
  skos:broader :Ptb;
  skos:definition "Penn Treebank chunked format"@en;
  skos:inScheme :DataFormatScheme;
  skos:prefLabel "PTB-chunked"@en .

:LexiconVisualization a skos:Concept;
  rdfs:label "Lexicon visualization"@en;
  skos:altLabel "Lexicon visualisation"@en-uk;
  skos:broader :SupportOperationForKnowledgeResources, :Visualization;
  skos:definition "The task/process of visualizing information (e.g. using diagrams, 3-d images, word clouds etc.) contained in lexical/conceptual resources"@en;
  skos:inScheme :OperationScheme;
  skos:prefLabel "Lexicon visualization"@en .

:MorphologicalAnnotationType a skos:Concept;
  rdfs:label "Morphological annotation type"@en;
  skos:broader :AnnotationType;
  skos:definition "Any type of annotation pertaining to the morphological level"@en;
  skos:inScheme :AnnotationTypeScheme;
  skos:narrower :Compound, :DerivationalFeature, :Lemma, :MorphologicalFeature, :Stem,
    :Word;
  skos:prefLabel "Morphological annotation type"@en .

:NaturalLanguageGeneration a skos:Concept;
  rdfs:label "Natural Language Generation"@en;
  skos:altLabel "Generation"@en, "NLG"@en, "Synthesis"@en;
  skos:broader :Operation;
  skos:definition "Natural Language Generation (NLG) is concerned with turning some usually non-linguistic representation of information and intended effect into fluent text preserving both meaning and intention. NLG systems often identify the content to be verbalized. They structure the document into interrelated sentence-sized chunks, choose appropriate words, aggregate and elide information to ensure fluency, create contextually appropriate referring expressions, such as pronouns, and follow grammatical constraints of the chosen language. All this is achieved using knowledge about the world and the domain of dicsourse, about communication and about languages. NLG components are used for e.g. automatic report generation, document authoring, dialogue, concept-to-speech, multi-modal and machine translation systems. Evaluating the correctness and the appropriateness of generated text is a research theme on its own since there is usually no single correct solution. One important way to tackle the problem consists in creating reference corpora and performing shared evaluation tasks, e.g. on generating referring expressions. However, this is not intended to replace less formal evaluation strategies such as human assessments."@en,
    "The task/process of generating natural language text from some non-linguistic representation of information."@en;
  skos:inScheme :OperationScheme;
  skos:narrower :AutomaticSubtitling, :Conjugation, :LexicalSimplification, :LexicalSubstitution,
    :MultilingualGeneration, :NewsGeneration, :Paraphrasing, :SignLanguageGeneration,
    :SpeechSynthesis, :SpokenLanguageGeneration, :Summarization, :SyntacticStructureGeneration,
    :TextGeneration, :TextSimplification, :TextToSpeechSynthesis;
  skos:prefLabel "Natural Language Generation"@en .

:BiomedicalConceptNormalization a skos:Concept;
  rdfs:label "Biomedical concept normalization"@en;
  skos:altLabel "Biomedical concept normalisation"@en-uk;
  skos:broader :ConceptNormalization;
  skos:definition "The task of mapping free-form expressions to medical terms [source: Medical concept normalization in social media posts with recurrent neural networks]"@en;
  skos:inScheme :OperationScheme;
  skos:prefLabel "Biomedical concept normalization"@en .

:Transcription a skos:Concept;
  rdfs:label "Transcription"@en;
  skos:altLabel "Speech transcription"@en, "Speech-to-Text conversion"@en;
  skos:broader :SpeechRecognition;
  skos:inScheme :OperationScheme;
  skos:narrower :OrthographicTranscription, :PhoneticTranscription;
  skos:prefLabel "Transcription"@en .

:FrameSemanticParsing a skos:Concept;
  rdfs:label "Frame-semantic parsing"@en;
  skos:broader :Parsing, :SemanticAnnotation;
  skos:definition "The task/process of recognising and labelling in a text predicate argument structures and the semantic roles of the constituents, in accordance to the frame semantics theory."@en;
  skos:inScheme :OperationScheme;
  skos:prefLabel "Frame-semantic parsing"@en .

:AudioProcessing a skos:Concept;
  rdfs:label "Audio processing"@en;
  skos:broader :ModelFunction, :OperationWithMultimediaInputOrOutput;
  skos:inScheme :OperationScheme;
  skos:prefLabel "Audio processing"@en .

:text_x_org_dkpro_conll2012 skos:broader :Mimetype;
  skos:inScheme :MimeTypeScheme .

:text_x_org_dkpro_conll2008 a skos:Concept;
  rdfs:label "text/x.org.dkpro.conll-2008";
  skos:broader :Mimetype;
  skos:inScheme :MimeTypeScheme .

:SentenceSplitting a skos:Concept;
  rdfs:label "Sentence splitting"@en;
  skos:altLabel "Segmentation into sentences"@en, "Sentence segmentation"@en;
  skos:broader :StructuralAnnotation;
  skos:definition "The task/process of recognizing and tagging sentence boundaries in a text"@en;
  skos:inScheme :OperationScheme;
  skos:prefLabel "Sentence splitting"@en .

:RdfFormats a skos:Concept;
  rdfs:label "RDF formats"@en;
  owl:deprecated true;
  skos:broader :DataFormat;
  skos:definition "Formats for RDF (Resource Description Framework) resources"@en;
  skos:inScheme :DataFormatScheme;
  skos:narrower :Nif, :Obo, :Owl, :Rdf_xml, :Turtle;
  skos:prefLabel "RDF formats"@en .

:Crawler a skos:Concept;
  :performsOperation :Crawling;
  rdfs:label "Crawler"@en;
  skos:altLabel "web crawler"@en;
  skos:broader :DataCollector;
  skos:definition "A component that crawls the web and collects data from various web sites"@en;
  skos:inScheme :ComponentTypeScheme;
  skos:prefLabel "Crawler"@en .

:ArgumentMining rdfs:label "Argument mining"@en;
  skos:altLabel "Argumentation mining"@en;
  skos:broader :ComputationalArgumentation;
  skos:definition "The automatic extraction and identification of argumentative structures from natural language text"@en;
  skos:inScheme :OperationScheme;
  skos:prefLabel "Argument mining"@en .

:InformationExtractionAndInformationRetrievalCollection skos:member :ArgumentMining .

:ProsodicInformationProcessing skos:broader :OperationWithMultimediaInputOrOutput .

:TermExtractor a skos:Concept;
  :performsOperation :TermExtraction;
  rdfs:label "Term extractor"@en;
  skos:altLabel "Terminology extractor"@en;
  skos:broader :Analyzer;
  skos:definition "A component that tries to extract terms from a corpus"@en;
  skos:inScheme :ComponentTypeScheme;
  skos:prefLabel "Term extractor"@en .

:application_postscript a skos:Concept;
  rdfs:label "application/postscript";
  skos:broader :Mimetype;
  skos:inScheme :MimeTypeScheme .

:text_x_org_dkpro_conll2009 a skos:Concept;
  rdfs:label "text/x.org.dkpro.conll-2009";
  skos:broader :Mimetype;
  skos:inScheme :MimeTypeScheme .

:SpeechSynthesis a skos:Concept;
  rdfs:label "Speech Synthesis"@en;
  skos:altLabel "Synthetic Speech Generation"@en;
  skos:broader :NaturalLanguageGeneration;
  skos:inScheme :OperationScheme;
  skos:prefLabel "Speech Synthesis"@en .

:Conll2008 a skos:Concept;
  :documentationUrl "https://zoidberg.ukp.informatik.tu-darmstadt.de/jenkins/job/DKPro%20Core%20Documentation%20(GitHub)/de.tudarmstadt.ukp.dkpro.core$de.tudarmstadt.ukp.dkpro.core.doc-asl/doclinks/5/format-reference.html#format-Conll2008";
  :hasMimetype :text_x_org_dkpro_conll2008;
  rdfs:label "CoNLL-2008"@en;
  skos:broader :ConllFormat;
  skos:definition "The CoNLL 2008 format targets syntactic and semantic dependencies. Columns are tab-separated. Sentences are separated by a blank new line."@en;
  skos:inScheme :DataFormatScheme;
  skos:prefLabel "CoNLL-2008"@en .

:WebAnnotationFormat a skos:Concept;
  :documentationUrl "https://www.w3.org/TR/annotation-model/";
  :hasMimetype :application_anno_json, :application_ld_json_profile_http_www_w3_org_ns_anno_jsonld;
  rdfs:label "Web annotation format"@en;
  skos:broader :AnnotationFormat, :Json;
  skos:definition "A structured model and format to enable annotations to be shared and reused across different hardware and software platforms."@en;
  skos:inScheme :DataFormatScheme;
  skos:prefLabel "Web annotation format"@en .

:Emotion a skos:Concept;
  rdfs:label "Emotion"@en;
  skos:broader :SemanticAnnotationType;
  skos:definition "An affective state of consciousness in which joy, sorrow, fear, hate, or the like, is experienced, as distinguished from cognitive and volitional states of consciousness [http://www.dictionary.com/browse/emotion]"@en;
  skos:inScheme :AnnotationTypeScheme;
  skos:prefLabel "Emotion"@en .

:GrapeVariety a skos:Concept;
  rdfs:label "Grape variety"@en;
  skos:broader :AgriculturalEntity;
  skos:definition "A type of grape"@en;
  skos:inScheme :AnnotationTypeScheme;
  skos:prefLabel "Grape variety"@en .

:VariablesDectector a skos:Concept;
  rdfs:label "Variables dectector"@en;
  skos:altLabel "Variables detection component"@en;
  skos:broader :Analyzer;
  skos:definition "A component that tries to identify variables (in social sciences) in a text"@en;
  skos:inScheme :ComponentTypeScheme;
  skos:prefLabel "Variables dectector"@en .

:ScholarlyCommunicationAnnotation a skos:Concept;
  rdfs:label "Scholarly analytics entity"@en;
  owl:deprecated true;
  skos:broader :DomainSpecificAnnotationType;
  skos:definition "Any type of annotation that is relevant to scholarly analtyics (e.g. citations, funding information etc.)"@en;
  skos:inScheme :AnnotationTypeScheme;
  skos:narrower :Citation, :DocumentSection, :Funding, :Keyword, :Topic;
  skos:prefLabel "Scholarly analytics entity"@en .

:ScientificUnit skos:broader :DomainSpecificAnnotationType .

:LipMovement a skos:Concept;
  rdfs:label "Lip movement"@en;
  skos:broader :ModalityAnnotationType;
  skos:inScheme :AnnotationTypeScheme;
  skos:prefLabel "Lip movement"@en .

:BrainRegion a skos:Concept;
  rdfs:label "Brain region"@en;
  skos:broader :BiologicalEnity, :NamedEntity;
  skos:inScheme :AnnotationTypeScheme;
  skos:prefLabel "Brain region"@en .

:RegressionAnalysis a skos:Concept;
  dc:source "Wikipedia (https://en.wikipedia.org/wiki/Regression_analysis)"@en;
  rdfs:label "Regression Analysis"@en;
  skos:broader :MachineAndStatisticalLearningMethod;
  skos:definition "A statistical process for estimating the relationships among variables. It includes many techniques for modeling and analyzing several variables, when the focus is on the relationship between a dependent variable and one or more independent variables (or 'predictors')."@en;
  skos:inScheme :TdmMethodScheme;
  skos:prefLabel "Regression Analysis"@en .

:Owl_xml a skos:Concept;
  :hasMimetype :application_xml;
  rdfs:label "OWL/XML"@en;
  skos:broader :Owl, :Xml;
  skos:definition "XML format for OWL ontologies"@en;
  skos:inScheme :DataFormatScheme;
  skos:prefLabel "OWL/XML"@en .

:EntityMentionLabelling a skos:Concept;
  rdfs:label "Entity mention labelling"@en;
  skos:altLabel "Entity mention labeling [en-US]"@en-us;
  skos:broader :InformationExtraction;
  skos:inScheme :OperationScheme;
  skos:prefLabel "Entity mention labelling"@en .

:application_tei_xml a skos:Concept;
  rdfs:label "application/tei+xml";
  skos:broader :Mimetype;
  skos:inScheme :MimeTypeScheme .

:Debugger a skos:Concept;
  :performsOperation :Debugging;
  rdfs:label "Debugger"@en;
  skos:broader :SupportComponent;
  skos:definition "A component that is used in the debugging process"@en;
  skos:inScheme :ComponentTypeScheme;
  skos:prefLabel "Debugger"@en .

:WikipediaFormat a skos:Concept;
  rdfs:label "Wikipedia format"@en;
  skos:broader :DataFormat;
  skos:definition "Formats used for wikipedia"@en;
  skos:inScheme :DataFormatScheme;
  skos:narrower :Blikiwikipedia, :WikipediaArticle, :WikipediaArticleInfo, :WikipediaDiscussion,
    :WikipediaLink, :WikipediaPage, :WikipediaQuery, :WikipediaRevision, :WikipediaRevisionPair,
    :WikipediaTemplateFilteredArticle;
  skos:prefLabel "Wikipedia format"@en .

:DatabaseFormat a skos:Concept;
  rdfs:label "Database format"@en;
  skos:broader :DataFormat;
  skos:definition "Formats used for databases"@en;
  skos:inScheme :DataFormatScheme;
  skos:narrower :ANNIS, :Jdbc, :MsAccessDatabase;
  skos:prefLabel "Database format"@en .

:KeywordExtraction a skos:Concept;
  rdfs:label "Keyword extraction"@en;
  skos:altLabel "KWS"@en, "Key phrase Extraction"@en, "Keyword search"@en, "Keyword spotting"@en;
  skos:broader :InformationExtraction;
  skos:definition "The task/process of identifying keywords (words deemed indicative of the topic/subject) in a text/corpus"@en;
  skos:inScheme :OperationScheme;
  skos:prefLabel "Keyword extraction"@en .

:Translation a skos:Concept;
  rdfs:label "Translation"@en;
  skos:broader :Operation;
  skos:definition "", "The task/process of expressing the sense of a sequence of words in one language into another language"@en;
  skos:inScheme :OperationScheme;
  skos:narrower :ImageTranslation, :Localization, :SpeechToSpeechTranslation;
  skos:prefLabel "Translation"@en .

:SentenceAlignment skos:definition "Alignment at sentence level"@en .

:UnicodeConformTokenizing a skos:Concept;
  rdfs:label "Unicode-conform tokenizing"@en;
  skos:broader :SupportOperation;
  skos:definition "";
  skos:inScheme :OperationScheme;
  skos:prefLabel "Unicode-conform tokenizing"@en .

:TopicDetection skos:broader :KnowledgeDiscovery .

:Graf a skos:Concept;
  :documentationUrl "http://dl.acm.org/citation.cfm?id=1642060", "https://zoidberg.ukp.informatik.tu-darmstadt.de/jenkins/job/DKPro%20Core%20Documentation%20(GitHub)/de.tudarmstadt.ukp.dkpro.core$de.tudarmstadt.ukp.dkpro.core.doc-asl/doclinks/5/format-reference.html#format-Graf";
  :hasMimetype :application_x_org_dkpro_graf_xml;
  rdfs:label "GrAF"@en;
  skos:altLabel "Graph Annotation Format"@en;
  skos:broader :AnnotationFormat;
  skos:definition "GrAF (Graph Annotation Format) is an extension of the Linguistic Annotation Framework (LAF)"@en;
  skos:inScheme :DataFormatScheme;
  skos:prefLabel "GrAF"@en .

:ConversationalSystemsBuilding a skos:Concept;
  rdfs:label "Conversational systems building"@en;
  skos:altLabel "Chatbots building"@en, "Conversational agents building"@en, "Dialogue systems building"@en,
    "Embodied agents building"@en, "Virtual agents building"@en;
  skos:broader :HumanComputerInteraction;
  skos:definition "All activities related to the creation of conversational/dialogue systems (i.e. computer systems intended to converse with humans, through one or more communication modalities, such as text, speech, graphics, haptics, gestures)"@en;
  skos:editorialNote "I have put all terms together as alternative labels, but maybe they should be distinguished at a later stage"@en;
  skos:inScheme :OperationScheme;
  skos:prefLabel "Conversational systems building"@en .

:PersuasiveExpression a skos:Concept;
  rdfs:label "Persuasive expression"@en;
  skos:broader :SemanticAnnotationType;
  skos:definition "A word or phrase used for persuasion purposes"@en;
  skos:inScheme :AnnotationTypeScheme;
  skos:prefLabel "Persuasive expression"@en .

:RawAudioFormat a skos:Concept;
  :documentationUrl "https://en.wikipedia.org/wiki/Raw_audio_format#:~:text=RAW%20Audio%20format%20or%20just,%2C%20or%20number%20of%20channels";
  rdfs:label "Raw audio format"@en;
  skos:broader :AudioFormat;
  skos:inScheme :DataFormatScheme;
  skos:prefLabel "Raw audio format"@en .

:InformationExtraction a skos:Concept;
  rdfs:label "Information Extraction"@en;
  skos:altLabel "IE & Text Analysis"@en, "Information Discovery"@en, "Information Retrieval"@en;
  skos:broader :TextAndDataMining;
  skos:definition "The goal of information extraction (IE) is to build systems that find and link relevant information from natural language text ignoring irrelevant information. The information of interest is typically pre-specified in form of uninstantiated frame-like structures also called templates. The templates are domain and task specific. The major task of an IE-system is then the identification of the relevant parts of the text which are used to fill a template's slots."@en,
    "The process/task of automatically extracting structured information from unstructured and/or semi-structured data"@en;
  skos:inScheme :OperationScheme;
  skos:narrower :AgeBracketDetection, :AuthorClassification, :AutomaticHyperlinking,
    :BotDetection, :ComputationalArgumentation, :ContradictionDetection, :EmotionDetection,
    :EmotionLabelling, :EntityMentionLabelling, :EntityMentionRecognition, :EventDetection,
    :ExtractionOfDomainSpecificInformation, :ExtractionOfQuantitativeInformation, :FactChecking,
    :FakeNewsDetection, :FrameExtraction, :GenderDetection, :HateSpeechRecognition, :HumourDetection,
    :IronyDetection, :KeywordExtraction, :LanguageDetection, :MultimediaInformationExtraction,
    :NegationDetection, :PersuasiveExpressionMining, :PolarityDetection, :QuestionAnswering,
    :RecognizingTextualEntailment, :RelationExtraction, :RepresentationOfSpaceAndTime,
    :RumoursStanceClassification, :SemanticReasoning, :SpeechRetrieval, :StanceDetection,
    :TableQuestionAnswering, :TemporalExpressionRecognition, :TermExtraction, :TextAnalysis,
    :TruthLabelling, :VerbalAggressionAnalysis;
  skos:prefLabel "Information Extraction"@en .

:Blikiwikipedia skos:definition "The Java Wikipedia API (Bliki engine) is a parser library for converting Wikipedia wikitext notation to HTML."@en .

:EAF a skos:Concept;
  :documentationUrl "https://www.mpi.nl/corpus/html/elan_ug/ch01.html";
  :hasMimetype :text_x_eaf_xml;
  rdfs:label "EUDICO annotation format"@en;
  skos:altLabel "eaf"@en;
  skos:broader :AnnotationFormat, :Xml;
  skos:definition "Format for annotations of video files with the ELAN annotator"@en;
  skos:inScheme :DataFormatScheme;
  skos:prefLabel "EUDICO annotation format"@en .

:LexiconMerging a skos:Concept;
  rdfs:label "Lexicon merging"@en;
  skos:broader :SupportOperationForKnowledgeResources;
  skos:definition "The task/process of merging (combining together) information coming from various lexical/conceptual resources"@en;
  skos:inScheme :OperationScheme;
  skos:prefLabel "Lexicon merging"@en .

:Xmi a skos:Concept;
  :documentationUrl "https://www.iana.org/assignments/media-types/application/vnd.xmi+xml";
  :hasFileExtension "xmi";
  :hasMimetype :application_vnd_xmi_xml;
  rdfs:label "XMI"@en;
  skos:broader :DocumentFormat, :Xml;
  skos:definition "Data format for the XML Metadata Interchange (XMI), which is an Object Management Group (OMG) standard for exchanging metadata information via Extensible Markup Language (XML)"@en;
  skos:inScheme :DataFormatScheme;
  skos:prefLabel "XMI"@en .

:Anonymization a skos:Concept;
  rdfs:label "Anonymization"@en;
  skos:altLabel "Anonymisation [en-UK]"@en-uk;
  skos:broader :Annotation;
  skos:definition "The task/process through which particular text segments or data units that allow the identification of a person are removed or replaced"@en;
  skos:inScheme :OperationScheme;
  skos:narrower :DataMasking, :TextEncryption;
  skos:prefLabel "Anonymization"@en .

:BelowPosTagging a skos:Concept;
  rdfs:label "Below Part-of-Speech Tagging"@en;
  skos:altLabel "Annotation of morphological features"@en, "B-PoS Tagging"@en, "Below PoS Tagging"@en;
  skos:broader :MorphologicalAnnotation, :MorphosyntacticTagging;
  skos:definition "The annotation of words with morphological information besides the part of speech and dependent upon it (e.g. for nouns: gender, number and case; for verbs: tense, number, person etc.)"@en;
  skos:inScheme :OperationScheme;
  skos:prefLabel "Below Part-of-Speech Tagging"@en .

:application_x_org_dkpro_graf_xml skos:inScheme :MimeTypeScheme .

:AnnotationOfMultiWordUnits a skos:Concept;
  rdfs:label "Annotation of multi-word units"@en;
  skos:broader :MorphologicalAnnotation;
  skos:definition "The task/process of annotating multi-word units, i.e. combinations of words that are considered as one"@en;
  skos:inScheme :OperationScheme;
  skos:prefLabel "Annotation of multi-word units"@en .

:application_xml a skos:Concept;
  rdfs:label "application/xml";
  skos:broader :Mimetype;
  skos:inScheme :MimeTypeScheme .

:ImageUnderstanding a skos:Concept;
  rdfs:label "Image Understanding"@en;
  skos:broader :TextAndDataMining;
  skos:definition "", "Advanced image processing in which artificial-intelligence techniques are used to interpret images by locating, characterizing, and recognizing objects and other features in the scene. [from https://www.encyclopedia.com/computing/dictionaries-thesauruses-pictures-and-press-releases/image-understanding]"@en;
  skos:inScheme :OperationScheme;
  skos:prefLabel "Image Understanding"@en .

:MachineLearningPredictor a skos:Concept;
  :performsOperation :Prediction;
  rdfs:label "Machine Learning predictor"@en;
  skos:broader :SupportComponent;
  skos:definition "A component that is used in predicting based on machine learning models"@en;
  skos:editorialNote "maybe create another class for predictors, analytics"@en;
  skos:inScheme :ComponentTypeScheme;
  skos:prefLabel "Machine Learning predictor"@en .

:QuestionTopicalTarget a skos:Concept;
  rdfs:label "Question Topical Target"@en;
  skos:altLabel "QTT"@en, "Question topic"@en;
  skos:broader :SemanticAnnotationType;
  skos:definition "The segment of a question that describes the entity about which the question is made"@en;
  skos:inScheme :AnnotationTypeScheme;
  skos:prefLabel "Question Topical Target"@en .

:IonicCurrent a skos:Concept;
  rdfs:label "Ionic current"@en;
  skos:altLabel "Ion current"@en;
  skos:broader :BiologicalEnity, :NamedEntity;
  skos:definition "The influx and/or efflux of ions through an ion channel"@en;
  skos:inScheme :AnnotationTypeScheme;
  skos:prefLabel "Ionic current"@en .

:Ptb a skos:Concept;
  rdfs:label "PTB"@en;
  skos:broader :AnnotationFormat;
  skos:definition "Penn Tree Bank formats"@en;
  skos:inScheme :DataFormatScheme;
  skos:narrower :PtbChunked, :PtbCombined;
  skos:prefLabel "PTB"@en .

:text_xCochrane a skos:Concept;
  rdfs:label "text/x-cochrane";
  skos:broader :Mimetype;
  skos:inScheme :MimeTypeScheme .

:TalkingHeadSynthesis a skos:Concept;
  rdfs:label "Talking head synthesis"@en;
  skos:broader :OperationWithMultimediaInputOrOutput;
  skos:inScheme :OperationScheme;
  skos:prefLabel "Talking head synthesis"@en .

:EntityLinking a skos:Concept;
  rdfs:label "Entity linking"@en;
  skos:broader :SemanticAnnotation;
  skos:definition "The task/process of attaching tags to all the mentions of an entity in a text linking them together with the entity."@en;
  skos:inScheme :OperationScheme;
  skos:prefLabel "Entity linking"@en .

:MalletLdaTopicProportions a skos:Concept;
  :documentationUrl "http://dkpro.github.io/dkpro-core/releases/1.8.0/docs/format-reference.html#format-MalletTopicProportions",
    "https://dkpro.github.io/dkpro-core/releases/1.8.0/docs/format-reference.html#format-de.tudarmstadt.ukp.dkpro.core.mallet-asl";
  rdfs:label "Mallet LDA Topic Proportions"@en;
  skos:broader :AnnotationFormat;
  skos:definition "Topic proportions in the shape [\\t]\\t\\t..."@en;
  skos:inScheme :DataFormatScheme;
  skos:prefLabel "Mallet LDA Topic Proportions"@en .

:EvaluationOfMachineTranslationAndTranslationTools a skos:Concept;
  rdfs:label "Evaluation of Machine Translation and translation tools"@en;
  skos:altLabel "Evaluation of MT"@en, "Evaluation of MT Systems"@en, "MT Evaluation"@en;
  skos:broader :Evaluation;
  skos:definition "The growing number of MT systems on the market that span a wide range of quality levels has motivated activities towards evaluation standards from national and international organizations. Evaluation of MT systems depends strongly on whether such a system is used for information dissemination, assimilation, or in a conversational context, the types of texts to be translated, whether there is a well-defined and limited application domain and many more factors."@en,
    "The task/process of assessing the quality performance of machine translation tools"@en;
  skos:inScheme :OperationScheme;
  skos:prefLabel "Evaluation of Machine Translation and translation tools"@en .

:hasFileExtension a owl:DatatypeProperty .

:application_anno_json a skos:Concept;
  rdfs:label "application/anno+json";
  skos:broader :Mimetype;
  skos:inScheme :MimeTypeScheme .

:text_x_org_dkpro_imscwb a skos:Concept;
  rdfs:label "text/x.org.dkpro.imscwb";
  skos:broader :Mimetype;
  skos:inScheme :MimeTypeScheme .

:I2b2 a skos:Concept;
  :documentationUrl "https://builds.openminted.eu/job/WP%205.2%20-%20Typesystem%20alignment/eu.openminted.interop$mapping-conversion/doclinks/1/components.html#I2B2Reader",
    "https://www.i2b2.org/NLP/RDoCforPsychiatry/PreviousChallenges.php";
  rdfs:label "I2B2"@en;
  skos:broader :AnnotationFormat;
  skos:definition "Format of the I2B2 challenge"@en;
  skos:inScheme :DataFormatScheme;
  skos:prefLabel "I2B2"@en .

:application_xXml_alvis a skos:Concept;
  rdfs:label "application/x-xml+alvis";
  skos:broader :Mimetype;
  skos:inScheme :MimeTypeScheme .

:MachineAndStatisticalLearningMethod a skos:Concept;
  rdfs:label "Machine and Statistical Learning Method"@en;
  skos:broader :TdmMethod;
  skos:definition "Methods and techniques used either in machine learning or statistical learning"@en;
  skos:inScheme :TdmMethodScheme;
  skos:narrower :ArtificialNeuralNetwork, :AssociationRuleLearning, :Bayesian, :ClusteringMethod,
    :DecisionTrees, :DeepLearning, :DimensionalityReduction, :EnsembleMethod, :InstanceBasedLearning,
    :KernelMethod, :RegressionAnalysis, :Regularisation;
  skos:prefLabel "Machine and Statistical Learning Method"@en .

:DialogueModelling a skos:Concept;
  rdfs:label "Dialogue modelling"@en;
  skos:altLabel "Dialog modeling [en-US]"@en-us;
  skos:broader :LanguageModelling, :ModelFunction;
  skos:definition "A Dialogue model is a system that simulates the behavior of dialogue participants. This includes formal models that instantiate linguistic theories of dialogue interaction and statistical models of dialogue behaviors."@en,
    "The task/process of building models of dialogues to be used in dialogue systems"@en;
  skos:inScheme :OperationScheme;
  skos:prefLabel "Dialogue modelling"@en .

:Sgml a skos:Concept;
  :hasMimetype :text_sgml;
  rdfs:label "SGML"@en;
  skos:broader :DocumentFormat;
  skos:definition "SGML format"@en;
  skos:inScheme :DataFormatScheme;
  skos:prefLabel "SGML"@en .

:ConstituencyTree a skos:Concept;
  rdfs:label "Constituency tree"@en;
  skos:broader :SyntacticAnnotationType;
  skos:definition "An ordered, rooted tree that represents the syntactic structure of a string according to a constituency grammar (= phrase structure grammars). It distinguishes between terminal and non-terminal nodes. The interior nodes are labeled by non-terminal categories of the grammar (phrases), while the leaf nodes are labeled by terminal categories (parts of speech). [adapted from https://en.wikipedia.org/wiki/Parse_tree]"@en;
  skos:inScheme :AnnotationTypeScheme;
  skos:prefLabel "Constituency tree"@en .

:BinaryFormat a skos:Concept;
  rdfs:label "Binary format"@en;
  skos:broader :DataFormat;
  skos:definition "Any format of a computer file in which information is stored in the form of ones and zeros, or in some other binary (two-state) sequence; used mainly for executable files or files that need to be interpreted by a computer program"@en;
  skos:inScheme :DataFormatScheme;
  skos:narrower :CBOR, :FastInfoset, :Pdf;
  skos:prefLabel "Binary format"@en .

:SpeechAnnotationType a skos:Concept;
  rdfs:label "Speech annotation type"@en;
  skos:broader :AnnotationType;
  skos:inScheme :AnnotationTypeScheme;
  skos:narrower :ProsodicBoundary, :Transcription1;
  skos:prefLabel "Speech annotation type"@en .

:RecognizingTextualEntailment a skos:Concept;
  rdfs:label "Recognizing Textual Entailment"@en;
  skos:broader :InformationExtraction, :KnowledgeDiscovery;
  skos:definition "A task/process that intends to recognize for two text fragments whether the meaning of one text is entailed in that of the other, i.e. whether the truth of one text fragment follows from that of the other fragment."@en;
  skos:inScheme :OperationScheme;
  skos:prefLabel "Recognizing Textual Entailment"@en .

:Pseudonymization skos:altLabel "pseudonymisation"@en-GB .

:EvaluationOfBroadCoverageNaturalLanguageParsers a skos:Concept;
  rdfs:label "Evaluation of broad-coverage natural language parsers"@en;
  skos:broader :Evaluation;
  skos:definition "The taks of parser evaluation is the measure the speed and accuracy of (symbolic or stochastic) parsers with respect to a manually parsed test corpus. Test data can either be a treebank constructed naturally occurring data, such as the \"\"Wall Street Corpus\"\", or a \"\"test suite\"\" containing constructed examples which cover all interesting linguistic phenomena. An important issue in parser evaluation is the comparison of parsers and grammars based on different linguistic theories. Evaluations have focussed on phrase structure or dependency structures."@en,
    "The task/process of assessing the quality performance of parsers"@en;
  skos:inScheme :OperationScheme;
  skos:prefLabel "Evaluation of broad-coverage natural language parsers"@en .

:audio_basic rdfs:label "audio/basic" .

:LinguisticEntity a skos:Concept;
  rdfs:label "Linguistic entity"@en;
  skos:broader :DomainSpecificAnnotationType;
  skos:definition "Any kind of annotation pertaining to entities of linguistics; the use of OLIA is recommended"@en;
  skos:inScheme :AnnotationTypeScheme;
  skos:prefLabel "Linguistic entity"@en .

:ScientificUnit skos:broader :NamedEntity .

:FrameExtraction a skos:Concept;
  rdfs:label "Frame extraction"@en;
  skos:broader :InformationExtraction;
  skos:definition "The task of recognizing words and phrases that evoke semantic frames as defined in the FrameNet project, and their semantic dependents."@en;
  skos:inScheme :OperationScheme;
  skos:prefLabel "Frame extraction"@en .

:NormalizationOfNumbers a skos:Concept;
  rdfs:label "Normalization of numbers"@en;
  skos:broader :Normalization;
  skos:definition "The task/process of substituting numbers with normalized values"@en;
  skos:inScheme :OperationScheme;
  skos:prefLabel "Normalization of numbers"@en .

:LD_json a skos:Concept;
  :hasMimetype :application_ld_json;
  rdfs:label "JSON/LD"@en;
  skos:altLabel "JSON linked data"@en, "LD-Json"@en;
  skos:broader :DocumentFormat, :Json, :LinkedDataFormat;
  skos:definition "Data format encoding Linked Data using JSON"@en;
  skos:inScheme :DataFormatScheme;
  skos:prefLabel "JSON/LD"@en .

:AssociationRuleLearning a skos:Concept;
  rdfs:label "Association Rule Learning"@en;
  skos:altLabel "ANN"@en;
  skos:broader :MachineAndStatisticalLearningMethod;
  skos:definition "A machine learning method used in recognising relationships among variables in databases and extracted in the form of rules."@en;
  skos:inScheme :TdmMethodScheme;
  skos:prefLabel "Association Rule Learning"@en .

:Uima_json a skos:Concept;
  :documentationUrl "https://dkpro.github.io/dkpro-core/releases/1.8.0/docs/format-reference.html#format-de.tudarmstadt.ukp.dkpro.core.io.json-asl";
  :hasMimetype :application_x_org_dkpro_uima_json;
  rdfs:label "UIMA/JSON"@en;
  skos:broader :Json, :UimaCasFormat;
  skos:definition "UIMA serialisation in JSON"@en;
  skos:inScheme :DataFormatScheme;
  skos:prefLabel "UIMA/JSON"@en .

:audio_aiff a skos:Concept;
  rdfs:label "audio/aiff";
  skos:broader :Mimetype;
  skos:inScheme :MimeTypeScheme .

:TemporalExpressionsLabelling a skos:Concept;
  rdfs:label "Temporal expressions labelling"@en;
  skos:altLabel "Annotation of time"@en;
  skos:broader :SemanticAnnotation;
  skos:definition "The task/process of determining the boundaries of units of text that denote time-related concepts and attaching to them tags that name these concepts (e.g. date, time, duration etc.)"@en;
  skos:inScheme :OperationScheme;
  skos:narrower :AnnotationOfDates;
  skos:prefLabel "Temporal expressions labelling"@en .

:DependencyParser a skos:Concept;
  :performsOperation :DependencyParsing;
  rdfs:label "Dependency parser"@en;
  skos:broader :Parser;
  skos:definition "A component that generates a dependency tree from typically token and part-of-speech annotations"@en;
  skos:inScheme :ComponentTypeScheme;
  skos:prefLabel "Dependency parser"@en .

:SpokenLanguageGeneration a skos:Concept;
  rdfs:label "Spoken Language Generation"@en;
  skos:altLabel "CTS"@en, "Concept-to-Speech generation"@en, "SLG"@en;
  skos:broader :NaturalLanguageGeneration;
  skos:definition "Whereas the generation of spoken language from semantic representations can be sequentialized into generation of text followed by text-to-speech, using text as an intermediate representation may lose information that was available in the original input, in particular related to information structure relevant for speech output. An integrated solution can avoid this problem and thereby lead to improved quality and/or simpler system architecture."@en;
  skos:inScheme :OperationScheme;
  skos:prefLabel "Spoken Language Generation"@en .

:text_x_org_dkpro_conll2012 a skos:Concept .

:TheoreticalFrame a skos:Concept;
  rdfs:label "Theoretical frame"@en;
  skos:broader :NamedEntity, :SocialSciencesEntity;
  skos:inScheme :AnnotationTypeScheme;
  skos:prefLabel "Theoretical frame"@en .

:documentationUrl a owl:DatatypeProperty;
  rdfs:comment "The URL link in which a concept is documented"@en;
  rdfs:domain owl:Thing;
  rdfs:label "documentation URL"@en;
  rdfs:range xsd:anyURI;
  rdfs:subPropertyOf owl:topDataProperty .

:AvatarSynthesis a skos:Concept;
  rdfs:label "Avatar synthesis"@en;
  skos:broader :HumanComputerInteraction;
  skos:inScheme :OperationScheme;
  skos:prefLabel "Avatar synthesis"@en .

:MachineTranslationSupport skos:inScheme :OperationScheme .

:SpokenLanguageUnderstanding skos:broader :NaturalLanguageUnderstanding .

:SentenceSplitter a skos:Concept;
  rdfs:label "Sentence splitter"@en;
  skos:broader :Segmenter;
  skos:definition "A component that splits a text into sentences"@en;
  skos:inScheme :ComponentTypeScheme;
  skos:prefLabel "Sentence splitter"@en .

:Simplifier a skos:Concept;
  rdfs:label "Simplifier"@en;
  skos:broader :Generator;
  skos:definition "A component that outputs a simpler rendition of a given item (sentence, text etc.)"@en;
  skos:inScheme :ComponentTypeScheme;
  skos:prefLabel "Simplifier"@en .

:IronyDetection a skos:Concept;
  rdfs:label "Irony detection"@en;
  skos:broader :InformationExtraction;
  skos:definition "The task of identifying in a text segments expressing irony and classifying  them into types"@en;
  skos:inScheme :OperationScheme;
  skos:prefLabel "Irony detection"@en .

:Alignment a skos:Concept;
  rdfs:label "Alignment"@en;
  skos:definition "Establishment of translational equivalences between structural units (words, sentences etc.) of a text in a given language and a text with similar meaning in other language(s)"@en;
  skos:inScheme :OperationScheme;
  skos:narrower :PhraseAlignment, :SentenceAlignment, :WordAlignment;
  skos:prefLabel "Alignment"@en .

:FillMask skos:definition "Masked Language Modeling is a fill-in-the-blank task, where a model uses the context words surrounding a mask token to try to predict what the masked word should be. [Source: https://keras.io/examples/nlp/masked_language_modeling/]";
  skos:inScheme :OperationScheme .

:Word a skos:Concept;
  rdfs:label "Word"@en;
  owl:equivalentClass <http://purl.org/olia/olia-top.owl#Word>;
  skos:broader :MorphologicalAnnotationType, :StructuralAnnotationType;
  skos:definition """A word is a unit which is a constituent at the phrase level and above. It is sometimes identifiable according to such criteria as (a) being the minimal possible unit in a reply, (b) having features such as a regular stress pattern, and phonological changes conditioned by or blocked at word boundaries, (c) being the largest unit resistant to insertion of new constituents within its boundaries, or (d) being the smallest constituent that can be moved within a sentence without making the sentence ungrammatical. A word is sometimes placed, in a hierarchy of grammatical constituents, above the morpheme level and below the phrase level. [http://www.glossary.sil.org/term/word]
In annotation, words are often used as equivalent to tokens; thus, for instance, punctuation marks (traditionally not considered as words) will also be annotated as \"word\"."""@en;
  skos:inScheme :AnnotationTypeScheme;
  skos:prefLabel "Word"@en .

:Chunk a skos:Concept;
  :documentationUrl "http://dkpro.github.io/dkpro-core/releases/1.8.0/docs/typesystem-reference.html#de.tudarmstadt.ukp.dkpro.core.api.syntax.type.chunk.Chunk";
  rdfs:label "Chunk"@en;
  skos:broader :SyntacticAnnotationType;
  skos:definition "Group of words that function together; a chunk normally includes a head and some consecutive (i.e. without gaps) preceding words"@en;
  skos:inScheme :AnnotationTypeScheme;
  skos:prefLabel "Chunk"@en .

:TermExtraction a skos:Concept;
  rdfs:label "Term extraction"@en;
  skos:altLabel "Corpus based term recognition"@en, "Term recognition"@en, "Terminology extraction"@en,
    "Terminology recognition"@en;
  skos:broader :InformationExtraction;
  skos:definition "The act/process of identifying and extracting candidate terms from a domain-specific corpus"@en;
  skos:inScheme :OperationScheme;
  skos:prefLabel "Term extraction"@en .

:EventLabelling a skos:Concept;
  rdfs:label "Event labelling"@en;
  skos:altLabel "Annotation of events"@en, "Event labeling [en-US]"@en-us;
  skos:broader :SemanticAnnotation;
  skos:definition "The process/act of marking events and classifying them into types of events in a text"@en;
  skos:inScheme :OperationScheme;
  skos:prefLabel "Event labelling"@en .

:Marker a skos:Concept;
  rdfs:label "Marker"@en;
  skos:broader :AgriculturalEntity;
  skos:inScheme :AnnotationTypeScheme;
  skos:prefLabel "Marker"@en .

:InlineXml a skos:Concept;
  :documentationUrl "https://dkpro.github.io/dkpro-core/releases/1.8.0/docs/format-reference.html#format-de.tudarmstadt.ukp.dkpro.core.io.xml-asl";
  :hasMimetype :application_xml;
  rdfs:label "Inline XML"@en;
  skos:broader :AnnotationFormat, :Xml;
  skos:definition "Inline XML file format"@en;
  skos:inScheme :DataFormatScheme;
  skos:prefLabel "Inline XML"@en .

:ManagementOfAnnotations a skos:Concept;
  rdfs:label "Management of annotations"@en;
  skos:altLabel "Management of annotated texts"@en, "Monitoring of annotated texts"@en,
    "Monitoring of annotations"@en;
  skos:broader :CorpusManagement;
  skos:definition "The task/process of managing (manually or (semi-)automatically) annotated texts, distributing them among annotators and monitoring their work"@en;
  skos:inScheme :OperationScheme;
  skos:prefLabel "Management of annotations"@en .

:ContradictionDetector a skos:Concept;
  :performsOperation :ContradictionDetection;
  rdfs:label "Contradiction detector"@en;
  skos:broader :Analyzer;
  skos:definition "A component that tries to automatically recognize elements that reveal contradiction in a text"@en;
  skos:editorialNote "could also be an annotator"@en;
  skos:inScheme :ComponentTypeScheme;
  skos:prefLabel "Contradiction detector"@en .

:WheatRelatedSpecies a skos:Concept;
  rdfs:label "Wheat-related species"@en;
  skos:broader :AgriculturalEntity, :Species;
  skos:inScheme :AnnotationTypeScheme;
  skos:prefLabel "Wheat-related species"@en .

:Phenotype a skos:Concept;
  rdfs:label "Phenotype"@en;
  skos:broader :AgriculturalEntity;
  skos:definition "The physical appearance or biochemical characteristic of an organism as a result of the interaction of its genotype and the environment [http://www.biology-online.org/dictionary/Phenotype]"@en;
  skos:inScheme :AnnotationTypeScheme;
  skos:prefLabel "Phenotype"@en .

:ConllU a skos:Concept;
  :documentationUrl "http://universaldependencies.org/docs/format.html";
  :hasMimetype :text_x_org_dkpro_conllU;
  rdfs:label "CoNLL-U"@en;
  skos:broader :ConllFormat;
  skos:definition "Format used for CoNLL."@en;
  skos:inScheme :DataFormatScheme;
  skos:prefLabel "CoNLL-U"@en .

:ImageProcessing a skos:Concept;
  rdfs:label "Image processing"@en;
  skos:broader :ModelFunction, :OperationWithMultimediaInputOrOutput;
  skos:inScheme :OperationScheme;
  skos:prefLabel "Image processing"@en .

:audio_x_wav skos:broader :Mimetype .

:Filter a skos:Concept;
  rdfs:label "Filter"@en;
  skos:broader :PreOrPostProcessor;
  skos:definition "A component that is used for filtering text input or annotations based on specific criteria"@en;
  skos:inScheme :ComponentTypeScheme;
  skos:prefLabel "Filter"@en .

:Phrase a skos:Concept;
  rdfs:label "Phrase"@en;
  owl:equivalentClass <http://purl.org/olia/olia-top.owl#Phrase>;
  skos:broader :StructuralAnnotationType;
  skos:definition "A phrase is a syntactic structure that consists of more than one word but lacks the subject-predicate organization of a clause. [http://www.glossary.sil.org/term/phrase]"@en;
  skos:inScheme :AnnotationTypeScheme;
  skos:prefLabel "Phrase"@en .

:LexiconAccess a skos:Concept;
  rdfs:label "Lexicon access"@en;
  skos:broader :SupportOperationForKnowledgeResources;
  skos:definition "The task/process of accessing lexical/conceptual resources (either by humans or computer programs)"@en;
  skos:inScheme :OperationScheme;
  skos:prefLabel "Lexicon access"@en .

:text_turtle a skos:Concept;
  rdfs:label "text/turtle";
  skos:broader :Mimetype;
  skos:inScheme :MimeTypeScheme .

:Segmenter a skos:Concept;
  rdfs:label "Segmenter"@en;
  skos:broader :Annotator;
  skos:definition "A component that segments a text into structural untis (chapters, paragraphs, sentences, words, tokens etc.)"@en;
  skos:inScheme :ComponentTypeScheme;
  skos:narrower :SentenceSplitter, :Tokenizer;
  skos:prefLabel "Segmenter"@en .

:ModelFunctionScheme a skos:ConceptScheme;
  rdfs:label "Model function Taxonomy"@en;
  skos:hasTopConcept :ModelFunction;
  skos:prefLabel "Model function Taxonomy"@en .

:MimeTypeScheme a skos:ConceptScheme;
  rdfs:label "Mimetypes Taxonomy"@en;
  skos:prefLabel "Mimetypes Taxonomy"@en .

:Tika a skos:Concept;
  :hasMimetype :application_tika;
  rdfs:label "Tika"@en;
  skos:broader :DocumentFormat;
  skos:inScheme :DataFormatScheme;
  skos:prefLabel "Tika"@en .

:DomainSpecificAnnotationType a skos:Concept;
  rdfs:label "Domain-specific annotation type"@en;
  skos:broader :AnnotationType;
  skos:definition "Any kind of annotation that is used for specific domains (e.g. genes and proteins from the biomedical domain, plants from agriculture etc.)"@en;
  skos:inScheme :AnnotationTypeScheme;
  skos:narrower :AgriculturalEntity, :BiologicalEnity, :ChemicalEntity, :LinguisticEntity,
    :NeuroscienceEntity, :Relation, :ScholarlyAnalyticsEntity, :ScholarlyCommunicationAnnotation,
    :ScientificUnit, :ScientificValue, :SocialSciencesEntity;
  skos:prefLabel "Domain-specific annotation type"@en .

:text_csv skos:broader :Mimetype;
  skos:inScheme :MimeTypeScheme .

:PosTagging a skos:Concept;
  rdfs:label "Part-of-Speech Tagging"@en;
  skos:altLabel "Grammatical annotation"@en, "Grammatical tagging"@en, "PoS Tagging"@en;
  skos:broader :MorphosyntacticTagging;
  skos:definition "The task/process of marking words with the part of speech (word category, e.g. noun, verb etc.) to which they belong"@en,
    "The technologies for or the process of determining the correct part-of-speech tag for a word given its local context. The task comprises disambiguation of multiple part-of-speech tags and guessing of the correct part-of-speech tag for unknown words. Part-of-speech tagging is frequently used as a preprocessing step for shallow and deep parsers."@en;
  skos:inScheme :OperationScheme;
  skos:prefLabel "Part-of-Speech Tagging"@en .

:ParalanguageAnnotation a skos:Concept;
  rdfs:label "Paralanguage annotation"@en;
  skos:broader :SpeechAnnotation;
  skos:definition "The task/process of annotating paralinguistic features, i.e. vocal features that accompany speech and contribute to communication but are not generally considered to be part of the language system (e.g. vocal quality, loudness, and tempo); facial expressions and gestures are also considered as paralinguistic features [adapted from https://www.dictionary.com/browse/paralanguage]"@en;
  skos:inScheme :OperationScheme;
  skos:prefLabel "Paralanguage annotation"@en .

:InformationRetrieval a skos:Concept;
  rdfs:label "Information Retrieval"@en;
  skos:broader :TextAndDataMining;
  skos:definition "Information Retrieval is the process of locating information that fits a user's information need, which is usually expressed as a search query. The fit of the retrieved information with the information need is referred to as \"\"relevance\"\". The information can be retrieved from databases (data retrieval) or from document collections (document retrieval), where documents can either be text documents or other media (audio, video, semi-structured data, multimedia). Success in information retrieval is generally defined by retrieving as much relevant information as possible (measured by \"\"recall\"\") while minimising the irrelevant information retrieved (measured by \"\"precision\"\"). The most widely used information retrieval systems today are Internet search engines."@en,
    "The activity of obtaining information resources relevant to an information need from a collection of information resources; searches can be based on full-text or other content-based indexing"@en;
  skos:inScheme :OperationScheme;
  skos:narrower :CrossLingualSearch, :ExploratorySearch, :InformationFiltering, :MultilingualInformationRetrieval,
    :MultimediaRetrieval, :SemanticSearch, :TerminologySearch;
  skos:prefLabel "Information Retrieval"@en .

:TranslationTechnologiesCollection a skos:Collection;
  rdfs:label "Translation Technologies Collection"@en;
  skos:member :Alignment, :ComputerAidedTranslation, :CrossLingualSearch, :EvaluationOfMachineTranslationAndTranslationTools,
    :HumanAidedMachineTranslation, :ImageTranslation, :Localization, :MachineTranslation,
    :MachineTranslationSupport, :ParallelSentenceExtraction, :PhraseAlignment, :SentenceAlignment,
    :SpeechToSpeechTranslation, :SpeechToTextTranslation, :Translation, :TranslationMemoryManagement,
    :WordAlignment;
  skos:prefLabel "Translation Technologies Collection"@en .

:TranslationTechnologies owl:deprecated true .

:InformationFiltering a skos:Concept;
  rdfs:label "Information filtering"@en;
  skos:broader :InformationRetrieval;
  skos:definition "The process/task of removing (filtering out) redundant or unwanted information from an information stream using (semi)automated or computerized methods prior to presentation to a human user; the selection of the items is based on the correlation between the content of the items and the user's preferences (content-based filtering) or the correlation between people with similar preferences (collaborative filtering)"@en;
  skos:inScheme :OperationScheme;
  skos:narrower :InformationFilteringByRecommenderSystems;
  skos:prefLabel "Information filtering"@en .

:ImageGeneration a skos:Concept;
  rdfs:label "Image generation"@en;
  skos:broader :ModelFunction, :OperationWithMultimediaInputOrOutput;
  skos:inScheme :OperationScheme;
  skos:narrower :TextToImageGeneration;
  skos:prefLabel "Image generation"@en .

:audio_x_wav a skos:Concept .

:AgriculturalEntity a skos:Concept;
  rdfs:label "Agricultural entity"@en;
  skos:broader :DomainSpecificAnnotationType;
  skos:definition "Any kind of annotation pertaining to entities of the agricultural domain; the use of the AGROVOC thesaurus is recommended"@en;
  skos:inScheme :AnnotationTypeScheme;
  skos:narrower :Gene, :GeneFamily, :GrapeVariety, :Habitat, :Marker, :Organism, :Phenotype,
    :PhysicoChemicalProperty, :ProteinFamily, :Rna, :WheatRelatedSpecies;
  skos:prefLabel "Agricultural entity"@en .

:Diaml a skos:Concept;
  :documentationUrl "https://www.iso.org/standard/51967.html";
  rdfs:label "DIAML"@en;
  skos:broader :AnnotationFormat;
  skos:definition "Format following Dialogue Act Markup Language (DiAML) which is defined within the ISO standard 24617-2"@en;
  skos:inScheme :DataFormatScheme;
  skos:prefLabel "DIAML"@en .

:SignLanguageRecognition a skos:Concept;
  rdfs:label "Sign language recognition"@en;
  skos:broader :OperationWithMultimediaInputOrOutput;
  skos:definition "The task/process of recognizing from images and videos hand gestures performed in sign language"@en;
  skos:inScheme :OperationScheme;
  skos:prefLabel "Sign language recognition"@en .

:text_sgml rdfs:label "text/sgml" .

:application_x_org_dkpro_uima_binary a skos:Concept;
  rdfs:label "application/x.org.dkpro.uima+binary";
  skos:broader :Mimetype;
  skos:inScheme :MimeTypeScheme .

:RelationExtraction a skos:Concept;
  rdfs:label "Relation Extraction"@en;
  skos:altLabel "Relationship Extraction"@en;
  skos:broader :InformationExtraction;
  skos:definition "Automated or human-assisted acquisition of relations between concepts from textual or other data, usu. within a selected domain."@en,
    "The process/task of identifying and classifying relation mentions between entities in text and/or data."@en;
  skos:editorialNote "can also be annotation"@en;
  skos:inScheme :OperationScheme;
  skos:prefLabel "Relation Extraction"@en .

:FacialExpressionRecognition skos:altLabel "Face expression detection"@en .

:ComponentTypeScheme a skos:ConceptScheme;
  rdfs:label "Component type Taxonomy"@en;
  skos:hasTopConcept :ComponentType;
  skos:prefLabel "Component type Taxonomy"@en .

:Habitat a skos:Concept;
  rdfs:label "Habitat"@en;
  skos:broader :AgriculturalEntity;
  skos:definition "The place or environment where an organism, plant or animal naturally or normally lives and grows"@en;
  skos:inScheme :AnnotationTypeScheme;
  skos:prefLabel "Habitat"@en .

:PersonIdentification a skos:Concept;
  rdfs:label "Person identification"@en;
  skos:broader :OperationWithMultimediaInputOrOutput;
  skos:definition "A process that identifies an individual uniquely by using unique personal identification number (PIN) and/or biometrics like fingerprint, face recognition etc."@en;
  skos:inScheme :OperationScheme;
  skos:prefLabel "Person identification"@en .

:OpticalCharacterRecognition skos:broader :OperationWithMultimediaInputOrOutput .

:DkproTokenized a skos:Concept;
  :documentationUrl "https://dkpro.github.io/dkpro-core/releases/1.8.0/docs/format-reference.html#format-TokenizedText",
    "https://dkpro.github.io/dkpro-core/releases/1.8.0/docs/format-reference.html#format-de.tudarmstadt.ukp.dkpro.core.io.text-asl";
  rdfs:label "DKPro tokenized"@en;
  skos:broader :AnnotationFormat;
  skos:definition "DkPro format for tokenized files containing one sentence per line and tokens split by whitespaces."@en;
  skos:inScheme :DataFormatScheme;
  skos:prefLabel "DKPro tokenized"@en .

:FeatureExtractor a skos:Concept;
  :performsOperation :FeatureExtraction;
  rdfs:label "Feature extractor"@en;
  skos:broader :SupportComponent;
  skos:definition "A component that is used for extracting features"@en;
  skos:editorialNote "could also be under analyzer as a general term"@en;
  skos:inScheme :ComponentTypeScheme;
  skos:prefLabel "Feature extractor"@en .

:EntityMentionRecognition a skos:Concept;
  rdfs:label "Entity mention recognition"@en;
  skos:altLabel "Entity mention detection"@en, "Mention detection"@en;
  skos:broader :InformationExtraction;
  skos:definition "The task/process of detecting in a text mentions of a specific class of entities (e.g. biochemical entities, historical persons)"@en;
  skos:inScheme :OperationScheme;
  skos:prefLabel "Entity mention recognition"@en;
  skos:related :NamedEntityRecognition .

:Tsv a skos:Concept;
  :hasMimetype :text_tabSeparatedValues;
  rdfs:label "TSV"@en;
  skos:altLabel "Tab-separated values"@en;
  skos:broader :TabularFormat;
  skos:definition "Format for files with tab-separated values"@en;
  skos:inScheme :DataFormatScheme;
  skos:prefLabel "TSV"@en .

:SupportOfCrowdsourcingTasks a skos:Concept;
  rdfs:label "Support of crowdsourcing tasks"@en;
  skos:broader :SupportOperation;
  skos:definition "Any operation that can support tasks that are accomplished through crowdsourcing"@en;
  skos:example "Collection of data, their transformation and organization into crowdsourcing units; automatic generation of reusable crowdsourcing interfaces for specific tasks (e.g. annotation)"@en;
  skos:inScheme :OperationScheme;
  skos:prefLabel "Support of crowdsourcing tasks"@en .

:Folia a skos:Concept;
  :documentationUrl "https://proycon.github.io/folia/";
  rdfs:label "FoLiA"@en;
  skos:altLabel "Format for Linguistic Annotation"@en;
  skos:broader :AnnotationFormat, :Xml;
  skos:definition "FoLiA is an XML-based annotation format, suitable for the representation of linguistically annotated language resources"@en;
  skos:inScheme :DataFormatScheme;
  skos:prefLabel "FoLiA"@en .

:VerbalAggressionAnalysis a skos:Concept;
  rdfs:label "Verbal aggression analysis"@en;
  skos:altLabel "Verbal aggression classification"@en, "Verbal aggression detection"@en,
    "Verbal aggression identification"@en;
  skos:broader :InformationExtraction;
  skos:definition "The task/process of recognizing evidence and the target(s) of verbal aggression usually in social media texts"@en;
  skos:inScheme :OperationScheme;
  skos:prefLabel "Verbal aggression analysis"@en .

:SemanticRelationLabelling a skos:Concept;
  rdfs:label "Semantic relation labelling"@en;
  skos:altLabel "Semantic relation labeling [en-US]"@en-us;
  skos:broader :SemanticAnnotation;
  skos:definition "The task/process of attaching tags indicating the semantic relation that holds between units of a text."@en;
  skos:inScheme :OperationScheme;
  skos:prefLabel "Semantic relation labelling"@en .

:Html a skos:Concept;
  :hasMimetype :text_html;
  rdfs:label "HTML"@en;
  skos:broader :DocumentFormat;
  skos:definition "HTML format"@en;
  skos:inScheme :DataFormatScheme;
  skos:narrower :Html5Microdata;
  skos:prefLabel "HTML"@en .

:text_xml a skos:Concept;
  rdfs:label "text/xml";
  skos:broader :Mimetype;
  skos:inScheme :MimeTypeScheme .

:DialogueAct a skos:Concept;
  rdfs:label "Dialogue act"@en;
  skos:broader :SpeechAct;
  skos:definition "A dialogue act has two main components:  a communicative function and a semantic content.   The semantic content specifies the objects, relations, actions, events, etc. that the dialogue act is about; the communicative function can be viewed as a specification of the way an addressee uses the semantic content to update his or her information state when  he  or  she  understands  the  corresponding  stretch  of dialogue. [http://www.lrec-conf.org/proceedings/lrec2010/pdf/560_Paper.pdf]"@en;
  skos:inScheme :AnnotationTypeScheme;
  skos:prefLabel "Dialogue act"@en .

:Argumentation a skos:Concept;
  rdfs:label "Annotation of argumentation"@en;
  skos:broader :DiscourseAnnotation;
  skos:definition "The task/process of marking argumentative structures, components and relations in a text"@en;
  skos:inScheme :OperationScheme;
  skos:prefLabel "Annotation of argumentation"@en .

:CommentFiltering a skos:Concept;
  rdfs:label "Comment filtering"@en;
  skos:broader :SupportOperation;
  skos:definition "The identification and removal of abusive, bullying, etc. comments from texts"@en;
  skos:inScheme :OperationScheme;
  skos:prefLabel "Comment filtering"@en .

:TemporalExpression a skos:Concept;
  skos:definition "A linguistic expression (word, group of words, group of numbers etc.) that denotes time (a point in time, duration, frequency)"@en .

:FastInfoset a skos:Concept;
  :documentationUrl "https://gate.ac.uk/sale/tao/splitch23.html#x28-59400023.31";
  :hasMimetype :application_fastinfoset;
  rdfs:label "Fast Infoset"@en;
  skos:broader :BinaryFormat, :GateFormat;
  skos:definition "A compressed binary encoding of GATE XML"@en;
  skos:inScheme :DataFormatScheme;
  skos:prefLabel "Fast Infoset"@en .

:BodyMovement a skos:Concept;
  rdfs:label "Body movement"@en;
  skos:broader :ModalityAnnotationType;
  skos:inScheme :AnnotationTypeScheme;
  skos:prefLabel "Body movement"@en .

:application_xMsaccess a skos:Concept;
  rdfs:label "application/x-msaccess";
  skos:broader :Mimetype;
  skos:inScheme :MimeTypeScheme .

:QuantititativeInformation a skos:Concept;
  rdfs:label "Quantitative information"@en;
  skos:altLabel "Statistical information"@en;
  skos:broader :AnnotationType;
  skos:inScheme :AnnotationTypeScheme;
  skos:narrower :Frequency;
  skos:prefLabel "Quantitative information"@en .

:application_x_org_dkpro_reuters21578_sgml a skos:Concept;
  rdfs:label "application/x.org.dkpro.reuters21578+sgml";
  skos:broader :Mimetype;
  skos:inScheme :MimeTypeScheme .

:wav a skos:Concept;
  :hasFileExtension "wav";
  :hasMimetype :audio_vnd_wave, :audio_wav, :audio_wave, :audio_x_wav;
  rdfs:label "audio wav"@en;
  skos:broader :AudioFormat;
  skos:inScheme :DataFormatScheme;
  skos:prefLabel "audio wav"@en .

:DataMerging a skos:Concept;
  rdfs:label "Data merging"@en;
  skos:broader :SupportOperation;
  skos:definition "The task/process of merging (combining) together data from various sources"@en;
  skos:inScheme :OperationScheme;
  skos:prefLabel "Data merging"@en .

:mpg a skos:Concept;
  :hasFileExtension "mpg";
  :hasMimetype :audio_mpa, :audio_mpa_robust, :audio_mpeg;
  rdfs:label "audio mpg"@en;
  skos:broader :AudioFormat;
  skos:inScheme :DataFormatScheme;
  skos:prefLabel "audio mpg"@en .

:Pml a skos:Concept;
  :documentationUrl "http://ufal.mff.cuni.cz/jazz/PML/index_en.html", "https://builds.openminted.eu/job/WP%205.2%20-%20Typesystem%20alignment/eu.openminted.interop$mapping-conversion/doclinks/1/components.html#_prague_markup_language_1";
  :hasMimetype :application_x-SDL-TM, :application_xml;
  rdfs:label "PML"@en;
  skos:altLabel "Prague Markup Language"@en;
  skos:broader :AnnotationFormat, :Xml;
  skos:definition "Format according to the Prague Markup Language (http://ufal.mff.cuni.cz/jazz/PML/index_en.html); PML is a generic data format based on XML intended for storing linguistically annotated data, such as the Prague Dependency Treebank, also annotation lexicons, etc."@en;
  skos:inScheme :DataFormatScheme;
  skos:prefLabel "PML"@en .

:flac a skos:Concept;
  :hasFileExtension "flac";
  :hasMimetype :audio_flac;
  rdfs:label "flac"@en;
  skos:broader :AudioFormat;
  skos:editorialNote "both mimetypes appeat at various pages (e.g. europeana supported mimetypes https://pro.europeana.eu/page/media-formats-mime-types) but none of them is found in IANA official pages"@en;
  skos:inScheme :DataFormatScheme;
  skos:prefLabel "flac"@en .

:PhraseAlignment a skos:Concept;
  rdfs:label "Phrase alignment"@en;
  skos:broader :Alignment;
  skos:definition "Alignment at phrase level"@en;
  skos:inScheme :OperationScheme;
  skos:prefLabel "Phrase alignment"@en .

:Pdf a skos:Concept;
  :hasFileExtension "pdf";
  :hasMimetype :application_pdf;
  rdfs:label "PDF"@en;
  skos:broader :BinaryFormat, :DocumentFormat;
  skos:definition "Data format for PDF files (Portable Document Format)"@en;
  skos:inScheme :DataFormatScheme;
  skos:prefLabel "PDF"@en .

:Lemmatization a skos:Concept;
  rdfs:label "Lemmatization"@en;
  skos:altLabel "Lemmatisation"@en-uk;
  skos:broader :TextAnnotation;
  skos:definition "Lemmatisation  (or lemmatization) in linguistics is the process of grouping together the inflected forms of a word so they can be analysed as a single item, identified by the word's lemma, or dictionary form. [Wikipedia]"@en;
  skos:inScheme :OperationScheme;
  skos:prefLabel "Lemmatization"@en .

:SpeechProcessingCollection skos:member :MultimodalSynthesis .

:InformationExtractor a skos:Concept;
  :performsOperation :InformationExtraction;
  rdfs:label "Information extractor"@en;
  skos:broader :Analyzer;
  skos:definition "A component that automatically extracts structured information from unstructured and/or semi-structured machine-readable documents"@en;
  skos:inScheme :ComponentTypeScheme;
  skos:prefLabel "Information extractor"@en .

:AgeBracketDetection a skos:Concept;
  rdfs:label "Age-bracket detection"@en;
  skos:broader :InformationExtraction;
  skos:definition "The task/process of identifying in a text a segment inside parentheses that describes an age group or age-related utterance"@en;
  skos:inScheme :OperationScheme;
  skos:prefLabel "Age-bracket detection"@en .

:GateFormat a skos:Concept;
  rdfs:label "GATE format"@en;
  skos:broader :DataFormat;
  skos:definition "Formats used for the GATE framework"@en;
  skos:inScheme :DataFormatScheme;
  skos:narrower :Datasift_json, :FastInfoset, :GateXml, :Gate_twitter_json;
  skos:prefLabel "GATE format"@en .

:XmlBioc a skos:Concept;
  :documentationUrl "http://bioc.sourceforge.net/";
  :hasMimetype :application_xml;
  rdfs:label "XML BioC"@en;
  skos:broader :Xml;
  skos:definition "BioC is a simple format to share text data and annotations."@en;
  skos:inScheme :DataFormatScheme;
  skos:prefLabel "XML BioC"@en .

:DiscourseAnnotation a skos:Concept;
  rdfs:label "Discourse annotation"@en;
  skos:broader :TextAnnotation;
  skos:definition "The task/process of adding annotations relevant to discourse, such as discourse structure, discourse markers etc."@en;
  skos:inScheme :OperationScheme;
  skos:narrower :AnaphoraAnnotation, :Argumentation, :CoreferenceAnnotation, :DiscourseModelling;
  skos:prefLabel "Discourse annotation"@en .

:MultimediaAnnotation a skos:Concept;
  rdfs:label "Multimedia annotation"@en;
  skos:broader :Annotation;
  skos:inScheme :OperationScheme;
  skos:prefLabel "Multimedia annotation"@en .

:ImageUnderstanding skos:broader :OperationWithMultimediaInputOrOutput .

:application_msword a skos:Concept;
  rdfs:label "application/msword";
  skos:broader :Mimetype;
  skos:inScheme :MimeTypeScheme .

:RuleBasedMethod a skos:Concept;
  rdfs:label "Rule-based Method"@en;
  skos:broader :TdmMethod;
  skos:definition "A type of method that makes use of set(s) of rules to perform the relevant task."@en;
  skos:inScheme :TdmMethodScheme;
  skos:prefLabel "Rule-based Method"@en .

:ProsodicSegmentation a skos:Concept;
  rdfs:label "Prosodic segmentation"@en;
  skos:broader :ProsodicAnnotation;
  skos:inScheme :OperationScheme;
  skos:prefLabel "Prosodic segmentation"@en .

:AnnotationOfCompounds a skos:Concept;
  rdfs:label "Annotation of compounds"@en;
  skos:broader :MorphologicalAnnotation;
  skos:definition "The task/process of marking compounds (single words composed of two or more free morphemes) and their parts"@en;
  skos:inScheme :OperationScheme;
  skos:prefLabel "Annotation of compounds"@en .

:OasisText a skos:Concept;
  :hasMimetype :application_vnd_oasis_opendocument_text;
  rdfs:label "Oasis text"@en;
  skos:broader :DocumentFormat, :OpenFormat;
  skos:inScheme :DataFormatScheme;
  skos:prefLabel "Oasis text"@en .

:Tcf a skos:Concept;
  :documentationUrl "https://weblicht.sfs.uni-tuebingen.de/weblichtwiki/index.php/The_TCF_Format";
  :hasMimetype :text_tcf_xml;
  rdfs:label "TCF"@en;
  skos:altLabel "Text Corpus Format"@en;
  skos:broader :AnnotationFormat, :CorpusFormat, :Xml;
  skos:definition "An XML data exchange format developed within the WebLicht architecture to facilitate efficient interoperability between the tools; it allows the various linguistic annotations produced by the tools within WebLicht to be stored in one document; it supports incremental enrichment of linguistic annotations at various levels of analysis in a stand-­off XML‐based format"@en;
  skos:inScheme :DataFormatScheme;
  skos:prefLabel "TCF"@en .

:application_pdf a skos:Concept;
  rdfs:label "application/pdf";
  skos:broader :Mimetype;
  skos:inScheme :MimeTypeScheme .

:NewsGeneration a skos:Concept;
  rdfs:label "News generation"@en;
  skos:broader :NaturalLanguageGeneration;
  skos:inScheme :OperationScheme;
  skos:prefLabel "News generation"@en .

:performsOperation a owl:ObjectProperty;
  rdfs:comment "Component A performs Operation B"@en;
  rdfs:label "performs operation"@en;
  rdfs:range _:node1fu4q14cjx42;
  rdfs:subPropertyOf owl:topObjectProperty;
  skos:altLabel "performs Task"@en .

:ZeroShotClassification a skos:Concept;
  rdfs:label "Zero-Shot classification"@en;
  skos:broader :ModelFunction, :SupportOperation;
  skos:inScheme :OperationScheme;
  skos:prefLabel "Zero-Shot classification"@en .

:InformationStorage a skos:Concept;
  rdfs:label "Information storage"@en;
  skos:altLabel "Data storage"@en;
  skos:broader :SupportOperation;
  skos:definition "";
  skos:inScheme :OperationScheme;
  skos:prefLabel "Information storage"@en .

:EmotionRecognizer a skos:Concept;
  :performsOperation :EmotionDetection;
  rdfs:label "Emotion recognizer"@en;
  skos:altLabel "Emotion detector"@en;
  skos:broader :Analyzer;
  skos:definition "A component that tries to recognize and annotate emotions (e.g. fear, anger, happiness etc.) from text, video, audio and image"@en;
  skos:editorialNote "could also be an annotator"@en;
  skos:inScheme :ComponentTypeScheme;
  skos:prefLabel "Emotion recognizer"@en .

:Chat a skos:Concept;
  :documentationUrl "http://talkbank.org/manuals/CHAT.pdf";
  rdfs:label "CHAT"@en;
  skos:altLabel "Codes for the Human Analysis of Transcripts"@en;
  skos:broader :AnnotationFormat;
  skos:definition "CHAT (Codes for the Human Analysis of Transcripts) transcription format; used by CHILDES corpora"@en;
  skos:inScheme :DataFormatScheme;
  skos:prefLabel "CHAT"@en .

:ScriptBasedAnalysis a skos:Concept;
  rdfs:label "Script-based analysis"@en;
  skos:altLabel "Script based analysis"@en;
  skos:broader :SupportOperation;
  skos:definition "The task/process of analysing a resource following a script"@en;
  skos:inScheme :OperationScheme;
  skos:prefLabel "Script-based analysis"@en .

:ConstituencyParsing a skos:Concept;
  rdfs:label "Constituency parsing"@en;
  skos:altLabel "Natural Language Parsing"@en, "Phrase parsing"@en;
  skos:broader :Parsing;
  skos:definition "Parsing (from Latin \"\"pars orationis\"\" = parts of speech) is the syntactic analysis of languages. Natural Language Parsing is the syntactic analysis of natural languages, such as Finnish or Chinese. The objective of Natural Language Parsing is to determine parts of sentences (such as verbs, noun phrases, or relative clauses), and the relationships between them (such as subject or object). Unlike parsing of formally defined artificial languages (such as Java or predicate logic), parsing of natural languages presents problems due to ambiguity, and the productive and creative use of language."@en,
    "The task/process of identifying and marking constituents (phrases, governed by a head and including function words and/or modifiers ) in a text or text segment"@en;
  skos:inScheme :OperationScheme;
  skos:prefLabel "Constituency parsing"@en .

:Disambiguator a skos:Concept;
  rdfs:label "Disambiguator"@en;
  skos:broader :Analyzer;
  skos:definition "A component that is used to disambiguate between two or more ambiguous items"@en;
  skos:inScheme :ComponentTypeScheme;
  skos:narrower :WordSenseDisambiguator;
  skos:prefLabel "Disambiguator"@en .

:aif a skos:Concept;
  :hasFileExtension "aif";
  :hasMimetype :audio_aiff;
  rdfs:label "aif"@en;
  skos:broader :AudioFormat;
  skos:inScheme :DataFormatScheme;
  skos:prefLabel "aif"@en .

:audio_mpeg3 a skos:Concept;
  rdfs:label "audio/mpeg3";
  skos:broader :Mimetype;
  skos:inScheme :MimeTypeScheme .

:TableQuestionAnswering a skos:Concept;
  rdfs:label "Table question answering"@en;
  skos:broader :InformationExtraction;
  skos:inScheme :OperationScheme;
  skos:prefLabel "Table question answering"@en .

:Validator a skos:Concept;
  :performsOperation :Validation;
  rdfs:label "Validator"@en;
  skos:broader :SupportComponent;
  skos:definition "A component used to confirm that a system/resource meets the specifications and fulfills its intended purpose"@en;
  skos:inScheme :ComponentTypeScheme;
  skos:prefLabel "Validator"@en .

:Organism a skos:Concept;
  rdfs:label "Organism"@en;
  skos:broader :AgriculturalEntity;
  skos:definition "An individual animal, plant, or single-celled life form [https://en.oxforddictionaries.com/definition/organism]"@en;
  skos:inScheme :AnnotationTypeScheme;
  skos:prefLabel "Organism"@en .

:application_vnd_oasis_opendocument_text a skos:Concept;
  rdfs:label "application/vnd.oasis.opendocument.text";
  skos:broader :Mimetype;
  skos:inScheme :MimeTypeScheme .

:StructuralAnnotation a skos:Concept;
  rdfs:label "Structural annotation"@en;
  skos:altLabel "Segmentation"@en;
  skos:broader :TextAnnotation;
  skos:definition "The task/process of segmenting a text and recognizing textual structural units (paragraphs, sentences, words etc.)"@en;
  skos:inScheme :OperationScheme;
  skos:narrower :AnnotationOfDocumentStructure, :ParagraphSplitting, :SentenceSplitting,
    :Tokenization;
  skos:prefLabel "Structural annotation"@en .

:AuthorClassification a skos:Concept;
  rdfs:label "Author classification"@en;
  skos:broader :InformationExtraction;
  skos:definition "The task/process of organizing documents into groups/classes on the basis of their author"@en;
  skos:inScheme :OperationScheme;
  skos:prefLabel "Author classification"@en .

:OfficialText skos:broader :NamedEntity .

:WordSenseDisambiguation a skos:Concept;
  rdfs:label "Word Sense Disambiguation"@en;
  skos:altLabel "WSD"@en;
  skos:broader :SupportOperation;
  skos:definition "The process/task of identifying which sense of a word with multiple meanings is used in a particular context; the selection of the sense is made from a list of the word's senses."@en,
    "Word Sense Disambiguation is a subtask of semantic tagging, which consists of assigning a semantic class (sense) to a lexical item as specified by a semantic lexicon. If the semantic lexicon specifies more than one sense for a particular lexical item, a disambiguation procedure is needed to decide upon the most appropriate sense(s) for any given instance of the lexical item in text. WSD is not a self-contained application, but it may be included as an integrated part of a semantic processor."@en;
  skos:inScheme :OperationScheme;
  skos:prefLabel "Word Sense Disambiguation"@en .

:Tmx a skos:Concept;
  :documentationUrl "http://www.ttt.org/oscarstandards/tmx/tmx14-20020710.htm";
  :hasMimetype :application_xTmx_xml;
  rdfs:label "TMX"@en;
  skos:altLabel "Translation Memory Exchange"@en;
  skos:broader :AnnotationFormat, :Xml;
  skos:definition "The purpose of the TMX format is to provide a standard method to describe translation memory data that is being exchanged among tools and/or translation vendors, while introducing little or no loss of critical data during the process."@en;
  skos:inScheme :DataFormatScheme;
  skos:prefLabel "TMX"@en .

:SpeechEnhancement a skos:Concept;
  rdfs:label "Speech Enhancement"@en;
  skos:broader :SpeechRecognition;
  skos:definition "The improvement of speech intelligibility by removing background noise from the speech signal"@en,
    "The improvement of speech intelligibility by removing background noise from the speech signal. Due to the complexity of speech acoustics and perception, no simple mathematical error criterion can be applied; instead, algorithms and measures need to be developed which accomodate human perception."@en;
  skos:inScheme :OperationScheme;
  skos:prefLabel "Speech Enhancement"@en .

:HumanComputerInteraction a skos:Concept;
  rdfs:label "Human Computer Interaction"@en;
  skos:altLabel "HCI"@en, "Human Machine Interaction"@en;
  skos:broader :OperationWithMultimediaInputOrOutput;
  skos:definition "A multi-disciplinary research area focusing on the design and use of computer technology deployed in interfaces between humans and computers"@en;
  skos:inScheme :OperationScheme;
  skos:narrower :AvatarSynthesis, :ConversationalSystemsBuilding;
  skos:prefLabel "Human Computer Interaction"@en .

:Constituent a skos:Concept;
  :documentationUrl "http://dkpro.github.io/dkpro-core/releases/1.8.0/docs/typesystem-reference.html#de.tudarmstadt.ukp.dkpro.core.api.syntax.type.constituent.Constituent";
  rdfs:label "Constituent"@en;
  owl:equivalentClass <http://purl.org/olia/olia-top.owl#Constituent>, <http://vocab.lappsgrid.org/Constituent>;
  skos:broader :SyntacticAnnotationType;
  skos:definition "A word or group of words that function as a single unit in a syntactic structure"@en;
  skos:inScheme :AnnotationTypeScheme;
  skos:prefLabel "Constituent"@en .

:Rtf a skos:Concept;
  :hasFileExtension "rtf";
  :hasMimetype :application_rtf;
  rdfs:label "RTF"@en;
  skos:broader :DocumentFormat;
  skos:definition "Rich Text Format; proprietary data format of Microsoft"@en;
  skos:inScheme :DataFormatScheme;
  skos:prefLabel "RTF"@en .

:Naf a skos:Concept;
  :documentationUrl "http://wordpress.let.vupr.nl/naf/", "https://github.com/newsreader/NAF";
  rdfs:label "NAF"@en;
  skos:altLabel "NLP Annotation Format"@en;
  skos:broader :AnnotationFormat;
  skos:definition "The NAF format is linguistic annotation format designed for complex NLP pipelines. NAF combines strengths of the Linguistic Annotation Framework (LAF) as described in Ide et al. (2003) and the NLP Interchange Format (Hellman et al. 2013, NIF)."@en;
  skos:inScheme :DataFormatScheme;
  skos:prefLabel "NAF"@en .

:Organization a skos:Concept;
  :documentationUrl "http://dkpro.github.io/dkpro-core/releases/1.8.0/docs/typesystem-reference.html#de.tudarmstadt.ukp.dkpro.core.api.ner.type.Organization";
  rdfs:label "Organization"@en;
  skos:broader :NamedEntity;
  skos:definition "A word or group of words that denotes an organization, such as company, association, institution etc."@en;
  skos:inScheme :AnnotationTypeScheme;
  skos:prefLabel "Organization"@en .

:svg a skos:Concept;
  :hasFileExtension "svg";
  :hasMimetype :image_svg;
  rdfs:label "SVG"@en;
  skos:altLabel "Scalable Vector Graphics"@en;
  skos:broader :ImageFormat;
  skos:inScheme :DataFormatScheme;
  skos:prefLabel "SVG"@en .

:TextToImageGeneration a skos:Concept;
  rdfs:label "Text to Image generation"@en;
  skos:broader :ImageGeneration;
  skos:inScheme :OperationScheme;
  skos:prefLabel "Text to Image generation"@en .

:AnnotationOfTextualEntailment a skos:Concept;
  rdfs:label "Annotation of textual entailment"@en;
  skos:broader :SemanticAnnotation;
  skos:definition "The task/process of annotating textual entailments, most usually indicating whether a text entails or contradicts a hypothesis sentence or does neither."@en;
  skos:inScheme :OperationScheme;
  skos:prefLabel "Annotation of textual entailment"@en .

:TextSimplification a skos:Concept;
  rdfs:label "Text simplification"@en;
  skos:broader :NaturalLanguageGeneration;
  skos:definition "The task of replacing textual segments (phrases, clauses, etc.) with other segments that have similar meaning but are easier to understand"@en;
  skos:inScheme :OperationScheme;
  skos:prefLabel "Text simplification"@en;
  skos:related :LexicalSimplification .

:application_vnd_openxmlformats_officedocument_spreadsheetml_sheet skos:broader :Mimetype .

:TopicDetection a skos:Concept;
  rdfs:label "Topic Detection"@en;
  skos:altLabel "TD"@en, "TDT"@en, "TT"@en, "Topic Detection and Tracking"@en, "Topic Tracking"@en,
    "Topic classification"@en, "Topic extraction"@en;
  skos:definition "The task/process of identifying the topic of a text or dataset (e.g. by clustering keywords or using topic models)"@en,
    "Topic Detection and Tracking (TDT) refers to automatic techniques for discovering, threading, and retrieving topically related material in streams of data."@en;
  skos:inScheme :OperationScheme;
  skos:prefLabel "Topic Detection"@en;
  skos:related :TextCategorization .

:PartOfSpeechTagger skos:broader :MorphologicalTagger .

:Reuters21578Sgml a skos:Concept;
  :documentationUrl "https://dkpro.github.io/dkpro-core/releases/1.8.0/docs/format-reference.html#format-Reuters21578Sgml";
  :hasMimetype :application_x_org_dkpro_reuters21578_sgml;
  rdfs:label "Reuters21578 SGML"@en;
  skos:broader :CorpusFormat;
  skos:definition "Reuters-21578 corpus in SGML format"@en;
  skos:inScheme :DataFormatScheme;
  skos:prefLabel "Reuters21578 SGML"@en .

:IntraDocumentCoReferenceResolution a skos:Concept;
  rdfs:label "Intra-document co-reference resolution"@en;
  skos:altLabel "Intra-document coreference resolution"@en;
  skos:broader :CoReferenceResolution;
  skos:inScheme :OperationScheme;
  skos:prefLabel "Intra-document co-reference resolution"@en .

:BionlpSt2013A1_a2 a skos:Concept;
  :documentationUrl "https://builds.openminted.eu/job/WP%205.2%20-%20Typesystem%20alignment/eu.openminted.interop$mapping-conversion/doclinks/1/components.html#_bionlp_st_2013_a1_a2_1";
  rdfs:label "BioNLP-ST 2013 a1/a2"@en;
  skos:altLabel "bioNLP; format-variant=ST2013a1_a2"@en;
  skos:broader :BionlpFormat, :BionlpFormats;
  skos:definition "Format used in BioNLP Shared Task 2013"@en;
  skos:inScheme :DataFormatScheme;
  skos:prefLabel "BioNLP-ST 2013 a1/a2"@en .

:WordSenseInduction a skos:Concept;
  rdfs:label "Word sense induction"@en;
  skos:altLabel "WSI"@en;
  skos:broader :KnowledgeDiscovery;
  skos:definition "The task of automatically identifying the senses of a word"@en;
  skos:inScheme :OperationScheme;
  skos:prefLabel "Word sense induction"@en;
  skos:related :WordSenseDisambiguation .

:Event a skos:Concept;
  :documentationUrl "http://dkpro.github.io/dkpro-core/releases/1.8.0/docs/typesystem-reference.html#de.tudarmstadt.ukp.dkpro.core.api.ner.type.Event";
  rdfs:label "Event"@en;
  skos:broader :SemanticAnnotationType;
  skos:definition "A thing that happens or takes place, especially one of importance [https://en.oxforddictionaries.com/definition/event]"@en;
  skos:inScheme :AnnotationTypeScheme;
  skos:prefLabel "Event"@en .

:Normalization a skos:Concept;
  rdfs:label "Normalization"@en;
  skos:broader :SupportOperation;
  skos:definition "The task/process of editing a text in order to remove unwanted material (e.g. quotation marks, hyphenations etc.) or to substitute/represent specific items (tokens, dates,  etc.) with normalized values"@en;
  skos:inScheme :OperationScheme;
  skos:narrower :ConceptNormalization, :NormalizationOfMeasurements, :NormalizationOfNumbers;
  skos:prefLabel "Normalization"@en .

:FacialExpressionRecognition skos:definition "The task/process of detecting emotions on human face based on biometric markers [adapted from https://sightcorp.com/knowledge-base/facial-expression-recognition/]"@en .

:AnnotationOfNumbers a skos:Concept;
  rdfs:label "Annotation of numbers"@en;
  skos:altLabel "Number detection"@en;
  skos:broader :SemanticAnnotation;
  skos:definition "The task/process of annotating numbers in a text"@en;
  skos:inScheme :OperationScheme;
  skos:prefLabel "Annotation of numbers"@en .

:InformationFilteringByRecommenderSystems a skos:Concept;
  rdfs:label "Information filtering by recommender systems"@en;
  skos:broader :InformationFiltering;
  skos:definition "The delivery of information in the form of suggestions by recommender systems; recommender systems seek to predict the \"\"rating\"\" or \"\"preference\"\" that a user would give to an item"@en;
  skos:inScheme :OperationScheme;
  skos:prefLabel "Information filtering by recommender systems"@en .

:MediaWikiMarkup a skos:Concept;
  :documentationUrl "https://www.mediawiki.org/wiki/Help:Formatting";
  rdfs:label "Media Wiki markup"@en;
  skos:broader :WikiFormat, :WikiFormats;
  skos:definition "Wiki markup for formatting"@en;
  skos:inScheme :DataFormatScheme;
  skos:prefLabel "Media Wiki markup"@en .

:application_vnd_ms_powerpoint a skos:Concept;
  rdfs:label "application/vnd.ms-powerpoint";
  skos:broader :Mimetype;
  skos:inScheme :MimeTypeScheme .

:TrainingOfLanguageModels a skos:Concept;
  dc:source "Adapted from http://homepages.inf.ed.ac.uk/lzhang10/slm.html";
  rdfs:label "Training of language models"@en;
  skos:broader :LanguageModelling;
  skos:definition "The task/process of training (statistical) language models that  that can estimate the distribution of natural language as accurately as possible."@en;
  skos:inScheme :OperationScheme;
  skos:prefLabel "Training of language models"@en .

:AudioSegmentation a skos:Concept;
  rdfs:label "Audio segmentation"@en;
  skos:broader :SpeechAnnotation;
  skos:definition "The task/process of partitioning audio stream into homogeneous segments and classifying them into speech and non-speech segments"@en;
  skos:inScheme :OperationScheme;
  skos:prefLabel "Audio segmentation"@en .

:TruthLabelling a skos:Concept;
  rdfs:label "Truth labelling"@en;
  skos:altLabel "Truth detection"@en, "Truth labeling"@en-us;
  skos:broader :InformationExtraction;
  skos:definition "The task of assigning a true/false tag to a news item, headline, claim, etc."@en;
  skos:inScheme :OperationScheme;
  skos:prefLabel "Truth labelling"@en .

:audio_vnd_wave a skos:Concept;
  rdfs:label "audio/vnd.wave";
  skos:broader :Mimetype;
  skos:inScheme :MimeTypeScheme .

:TrainingOfNmtModels a skos:Concept;
  rdfs:label "Training of NMT models"@en;
  skos:altLabel "Training of Neural Machine Translation models"@en;
  skos:broader :LanguageModelling;
  skos:inScheme :OperationScheme;
  skos:prefLabel "Training of NMT models"@en .

:MLModelFormat a skos:Concept;
  rdfs:label "Machine Learning Model format"@en;
  skos:altLabel "ML model format"@en;
  skos:broader :DataFormat;
  skos:definition "Format used for ML models"@en;
  skos:inScheme :DataFormatScheme;
  skos:narrower :ONNX, :TFSavedModel;
  skos:prefLabel "Machine Learning Model format"@en .

:Tgrep2 a skos:Concept;
  :documentationUrl "https://dkpro.github.io/dkpro-core/releases/1.8.0/docs/format-reference.html#format-de.tudarmstadt.ukp.dkpro.core.io.tgrep-gpl";
  :hasMimetype :application_x_org_dkpro_tgrep2;
  rdfs:label "TGrep2"@en;
  skos:broader :AnnotationFormat;
  skos:definition "Format for TGrep2 (search engine for searching syntactic parse trees represented as bracketed structures)"@en;
  skos:inScheme :DataFormatScheme;
  skos:prefLabel "TGrep2"@en .

:CorpusViewer a skos:Concept;
  :performsOperation :CorpusViewing;
  rdfs:label "Corpus viewer"@en;
  skos:broader :Viewer;
  skos:definition "A component that supports humans in accessing the contents of a corpus"@en;
  skos:inScheme :ComponentTypeScheme;
  skos:prefLabel "Corpus viewer"@en .

:Normalizer a skos:Concept;
  :performsOperation :Normalization;
  rdfs:label "Normalizer"@en;
  skos:broader :PreOrPostProcessor;
  skos:definition "A component that removes unwanted material from text (e.g. quotation marks, hyphenations etc.) or performs edits so that specific items (tokens, dates,  etc.) are substituted/represented with normalized values"@en;
  skos:inScheme :ComponentTypeScheme;
  skos:prefLabel "Normalizer"@en .

:Conll2003 a skos:Concept;
  :documentationUrl "https://zoidberg.ukp.informatik.tu-darmstadt.de/jenkins/job/DKPro%20Core%20Documentation%20(GitHub)/de.tudarmstadt.ukp.dkpro.core$de.tudarmstadt.ukp.dkpro.core.doc-asl/doclinks/5/format-reference.html#format-Conll2003";
  :hasMimetype :text_x_org_dkpro_conll2003;
  rdfs:label "CoNLL-2003"@en;
  skos:broader :ConllFormat;
  skos:definition "The CoNLL 2004 format encodes named entity spans and chunk spans. Fields are separated by a single space. Sentences are separated by a blank new line. Named entities and chunks are encoded in the IOB1 format. I.e. a B prefix is only used if the category of the following span differs from the category of the current span."@en;
  skos:inScheme :DataFormatScheme;
  skos:prefLabel "CoNLL-2003"@en .

:InstanceBasedLearning a skos:Concept;
  dc:source "adapted from Wikipedia (https://en.wikipedia.org/wiki/Instance-based_learning)"@en;
  rdfs:label "Instance-based Learning"@en;
  skos:broader :MachineAndStatisticalLearningMethod;
  skos:definition "A family of learning algorithms that, instead of performing explicit generalization, compares new problem instances with instances seen in training, which have been stored in memory."@en;
  skos:example "Examples of instance-based learning algorithm are the k-nearest neighbor algorithm, kernel machines and RBF networks."@en;
  skos:inScheme :TdmMethodScheme;
  skos:prefLabel "Instance-based Learning"@en .

:basic a skos:Concept;
  :hasFileExtension "au", "snd";
  :hasMimetype :audio_basic;
  rdfs:label "basic"@en;
  skos:broader :AudioFormat;
  skos:inScheme :DataFormatScheme;
  skos:prefLabel "basic"@en .

:OpenFormat a skos:Concept;
  rdfs:label "Open format"@en;
  skos:broader :DataFormat;
  skos:inScheme :DataFormatScheme;
  skos:narrower :OasisPresentation, :OasisSpreadsheet, :OasisText, :OpenOfficeDocument,
    :OpenOfficePresentation, :OpenOfficeSpreadsheet;
  skos:prefLabel "Open format"@en .

:Viewing a skos:Concept;
  rdfs:label "Viewing"@en;
  skos:broader :SupportOperation;
  skos:definition "The task/process of viewing the contents of a resource as performed by human beings"@en;
  skos:inScheme :OperationScheme;
  skos:narrower :CorpusViewing, :LexiconViewing;
  skos:prefLabel "Viewing"@en .

:ProteinFamily a skos:Concept;
  rdfs:label "Protein family"@en;
  skos:broader :AgriculturalEntity;
  skos:definition "A protein family is a group of proteins that share a common evolutionary origin, reflected by their related functions and similarities in sequence or structure [https://www.ebi.ac.uk/training/online/course/introduction-protein-classification-ebi/protein-classification/what-are-protein-families]"@en;
  skos:inScheme :AnnotationTypeScheme;
  skos:prefLabel "Protein family"@en .

:StatisticalLanguageModelling a skos:Concept;
  rdfs:label "Statistical Language Modelling"@en;
  skos:altLabel "SLM"@en, "Statistical Language Modeling"@en;
  skos:broader :LanguageModelling;
  skos:inScheme :OperationScheme;
  skos:prefLabel "Statistical Language Modelling"@en .

:KnowledgeRepresentation a skos:Concept;
  rdfs:label "Knowledge Representation"@en;
  skos:altLabel "KR"@en;
  skos:broader :TextAndDataMining;
  skos:definition "", "The task/process of representing information about entities in a form that machines are capable of understanding it"@en;
  skos:inScheme :OperationScheme;
  skos:prefLabel "Knowledge Representation"@en .

:SoundEventAnnotation a skos:Concept;
  rdfs:label "Sound event annotation"@en;
  skos:broader :SpeechAnnotation;
  skos:inScheme :OperationScheme;
  skos:prefLabel "Sound event annotation"@en .

:SpeechUnderstanding a skos:Concept;
  rdfs:label "Speech understanding"@en;
  skos:broader :NaturalLanguageUnderstanding, :SpeechRecognition;
  skos:inScheme :OperationScheme;
  skos:prefLabel "Speech understanding"@en .

:TextAndDataMining a skos:Concept;
  rdfs:label "Text and Data Mining"@en;
  skos:altLabel "DM"@en, "Data Mining"@en, "TDM"@en, "TM"@en, "Text Data Mining"@en,
    "Text Mining"@en;
  skos:broader :Operation;
  skos:definition "Text data mining concerns the application of data mining (knowledge discovery in databases, KDD) to unstructured textual data. The goal of data mining is to discover or derive new information from data, finding patterns across datasets, and/or separating signal from noise. Core text mining algorithms decompose text in meaningful chunks that can then be used for true data mining purposes."@en,
    "The automated processing of unstructured text and/or structured data leading to the extraction of previously hidden knowledge."@en;
  skos:inScheme :OperationScheme;
  skos:narrower :InformationExtraction, :KnowledgeAcquisition, :KnowledgeDiscovery,
    :Prediction;
  skos:prefLabel "Text and Data Mining"@en .

:text_x_anafora rdfs:label "text/x-anafora" .

:TerminologySearch a skos:Concept;
  rdfs:label "Terminology search"@en;
  skos:altLabel "Term search"@en;
  skos:broader :InformationRetrieval;
  skos:inScheme :OperationScheme;
  skos:prefLabel "Terminology search"@en .

:TextToTextGeneration a skos:Concept;
  rdfs:label "Text to Text Generation"@en;
  skos:broader :TextGeneration;
  skos:inScheme :OperationScheme;
  skos:prefLabel "Text to Text Generation"@en .

:Term a skos:Concept;
  rdfs:label "Term"@en;
  skos:broader :AnnotationType;
  skos:definition "A term is a designation consisting of one or more words representing a general concept in a special language in a specific subject field [ISO 704:2009]"@en;
  skos:inScheme :AnnotationTypeScheme;
  skos:prefLabel "Term"@en .

:FeatureExtraction a skos:Concept;
  dc:source <http://scikit-learn.org/stable/modules/feature_extraction.html>;
  rdfs:label "Feature extraction"@en;
  skos:broader :ModelFunction, :SupportOperation;
  skos:definition "Feature extraction consists in transforming arbitrary data, such as text or images, into numerical features usable for machine learning"@en;
  skos:inScheme :OperationScheme;
  skos:narrower :FrequencyCount;
  skos:prefLabel "Feature extraction"@en .

:SDL_tm_xliff a skos:Concept;
  :documentationUrl "http://sdl.com/FileTypes/SdlXliff/1.0";
  rdfs:label "SDL alignment format"@en;
  skos:broader :Xml;
  skos:inScheme :DataFormatScheme;
  skos:prefLabel "SDL alignment format"@en .

:AclAnthologyCorpusFormat a skos:Concept;
  :documentationUrl "https://dkpro.github.io/dkpro-core/releases/1.8.0/docs/format-reference.html#format-AclAnthology",
    "https://dkpro.github.io/dkpro-core/releases/1.8.0/docs/format-reference.html#format-de.tudarmstadt.ukp.dkpro.core.io.aclanthology-asl";
  :hasMimetype :text_plain;
  rdfs:label "ACL Anthology Corpus format"@en;
  skos:broader :CorpusFormat;
  skos:definition "Data format specific to the ACL Anthology Reference Corpus (http://acl-arc.comp.nus.edu.sg/), most probably version 20080325"@en;
  skos:inScheme :DataFormatScheme;
  skos:prefLabel "ACL Anthology Corpus format"@en .

:gif a skos:Concept;
  :hasFileExtension "gif";
  :hasMimetype :image_gif;
  rdfs:label "GIF"@en;
  skos:altLabel "Graphics Interchange Format"@en;
  skos:broader :ImageFormat;
  skos:inScheme :DataFormatScheme;
  skos:prefLabel "GIF"@en .

:MachineLearningMethod a skos:Concept;
  dc:source "adapted from https://www.sas.com/en-US/insights/analytics/machine-learning.html"@en;
  rdfs:label "Machine Learning Method"@en;
  skos:broader :TdmMethod;
  skos:definition "A method of data analysis that automates model building. Using algorithms that iteratively learn from data, machine learning allows computers to find hidden insights without being explicitly programmed where to look."@en;
  skos:inScheme :TdmMethodScheme;
  skos:prefLabel "Machine Learning Method"@en .

:ScriptBasedAnalyser a skos:Concept;
  :performsOperation :ScriptBasedAnalysis;
  rdfs:label "Script-based analyser"@en;
  skos:broader :SupportComponent;
  skos:definition "A component that performs analysis tasks based on a script"@en;
  skos:inScheme :ComponentTypeScheme;
  skos:prefLabel "Script-based analyser"@en .

:Converter a skos:Concept;
  :performsOperation :FormatConversion;
  rdfs:label "Converter"@en;
  skos:broader :SupportComponent;
  skos:definition "A component that performs conversion between formats of a resource"@en;
  skos:inScheme :ComponentTypeScheme;
  skos:narrower :DependencyConverter;
  skos:prefLabel "Converter"@en .

:application_xTex a skos:Concept;
  rdfs:label "application/x-tex";
  skos:broader :Mimetype;
  skos:inScheme :MimeTypeScheme .

:Aligner a skos:Concept;
  rdfs:label "Aligner"@en;
  skos:broader :Annotator;
  skos:definition "A component that detects and annotates equivalence relations between items (corpora, texts, paragraphs, sentences, phrases, words) in two languages"@en;
  skos:inScheme :ComponentTypeScheme;
  skos:prefLabel "Aligner"@en .

:Pubmed a skos:Concept;
  :documentationUrl "https://gate.ac.uk/sale/tao/splitch23.html#sec:creole:pubmed";
  :hasMimetype :text_xPubmed;
  rdfs:label "PubMed"@en;
  skos:broader :DocumentFormat;
  skos:definition "Textual format used for PubMed articles"@en;
  skos:inScheme :DataFormatScheme;
  skos:prefLabel "PubMed"@en .

:EmotionDetection a skos:Concept;
  rdfs:label "Emotion recognition"@en;
  skos:altLabel "Emotion detection"@en;
  skos:broader :InformationExtraction;
  skos:definition "The recognition of emotions from text, speech, facial expressions, gestures and/or physiological measures. A key challenge is the appropriate representation of emotional states."@en;
  skos:inScheme :OperationScheme;
  skos:prefLabel "Emotion recognition"@en .

:CertaintyLevel a skos:Concept;
  rdfs:label "Certainty level"@en;
  skos:broader :SemanticAnnotationType;
  skos:definition "Degree of certainty about the validity of what is being asserted in the text"@en;
  skos:inScheme :AnnotationTypeScheme;
  skos:prefLabel "Certainty level"@en .

:FlowControl a skos:Concept;
  dc:source <https://en.wikipedia.org/wiki/Flow_control_(data)>;
  rdfs:label "Flow control"@en;
  skos:broader :SupportOperation;
  skos:inScheme :OperationScheme;
  skos:prefLabel "Flow control"@en .

:MultilingualGeneration a skos:Concept;
  rdfs:label "Multilingual generation"@en;
  skos:broader :NaturalLanguageGeneration;
  skos:definition "Multilingual generation is the verbalization of a non-linguistic semantic representation in different human languages. The language of choice is usually a parameter to a multilingual generation system. A typical instance of multilingual generation is found in interlingual machine translation, when multiple target languages are involved. Other instances include report generation systems for multiple languages (such as Temsis-Gen) and grammar-based realizers (such as FUF/SURGE)."@en,
    "The task/process of generating content in multiple languages"@en;
  skos:inScheme :OperationScheme;
  skos:prefLabel "Multilingual generation"@en .

:Text a skos:Concept;
  :hasFileExtension "txt";
  :hasMimetype :text_plain;
  rdfs:label "text/plain"@en;
  skos:altLabel "plain text"@en;
  skos:broader :DocumentFormat;
  skos:definition "Default value for the format of textual files; a textual file should be human-readable and must not contain binary data"@en;
  skos:inScheme :DataFormatScheme;
  skos:prefLabel "text/plain"@en .

:OperationScheme a skos:ConceptScheme;
  rdfs:label "Operation Taxonomy"@en;
  skos:hasTopConcept :Operation;
  skos:prefLabel "Operation Taxonomy"@en .

:Conll2009 a skos:Concept;
  :documentationUrl "https://dkpro.github.io/dkpro-core/releases/1.8.0/docs/format-reference.html#format-Conll2009";
  :hasMimetype :text_x_org_dkpro_conll2009;
  rdfs:label "CoNLL-2009"@en;
  skos:broader :ConllFormat;
  skos:definition "The CoNLL 2009 format targets semantic role labeling. Columns are tab-separated. Sentences are separated by a blank new line."@en;
  skos:inScheme :DataFormatScheme;
  skos:prefLabel "CoNLL-2009"@en .

:DiscourseRelation a skos:Concept;
  rdfs:label "Discourse relation"@en;
  skos:broader :DiscourseAnnotationType;
  skos:definition "The relation that holds between two segments of discourse; e.g. causal, temporal etc."@en;
  skos:inScheme :AnnotationTypeScheme;
  skos:prefLabel "Discourse relation"@en .

:WikipediaLink a skos:Concept;
  :documentationUrl "https://dkpro.github.io/dkpro-core/releases/1.8.0/docs/format-reference.html#format-WikipediaLink";
  rdfs:label "Wikipedia link"@en;
  skos:broader :WikipediaFormat;
  skos:definition "Format for wikipedia links"@en;
  skos:inScheme :DataFormatScheme;
  skos:prefLabel "Wikipedia link"@en .

:NamedEntityDisambiguation a skos:Concept;
  rdfs:label "Named Entity Disambiguation"@en;
  skos:altLabel "NED"@en;
  skos:broader :NamedEntityRecognition;
  skos:definition "The task/process of selecting among candidate entities from a knowledge base (or other information resource) the ones to which the named entities in a text refer to"@en;
  skos:inScheme :OperationScheme;
  skos:prefLabel "Named Entity Disambiguation"@en .

:Transcription1 a skos:Concept;
  rdfs:label "Transcription"@en;
  skos:broader :SpeechAnnotationType;
  skos:inScheme :AnnotationTypeScheme;
  skos:narrower :OrthographicTranscription1, :PhoneticTranscription1;
  skos:prefLabel "Transcription"@en .

:SpeakerDiarization a skos:Concept;
  rdfs:label "Speaker diarization"@en;
  skos:altLabel "Speaker diarisation"@en-uk;
  skos:broader :SpeechAnnotation;
  skos:definition "Partitioning of audio stream into homogeneous segments according to speaker properties and acoustic conditions"@en;
  skos:inScheme :OperationScheme;
  skos:prefLabel "Speaker diarization"@en .

:Lemma a skos:Concept;
  :documentationUrl "http://dkpro.github.io/dkpro-core/releases/1.8.0/docs/typesystem-reference.html#de.tudarmstadt.ukp.dkpro.core.api.segmentation.type.Lemma";
  rdfs:label "Lemma"@en;
  skos:broader :MorphologicalAnnotationType;
  skos:definition "The canonical or citation form used for referring to a word and its inflected forms"@en;
  skos:inScheme :AnnotationTypeScheme;
  skos:prefLabel "Lemma"@en .

:NegraExport a skos:Concept;
  :documentationUrl "http://www.coli.uni-saarland.de/~thorsten/publications/Brants-CLAUS98.pdf";
  :hasMimetype :application_x_org_dkpro_negra3, :application_x_org_dkpro_negra4;
  rdfs:label "NeGra export"@en;
  skos:broader :AnnotationFormat;
  skos:definition "Export format for annotated corpora in the NeGra project"@en;
  skos:inScheme :DataFormatScheme;
  skos:prefLabel "NeGra export"@en .

:EnsembleMethod a skos:Concept;
  dc:source "adapted from Wikipedia (https://en.wikipedia.org/wiki/Ensemble_learning)"@en;
  rdfs:label "Ensemble Method"@en;
  skos:broader :MachineAndStatisticalLearningMethod;
  skos:definition "Any method that uses multiple learning algorithms in an attempt to improve predictive performance not obtainable otherwise with any of the constituent learning algorithms."@en;
  skos:inScheme :TdmMethodScheme;
  skos:prefLabel "Ensemble Method"@en .

:MultiWordUnit a skos:Concept;
  rdfs:label "Multi-word unit"@en;
  skos:broader :StructuralAnnotationType;
  skos:definition "A combination of words that are considered as forming one semantic unit"@en;
  skos:inScheme :AnnotationTypeScheme;
  skos:prefLabel "Multi-word unit"@en .

:KernelMethod a skos:Concept;
  dc:source "adapted from wikipedia (https://en.wikipedia.org/wiki/Kernel_method)"@en;
  rdfs:label "Kernel Method"@en;
  skos:broader :MachineAndStatisticalLearningMethod;
  skos:definition "Any method used in pattern analysis that relies on kernel functions, which enable it to operate in a high-dimensional, implicit feature space without ever computing the coordinates of the data in that space, but rather by simply computing the inner products between the images of all pairs of data in the feature space."@en;
  skos:inScheme :TdmMethodScheme;
  skos:prefLabel "Kernel Method"@en .

:Brat a skos:Concept;
  :documentationUrl "http://brat.nlplab.org/standoff.html", "https://dkpro.github.io/dkpro-core/releases/1.8.0/docs/format-reference.html#format-de.tudarmstadt.ukp.dkpro.core.io.brat-asl";
  :hasMimetype :text_x_brat;
  rdfs:label "BRAT"@en;
  skos:broader :AnnotationFormat;
  skos:definition "BRAT stand-off format for annotations (BRAT is a online environment for collaborative text annotation, cf. http://brat.nlplab.org/)"@en;
  skos:inScheme :DataFormatScheme;
  skos:prefLabel "BRAT"@en .

:MachineTranslation a skos:Concept;
  rdfs:label "Machine Translation"@en;
  skos:altLabel "Automated Translation"@en, "Automatic Translation"@en, "Computer Translation"@en,
    "MT"@en;
  skos:broader :Translation;
  skos:definition "Machine Translation (MT) is the fully automatic translation from one human language into another one. Machine translation has been worked on since the 1950s. There are a number of commercial products available and in daily use, but there are still open research problems. Tranfer-based MT has a set of transfer rules for each language pair, so that n*(n-1) rule sets are necessary for MT between n languages. In contract, interlingua-based MT uses a language-independent representation into which all source languages are analysed and from which all target languages is generated. Most practically usable MT systems are tranfser-based. Recently, there have been interestinv developments in statistical MT algorithms which are trained on parallel corpora of translated texts, and are very useful for constructing MT systems for new language pairs."@en,
    "The automatic translation of a text from one language into another performed by software without human involvement"@en;
  skos:inScheme :OperationScheme;
  skos:prefLabel "Machine Translation"@en .

:Coreference a skos:Concept;
  rdfs:label "Coreference"@en;
  owl:equivalentClass <http://vocab.lappsgrid.org/Coreference>;
  skos:altLabel "Co-reference"@en;
  skos:broader :DiscourseAnnotationType;
  skos:definition "Coreference is the reference in one expression to the same referent in another expression. [http://www.glossary.sil.org/term/coreference]"@en;
  skos:editorialNote "As defined here it refers more to the phenomenon than the actual annotation types; referent and co-referent might be more appropriate"@en;
  skos:inScheme :AnnotationTypeScheme;
  skos:narrower :EntityMentionPair;
  skos:prefLabel "Coreference"@en .

:ONNX a skos:Concept;
  :documentationUrl "https://onnx.ai/";
  rdfs:label "ONNX"@en;
  skos:altLabel "Open Neural Network Exchange"@en;
  skos:broader :MLModelFormat;
  skos:definition "Open format built to represent machine learning models"@en;
  skos:inScheme :DataFormatScheme;
  skos:prefLabel "ONNX"@en .

:AnnotationOfDerivationalFeatures a skos:Concept;
  rdfs:label "Annotation of derivational features"@en;
  skos:broader :MorphologicalAnnotation;
  skos:definition "The task/process of adding annotations relevant to the derivational level of analysis (e.g. recognizing derivational affixes, tagging their meaning etc.)"@en;
  skos:inScheme :OperationScheme;
  skos:prefLabel "Annotation of derivational features"@en .

:ExtractionOfQuantitativeInformation a skos:Concept;
  rdfs:label "Extraction of quantitative information"@en;
  skos:broader :InformationExtraction;
  skos:definition "The task of computing and extracting quantitative properties (e.g. of strings, words, etc.)"@en;
  skos:inScheme :OperationScheme;
  skos:prefLabel "Extraction of quantitative information"@en .

:Xpath a skos:Concept;
  :documentationUrl "https://www.w3.org/TR/xpath/", "https://zoidberg.ukp.informatik.tu-darmstadt.de/jenkins/job/DKPro%20Core%20Documentation%20(GitHub)/de.tudarmstadt.ukp.dkpro.core$de.tudarmstadt.ukp.dkpro.core.doc-asl/doclinks/5/format-reference.html#format-XmlXPath";
  :hasMimetype :application_xml;
  rdfs:label "XPath"@en;
  skos:broader :Xml;
  skos:definition "XPath is a language for addressing parts of an XML document, designed to be used by both XSLT and XPointer."@en;
  skos:inScheme :DataFormatScheme;
  skos:prefLabel "XPath"@en .

:image_gif a skos:Concept;
  rdfs:label "image/gif";
  skos:broader :Mimetype;
  skos:inScheme :MimeTypeScheme .

:AnnotationOfQuestionTopics a skos:Concept;
  rdfs:label "Annotation of question topics"@en;
  skos:altLabel "Annotation of question topical targets"@en;
  skos:broader :SemanticAnnotation;
  skos:definition "The task/process of attaching tags to the segment of a question that functions as the topic of that question"@en;
  skos:inScheme :OperationScheme;
  skos:prefLabel "Annotation of question topics"@en .

:MsPowerpoint a skos:Concept;
  :hasMimetype :application_vnd_ms_powerpoint;
  rdfs:label "MS-Powerpoint"@en;
  skos:broader :DocumentFormat;
  skos:definition "Data format for Microsoft Powerpoint files";
  skos:inScheme :DataFormatScheme;
  skos:prefLabel "MS-Powerpoint"@en .

:Topic a skos:Concept;
  rdfs:label "Topic"@en;
  skos:broader :SemanticAnnotationType;
  skos:definition "The subject of a text or conversation, what it is about"@en;
  skos:inScheme :AnnotationTypeScheme;
  skos:prefLabel "Topic"@en .

:StructuralAnnotation skos:inScheme :ModelFunctionScheme .

:Zip a skos:Concept;
  rdfs:label "zip"@en .

:DeepLearning a skos:Concept;
  dc:source "adapted from wikipedia (https://en.wikipedia.org/wiki/Deep_learning)"@en;
  rdfs:label "Deep Learning"@en;
  skos:broader :MachineAndStatisticalLearningMethod;
  skos:definition "A branch of machine learning based on deep neural networks. A deep neural network (DNN) is an artificial neural network (ANN) with multiple hidden layers of units between the input and output layers."@en;
  skos:inScheme :TdmMethodScheme;
  skos:prefLabel "Deep Learning"@en .

:OpenOfficePresentation a skos:Concept;
  :hasMimetype :application_vnd_openxmlformats_officedocument_presentationml_presentation;
  rdfs:label "Open office presentation"@en;
  skos:broader :DocumentFormat, :OpenFormat, :Xml;
  skos:inScheme :DataFormatScheme .

:DataToTextGeneration skos:inScheme :ModelFunctionScheme .

:text_x_eaf_xml a skos:Concept;
  rdfs:label "text/x-eaf+xml";
  skos:broader :Mimetype;
  skos:inScheme :MimeTypeScheme .

:HistoricalEvent a skos:Concept;
  rdfs:label "Historical event"@en;
  skos:broader :NamedEntity, :SocialSciencesEntity;
  skos:inScheme :AnnotationTypeScheme;
  skos:prefLabel "Historical event"@en .

:ConstituencyParser a skos:Concept;
  :performsOperation :ConstituencyParsing;
  rdfs:label "Constituency parser"@en;
  skos:broader :Parser;
  skos:definition "A component that builds a constituency tree from typically token and part-of-speech annotations"@en;
  skos:inScheme :ComponentTypeScheme;
  skos:prefLabel "Constituency parser"@en .

:LanguageIdentification a skos:Concept;
  rdfs:label "Language identification"@en;
  skos:altLabel "Automatic Language Identification"@en, "Language recognition"@en;
  skos:broader :InformationExtraction;
  skos:definition "Automatic Language Identification (LID) is the process of identifying the natural language of a sample of speech or written text by an unknown speaker. Several important applications exist for LID, viz., as a front-end to, e.g., a call router in a telephone-based application or a multi-lingual speech recognition system."@en,
    "The task/process of guessing what natural language a text or text segment is written in"@en;
  skos:inScheme :OperationScheme;
  skos:prefLabel "Language identification"@en .

:StatisticalLearningMethod a skos:Concept;
  dc:source "\"R: Statistical learning primer\", https://www.pressreader.com/australia/linux-format/20161025/283626759591113"@en;
  rdfs:label "Statistical Learning Method"@en;
  skos:broader :TdmMethod;
  skos:definition "The process of using statistics and techniques related to statistics in order to understand and learn from your data so that you can predict its future."@en;
  skos:inScheme :TdmMethodScheme;
  skos:prefLabel "Statistical Learning Method"@en .

:GazeteerBasedMatching a skos:Concept;
  rdfs:label "Gazeteer based matching"@en;
  skos:altLabel "Gazeteer-based matching"@en;
  skos:broader :Matching;
  skos:definition "The task/process of performing a comparison between a text/dataset and a gazeteer and identifying in the text/dataset units that are included in the gazeteer"@en;
  skos:inScheme :OperationScheme;
  skos:prefLabel "Gazeteer based matching"@en .

:EmotionGeneration a skos:Concept;
  rdfs:label "Emotion generation"@en;
  skos:broader :OperationWithMultimediaInputOrOutput;
  skos:inScheme :OperationScheme;
  skos:prefLabel "Emotion generation"@en .

:DocumentImageAnalysis skos:broader :SupportOperation .

:WikipediaRevisionPair a skos:Concept;
  :documentationUrl "https://dkpro.github.io/dkpro-core/releases/1.8.0/docs/format-reference.html#format-WikipediaRevisionPair";
  rdfs:label "Wikipedia revision pair"@en;
  skos:broader :WikipediaFormat;
  skos:definition "Pairs of adjacent revisions of all articles"@en;
  skos:inScheme :DataFormatScheme;
  skos:prefLabel "Wikipedia revision pair"@en .

:Matching a skos:Concept;
  rdfs:label "Matching"@en;
  skos:broader :SupportOperation;
  skos:definition "The task/performance of identifying similar elements in two resources"@en;
  skos:inScheme :OperationScheme;
  skos:narrower :GazeteerBasedMatching;
  skos:prefLabel "Matching"@en .

:tiff a skos:Concept;
  :hasFileExtension "tif", "tiff";
  :hasMimetype :image_tiff;
  rdfs:label "TIFF"@en;
  skos:altLabel "Tagged Image File Format"@en;
  skos:broader :ImageFormat;
  skos:inScheme :DataFormatScheme;
  skos:prefLabel "TIFF"@en .

:PhysicoChemicalProperty a skos:Concept;
  rdfs:label "Physico-chemical property"@en;
  skos:broader :AgriculturalEntity;
  skos:definition "Physical and chemical property of substances"@en;
  skos:inScheme :AnnotationTypeScheme;
  skos:prefLabel "Physico-chemical property"@en .

:Conjugation a skos:Concept;
  rdfs:label "Conjugation"@en;
  skos:broader :NaturalLanguageGeneration;
  skos:definition "The act of generating (listing in a prescribed order) the various inflectional forms of a word"@en;
  skos:inScheme :OperationScheme;
  skos:prefLabel "Conjugation"@en .

:OasisPresentation a skos:Concept;
  :hasMimetype :application_vnd_oasis_opendocument_presentation;
  rdfs:label "Oasis Presentation"@en;
  skos:broader :DocumentFormat, :OpenFormat;
  skos:inScheme :DataFormatScheme;
  skos:prefLabel "Oasis Presentation"@en .

:application_vnd_xmi_xml a skos:Concept;
  rdfs:label "application/vnd.xmi+xml";
  skos:broader :Mimetype;
  skos:inScheme :MimeTypeScheme .

:Editing a skos:Concept;
  rdfs:label "Editing"@en;
  skos:broader :SupportOperation;
  skos:definition "The task/process of changing the contents of a resource"@en;
  skos:inScheme :OperationScheme;
  skos:prefLabel "Editing"@en .

:application_x_org_dkpro_negra3 skos:broader :Mimetype .

:AnnotationOfDocumentStructure a skos:Concept;
  rdfs:label "Annotation of document structure"@en;
  skos:broader :StructuralAnnotation;
  skos:definition "The task/process of annotating the internal structure of a document (e.g. book chapters, sections in a journal article, title, preface, images/figures etc.)"@en;
  skos:inScheme :OperationScheme;
  skos:prefLabel "Annotation of document structure"@en .

:ExtractionOfFundingInformation a skos:Concept;
  rdfs:label "Extraction of funding information"@en;
  skos:altLabel "Mining of funding information"@en;
  skos:broader :ExtractionOfDomainSpecificInformation;
  skos:definition "The task/process of detecting in a text and extracting information relevant to funding (e.g. funding programme, award, funder etc.)"@en;
  skos:inScheme :OperationScheme;
  skos:prefLabel "Extraction of funding information"@en .

:DataCollection a skos:Concept;
  dc:source <https://en.wikipedia.org/wiki/Data_collection>;
  rdfs:label "Data collection"@en;
  skos:broader :SupportOperation;
  skos:definition "The process of gathering and measuring information on targeted variables in an established systematic fashion, which then enables one to answer relevant questions and evaluate outcomes."@en;
  skos:inScheme :OperationScheme;
  skos:narrower :Crawling;
  skos:prefLabel "Data collection"@en .

:TemporalExpression skos:inScheme :AnnotationTypeScheme .

:mp4 a skos:Concept;
  :hasFileExtension "mp4";
  :hasMimetype :video_mp4;
  rdfs:label "MPEG-4"@en;
  skos:altLabel "MP4"@en;
  skos:broader :VideoFormat;
  skos:inScheme :DataFormatScheme;
  skos:prefLabel "MPEG-4"@en .

:SentimentAnalysis a skos:Concept;
  rdfs:label "Sentiment analysis"@en;
  skos:altLabel "Opinion extraction"@en, "Opinion mining"@en, "Polarity detection"@en,
    "Sentiment detection"@en;
  skos:broader :InformationExtraction;
  skos:definition "The process/task of computationally identifying and categorizing opinions expressed in a piece of text, especially in order to determine whether the writer's attitude towards a particular topic, product, etc. is positive, negative, or neutral"@en;
  skos:inScheme :OperationScheme;
  skos:prefLabel "Sentiment analysis"@en .

:DiscourseModelling a skos:Concept;
  rdfs:label "Discourse modelling"@en;
  skos:altLabel "Discourse modeling [en-US]"@en-us;
  skos:broader :DiscourseAnnotation;
  skos:definition "Discourse modelling describes all aspects of the relations between groups of sentences in monologue (text), dialogue, or multiparty interactions, e.g. text coherence, rhetorical relations, intentional and attentional state, centering, dialogue moves, dialogue acts, argument structures and reference phenomena, to name just a few. Recently, with the growing interest in multimodal discourse processing, discourse models extend their reach beyond the modality speech/language to other modalities like gesture, gaze or haptics, and cover also cross-modal phenomena."@en,
    "The task/process of building discourse models"@en;
  skos:inScheme :OperationScheme;
  skos:prefLabel "Discourse modelling"@en .

:Bayesian a skos:Concept;
  dc:source "adapted from Wikipedia (https://en.wikipedia.org/wiki/Bayesian_inference)"@en;
  rdfs:label "Bayesian"@en;
  skos:broader :MachineAndStatisticalLearningMethod;
  skos:definition "A method in probability and statistics based on Bayes' theorem, mainly related to statistical inference."@en;
  skos:inScheme :TdmMethodScheme;
  skos:prefLabel "Bayesian"@en .

:Pseudonymization a skos:Concept;
  rdfs:label "Pseudonymization"@en;
  skos:broader :SupportOperation;
  skos:definition "The processing of personal data in such a way that the data can no longer be attributed to a specific data subject without the use of additional information (from GDPR)"@en;
  skos:inScheme :OperationScheme;
  skos:prefLabel "Pseudonymization"@en .

:TFSavedModel a skos:Concept;
  :documentationUrl "https://www.tensorflow.org/guide/saved_model";
  rdfs:label "TensorFlow SavedModel"@en;
  skos:broader :MLModelFormat;
  skos:inScheme :DataFormatScheme .

:application_x_org_dkpro_graf_xml skos:broader :Mimetype .

:text_x_brat skos:broader :Mimetype;
  skos:inScheme :MimeTypeScheme .

:DataMerger a skos:Concept;
  :performsOperation :DataMerging;
  rdfs:label "Data merger"@en;
  skos:broader :SupportComponent;
  skos:definition "A component that supports data merging from various sources"@en;
  skos:inScheme :ComponentTypeScheme;
  skos:prefLabel "Data merger"@en .

:application_tika a skos:Concept;
  rdfs:label "application/tika";
  skos:broader :Mimetype;
  skos:inScheme :MimeTypeScheme .

:TextCompression a skos:Concept;
  rdfs:label "Text compression"@en;
  skos:definition "Methods for text compression identify and exploit redundancy in text documents in order to obtain a more condensed representation of the information, from which the original data can be recovered without modification (lossless compression). In theory, there is a close relation between compression and prediction: The better a statistical language model can estimate the probability of a word, given some context, the more the text as a whole can be compressed."@en;
  skos:inScheme :OperationScheme;
  skos:prefLabel "Text compression"@en .

:GrammarChecking a skos:Concept .

:Latex a skos:Concept;
  :documentationUrl "https://www.latex-project.org/about/";
  :hasMimetype :application_xLatex;
  rdfs:label "LATEX"@en;
  skos:broader :DocumentFormat;
  skos:definition "Data format for documents using LaTeX (a high-quality typesetting system very popular for scientific documents)"@en;
  skos:inScheme :DataFormatScheme;
  skos:prefLabel "LATEX"@en .

:LexicalSubstitution a skos:Concept;
  rdfs:label "Lexical substitution"@en;
  skos:broader :NaturalLanguageGeneration;
  skos:definition "The task of identifying a substitute for a word in the context of a clause [from Wikipedia]"@en;
  skos:inScheme :OperationScheme;
  skos:prefLabel "Lexical substitution"@en;
  skos:related :Paraphrasing .

:text_x_org_dkpro_ngram a skos:Concept;
  rdfs:label "text/x.org.dkpro.ngram";
  skos:broader :Mimetype;
  skos:inScheme :MimeTypeScheme .

:application_vnd_oasis_opendocument_spreadsheet a skos:Concept;
  rdfs:label "application/vnd.oasis.opendocument.spreadsheet";
  skos:broader :Mimetype;
  skos:inScheme :MimeTypeScheme .

:Citation a skos:Concept;
  rdfs:label "Citation"@en;
  skos:broader :ScholarlyAnalyticsEntity;
  skos:definition "Reference to a book, paper, or author, especially in a scholarly work."@en;
  skos:inScheme :AnnotationTypeScheme;
  skos:prefLabel "Citation"@en .

:AnnotationOfTextualEntailment skos:inScheme :ModelFunctionScheme .

:Protein a skos:Concept;
  rdfs:label "Protein"@en;
  skos:broader :BiologicalEnity, :NamedEntity;
  skos:definition "Any of various naturally occurring extremely complex substances that consist of amino-acid residues joined by peptide bonds, contain the elements carbon, hydrogen, nitrogen, oxygen, usually sulfur, and occasionally other elements (such as phosphorus or iron), and include many essential biological compounds (such as enzymes, hormones, or antibodies) [https://www.merriam-webster.com/dictionary/protein]"@en;
  skos:inScheme :AnnotationTypeScheme;
  skos:prefLabel "Protein"@en .

:AnaphoraResolution a skos:Concept;
  rdfs:label "Anaphora resolution"@en;
  skos:broader :LinguisticAnalysis;
  skos:definition "The process/task of identifying all linguistic expressions that appear in a certain text or across texts and refer to the same entity"@en;
  skos:inScheme :OperationScheme;
  skos:prefLabel "Anaphora resolution"@en;
  skos:related :CoReferenceResolution .

:DependencyParsing a skos:Concept;
  dc:source "adapted from https://nlp.stanford.edu/software/nndep.shtml"@en;
  rdfs:label "Dependency parsing"@en;
  skos:broader :Parsing;
  skos:definition "The task/process of identifying and marking the grammatical structure of a sentence, establishing relationships between \"\"head\"\" words and words that modify those heads"@en;
  skos:inScheme :OperationScheme;
  skos:prefLabel "Dependency parsing"@en .

:BotDetection a skos:Concept;
  rdfs:label "Bot detection"@en;
  skos:broader :InformationExtraction;
  skos:definition "The task/process of identifying segments of text or speech discourse that have been uttered by bots"@en;
  skos:inScheme :OperationScheme;
  skos:prefLabel "Bot detection"@en .

:Jdbc a skos:Concept;
  :documentationUrl "https://zoidberg.ukp.informatik.tu-darmstadt.de/jenkins/job/DKPro%20Core%20Documentation%20(GitHub)/de.tudarmstadt.ukp.dkpro.core$de.tudarmstadt.ukp.dkpro.core.doc-asl/doclinks/5/format-reference.html#format-Jdbc";
  rdfs:label "JDBC"@en;
  skos:altLabel "JAVA Database Connectivity"@en;
  skos:broader :DatabaseFormat;
  skos:definition "For JDBC databases"@en;
  skos:inScheme :DataFormatScheme;
  skos:prefLabel "JDBC"@en .

:Miscellaneous a skos:Concept;
  rdfs:label "Miscellaneous"@en;
  skos:altLabel "MISC"@en;
  skos:broader :NamedEntity;
  skos:definition "A general label for named entities other than the usual ones recognized by a system"@en;
  skos:inScheme :AnnotationTypeScheme;
  skos:prefLabel "Miscellaneous"@en .

:application_zip a skos:Concept;
  rdfs:label "application/zip";
  skos:broader :Mimetype;
  skos:inScheme :MimeTypeScheme .

:SpellChecking a skos:Concept;
  rdfs:label "Spell checking"@en;
  skos:altLabel "Spelling correction"@en;
  skos:broader :AuthoringSupport;
  skos:definition "Techniques for the identification of spelling or typing errors in textual documents, which may be applied interactively during the creation of the document, or off-line for existing documents. Spelling correction is an extension in which for each assumed error one or several hypothetical corrections are suggested."@en,
    "The task/process of checking the accuracy of spelling of a word (and usually correcting it) according to the accepted form"@en;
  skos:inScheme :OperationScheme;
  skos:prefLabel "Spell checking"@en .

:video_mp4 a skos:Concept;
  rdfs:label "video/mp4";
  skos:broader :Mimetype;
  skos:inScheme :MimeTypeScheme .

:application_x_org_dkpro_tiger_xml a skos:Concept;
  rdfs:label "application/x.org.dkpro.tiger+xml";
  skos:broader :Mimetype;
  skos:inScheme :MimeTypeScheme .

:Chunker a skos:Concept;
  rdfs:label "Chunker"@en;
  skos:broader :Annotator;
  skos:definition "A component that groups tokens of a text into chunks"@en;
  skos:inScheme :ComponentTypeScheme;
  skos:prefLabel "Chunker"@en .

:text_x_org_dkpro_reuters21578 a skos:Concept;
  rdfs:label "text/x.org.dkpro.reuters21578";
  skos:broader :Mimetype;
  skos:inScheme :MimeTypeScheme .

:WikipediaArticleInfo a skos:Concept;
  :documentationUrl "https://dkpro.github.io/dkpro-core/releases/1.8.0/docs/format-reference.html#format-WikipediaArticleInfo";
  rdfs:label "Wikipedia article info"@en;
  skos:broader :WikipediaFormat;
  skos:definition "Format of general article infos"@en;
  skos:inScheme :DataFormatScheme;
  skos:prefLabel "Wikipedia article info"@en .

:image_tiff a skos:Concept;
  rdfs:label "image/tiff";
  skos:broader :Mimetype;
  skos:inScheme :MimeTypeScheme .

:AnaphoraAnnotation a skos:Concept;
  rdfs:label "Anaphora annotation"@en;
  skos:broader :DiscourseAnnotation;
  skos:definition "The process/task of marking all linguistic expressions that appear in a certain text or across texts as referring to the same entity and linking it to this entity"@en;
  skos:inScheme :OperationScheme;
  skos:prefLabel "Anaphora annotation"@en;
  skos:related :CoReferenceAnnotation .

:ContradictionDetection a skos:Concept;
  rdfs:label "Contradiction detection"@en;
  skos:broader :InformationExtraction;
  skos:definition "The task/process of identifying conflicting statements (contradictions) in a dataset"@en;
  skos:inScheme :OperationScheme;
  skos:prefLabel "Contradiction detection"@en .

:Synapse a skos:Concept;
  rdfs:label "Synapse"@en;
  skos:broader :BiologicalEnity, :NamedEntity;
  skos:definition "A specialized structure or junction that allows cell to cell communication [http://www.biology-online.org/dictionary/Synapse]"@en;
  skos:inScheme :AnnotationTypeScheme;
  skos:prefLabel "Synapse"@en .

:SpeechAnalytics a skos:Concept;
  rdfs:label "Speech analytics"@en;
  skos:broader :TextSpeechDataAnalytics;
  skos:inScheme :OperationScheme;
  skos:prefLabel "Speech analytics"@en .

:application_xXces_xml a skos:Concept;
  skos:inScheme :MimeTypeScheme .

:text_x_org_dkpro_conll2012 rdfs:label "text/x.org.dkpro.conll-2012" .

:WordSegmentation a skos:Concept;
  rdfs:label "Word segmentation"@en;
  skos:broader :MorphologicalAnnotation;
  skos:definition "The task/process of segmenting (cutting) a word into root and affixes"@en;
  skos:inScheme :OperationScheme;
  skos:prefLabel "Word segmentation"@en .

:audio_wav a skos:Concept;
  rdfs:label "audio/wav";
  skos:broader :Mimetype;
  skos:inScheme :MimeTypeScheme .

:SyllableSegmentation a skos:Concept;
  rdfs:label "Syllable segmentation"@en;
  skos:broader :MorphologicalAnnotation;
  skos:definition "Segmentation of a word into syllables"@en;
  skos:inScheme :OperationScheme;
  skos:prefLabel "Syllable segmentation"@en .

:SpeechAnnotation a skos:Concept;
  rdfs:label "Speech annotation"@en;
  skos:broader :Annotation;
  skos:inScheme :OperationScheme;
  skos:narrower :AnnotationOfSpeakerTurns, :AudioSegmentation, :ParalanguageAnnotation,
    :ProsodicAnnotation, :SoundEventAnnotation, :SoundToTextAlignment, :SpeakerDiarization;
  skos:prefLabel "Speech annotation"@en .

:Zip skos:inScheme :DataFormatScheme .

:Search skos:broader :SupportOperation;
  skos:definition "The act of looking for a unit of text in a dataset"@en;
  skos:inScheme :OperationScheme;
  skos:prefLabel "Search"@en .

:SupportOperation skos:narrower :Search .

:InformationExtractionAndInformationRetrievalCollection skos:member :Search .

:Stemmer a skos:Concept;
  :performsOperation :Stemming;
  rdfs:label "Stemmer"@en;
  skos:broader :Annotator;
  skos:definition "A component that extracts stems from words in a text, usually by removing the most common morphological and inflectional endings from words"@en;
  skos:inScheme :ComponentTypeScheme;
  skos:prefLabel "Stemmer"@en .

:Concordancing rdfs:label "Concordancing"@en;
  skos:broader :Reading;
  skos:definition "The automatic generation of concordances, i.e. formatted displays of all the occurrences of a particular types in a corpus"@en;
  skos:inScheme :OperationScheme;
  skos:prefLabel "Concordancing"@en .

:SupportOperationCollection skos:member :Concordancing .

:SemanticReasoning a skos:Concept;
  rdfs:label "Semantic reasoning"@en;
  skos:broader :InformationExtraction;
  skos:definition "The inferrence of logical consequences from a set of asserted facts or axioms [from wikipedia]"@en;
  skos:inScheme :OperationScheme;
  skos:prefLabel "Semantic reasoning"@en .

:DocumentAnnotationType a skos:Concept;
  rdfs:label "Document annotation type"@en;
  owl:equivalentClass <http://vocab.lappsgrid.org/Document>;
  skos:altLabel "Document information"@en, "Document metadata"@en;
  skos:broader :AnnotationType;
  skos:definition "Any kind of annotation that is used to describe a document (e.g. identifier, size, location, language etc.)"@en;
  skos:inScheme :AnnotationTypeScheme;
  skos:prefLabel "Document annotation type"@en .

:text_html a skos:Concept;
  rdfs:label "text/html";
  skos:broader :Mimetype;
  skos:inScheme :MimeTypeScheme .

:Dependency a skos:Concept;
  :documentationUrl "http://dkpro.github.io/dkpro-core/releases/1.8.0/docs/typesystem-reference.html#de.tudarmstadt.ukp.dkpro.core.api.syntax.type.dependency.Dependency";
  rdfs:label "Dependency"@en;
  owl:equivalentClass <http://vocab.lappsgrid.org/Dependency>;
  skos:broader :SyntacticAnnotationType;
  skos:definition "A type of syntactic relation that holds between linguistic units, where we try to recognise the head (governor) and its dependents"@en;
  skos:inScheme :AnnotationTypeScheme;
  skos:prefLabel "Dependency"@en .

:application_rtf a skos:Concept;
  rdfs:label "application/rtf";
  skos:broader :Mimetype;
  skos:inScheme :MimeTypeScheme .

:ANNIS a skos:Concept;
  :documentationUrl "http://korpling.github.io/ANNIS/3.6/user-guide/import-and-config-convert.html";
  rdfs:label "ANNIS"@en;
  skos:altLabel "relANNIS"@en;
  skos:broader :AnnotationFormat, :DatabaseFormat;
  skos:definition "Relational database format used in the ANNIS architecture (https://corpus-tools.org/annis/)"@en;
  skos:inScheme :DataFormatScheme;
  skos:prefLabel "ANNIS"@en .

:MultimodalIntegration a skos:Concept;
  rdfs:label "Multimodal integration"@en;
  skos:altLabel "Modality integration"@en, "Multisensory integration"@en;
  skos:broader :OperationWithMultimediaInputOrOutput;
  skos:definition "Multimodal fusion combines the output of speech understanding, gestures and mimic recognition (if available) to an uniform representation of the user intention."@en,
    "The study of how information from the different sensory modalities, such as sight, sound, touch, smell, self-motion and taste, may be integrated by the nervous system. [from Wikipedia]"@en;
  skos:inScheme :OperationScheme;
  skos:prefLabel "Multimodal integration"@en .

:LanguageIdentifier skos:prefLabel "Language identifier"@en .

:ProsodicAnnotation a skos:Concept;
  rdfs:label "Prosodic annotation"@en;
  skos:broader :SpeechAnnotation;
  skos:inScheme :OperationScheme;
  skos:narrower :ProsodicSegmentation;
  skos:prefLabel "Prosodic annotation"@en .

:ComputerAidedTranslation a skos:Concept;
  rdfs:label "Computer-aided translation"@en;
  skos:altLabel "CAT"@en, "Computer-assisted translation"@en, "MAHT"@en, "Machine-aided human translation"@en;
  skos:definition "A form of translation performed by a human translator with the aid of software programmes"@en,
    "Techniques that help to increase the productivity of human translators via suitable computational infrastructure, including translation memories, terminology management, partial machine translation, online lexicons, or other techniques that automate parts of the translator's work, such as speech recognition or accelerated typing techniques applied to human translations."@en;
  skos:inScheme :OperationScheme;
  skos:prefLabel "Computer-aided translation"@en .

:FillMask a skos:Concept .

:SemanticClass a skos:Concept;
  :documentationUrl "http://dkpro.github.io/dkpro-core/releases/1.8.0/docs/typesystem-reference.html#de.tudarmstadt.ukp.dkpro.core.api.semantics.type.SemanticField";
  rdfs:label "Semantic class"@en;
  skos:altLabel "Semantic type"@en;
  skos:broader :SemanticAnnotationType;
  skos:definition "A division of words into classes based on their common semantic features"@en;
  skos:inScheme :AnnotationTypeScheme;
  skos:prefLabel "Semantic class"@en .

:Stemming a skos:Concept;
  rdfs:label "Stemming"@en;
  skos:broader :TextAnnotation;
  skos:definition "The task/process of cutting off the ends of words (mainly inflectional affixes but sometimes also derivational affixes) aiming to relate words to a base form."@en;
  skos:inScheme :OperationScheme;
  skos:prefLabel "Stemming"@en;
  skos:related :Lemmatization .

:Subjectivity a skos:Concept;
  rdfs:label "Subjectivity"@en;
  skos:broader :SemanticAnnotationType;
  skos:definition "The linguistic expression of somebody’s opinions, sentiments, emotions, evaluations, beliefs, speculations (private states, i.e. states that are not open to objective observation or verification). [http://www.mavir.net/docs/JWiebe-Subjectivity-nov2010.pdf]"@en;
  skos:inScheme :AnnotationTypeScheme;
  skos:prefLabel "Subjectivity"@en .

:DerivationalFeature a skos:Concept;
  rdfs:label "Derivational feature"@en;
  skos:broader :MorphologicalAnnotationType;
  skos:definition "Any feature relevant to the derivation process of a word (e.g. marking affixes, their meaning etc.)"@en;
  skos:inScheme :AnnotationTypeScheme;
  skos:prefLabel "Derivational feature"@en .

:Geo-politicalEntity a skos:Concept;
  rdfs:label "Geo-political entity"@en;
  skos:altLabel "GPE"@en;
  skos:broader :NamedEntity;
  skos:definition "A geographical area associated with some sort of political structure"@en;
  skos:inScheme :AnnotationTypeScheme;
  skos:prefLabel "Geo-political entity"@en .

:LexiconAcquisitionFromCorpora a skos:Concept;
  rdfs:label "Lexicon acquisition from corpora"@en;
  skos:broader :KnowledgeAcquisition, :SupportOperationForKnowledgeResources;
  skos:definition "The task/process of constructing lexical resources from corpora"@en;
  skos:inScheme :OperationScheme;
  skos:prefLabel "Lexicon acquisition from corpora"@en .

:LexiconEnhancement a skos:Concept;
  rdfs:label "Lexicon enhancement"@en;
  skos:broader :KnowledgeAcquisition, :SupportOperationForKnowledgeResources;
  skos:definition "The task/process of improving (e.g. increasing the size of entries, improving the information, adding new types of information, etc.) a lexicon"@en;
  skos:inScheme :OperationScheme;
  skos:prefLabel "Lexicon enhancement"@en .

:FlowController a skos:Concept;
  :performsOperation :FlowControl;
  rdfs:label "Flow controller"@en;
  skos:broader :SupportComponent;
  skos:definition "A component that supports controlling flows"@en;
  skos:inScheme :ComponentTypeScheme;
  skos:prefLabel "Flow controller"@en .

:audio_wave a skos:Concept;
  rdfs:label "audio/wave";
  skos:broader :Mimetype;
  skos:inScheme :MimeTypeScheme .

:MsExcel a skos:Concept;
  :hasMimetype :application_vnd_msExcel;
  rdfs:label "MS-Excel"@en;
  skos:broader :AnnotationFormat, :DocumentFormat, :TabularFormat;
  skos:definition "Data format for Microsoft Excel documents"@en;
  skos:inScheme :DataFormatScheme;
  skos:prefLabel "MS-Excel"@en .

:Tuepp a skos:Concept;
  :documentationUrl "http://dkpro.github.io/dkpro-core/releases/1.8.0/docs/format-reference.html#format-de.tudarmstadt.ukp.dkpro.core.io.tuepp-asl",
    "https://zoidberg.ukp.informatik.tu-darmstadt.de/jenkins/job/DKPro%20Core%20Documentation%20(GitHub)/de.tudarmstadt.ukp.dkpro.core$de.tudarmstadt.ukp.dkpro.core.doc-asl/doclinks/5/format-reference.html#format-Tuepp";
  :hasMimetype :application_x_org_dkpro_tuepp_xml;
  rdfs:label "Tuepp"@en;
  skos:broader :AnnotationFormat, :CorpusFormat, :Xml;
  skos:definition "Format of the Tübingen Partially Parsed Corpus of Written German (TüPP-D/Z) XML files; TüPP D/Z (http://www.sfs.uni-tuebingen.de/de/ascl/ressourcen/corpora/tuepp-dz.html) is a collection of articles from the German newspaper taz (die tageszeitung) annotated and encoded in a XML format."@en;
  skos:inScheme :DataFormatScheme;
  skos:prefLabel "Tuepp"@en .

:ImageClassification a skos:Concept;
  rdfs:label "Image classification"@en;
  skos:broader :OperationWithMultimediaInputOrOutput;
  skos:inScheme :OperationScheme;
  skos:prefLabel "Image classification"@en .

:HandwritingRecognition skos:broader :SupportOperation .

:SemanticFrame a skos:Concept;
  dc:source <https://framenet.icsi.berkeley.edu/fndrupal/glossary>;
  :documentationUrl "http://dkpro.github.io/dkpro-core/releases/1.8.0/docs/typesystem-reference.html#de.tudarmstadt.ukp.dkpro.core.api.semantics.type.SemanticPredicate";
  rdfs:label "Semantic frame"@en;
  owl:equivalentClass <http://purl.org/olia/olia-top.owl#Frame>;
  skos:altLabel "Frame"@en;
  skos:broader :SemanticAnnotationType;
  skos:definition "A schematic representation of a situation involving various participants, props and other conceptual roles, each of which is a frame element"@en;
  skos:inScheme :AnnotationTypeScheme;
  skos:prefLabel "Semantic frame"@en .

:RumoursStanceClassification a skos:Concept;
  rdfs:label "Rumours stance classification"@en;
  skos:broader :InformationExtraction;
  skos:definition "The task of identifying the attitude of a person towards the truthfulness of a rumour"@en;
  skos:inScheme :OperationScheme;
  skos:prefLabel "Rumours stance classification"@en .

:MsWord a skos:Concept;
  :hasFileExtension "doc";
  :hasMimetype :application_msword;
  rdfs:label "MS-Word"@en;
  skos:broader :DocumentFormat;
  skos:definition "Data format for Microsoft Word documents"@en;
  skos:inScheme :DataFormatScheme;
  skos:prefLabel "MS-Word"@en .

:BLAST a skos:Concept;
  :documentationUrl "https://cl.lingfil.uu.se/~sara/blast/README";
  :hasFileExtension "blast";
  rdfs:label "BLAST"@en;
  skos:broader :AnnotationFormat;
  skos:inScheme :DataFormatScheme;
  skos:prefLabel "BLAST"@en .

:WikipediaArticle a skos:Concept;
  :documentationUrl "https://zoidberg.ukp.informatik.tu-darmstadt.de/jenkins/job/DKPro%20Core%20Documentation%20(GitHub)/de.tudarmstadt.ukp.dkpro.core$de.tudarmstadt.ukp.dkpro.core.doc-asl/doclinks/5/format-reference.html#format-WikipediaArticle";
  rdfs:label "Wikipedia article"@en;
  skos:broader :WikipediaFormat;
  skos:definition "Format for wikipedia articles"@en;
  skos:inScheme :DataFormatScheme;
  skos:prefLabel "Wikipedia article"@en .

:application_x_json_twitter a skos:Concept;
  rdfs:label "application/x-json-twitter";
  skos:broader :Mimetype;
  skos:inScheme :MimeTypeScheme .

:DeepParserPerformanceEvaluation a skos:Concept;
  rdfs:label "Deep parser performance evaluation"@en;
  skos:broader :Evaluation;
  skos:definition "The task of parser evaluation is to measure the speed and accuracy of parsers with respect to a manually parsed test corpus. In the evaluation of so-called deep parsers, which are based on comprehensive linguistic theories, the assignment of the correct semantic analysis plays an important role. Another aspect is the handling and reduction of ambiguities, which is important not only from the linguistic point of view but because it plays a major role in the time and memory requirements of deep parsers. Test data can either be a treebank constructed from naturally occurring data, such as the \"\"Wall Street Corpus\"\", or a \"\"test suite\"\" containing constructed examples which cover all interesting linguistic phenomena. An important issue in deep parser evaluation is the comparison of parsers and grammars based on different linguistic theories."@en,
    "The task/process of measuring the speed and accuracy of deep parsers with respect to a manually parsed test corpus."@en;
  skos:inScheme :OperationScheme;
  skos:prefLabel "Deep parser performance evaluation"@en .

:image_jpeg skos:inScheme :MimeTypeScheme .

:Sentence a skos:Concept;
  :documentationUrl "http://dkpro.github.io/dkpro-core/releases/1.8.0/docs/typesystem-reference.html#de.tudarmstadt.ukp.dkpro.core.api.segmentation.type.Sentence";
  rdfs:label "Sentence"@en;
  owl:equivalentClass <http://purl.org/olia/olia-top.owl#Sentence>;
  skos:broader :StructuralAnnotationType;
  skos:definition "A group of words, usually containing a verb, that expresses a thought in the form of a statement, question, instruction, or exclamation and starts with a capital letter when written [https://dictionary.cambridge.org/dictionary/english/sentence]"@en;
  skos:inScheme :AnnotationTypeScheme;
  skos:prefLabel "Sentence"@en .

:Chemical a skos:Concept;
  rdfs:label "Chemical"@en;
  skos:broader :BiologicalEnity, :NamedEntity;
  skos:definition "Any substance (as an acid) that is formed when two or more other substances act upon one another or that is used to produce a change in another substance [https://www.merriam-webster.com/dictionary/chemical]"@en;
  skos:inScheme :AnnotationTypeScheme;
  skos:prefLabel "Chemical"@en .

:DocumentComparison a skos:Concept;
  rdfs:label "Document comparison"@en;
  skos:broader :SupportOperation;
  skos:definition "The task/process of comparing different versions of the same document"@en;
  skos:inScheme :OperationScheme;
  skos:prefLabel "Document comparison"@en .

:SignLanguageGeneration a skos:Concept;
  rdfs:label "Sign language generation"@en;
  skos:broader :NaturalLanguageGeneration, :OperationWithMultimediaInputOrOutput;
  skos:definition "The task/process of generating videos in sign language"@en;
  skos:inScheme :OperationScheme;
  skos:prefLabel "Sign language generation"@en .

:LanguageIdentifier a skos:Concept .

:Visualiser a skos:Concept;
  :performsOperation :Visualization;
  rdfs:label "Visualiser"@en;
  skos:broader :SupportComponent;
  skos:definition "A component or interface that renders the contents of a resource in a graphic way for visualisation purposes"@en;
  skos:inScheme :ComponentTypeScheme;
  skos:prefLabel "Visualiser"@en .

:CertaintyLevelLabelling a skos:Concept;
  rdfs:label "Certainty level labelling"@en;
  skos:altLabel "Certainty level labeling [en-US]"@en-us;
  skos:broader :SemanticAnnotation;
  skos:definition "The task/process of adding to statements in a text annotations that indicate the level of certainty of the author vis-a-vis the statement"@en;
  skos:inScheme :OperationScheme;
  skos:prefLabel "Certainty level labelling"@en .

:application_x_kaf_json a skos:Concept;
  rdfs:label "application/x-kaf+json";
  skos:broader :Mimetype;
  skos:inScheme :MimeTypeScheme .

:Sentiment a skos:Concept;
  :documentationUrl "http://dkpro.github.io/dkpro-core/releases/1.8.0/docs/typesystem-reference.html#de.tudarmstadt.ukp.dkpro.core.sentiment.type.StanfordSentimentAnnotation";
  rdfs:label "Sentiment"@en;
  skos:altLabel "Opinion"@en;
  skos:broader :SemanticAnnotationType;
  skos:definition "The affective state (judgement, feeling) of a person or group towards an entity or event"@en;
  skos:inScheme :AnnotationTypeScheme;
  skos:prefLabel "Sentiment"@en .

:OpenOfficeDocument a skos:Concept;
  :hasMimetype :application_vnd_openxmlformats_officedocument_wordprocessingml_document;
  rdfs:label "Open office document"@en;
  skos:broader :DocumentFormat, :OpenFormat, :Xml;
  skos:inScheme :DataFormatScheme;
  skos:prefLabel "Open office document"@en .

:OntologyEnhancement a skos:Concept;
  rdfs:label "Ontology enhancement"@en;
  skos:broader :KnowledgeAcquisition;
  skos:definition "The task/process of improving an ontology, typically by adding new relations or entities"@en;
  skos:inScheme :OperationScheme;
  skos:prefLabel "Ontology enhancement"@en .

:LanguageTechnology a skos:Concept;
  rdfs:label "Language Technology"@en;
  skos:altLabel "HLT"@en, "Human Language Technology"@en, "LT"@en;
  skos:broader :Operation;
  skos:definition "Language technology, often called human language technology, studies methods of how computer programs or electronic devices can analyze, produce, modify or respond to human texts and speech. It consists of natural language processing and computational linguistics on the one hand, and speech technology on the other. [Wikipedia]"@en;
  skos:inScheme :OperationScheme;
  skos:prefLabel "Language Technology"@en .

:LinkedDataFormat a skos:Concept;
  rdfs:label "Linked data format"@en;
  skos:broader :DataFormat;
  skos:definition "Formats used for linked data"@en;
  skos:inScheme :DataFormatScheme;
  skos:narrower :LD_json;
  skos:prefLabel "Linked data format"@en .

:ArtificialNeuralNetwork a skos:Concept;
  dc:source "adapted from wikipedia (https://en.wikipedia.org/wiki/Artificial_neural_network)"@en;
  rdfs:label "Artificial Neural Network"@en;
  skos:broader :MachineAndStatisticalLearningMethod;
  skos:definition "A computational model based on a large collection of simple neural units (artificial neurons), loosely analogous to the observed behavior of a biological brain's axons. These systems are self-learning and trained, rather than explicitly programmed."@en;
  skos:inScheme :TdmMethodScheme;
  skos:prefLabel "Artificial Neural Network"@en .

:application_x_org_dkpro_tgrep2 a skos:Concept;
  rdfs:label "application/x.org.dkpro.tgrep2";
  skos:broader :Mimetype;
  skos:inScheme :MimeTypeScheme .

:DependencyConverter a skos:Concept;
  :performsOperation :DependencyConversion;
  rdfs:label "Dependency converter"@en;
  skos:broader :Converter;
  skos:definition "A component that converts a constituency tree into a dependency tree"@en;
  skos:inScheme :ComponentTypeScheme;
  skos:prefLabel "Dependency converter"@en .

:MsAccessDatabase a skos:Concept;
  :hasFileExtension "mdb";
  :hasMimetype :application_vnd_msaccess, :application_xMsaccess;
  rdfs:label "MS-Access database"@en;
  skos:broader :DatabaseFormat;
  skos:definition "Data format for Microsoft Access database"@en;
  skos:inScheme :DataFormatScheme;
  skos:prefLabel "MS-Access database"@en .

:application_xhtml_xml a skos:Concept;
  rdfs:label "application/xhtml+xml";
  skos:broader :Mimetype;
  skos:inScheme :MimeTypeScheme .

:application_xTmx_xml a skos:Concept;
  rdfs:label "application/x-tmx+xml";
  skos:broader :Mimetype;
  skos:inScheme :MimeTypeScheme .

:ModelOrganism_species a skos:Concept;
  rdfs:label "Model organism/species"@en;
  skos:broader :BiologicalEnity, :NamedEntity;
  skos:inScheme :AnnotationTypeScheme;
  skos:prefLabel "Model organism/species"@en .

:SemanticSearch a skos:Concept;
  rdfs:label "Semantic search"@en;
  skos:broader :InformationRetrieval;
  skos:definition "A type of search that seeks to improve search accuracy by understanding the searcher's intent and the contextual meaning of terms as they appear in the searchable dataspace, whether on the Web or within a closed system, to generate more relevant results."@en;
  skos:inScheme :OperationScheme;
  skos:prefLabel "Semantic search"@en .

:Neuron a skos:Concept;
  rdfs:label "Neuron"@en;
  skos:broader :BiologicalEnity, :NamedEntity;
  skos:definition "A nerve cell that carries information between the brain and other parts of the body"@en;
  skos:inScheme :AnnotationTypeScheme;
  skos:prefLabel "Neuron"@en .

:text_tcf_xml a skos:Concept;
  rdfs:label "text/tcf+xml";
  skos:broader :Mimetype;
  skos:inScheme :MimeTypeScheme .

:NeuroscienceEntity a skos:Concept;
  rdfs:label "Neuroscience entity"@en;
  skos:broader :DomainSpecificAnnotationType;
  skos:definition "Any kind of annotation pertaining to entities of neuroscience"@en;
  skos:inScheme :AnnotationTypeScheme;
  skos:prefLabel "Neuroscience entity"@en .

:text_csv a skos:Concept .

:FakeNewsDetection a skos:Concept;
  rdfs:label "Fake news detection"@en;
  skos:altLabel "Fake news assessment"@en, "Fake news evaluation"@en;
  skos:broader :InformationExtraction;
  skos:definition "The process of detecting whether a certain news item is fake (i.e. a type of news items of yellow journalism or propaganda that consists of deliberate disinformation or hoaxes spread via traditional news media or online social media) [adapted from wikipedia]"@en;
  skos:inScheme :OperationScheme;
  skos:prefLabel "Fake news detection"@en .

:KeywordExtractor a skos:Concept;
  :performsOperation :KeywordExtraction;
  rdfs:label "Keyword extractor"@en;
  skos:broader :Analyzer;
  skos:definition "A component that tries to extract keywords from a given text"@en;
  skos:inScheme :ComponentTypeScheme;
  skos:prefLabel "Keyword extractor"@en .

:CoReferenceResolution a skos:Concept;
  rdfs:label "Co-reference resolution"@en;
  skos:altLabel "Coreference resolution"@en;
  skos:broader :LinguisticAnalysis;
  skos:definition "The process/task of determining all linguistic expressions that refer to the same entity in a certain text or across texts."@en,
    "The process/task of identifying all linguistic expressions that appear in a certain text or across texts and refer to the same unique entity in the world"@en;
  skos:inScheme :OperationScheme;
  skos:narrower :IntraDocumentCoReferenceResolution;
  skos:prefLabel "Co-reference resolution"@en;
  skos:related :AnaphoraResolution .

:LexiconExtractorFromLexica a skos:Concept;
  :performsOperation :LexiconExtractionFromLexica;
  rdfs:label "Lexicon extractor from lexica"@en;
  skos:broader :Analyzer;
  skos:definition "A component that extracts specific lexical information contained in other lexica"@en;
  skos:inScheme :ComponentTypeScheme;
  skos:prefLabel "Lexicon extractor from lexica"@en .

:WARC a skos:Concept;
  :documentationUrl "http://archive-access.sourceforge.net/warc/", "https://en.wikipedia.org/wiki/Web_ARChive";
  rdfs:label "Web ARChive format"@en;
  skos:broader :CorpusFormat;
  skos:inScheme :DataFormatScheme;
  skos:prefLabel "Web ARChive format"@en .

:TerminologyManagement a skos:Concept;
  rdfs:label "Terminology management"@en;
  skos:broader :SupportOperation;
  skos:inScheme :OperationScheme;
  skos:prefLabel "Terminology management"@en .

:TranslationMemoryManagement a skos:Concept;
  rdfs:label "Translation memory management"@en;
  skos:broader :SupportOperation;
  skos:inScheme :OperationScheme;
  skos:prefLabel "Translation memory management"@en .

:SentenceAlignment skos:prefLabel "Sentence alignment"@en .

:WordSenseDisambiguator a skos:Concept;
  :performsOperation :WordSenseDisambiguation;
  rdfs:label "Word sense disambiguator"@en;
  skos:broader :Disambiguator;
  skos:definition "A component that tries to identify which sense of a word (i.e. meaning) is used in a sentence, when the word has multiple meanings"@en;
  skos:editorialNote "could also be an annotator and a support component (used in a lot of processes)"@en;
  skos:inScheme :ComponentTypeScheme;
  skos:prefLabel "Word sense disambiguator"@en .

:LexicalSimplification a skos:Concept;
  rdfs:label "Lexical simplification"@en;
  skos:broader :NaturalLanguageGeneration;
  skos:definition "The task of replacing individual words of a text with words that are easier to understand, so that the text as a whole becomes easier to comprehend, e.g. by people with learning disabilities or by children who learn to read [from https://link.springer.com/chapter/10.1007/978-3-642-28601-8_36]"@en;
  skos:inScheme :OperationScheme;
  skos:prefLabel "Lexical simplification"@en;
  skos:related :LexicalSubstitution .

:PreOrPostProcessor a skos:Concept;
  rdfs:label "Pre- or Post-Processor"@en;
  skos:broader :ComponentType;
  skos:definition "A component that is used at pre- or post-processing stages in order to normalize input/output"@en;
  skos:inScheme :ComponentTypeScheme;
  skos:narrower :Filter, :GrammarChecker, :Normalizer, :SpellingChecker;
  skos:prefLabel "Pre- or Post-Processor"@en .

:Summarizer a skos:Concept;
  :performsOperation :Summarization;
  rdfs:label "Summarizer"@en;
  skos:broader :Generator;
  skos:definition "A component that produces a natural language synopsis of a longer text"@en;
  skos:inScheme :ComponentTypeScheme;
  skos:prefLabel "Summarizer"@en .

:application_json a skos:Concept;
  rdfs:label "application/json";
  skos:broader :Mimetype;
  skos:inScheme :MimeTypeScheme .

:PolarityLabelling a skos:Concept;
  rdfs:label "Polarity labelling"@en;
  skos:broader :SemanticAnnotation;
  skos:definition "The task/process of adding to units of a text (especially in sentiment-intensive texts) tags that indicate polarity (negative, positive, neutral, mixed)"@en;
  skos:inScheme :OperationScheme;
  skos:prefLabel "Polarity labelling"@en .

:Chunking a skos:Concept;
  rdfs:label "Chunking"@en;
  skos:altLabel "Light parsing"@en, "Shallow Parsing"@en;
  skos:broader :Parsing;
  skos:definition "Shallow parsing refers to a class of techniques for identifying phrasal chunks in texts without assigning deep hierarchical structures. Cascaded finite-state models are often used for shallow parsing. Shallow parsing techniques are used because they are more time-efficient and more error-tolerant than \"\"deep\"\" parsers, and give rise to fewer ambiguities."@en,
    "The task/process of dividing a sentence into chunks (non-overlapping text segments consisting of a head and preceding function words and/or modifiers)"@en;
  skos:inScheme :OperationScheme;
  skos:narrower :NounPhraseChunking;
  skos:prefLabel "Chunking"@en .

:Crawling a skos:Concept;
  rdfs:label "Web crawling"@en;
  skos:altLabel "Crawling"@en, "Web Crawling and Spidering"@en;
  skos:broader :DataCollection;
  skos:definition "", "The use of bots that crawl the web (crawlers) in order to spot content that matches user-set criteria and download them to create large datasets"@en;
  skos:inScheme :OperationScheme;
  skos:prefLabel "Web crawling"@en .

:Processor a skos:Concept;
  rdfs:label "Processor"@en;
  skos:broader :ComponentType;
  skos:definition "A component that is used in processing operations"@en;
  skos:inScheme :ComponentTypeScheme;
  skos:narrower :Annotator, :Generator;
  skos:prefLabel "Processor"@en .

:FaceVerification a skos:Concept;
  rdfs:label "Face verification"@en;
  skos:altLabel "Face authentication"@en;
  skos:broader :OperationWithMultimediaInputOrOutput;
  skos:definition "The task/process of validating a claimed identity based on the image of a face, and either accepting or rejecting the identity claim [adapted from http://www.idiap.ch/~marcel/labs/faceverif.php]"@en;
  skos:inScheme :OperationScheme;
  skos:prefLabel "Face verification"@en .

:audio_x_wav rdfs:label "audio/x-wav" .

:FacialExpression a skos:Concept;
  rdfs:label "Facial expression"@en;
  skos:broader :ModalityAnnotationType;
  skos:inScheme :AnnotationTypeScheme;
  skos:prefLabel "Facial expression"@en .

:HumourDetection a skos:Concept;
  rdfs:label "Humour detection"@en;
  skos:altLabel "Humor detection"@en-us, "Humor recognition"@en-us, "Humor sensing"@en-us,
    "Humour recognition"@en, "Humour sensing"@en;
  skos:broader :InformationExtraction;
  skos:definition "The task of identifying in a text structures and phrases of humour"@en-us;
  skos:inScheme :OperationScheme;
  skos:prefLabel "Humour detection"@en .

:SpatialRoleLabelling a skos:Concept;
  rdfs:label "Spatial role labelling"@en;
  skos:altLabel "Spatial role labeling"@en-us;
  skos:broader :SemanticAnnotation;
  skos:definition "Τhe task of identifying and classifying the spatial arguments of the spatial expressions mentioned in a sentence"@en;
  skos:inScheme :OperationScheme;
  skos:prefLabel "Spatial role labelling"@en .

:audio_mpa a skos:Concept;
  rdfs:label "audio/MPA";
  skos:broader :Mimetype;
  skos:inScheme :MimeTypeScheme .

:IonicChannel a skos:Concept;
  rdfs:label "Ionic channel"@en;
  skos:altLabel "Ion channel"@en;
  skos:broader :BiologicalEnity, :NamedEntity;
  skos:definition "A single protein or protein complex that traverses the lipid bilayer of cell membrane and form a channel to facilitate the movement of ions through the membrane according to their electrochemical gradient [http://www.biology-online.org/dictionary/Ion_channel]"@en;
  skos:inScheme :AnnotationTypeScheme;
  skos:prefLabel "Ionic channel"@en .

:SyntacticStructureGeneration a skos:Concept;
  rdfs:label "Syntactic Structure Generation"@en;
  skos:broader :NaturalLanguageGeneration;
  skos:definition "";
  skos:inScheme :OperationScheme;
  skos:prefLabel "Syntactic Structure Generation"@en .

:GateXml a skos:Concept;
  :hasMimetype :application_xml;
  rdfs:label "GATE XML"@en;
  skos:broader :GateFormat, :Xml;
  skos:definition "XML-based format for GATE components"@en;
  skos:inScheme :DataFormatScheme;
  skos:prefLabel "GATE XML"@en .

:WordAlignment a skos:Concept;
  rdfs:label "Word alignment"@en;
  skos:broader :Alignment;
  skos:definition "Alignment at word level"@en;
  skos:inScheme :OperationScheme;
  skos:prefLabel "Word alignment"@en .

:CorpusViewing a skos:Concept;
  rdfs:label "Corpus viewing"@en;
  skos:broader :Viewing;
  skos:definition "The task/process of viewing the contents of a corpus as performed by human beings"@en;
  skos:inScheme :OperationScheme;
  skos:prefLabel "Corpus viewing"@en .

:JsonL a skos:Concept;
  :documentationUrl "https://jsonlines.org/";
  rdfs:label "JSON Lines"@en;
  skos:altLabel "JSONL"@en;
  skos:broader :Json;
  skos:inScheme :DataFormatScheme;
  skos:prefLabel "JSON Lines"@en .

:ResourceAccess a skos:Concept;
  rdfs:label "Resource access"@en;
  skos:broader :SupportOperation;
  skos:definition "Any operation that enables accessing a resource"@en;
  skos:inScheme :OperationScheme;
  skos:narrower :Reading, :Writing;
  skos:prefLabel "Resource access"@en .

:Cadixe_json a skos:Concept;
  :documentationUrl "https://builds.openminted.eu/job/WP%205.2%20-%20Typesystem%20alignment/eu.openminted.interop$mapping-conversion/doclinks/1/components.html#ExportCadixeJSON";
  :hasMimetype :application_json;
  rdfs:label "Cadixe/JSON"@en;
  skos:broader :AnnotationFormat, :Json;
  skos:definition "AlvisAE protocol format"@en;
  skos:inScheme :DataFormatScheme;
  skos:prefLabel "Cadixe/JSON"@en .

:FormatConversion a skos:Concept;
  rdfs:label "Format conversion"@en;
  skos:altLabel "Data conversion"@en, "File conversion"@en;
  skos:broader :SupportOperation;
  skos:definition "The task/process of converting (changing) the format of a resource into another (e.g. PDF to TXT or XML)"@en;
  skos:inScheme :OperationScheme;
  skos:narrower :DependencyConversion, :LexiconFormatConversion;
  skos:prefLabel "Format conversion"@en .

:hasMimetype rdfs:domain _:node1fu4q14cjx26 .

_:node1fu4q14cjx26 a owl:Class;
  owl:intersectionOf _:node1fu4q14cjx27 .

_:node1fu4q14cjx27 a rdf:List;
  rdf:first skos:Concept;
  rdf:rest _:node1fu4q14cjx28 .

_:node1fu4q14cjx28 a rdf:List;
  rdf:first _:node1fu4q14cjx25 .

_:node1fu4q14cjx25 a owl:Restriction;
  owl:hasValue :DataFormatScheme .

_:node1fu4q14cjx28 rdf:rest rdf:nil .

:TrainingOfMachineLearningModels a skos:Concept;
  dc:source "adapted from http://docs.aws.amazon.com/machine-learning/latest/dg/training-ml-models.html";
  rdfs:label "Training of Machine Learning models"@en;
  skos:broader :LanguageModelling;
  skos:definition "The task/process of creating Machine Learning (ML) models by providing a ML algorithm with training data that help the algorithm discover patterns in data, and construct the appropriate models using these discoveries"@en;
  skos:inScheme :OperationScheme;
  skos:prefLabel "Training of Machine Learning models"@en .

:OrthographicTranscription1 a skos:Concept;
  rdfs:label "Orthographic transcription"@en;
  skos:broader :Transcription1;
  skos:inScheme :AnnotationTypeScheme;
  skos:prefLabel "Orthographic transcription"@en .

:Compound a skos:Concept;
  :documentationUrl "http://dkpro.github.io/dkpro-core/releases/1.8.0/docs/typesystem-reference.html#de.tudarmstadt.ukp.dkpro.core.api.segmentation.type.Compound";
  rdfs:label "Compound"@en;
  skos:broader :MorphologicalAnnotationType;
  skos:definition "A single word composed of two or more free morphemes"@en;
  skos:inScheme :AnnotationTypeScheme;
  skos:prefLabel "Compound"@en .

:DependencyTree a skos:Concept;
  rdfs:label "Dependency tree"@en;
  skos:broader :SyntacticAnnotationType;
  skos:definition "A tree that represents the dependency relations in a sentence, i.e. showing the governor (head) and its dependents with directed links"@en;
  skos:inScheme :AnnotationTypeScheme;
  skos:prefLabel "Dependency tree"@en .

:Csv a skos:Concept;
  :hasMimetype :text_csv;
  rdfs:label "CSV"@en;
  skos:altLabel "Comma-separated values"@en;
  skos:broader :TabularFormat;
  skos:definition "Data format with comma-separated values"@en;
  skos:inScheme :DataFormatScheme;
  skos:prefLabel "CSV"@en .

:SoundToTextAlignment a skos:Concept;
  rdfs:label "Sound-to-Text alignment"@en;
  skos:broader :SpeechAnnotation;
  skos:inScheme :OperationScheme;
  skos:prefLabel "Sound-to-Text alignment"@en .

:SpeechToSpeechTranslation a skos:Concept;
  rdfs:label "Speech-to-Speech translation"@en;
  skos:broader :Translation;
  skos:definition "The process by which spoken utterances in one language are automatically translated and spoken aloud in another language"@en;
  skos:inScheme :OperationScheme;
  skos:prefLabel "Speech-to-Speech translation"@en .

:Zip skos:broader :PackageFormat .

:SubcategorizationFrame a skos:Concept;
  rdfs:label "Subcategorization frame"@en;
  skos:altLabel "Argument structure"@en, "Subcategorisation frame"@en;
  skos:broader :SyntacticAnnotationType;
  skos:definition "The number and types of syntactic arguments required by a certain lexical item (mainly verbs, but also nouns and adjectives)"@en;
  skos:inScheme :AnnotationTypeScheme;
  skos:prefLabel "Subcategorization frame"@en .

:WikipediaDiscussion a skos:Concept;
  :documentationUrl "https://dkpro.github.io/dkpro-core/releases/1.8.0/docs/format-reference.html#format-WikipediaDiscussion";
  rdfs:label "Wikipedia discussion"@en;
  skos:broader :WikipediaFormat;
  skos:definition "Format for wikipedia discussion pages"@en;
  skos:inScheme :DataFormatScheme;
  skos:prefLabel "Wikipedia discussion"@en .

:text_x_org_dkpro_ptbChunked a skos:Concept;
  rdfs:label "text/x.org.dkpro.ptb-chunked";
  skos:broader :Mimetype;
  skos:inScheme :MimeTypeScheme .

:application_x_org_dkpro_tuepp_xml a skos:Concept;
  rdfs:label "application/x.org.dkpro.tuepp+xml";
  skos:broader :Mimetype;
  skos:inScheme :MimeTypeScheme .

:Xhtml a skos:Concept;
  :documentationUrl "https://www.w3.org/TR/xhtml1/";
  :hasFileExtension "html";
  :hasMimetype :application_xhtml_xml;
  rdfs:label "XHTML"@en;
  skos:broader :DocumentFormat, :Xml;
  skos:definition "Data format for XHTML (Extensible HyperText Markup Language)"@en;
  skos:inScheme :DataFormatScheme;
  skos:prefLabel "XHTML"@en .

:MorphologicalFeature a skos:Concept;
  :documentationUrl "http://dkpro.github.io/dkpro-core/releases/1.8.0/docs/typesystem-reference.html#de.tudarmstadt.ukp.dkpro.core.api.lexmorph.type.morph.MorphologicalFeatures";
  rdfs:label "Morphological feature"@en;
  owl:equivalentClass <http://purl.org/olia/olia-top.owl#MorphosyntacticFeature>;
  skos:altLabel "Grammatical category"@en, "Grammatical feature"@en, "Morphosyntactic feature"@en;
  skos:broader :MorphologicalAnnotationType;
  skos:definition "Property of a word that is expressed in its inflected form; examples include person, tense, gender, case etc."@en;
  skos:inScheme :AnnotationTypeScheme;
  skos:prefLabel "Morphological feature"@en .

:WordSense a skos:Concept;
  :documentationUrl "http://dkpro.github.io/dkpro-core/releases/1.8.0/docs/typesystem-reference.html#de.tudarmstadt.ukp.dkpro.core.api.semantics.type.WordSense";
  rdfs:label "Word sense"@en;
  skos:broader :SemanticAnnotationType;
  skos:definition "Corresponds to the structural part of a lexical entry that contains the relevant semantic, grammatical, and anthropological information for a lexical unit. [adapted from http://www.glossary.sil.org/term/sense]"@en;
  skos:inScheme :AnnotationTypeScheme;
  skos:prefLabel "Word sense"@en .

:TextualEntailment a skos:Concept;
  rdfs:label "Textual entailment"@en;
  skos:altLabel "Entailment"@en;
  skos:broader :SemanticAnnotationType;
  skos:inScheme :AnnotationTypeScheme;
  skos:prefLabel "Textual entailment"@en .

:BionlpFormat a skos:Concept;
  dct:replaces :BionlpFormats;
  rdfs:label "BioNLP format"@en;
  skos:broader :DocumentFormat;
  skos:definition "Formats used  for BioNLP shared tasks"@en;
  skos:inScheme :DataFormatScheme;
  skos:narrower :Bionlp, :BionlpSt2013A1_a2, :Json_genia;
  skos:prefLabel "BioNLP format"@en .

:CoReferenceAnnotator a skos:Concept;
  rdfs:label "Co-reference annotator"@en;
  skos:broader :Annotator;
  skos:definition "A component that annotates tokens of a text with coreference labels, marking expressions that refer to the same entity in the text"@en;
  skos:inScheme :ComponentTypeScheme;
  skos:prefLabel "Co-reference annotator"@en .

:BinaryCas a skos:Concept;
  :documentationUrl "https://dkpro.github.io/dkpro-core/releases/1.8.0/docs/format-reference.html#format-de.tudarmstadt.ukp.dkpro.core.io.bincas-asl";
  :hasMimetype :application_x_org_dkpro_uima_binary;
  rdfs:label "Binary CAS"@en;
  skos:altLabel "UIMA Binary CAS"@en;
  skos:broader :UimaCasFormat;
  skos:definition "Binary format used for CAS data"@en;
  skos:inScheme :DataFormatScheme;
  skos:prefLabel "Binary CAS"@en .

:Funding a skos:Concept;
  rdfs:label "Funding"@en;
  skos:broader :ScholarlyAnalyticsEntity;
  skos:definition "Annotation related to the funding of a resource (e.g. funder, funding project, etc.)"@en;
  skos:inScheme :AnnotationTypeScheme;
  skos:prefLabel "Funding"@en .

:AnnotationOfNumbers skos:inScheme :ModelFunctionScheme .

:TextAnalysis a skos:Concept;
  rdfs:label "Text analysis"@en;
  skos:broader :InformationExtraction;
  skos:inScheme :OperationScheme;
  skos:prefLabel "Text analysis"@en .

:Keyword a skos:Concept;
  rdfs:label "Keyword"@en;
  skos:broader :ScholarlyAnalyticsEntity, :SemanticAnnotationType;
  skos:definition "A word or group of words used to describe or index the contents of a document"@en;
  skos:inScheme :AnnotationTypeScheme;
  skos:prefLabel "Keyword"@en .

:AudioSegmentation skos:inScheme :ModelFunctionScheme .

:Avro_json a skos:Concept;
  :documentationUrl "https://avro.apache.org/docs/1.8.1/spec.html";
  rdfs:label "Avro"@en;
  skos:broader :Json;
  skos:inScheme :DataFormatScheme;
  skos:prefLabel "Avro"@en .

:application_pls_xml a skos:Concept;
  rdfs:label "application/pls+xml";
  skos:broader :Mimetype;
  skos:inScheme :MimeTypeScheme .

:SpeechAnalysis a skos:Concept;
  rdfs:label "Speech analysis"@en;
  skos:broader :SpeechRecognition;
  skos:inScheme :OperationScheme;
  skos:prefLabel "Speech analysis"@en .

:L2WritingSupport a skos:Concept;
  rdfs:label "L2 writing support"@en;
  skos:altLabel "L2 writing assistant"@en;
  skos:broader :AuthoringSupport;
  skos:inScheme :OperationScheme;
  skos:prefLabel "L2 writing support"@en .

:BuildingOfFiniteStateAutomata a skos:Concept;
  rdfs:label "Building of finite state automata"@en;
  skos:broader :SupportOperation;
  skos:definition "The task/process of creating Finite State Automata (a mathematical model of computation)"@en;
  skos:inScheme :OperationScheme;
  skos:prefLabel "Building of finite state automata"@en;
  skos:related :FiniteStateTechnology .

:OfficialText a skos:Concept .

:Xces a skos:Concept;
  :hasMimetype :application_xXces_xml;
  rdfs:label "XCES"@en;
  skos:broader :AnnotationFormat, :Xml;
  skos:definition "Data format for documents and corpora using the XCES standard (Corpus Encoding Standard for XML), cf. http://www.xces.org/"@en;
  skos:inScheme :DataFormatScheme;
  skos:narrower :XcesIlspVariant;
  skos:prefLabel "XCES"@en .

:application_x-SDL-TM a skos:Concept;
  rdfs:label "application/x-SDL-TM";
  skos:broader :Mimetype;
  skos:inScheme :MimeTypeScheme .

:Editor a skos:Concept;
  :performsOperation :Editing;
  rdfs:label "Editor"@en;
  skos:broader :SupportComponent;
  skos:definition "A component that allows humans to edit the contents of a resource"@en;
  skos:inScheme :ComponentTypeScheme;
  skos:prefLabel "Editor"@en .

:video_avi a skos:Concept;
  rdfs:label "video/x-msvideo";
  skos:broader :Mimetype;
  skos:inScheme :MimeTypeScheme .

:FrequencyCount a skos:Concept;
  rdfs:label "Frequency count"@en;
  skos:altLabel "Computation of frequencies"@en;
  skos:broader :FeatureExtraction;
  skos:definition "The task of counting frequencies of entities (e.g. words, strings, sentences, specific tags, etc.)"@en;
  skos:inScheme :OperationScheme;
  skos:prefLabel "Frequency count"@en .

:SpeechAct a skos:Concept;
  rdfs:label "Speech act"@en;
  skos:broader :DiscourseAnnotationType;
  skos:definition "A speech act is an act that a speaker performs when making an utterance, including the following: (a) A general act (illocutionary act) that a speaker performs, analyzable as including: the uttering of words (utterance acts), making reference and predicating (propositional acts), and a particular intention in making the utterance (illocutionary force). (b) An act involved in the illocutionary act, including utterance acts and propositional acts, (c) The production of a particular effect in the addressee (perlocutionary act) [http://www.glossary.sil.org/term/speech-act]"@en;
  skos:inScheme :AnnotationTypeScheme;
  skos:narrower :DialogueAct;
  skos:prefLabel "Speech act"@en .

:TemporalExpressionRecognition a skos:Concept;
  rdfs:label "Temporal expressions recognition"@en;
  skos:broader :InformationExtraction;
  skos:definition "The task/process of identifying temporal expressions (also called timex) in a text in order to extract temporal information"@en;
  skos:inScheme :OperationScheme;
  skos:prefLabel "Temporal expressions recognition"@en .

:GeneFamily a skos:Concept;
  rdfs:label "Gene family"@en;
  skos:broader :AgriculturalEntity;
  skos:definition "A gene family is a set of several similar genes, formed by duplication of a single original gene, and generally with similar biochemical functions [https://en.wikipedia.org/wiki/Gene_family]"@en;
  skos:inScheme :AnnotationTypeScheme;
  skos:prefLabel "Gene family"@en .

:Viewer a skos:Concept;
  :performsOperation :Viewing;
  rdfs:label "Viewer"@en;
  skos:broader :SupportComponent;
  skos:definition "A component that supports humans in accessing the contents of a resource"@en;
  skos:inScheme :ComponentTypeScheme;
  skos:narrower :CorpusViewer, :LexiconViewer;
  skos:prefLabel "Viewer"@en .

:Location a skos:Concept;
  :documentationUrl "http://dkpro.github.io/dkpro-core/releases/1.8.0/docs/typesystem-reference.html#de.tudarmstadt.ukp.dkpro.core.api.ner.type.Location";
  rdfs:label "Location"@en;
  skos:broader :NamedEntity;
  skos:definition "A word or group of words that denotes a geographical entity"@en;
  skos:inScheme :AnnotationTypeScheme;
  skos:prefLabel "Location"@en .

:Tbx a skos:Concept;
  :documentationUrl "https://www.tbxinfo.net/tbx-about/";
  rdfs:label "tbx"@en;
  skos:broader :Xml;
  skos:definition "TermBase eXchange (TBX) is an international standard (ISO 30042:2019) for the representation of structured concept-oriented terminological data, copublished by ISO and the Localization Industry Standards Association (LISA) [wikipedia]"@en;
  skos:inScheme :DataFormatScheme;
  skos:prefLabel "tbx"@en .

:SemanticClassLabelling a skos:Concept;
  rdfs:label "Semantic class labelling"@en;
  skos:altLabel "Semantic class labeling [en-US]"@en-us;
  skos:broader :SemanticAnnotation;
  skos:definition "The task/process of classifying words in a text according to a set of semantic classes (types)."@en;
  skos:inScheme :OperationScheme;
  skos:prefLabel "Semantic class labelling"@en .

:PersuasiveExpressionMiner a skos:Concept;
  :performsOperation :PersuasiveExpressionMining;
  rdfs:label "Persuasive expression miner"@en;
  skos:broader :Analyzer;
  skos:definition "A component that tries to identify persuasive expressions in a given text"@en;
  skos:editorialNote "could also be an annotator"@en;
  skos:inScheme :ComponentTypeScheme;
  skos:prefLabel "Persuasive expression miner"@en .

:ComputationalArgumentation a skos:Concept;
  rdfs:label "Computational argumentation"@en;
  skos:broader :InformationExtraction;
  skos:definition "The process/task of identifying and representing argumentation in text, so that systems have the ability to use them in tasks, such as automated logical reasoning"@en;
  skos:inScheme :OperationScheme;
  skos:narrower :ArgumentMining;
  skos:prefLabel "Computational argumentation"@en .

:KeaCorpus skos:inScheme :DataFormatScheme .

:Debugging a skos:Concept;
  rdfs:label "Debugging"@en;
  skos:broader :SupportOperation;
  skos:definition "The task/process of removing errors from a computer programme"@en;
  skos:inScheme :OperationScheme;
  skos:prefLabel "Debugging"@en .

:text_plain a skos:Concept;
  rdfs:label "text/plain";
  skos:broader :Mimetype;
  skos:inScheme :MimeTypeScheme .

:CorpusManagement a skos:Concept;
  rdfs:label "Corpus management"@en;
  skos:broader :SupportOperation;
  skos:definition "The task/process of managing corpora, e.g. creating, viewing, etc. through an integrated environment"@en;
  skos:inScheme :OperationScheme;
  skos:narrower :ManagementOfAnnotations;
  skos:prefLabel "Corpus management"@en .

:DocumentClassifier a skos:Concept;
  :performsOperation :TextCategorization;
  rdfs:label "Document classifier"@en;
  skos:broader :Analyzer;
  skos:definition "A component that tries to classify a document into one or more categories"@en;
  skos:inScheme :ComponentTypeScheme;
  skos:prefLabel "Document classifier"@en .

:EntityMentionPair a skos:Concept;
  rdfs:label "Entity-Mention pair"@en;
  skos:broader :Coreference;
  skos:definition "The pair of an entity and all the mentions of this entity formulated in various ways; used in co-reference resolution"@en;
  skos:inScheme :AnnotationTypeScheme;
  skos:prefLabel "Entity-Mention pair"@en .

:Person a skos:Concept;
  :documentationUrl "http://dkpro.github.io/dkpro-core/releases/1.8.0/docs/typesystem-reference.html#de.tudarmstadt.ukp.dkpro.core.api.ner.type.Person";
  rdfs:label "Person"@en;
  skos:broader :NamedEntity;
  skos:definition "A word or group of words that refers to a person"@en;
  skos:inScheme :AnnotationTypeScheme;
  skos:prefLabel "Person"@en .

:SerializedCas a skos:Concept;
  :documentationUrl "http://dkpro.github.io/dkpro-core/releases/1.8.0/docs/format-reference.html#format-SerializedCas";
  rdfs:label "Serialized CAS"@en;
  skos:broader :UimaCasFormat;
  skos:definition "The CAS is the native data model used by UIMA; there are various ways of saving CAS data, using XMI, XCAS, or binary formats; this is for the serialized format"@en;
  skos:inScheme :DataFormatScheme;
  skos:prefLabel "Serialized CAS"@en .

:Transliteration a skos:Concept;
  rdfs:label "Transliteration"@en;
  skos:altLabel "Script conversion"@en;
  skos:broader :SupportOperation;
  skos:definition "Transliteration is the process of transferring a word from the alphabet of one language to another. [vocabulary.com]"@en;
  skos:inScheme :OperationScheme;
  skos:prefLabel "Transliteration"@en .

:TagsetConversion a skos:Concept;
  rdfs:label "Tagset conversion"@en;
  skos:broader :SupportOperation;
  skos:inScheme :OperationScheme;
  skos:prefLabel "Tagset conversion"@en .

:text_x_org_dkpro_conll2000 a skos:Concept;
  rdfs:label "text/x.org.dkpro.conll-2000";
  skos:broader :Mimetype;
  skos:inScheme :MimeTypeScheme .

:application_vnd_openxmlformats_officedocument_wordprocessingml_document a skos:Concept;
  rdfs:label "application/vnd.openxmlformats-officedocument.wordprocessingml.document";
  skos:broader :Mimetype;
  skos:inScheme :MimeTypeScheme .

:Reading a skos:Concept;
  rdfs:label "Reading"@en;
  skos:broader :ResourceAccess;
  skos:definition "Getting access to the contents of an input resource"@en;
  skos:inScheme :OperationScheme;
  skos:narrower :Concordancing;
  skos:prefLabel "Reading"@en .

:audio_mpeg a skos:Concept;
  rdfs:label "audio/mpeg";
  skos:broader :Mimetype;
  skos:inScheme :MimeTypeScheme .

:mp3 a skos:Concept;
  :hasFileExtension "mp3";
  :hasMimetype :audio_mpeg3, :audio_x_mpeg3;
  rdfs:label "audio mp3"@en;
  skos:broader :AudioFormat;
  skos:inScheme :DataFormatScheme;
  skos:prefLabel "audio mp3"@en .

:SpellingChecker a skos:Concept;
  rdfs:label "Spelling checker"@en;
  skos:broader :PreOrPostProcessor;
  skos:definition "A component that corrects spelling mistakes in a text"@en;
  skos:inScheme :ComponentTypeScheme;
  skos:prefLabel "Spelling checker"@en .

:application_ld_json a skos:Concept;
  rdfs:label "application/ld+json";
  skos:broader :Mimetype;
  skos:inScheme :MimeTypeScheme .

:Regularisation a skos:Concept;
  dc:source "adapted from Wikipedia (https://en.wikipedia.org/wiki/Regularization_(mathematics))"@en;
  rdfs:label "Regularisation"@en;
  skos:altLabel "Regularization"@en;
  skos:broader :MachineAndStatisticalLearningMethod;
  skos:definition "A process of introducing additional information in order to solve an ill-posed problem or to prevent overfitting."@en;
  skos:inScheme :TdmMethodScheme;
  skos:prefLabel "Regularisation"@en .

:SpokenLanguageUnderstanding a skos:Concept;
  rdfs:label "Spoken Language Understanding"@en;
  skos:broader :SpeechRecognition;
  skos:definition "Spoken language understanding is the task of assigning a semantic interpretation to a spoken input, by making use of syntactic and semantic knowledge, which is often specific to a particular application domain. Spoken language understanding can involve dealing with multiple recognition hypotheses from a speech recogniser, taking prosodic properties of utterances into account and having to deal with fragmentary and grammatically incorrect utterances. Commercial speech recognisers often are accompanied by analysis tools. In commercial applications such as dialogue systems and command and control, spoken language understanding generally involves the construction of a task and domain-specific interpretation of the utterance."@en;
  skos:inScheme :OperationScheme;
  skos:prefLabel "Spoken Language Understanding"@en .

:Relation a skos:Concept;
  rdfs:label "Relation"@en;
  skos:broader :DomainSpecificAnnotationType;
  skos:definition "Any type of relation that holds between two or more entities of a specific domain"@en;
  skos:inScheme :AnnotationTypeScheme;
  skos:prefLabel "Relation"@en .

:text_csv rdfs:label "text/csv" .

:text_tabSeparatedValues a skos:Concept;
  rdfs:label "text/tab-separated-values";
  skos:broader :Mimetype;
  skos:inScheme :MimeTypeScheme .

:SentenceSimilarityAssessment a skos:Concept;
  rdfs:label "Sentence similarity assessment"@en;
  skos:broader :TextSimilarityAssessment;
  skos:inScheme :OperationScheme;
  skos:prefLabel "Sentence similarity assessment"@en .

:text_x_org_dkpro_conll2006 a skos:Concept;
  rdfs:label "text/x.org.dkpro.conll-2006";
  skos:broader :Mimetype;
  skos:inScheme :MimeTypeScheme .

:MultimediaDocumentProcessing a skos:Concept;
  rdfs:label "Multimedia document processing"@en;
  skos:broader :OperationWithMultimediaInputOrOutput;
  skos:inScheme :OperationScheme;
  skos:prefLabel "Multimedia document processing"@en .

:LanguageIdentifier skos:broader :Analyzer .

:TextGeneration a skos:Concept;
  rdfs:label "Text generation"@en;
  skos:broader :ModelFunction, :NaturalLanguageGeneration;
  skos:inScheme :OperationScheme;
  skos:narrower :DataToTextGeneration, :TextToTextGeneration;
  skos:prefLabel "Text generation"@en .

:Obo a skos:Concept;
  :documentationUrl "http://owlcollab.github.io/oboformat/doc/obo-syntax.html";
  rdfs:label "OBO"@en;
  skos:broader :RdfFormat, :RdfFormats;
  skos:definition "Serialization format for ontologies according to the Open Biomedical Ontologies model."@en;
  skos:inScheme :DataFormatScheme;
  skos:prefLabel "OBO"@en .

:Visualization a skos:Concept;
  rdfs:label "Visualization"@en;
  skos:altLabel "Presentation and Visualisation"@en, "Visualisation"@en;
  skos:broader :Operation, :SupportOperation;
  skos:definition "The representation of an object, situation, or set of information as a chart, diagram or any other image that helps end users understand the contents or message"@en;
  skos:inScheme :OperationScheme;
  skos:narrower :LexiconVisualization;
  skos:prefLabel "Visualization"@en .

:application_emma_xml a skos:Concept;
  rdfs:label "application/emma+xml";
  skos:broader :Mimetype;
  skos:inScheme :MimeTypeScheme .

:AnnotationTypeScheme a skos:ConceptScheme;
  rdfs:label "Annotation type Taxonomy"@en;
  skos:hasTopConcept :AnnotationType;
  skos:prefLabel "Annotation type Taxonomy"@en .

:OrthographicTranscription a skos:Concept;
  rdfs:label "Orthographic transcription"@en;
  skos:broader :Transcription;
  skos:definition "The task/process of transcribing a source language word/phrase or an audio segment into the standard spelling system of a target language"@en;
  skos:inScheme :OperationScheme;
  skos:prefLabel "Orthographic transcription"@en .

:WikipediaTemplateFilteredArticle a skos:Concept;
  :documentationUrl "https://dkpro.github.io/dkpro-core/releases/1.8.0/docs/format-reference.html#format-WikipediaTemplateFilteredArticle";
  rdfs:label "Wikipedia template filtered article"@en;
  skos:broader :WikipediaFormat;
  skos:definition "Format for wikipedia pages that contain or do not contain the templates specified in the template whitelist and template blacklist"@en;
  skos:inScheme :DataFormatScheme;
  skos:prefLabel "Wikipedia template filtered article"@en .

:MultimediaDevelopment a skos:Concept;
  rdfs:label "Multimedia development"@en;
  skos:broader :OperationWithMultimediaInputOrOutput;
  skos:inScheme :OperationScheme;
  skos:prefLabel "Multimedia development"@en .

:MultimediaAnnotation skos:broader :OperationWithMultimediaInputOrOutput .

:Bionlp a skos:Concept;
  :documentationUrl "https://builds.openminted.eu/job/WP%205.2%20-%20Typesystem%20alignment/eu.openminted.interop$mapping-conversion/doclinks/1/components.html#_bionlp_shared_task_2";
  rdfs:label "BioNLP"@en;
  skos:broader :BionlpFormat, :BionlpFormats;
  skos:definition "File format used for the BioNLP Shared Task format"@en;
  skos:inScheme :DataFormatScheme;
  skos:prefLabel "BioNLP"@en .

:OntologyAcquisition a skos:Concept;
  rdfs:label "Ontology acquisition"@en;
  skos:broader :KnowledgeAcquisition;
  skos:definition "The task/process of creating an ontology based on other resources (corpora, other lexical resources, etc.)"@en;
  skos:inScheme :OperationScheme;
  skos:prefLabel "Ontology acquisition"@en .

:application_x_org_dkpro_negra4 a skos:Concept;
  rdfs:label "application/x.org.dkpro.negra4";
  skos:broader :Mimetype;
  skos:inScheme :MimeTypeScheme .

:application_vnd_msaccess a skos:Concept;
  rdfs:label "application/vnd.msaccess";
  skos:broader :Mimetype;
  skos:inScheme :MimeTypeScheme .

:PartOfSpeech a skos:Concept;
  :documentationUrl "http://dkpro.github.io/dkpro-core/releases/1.8.0/docs/typesystem-reference.html#de.tudarmstadt.ukp.dkpro.core.api.lexmorph.type.pos.POS";
  rdfs:label "Part of Speech"@en;
  owl:equivalentClass <http://purl.org/olia/olia-top.owl#MorphosyntacticCategory>;
  skos:altLabel "Grammatical category"@en, "Morphosyntactic category"@en, "Word category"@en;
  skos:broader :AnnotationType;
  skos:definition "A division of words based on common grammatical features"@en;
  skos:inScheme :AnnotationTypeScheme;
  skos:prefLabel "Part of Speech"@en .

:LexiconExtractorFromCorpora a skos:Concept;
  :performsOperation :LexiconAcquisitionFromCorpora;
  rdfs:label "Lexicon extractor from corpora"@en;
  skos:broader :Analyzer;
  skos:definition "A component that extracts lexical information from corpora in order to produce structured lexical resources"@en;
  skos:inScheme :ComponentTypeScheme;
  skos:prefLabel "Lexicon extractor from corpora"@en .

:MultimediaInformationExtraction a skos:Concept;
  rdfs:label "Multimedia Information Extraction"@en;
  skos:broader :InformationExtraction;
  skos:definition "Multimedia Information Extraction can be considered as an extension of textual information extraction to multimedia documents, in an integrated view."@en,
    "The process/task of automatically extracting structured information from multimedia data"@en;
  skos:inScheme :OperationScheme;
  skos:prefLabel "Multimedia Information Extraction"@en .

:LanguageIdentifier skos:definition "A component that identifies the language of a given text based on its contents"@en .

:BelowPosTagging owl:deprecated true .

:LexiconFormatConversion a skos:Concept;
  rdfs:label "Lexicon format conversion"@en;
  skos:broader :FormatConversion, :SupportOperationForKnowledgeResources;
  skos:definition "The task/process of converting the format of a lexical/conceptual resource into another (e.g. from TSV to XML)"@en;
  skos:inScheme :OperationScheme;
  skos:prefLabel "Lexicon format conversion"@en .

:application_ld_json_profile_http_www_w3_org_ns_anno_jsonld a skos:Concept;
  rdfs:label "application/ld+json;profile=\"http://www.w3.org/ns/anno.jsonld\"";
  skos:broader :Mimetype;
  skos:inScheme :MimeTypeScheme .

:GazeEyeMovement a skos:Concept;
  rdfs:label "Gaze eye movement"@en;
  skos:broader :ModalityAnnotationType;
  skos:inScheme :AnnotationTypeScheme;
  skos:prefLabel "Gaze eye movement"@en .

:DataToTextGeneration a skos:Concept;
  rdfs:label "Data to Text Generation"@en;
  skos:broader :TextGeneration;
  skos:inScheme :OperationScheme;
  skos:prefLabel "Data to Text Generation"@en .

:Crowdsourcing a skos:Concept;
  dc:source <https://www.merriam-webster.com/dictionary/crowdsourcing>;
  rdfs:label "Crowdsourcing"@en;
  skos:broader :TdmMethod;
  skos:definition "The practice of obtaining needed services, ideas, or content by soliciting contributions from a large group of people and especially from the online community rather than from traditional employees or suppliers"@en;
  skos:inScheme :TdmMethodScheme;
  skos:prefLabel "Crowdsourcing"@en .

:AnnotatorOfSemanticRoleLabels a skos:Concept;
  rdfs:label "Annotator of semantic role labels"@en;
  skos:broader :SemanticAnnotator;
  skos:definition "A component that annotates the tokens of a text with Semantic Role labels"@en;
  skos:inScheme :ComponentTypeScheme;
  skos:prefLabel "Annotator of semantic role labels"@en .

:image_bmp a skos:Concept;
  rdfs:label "image/bmp";
  skos:broader :Mimetype;
  skos:inScheme :MimeTypeScheme .

:HeadMovement a skos:Concept;
  rdfs:label "Head movement"@en;
  skos:broader :ModalityAnnotationType;
  skos:inScheme :AnnotationTypeScheme;
  skos:prefLabel "Head movement"@en .

:image_svg a skos:Concept;
  rdfs:label "image/svg+xml";
  skos:broader :Mimetype;
  skos:inScheme :MimeTypeScheme .

:audio_x_mpeg3 a skos:Concept;
  rdfs:label "audio/x-mpeg3";
  skos:broader :Mimetype;
  skos:inScheme :MimeTypeScheme .

:DataFormatScheme a skos:ConceptScheme;
  rdfs:label "Data format Taxonomy"@en;
  skos:hasTopConcept :DataFormat;
  skos:prefLabel "Data format Taxonomy"@en .

:LipTrackingAnalysis a skos:Concept;
  rdfs:label "Lip tracking analysis"@en;
  skos:broader :SpeechRecognition;
  skos:definition "The task/process of recognising the lip contour and tracking the movements of lips in lip reading"@en;
  skos:inScheme :OperationScheme;
  skos:prefLabel "Lip tracking analysis"@en .

:AutomaticHyperlinking a skos:Concept;
  rdfs:label "Automatic hyperlinking"@en;
  skos:broader :InformationExtraction;
  skos:definition "Automatic hyperlinking is the insertion of hyperlinks into text documents by automatic means. The automatic hyperlinking process consists of the identification of hyperlinkable entities (concepts, named entities) in the original text, and the assignment of link targets for each such entity. Named entity recognition is often used for identifying linkable entities, for example geographical locations or organisation names. The assignment of link targets depends on a database with link targets for each entity. In general, there can be several link targets for each entity, for example for a company: its homepage, a map, a stock quote etc. Multiple outgoing hyperlinks from one target are supported by the W3C standard XLINK/XPointer. Automatic hyperlinking is an important technology for enabling the Semantic Web."@en,
    "The identification of hyperlinkable entities (concepts, named entities) in a text and the assignment of hyperlinks (link targets) for each such entity."@en;
  skos:inScheme :OperationScheme;
  skos:prefLabel "Automatic hyperlinking"@en .

:AudienceReaction a skos:Concept;
  rdfs:label "Audience reaction"@en;
  skos:broader :DiscourseAnnotationType;
  skos:definition "The response of the target recipients (audience) to a system, process or event"@en;
  skos:inScheme :AnnotationTypeScheme;
  skos:prefLabel "Audience reaction"@en .

:audio_flac a skos:Concept;
  skos:broader :Mimetype;
  skos:inScheme :MimeTypeScheme .

:Alto rdfs:label "ALTO"@en;
  skos:prefLabel "ALTO"@en .

:text_sgml skos:prefLabel "text/sgml" .

:image_jpeg skos:prefLabel "image/jpeg" .

:application_x_org_dkpro_negra3 skos:prefLabel "application/x.org.dkpro.negra3" .

:audio_basic skos:prefLabel "audio/basic" .

:application_vnd_oasis_opendocument_presentation skos:prefLabel "application/vnd.oasis.opendocument.presentation" .

:application_fastinfoset skos:prefLabel "application/fastinfoset" .

:application_vnd_openxmlformats_officedocument_presentationml_presentation skos:prefLabel
    "application/vnd.openxmlformats-officedocument.presentationml.presentation" .

:application_xml_alto skos:prefLabel "application/xml+alto" .

:application_xLatex skos:prefLabel "application/x-latex" .

:image_png skos:prefLabel "image/png" .

:ModelFunction skos:inScheme :ModelFunctionScheme .

:text_xPubmed skos:prefLabel "text/x-pubmed" .

:application_x_org_dkpro_uima_json skos:prefLabel "application/x.org.dkpro.uima+json" .

:application_vnd_msExcel skos:prefLabel "application/vnd.msExcel" .

:text_x_org_dkpro_conllU skos:prefLabel "text/x.org.dkpro.conll-u" .

:text_x_org_dkpro_conll2008 skos:prefLabel "text/x.org.dkpro.conll-2008" .

:application_postscript skos:prefLabel "application/postscript" .

:text_x_org_dkpro_conll2009 skos:prefLabel "text/x.org.dkpro.conll-2009" .

:application_tei_xml skos:prefLabel "application/tei+xml" .

:application_xml skos:prefLabel "application/xml" .

:text_xCochrane skos:prefLabel "text/x-cochrane" .

:application_anno_json skos:prefLabel "application/anno+json" .

:text_x_org_dkpro_imscwb skos:prefLabel "text/x.org.dkpro.imscwb" .

:application_xXml_alvis skos:prefLabel "application/x-xml+alvis" .

:audio_aiff skos:prefLabel "audio/aiff" .

:text_x_org_dkpro_conll2012 skos:prefLabel "text/x.org.dkpro.conll-2012" .

:text_turtle skos:prefLabel "text/turtle" .

:audio_x_wav skos:prefLabel "audio/x-wav" .

:application_x_org_dkpro_uima_binary skos:prefLabel "application/x.org.dkpro.uima+binary" .

:text_xml skos:prefLabel "text/xml" .

:application_xMsaccess skos:prefLabel "application/x-msaccess" .

:application_x_org_dkpro_reuters21578_sgml skos:prefLabel "application/x.org.dkpro.reuters21578+sgml" .

:application_msword skos:prefLabel "application/msword" .

:application_pdf skos:prefLabel "application/pdf" .

:audio_mpeg3 skos:prefLabel "audio/mpeg3" .

:application_vnd_oasis_opendocument_text skos:prefLabel "application/vnd.oasis.opendocument.text" .

:application_vnd_ms_powerpoint skos:prefLabel "application/vnd.ms-powerpoint" .

:audio_vnd_wave skos:prefLabel "audio/vnd.wave" .

:application_xTex skos:prefLabel "application/x-tex" .

:image_gif skos:prefLabel "image/gif" .

:Zip :hasMimetype :application_zip;
  skos:prefLabel "zip"@en .

:OpenOfficePresentation skos:prefLabel "Open office presentation"@en .

:text_x_eaf_xml skos:prefLabel "text/x-eaf+xml" .

:application_vnd_xmi_xml skos:prefLabel "application/vnd.xmi+xml" .

:TFSavedModel skos:prefLabel "TensorFlow SavedModel"@en .

:application_tika skos:prefLabel "application/tika" .

:text_x_org_dkpro_ngram skos:prefLabel "text/x.org.dkpro.ngram" .

:application_vnd_oasis_opendocument_spreadsheet skos:prefLabel "application/vnd.oasis.opendocument.spreadsheet" .

:application_zip skos:prefLabel "application/zip" .

:video_mp4 skos:prefLabel "video/mp4" .

:application_x_org_dkpro_tiger_xml skos:prefLabel "application/x.org.dkpro.tiger+xml" .

:text_x_org_dkpro_reuters21578 skos:prefLabel "text/x.org.dkpro.reuters21578" .

:image_tiff skos:prefLabel "image/tiff" .

:audio_wav skos:prefLabel "audio/wav" .

:application_xXces_xml skos:prefLabel "application/x-xces+xml" .

:text_html skos:prefLabel "text/html" .

:application_rtf skos:prefLabel "application/rtf" .

:audio_wave skos:prefLabel "audio/wave" .

:application_x_json_twitter skos:prefLabel "application/x-json-twitter" .

:application_x_kaf_json skos:prefLabel "application/x-kaf+json" .

:application_x_org_dkpro_tgrep2 skos:prefLabel "application/x.org.dkpro.tgrep2" .

:application_xhtml_xml skos:prefLabel "application/xhtml+xml" .

:application_xTmx_xml skos:prefLabel "application/x-tmx+xml" .

:text_tcf_xml skos:prefLabel "text/tcf+xml" .

:text_csv skos:prefLabel "text/csv" .

:application_json skos:prefLabel "application/json" .

:audio_mpa skos:prefLabel "audio/MPA" .

:text_x_org_dkpro_ptbChunked skos:prefLabel "text/x.org.dkpro.ptb-chunked" .

:application_x_org_dkpro_tuepp_xml skos:prefLabel "application/x.org.dkpro.tuepp+xml" .

:application_pls_xml skos:prefLabel "application/pls+xml" .

:application_x-SDL-TM skos:prefLabel "application/x-SDL-TM" .

:video_avi skos:prefLabel "video/x-msvideo" .

:text_plain skos:prefLabel "text/plain" .

:text_x_org_dkpro_conll2000 skos:prefLabel "text/x.org.dkpro.conll-2000" .

:application_vnd_openxmlformats_officedocument_wordprocessingml_document skos:prefLabel
    "application/vnd.openxmlformats-officedocument.wordprocessingml.document" .

:audio_mpeg skos:prefLabel "audio/mpeg" .

:application_ld_json skos:prefLabel "application/ld+json" .

:text_tabSeparatedValues skos:prefLabel "text/tab-separated-values" .

:text_x_org_dkpro_conll2006 skos:prefLabel "text/x.org.dkpro.conll-2006" .

:application_emma_xml skos:prefLabel "application/emma+xml" .

:application_x_org_dkpro_negra4 skos:prefLabel "application/x.org.dkpro.negra4" .

:application_vnd_msaccess skos:prefLabel "application/vnd.msaccess" .

:application_ld_json_profile_http_www_w3_org_ns_anno_jsonld skos:prefLabel "application/ld+json;profile=\"http://www.w3.org/ns/anno.jsonld\"" .

:image_bmp skos:prefLabel "image/bmp" .

:image_svg skos:prefLabel "image/svg+xml" .

:audio_x_mpeg3 skos:prefLabel "audio/x-mpeg3" .

:audio_flac skos:prefLabel "audio/flac" .

:application_x_org_dkpro_graf_xml skos:prefLabel "application/x.org.dkpro.graf+xml" .

:application_rdf_xml skos:prefLabel "application/rdf+xml" .

:application_vnd_openxmlformats_officedocument_spreadsheetml_sheet skos:prefLabel
    "application/vnd.openxmlformats-officedocument.spreadsheetml.sheet" .

:text_x_brat skos:prefLabel "text/x-brat" .

:text_x_anafora skos:prefLabel "text/x-anafora" .

:text_x_org_dkpro_conll2003 skos:prefLabel "text/x.org.dkpro.conll-2003" .

:text_x_org_dkpro_ptbCombined skos:prefLabel "text/x.org.dkpro.ptb-combined" .

:audio_mpa_robust skos:prefLabel "audio/mpa-robust" .

:text_x_org_dkpro_conll2002 skos:prefLabel "text/x.org.dkpro.conll-2002" .

:performsOperation rdfs:domain _:node1fu4q14cjx38 .

_:node1fu4q14cjx38 a owl:Class;
  owl:intersectionOf _:node1fu4q14cjx39 .

_:node1fu4q14cjx39 a rdf:List;
  rdf:first skos:Concept;
  rdf:rest _:node1fu4q14cjx40 .

_:node1fu4q14cjx40 a rdf:List;
  rdf:first _:node1fu4q14cjx37 .

_:node1fu4q14cjx37 a owl:Restriction;
  owl:hasValue :ComponentTypeScheme;
  owl:onProperty skos:inScheme .

_:node1fu4q14cjx40 rdf:rest rdf:nil .

:SemanticAnnotation skos:inScheme :ModelFunctionScheme .

:CoreferenceAnnotation skos:inScheme :ModelFunctionScheme .

:SemanticRoleLabelling skos:inScheme :ModelFunctionScheme .

:AnnotationOfDates skos:inScheme :ModelFunctionScheme .

:ParagraphSplitting skos:inScheme :ModelFunctionScheme .

:MorphologicalAnnotation skos:inScheme :ModelFunctionScheme .

:TextAnnotation skos:inScheme :ModelFunctionScheme .

:ReadabilityAnnotation skos:inScheme :ModelFunctionScheme .

:Annotation skos:inScheme :ModelFunctionScheme .

:NounPhraseChunking skos:inScheme :ModelFunctionScheme .

:DataMasking skos:inScheme :ModelFunctionScheme .

:AnnotationOfMeasurements skos:inScheme :ModelFunctionScheme .

:DeepParsing skos:inScheme :ModelFunctionScheme .

:MorphosyntacticTagging skos:inScheme :ModelFunctionScheme .

:TerminologyMarkup skos:inScheme :ModelFunctionScheme .

:Tokenization skos:inScheme :ModelFunctionScheme .

:AnnotationOfSpeakerTurns skos:inScheme :ModelFunctionScheme .

:TextEncryption skos:inScheme :ModelFunctionScheme .

:Parsing skos:inScheme :ModelFunctionScheme .

:FrameSemanticParsing skos:inScheme :ModelFunctionScheme .

:SentenceSplitting skos:inScheme :ModelFunctionScheme .

:Anonymization skos:inScheme :ModelFunctionScheme .

:BelowPosTagging skos:inScheme :ModelFunctionScheme .

:AnnotationOfMultiWordUnits skos:inScheme :ModelFunctionScheme .

:EntityLinking skos:inScheme :ModelFunctionScheme .

:TemporalExpressionsLabelling skos:inScheme :ModelFunctionScheme .

:EventLabelling skos:inScheme :ModelFunctionScheme .

:PosTagging skos:inScheme :ModelFunctionScheme .

:ParalanguageAnnotation skos:inScheme :ModelFunctionScheme .

:SemanticRelationLabelling skos:inScheme :ModelFunctionScheme .

:Argumentation skos:inScheme :ModelFunctionScheme .

:Lemmatization skos:inScheme :ModelFunctionScheme .

:DiscourseAnnotation skos:inScheme :ModelFunctionScheme .

:MultimediaAnnotation skos:inScheme :ModelFunctionScheme .

:ProsodicSegmentation skos:inScheme :ModelFunctionScheme .

:AnnotationOfCompounds skos:inScheme :ModelFunctionScheme .

_:node1fu7rlrd8x1 a owl:Restriction;
  owl:hasValue :DataFormatScheme;
  owl:onProperty skos:inScheme .

_:node1fu7rlrd8x3 a rdf:List;
  rdf:first skos:Concept;
  rdf:rest _:node1fu7rlrd8x4 .

_:node1fu7rlrd8x4 a rdf:List;
  rdf:first _:node1fu7rlrd8x1;
  rdf:rest rdf:nil .

_:node1fu4q14cjx29 a owl:Restriction;
  owl:hasValue :DataFormatScheme;
  owl:onProperty skos:inScheme .

_:node1fu4q14cjx32 a rdf:List;
  rdf:first _:node1fu4q14cjx29;
  rdf:rest rdf:nil .

_:node1fu7rlrd8x2 a owl:Class;
  owl:intersectionOf _:node1fu7rlrd8x3 .

_:node1fu4q14cjx31 a rdf:List;
  rdf:first skos:Concept;
  rdf:rest _:node1fu4q14cjx32 .

_:node1fu4q14cjx18 a owl:Restriction;
  owl:hasValue :application_zip;
  owl:onProperty :hasMimetype .

_:node1fu4q14cjx21 a owl:Restriction;
  owl:hasValue :AnnotationTypeScheme;
  owl:onProperty skos:inScheme .

_:node1fu4q14cjx30 owl:intersectionOf _:node1fu4q14cjx31 .

_:node1fu4q14cjx22 a owl:Restriction;
  owl:hasValue :OperationScheme;
  owl:onProperty skos:inScheme .

_:node1fu4q14cjx41 a owl:Restriction;
  owl:hasValue :OperationScheme;
  owl:onProperty skos:inScheme .

_:node1fu4q14cjx23 a owl:Restriction;
  owl:hasValue :TdmMethodScheme;
  owl:onProperty skos:inScheme .

_:node1fu4q14cjx42 a owl:Class;
  owl:intersectionOf _:node1fu4q14cjx43 .

_:node1fu4q14cjx43 a rdf:List;
  rdf:first skos:Concept;
  rdf:rest _:node1fu4q14cjx44 .

_:node1fu4q14cjx44 a rdf:List;
  rdf:first _:node1fu4q14cjx41;
  rdf:rest rdf:nil .

_:node1fu4q14cjx24 a owl:Restriction;
  owl:hasValue :DataFormatScheme;
  owl:onProperty skos:inScheme .

_:node1fu4q14cjx25 owl:onProperty skos:inScheme .
